@prefix ex: <http://example.org/ontology/> .
@prefix imdrf: <http://imdrf.org/> .
@prefix owl: <http://www.w3.org/2002/07/owl#> .
@prefix rdfs: <http://www.w3.org/2000/01/rdf-schema#> .

imdrf:A010101 a owl:Class ;
    rdfs:label "Biocompatibility" ;
    rdfs:comment "Problem associated with undesirable local or systemic effects due to exposure to medical device materials or leachates from those materials by a patient who has an implant or is receiving treatment with a device made from them." ;
    rdfs:subClassOf imdrf:A0101 .

imdrf:A010102 a owl:Class ;
    rdfs:label "Device Appears to Trigger Rejection" ;
    rdfs:comment "The device appears to elicit undesired response in the patient to the presence of an implanted or invasive device, without inherent device failure, e.g. fibrous encapsulation, or inflammation of the tissue around the device, or extrusion of the device." ;
    rdfs:subClassOf imdrf:A0101 .

imdrf:A010103 a owl:Class ;
    rdfs:label "Inadequacy of Device Shape and/or Size" ;
    rdfs:comment "The physical size and/or shape of the device was inadequate with regard to the patient's anatomy." ;
    rdfs:subClassOf imdrf:A0101 .

imdrf:A010201 a owl:Class ;
    rdfs:label "Failure to Osseointegrate" ;
    rdfs:comment "Problem associated with the failure to see direct anchorage of an implant by the formation of bony tissue around the implant without the growth of fibrous tissue at the bone-implant interface." ;
    rdfs:subClassOf imdrf:A0102 .

imdrf:A010202 a owl:Class ;
    rdfs:label "Loss of Osseointegration" ;
    rdfs:comment "Problem associated with weakened integration of the device at the bone-implant interface due to loss of fibrous and/or bony tissue and leading to compromised anchorage of the device. i.e. Loosening/Lysis" ;
    rdfs:subClassOf imdrf:A0102 .

imdrf:A0103 a owl:Class ;
    rdfs:label "Loosening of Implant Not Related to Bone-Ingrowth" ;
    rdfs:comment "Problem associated with the loss of direct anchorage of an implanted device over time or due to an injury." ;
    rdfs:subClassOf imdrf:A01 .

imdrf:A010401 a owl:Class ;
    rdfs:label "Expulsion" ;
    rdfs:comment "Problem with all or part of an implanted or invasive device being completely expelled from its intended location within the body." ;
    rdfs:subClassOf imdrf:A0104 .

imdrf:A010402 a owl:Class ;
    rdfs:label "Migration" ;
    rdfs:comment "Problem with all or part of an implanted or invasive device moving from its intended location within the body." ;
    rdfs:subClassOf imdrf:A0104 .

imdrf:A0105 a owl:Class ;
    rdfs:label "Lack of Effect" ;
    ex:statusDescription "Term was added on 27 January 2022. For details, see comment No. 23 of the Change Log (Release Number 2022)." ;
    rdfs:comment "Problems associated with a product having less efficacy than expected. No other malfunctions could be identified." ;
    rdfs:subClassOf imdrf:A01 .

imdrf:A0106 a owl:Class ;
    rdfs:label "Device Stenosis" ;
    ex:statusDescription "Term was added on 27 January 2022. For details, see comment No. 148, 176 of the Change Log (Release Number 2022)." ;
    rdfs:comment "Problem associated with the narrowing or obstruction of the device (e.g. prosthetic heart valves, stents, etc.)." ;
    rdfs:subClassOf imdrf:A01 .

imdrf:A0107 a owl:Class ;
    rdfs:label "Implant subsidence" ;
    ex:statusDescription "Term added for Release Number 2024. See no. 44 of Change Log" ;
    rdfs:comment "Problem related to the settling or collapse of bone adjacent to an implanted device, in direction of the loading force." ;
    rdfs:subClassOf imdrf:A01 .

imdrf:A020101 a owl:Class ;
    rdfs:label "Dull, Blunt" ;
    rdfs:comment "Problem associated with a device not being as sharp as intended or expected." ;
    rdfs:subClassOf imdrf:A0201 .

imdrf:A020102 a owl:Class ;
    rdfs:label "Nonstandard Device" ;
    rdfs:comment "Problem associated with the device that does not meet the specifications or requirements for which it was manufactured (e.g. materials, parts, manufacturing process)." ;
    rdfs:subClassOf imdrf:A0201 .

imdrf:A0202 a owl:Class ;
    rdfs:label "Defective Component" ;
    ex:status "Retired" ;
    ex:statusDescription "Term retired for Release Number 2025. Use A020102 - Nonstandard Device or other codes which describe the specific defect with the component. See no. 1 of Change Request Log" ;
    rdfs:comment "Problem associated with a device component having flaws of dimensional deviations greater than acceptable for the intended use." ;
    rdfs:subClassOf imdrf:A02 .

imdrf:A0203 a owl:Class ;
    rdfs:label "Defective Device" ;
    ex:status "Retired" ;
    ex:statusDescription "Term retired for Release Number 2025. Use A020102 - Nonstandard Device or other codes which describe the specific defect with the device. See no. 1 of Change Request Log" ;
    rdfs:comment "Problem associated with having flaws or dimensional deviations greater than acceptable for the intended use of the device." ;
    rdfs:subClassOf imdrf:A02 .

imdrf:A0204 a owl:Class ;
    rdfs:label "Device Damaged Prior to Use" ;
    ex:status "Retired" ;
    ex:statusDescription "Term retired for Release Number 2025. Use A0207 - Device Damaged Prior to Receipt by User. See no. 106 of Change Request Log" ;
    rdfs:comment "Problem associated with packaging or shipping damage prior to the use of the device." ;
    rdfs:subClassOf imdrf:A02 .

imdrf:A020501 a owl:Class ;
    rdfs:label "Difficult to Open or Remove Packaging Material" ;
    rdfs:comment "Problem associated with difficulty for users to operate the device, specifically as it relates to the opening or removal of the outer wrapping." ;
    rdfs:subClassOf imdrf:A0205 .

imdrf:A020502 a owl:Class ;
    rdfs:label "Incomplete or Missing Packaging" ;
    rdfs:comment "Problem associated with the nonconformance to the device specifications due to incomplete or missing packaging that may compromise the device operation as intended." ;
    rdfs:subClassOf imdrf:A0205 .

imdrf:A020503 a owl:Class ;
    rdfs:label "Unsealed Device Packaging" ;
    rdfs:comment "Problem associated with the loss of packaging seal." ;
    rdfs:subClassOf imdrf:A0205 .

imdrf:A020504 a owl:Class ;
    rdfs:label "Tear, Rip or Hole in Device Packaging" ;
    rdfs:comment "Problem associated with packaging damage (tear, rip or hole) prior to the use of the device." ;
    rdfs:subClassOf imdrf:A0205 .

imdrf:A020505 a owl:Class ;
    rdfs:label "Device packaging look-alike" ;
    ex:statusDescription "Term added for Release Number 2024. See no. 116 of Change Log" ;
    rdfs:comment "Problem associated with medical device packaging that looks similar to another product leading to confusion. The other product may be another device or a different product such as a medicine or cleaning agent.  Use A210107 for Device label look-alike." ;
    rdfs:subClassOf imdrf:A0205 .

imdrf:A020601 a owl:Class ;
    rdfs:label "Component Misassembled" ;
    ex:statusDescription "Definition was modified on 27 January 2022 (Old definition: Component Misassembled: A device found to have one or more components incorrectly assembled when delivered to the user facility. For details, see comment No. 1 of the Change Log (Release Number 2022)." ;
    rdfs:comment "A device found to have one or more components incorrectly assembled when delivered to the user facility. This includes cases in which components are interchanged." ;
    rdfs:subClassOf imdrf:A0206 .

imdrf:A020602 a owl:Class ;
    rdfs:label "Component Missing" ;
    rdfs:comment "A device component(s) found to be missing when delivered to the user facility." ;
    rdfs:subClassOf imdrf:A0206 .

imdrf:A020603 a owl:Class ;
    rdfs:label "Extra Components" ;
    ex:statusDescription "Term was added on 27 January 2022. For details, see comment No. 222 of the Change Log (Release Number 2022)." ;
    rdfs:comment "More than the usual number of components present/additional components from this or other devices." ;
    rdfs:subClassOf imdrf:A0206 .

imdrf:A020701 a owl:Class ;
    rdfs:label "Delivered as Unsterile Product" ;
    rdfs:comment "Problem associated with a device being received in such a manner to indicate that its sterility has been compromised (e.g. sterile packaging breached, visible contaminate present)" ;
    rdfs:subClassOf imdrf:A0207 .

imdrf:A0301 a owl:Class ;
    rdfs:label "Device Emits Odor" ;
    rdfs:comment "Problem associated with an unexpected or inappropriate smell released by the device." ;
    rdfs:subClassOf imdrf:A03 .

imdrf:A030201 a owl:Class ;
    rdfs:label "Clumping in Device or Device Ingredient" ;
    rdfs:comment "Problem associated with the aggregation of particles into irregular masses." ;
    rdfs:subClassOf imdrf:A0302 .

imdrf:A030202 a owl:Class ;
    rdfs:label "Coagulation in Device or Device Ingredient" ;
    rdfs:comment "Problem associated with the undesired characterization of congealing, solidifying, thickening, curdling." ;
    rdfs:subClassOf imdrf:A0302 .

imdrf:A030203 a owl:Class ;
    rdfs:label "Precipitate in Device or Device Ingredient" ;
    rdfs:comment "Problem associated with the separation of solid particles from a liquid as the result of a chemical or physical change." ;
    rdfs:subClassOf imdrf:A0302 .

imdrf:A030204 a owl:Class ;
    rdfs:label "Cross Reactivity" ;
    rdfs:comment "Problem associated with the degree to which an antibody or antigen participates in cross reactions." ;
    rdfs:subClassOf imdrf:A0302 .

imdrf:A030205 a owl:Class ;
    rdfs:label "Particulates" ;
    rdfs:comment "Substances that consist of separate particles that are introduced by the device during use." ;
    rdfs:subClassOf imdrf:A0302 .

imdrf:A030206 a owl:Class ;
    rdfs:label "High pH" ;
    rdfs:comment "pH higher than expected and/or anticipated." ;
    rdfs:subClassOf imdrf:A0302 .

imdrf:A030207 a owl:Class ;
    rdfs:label "Low pH" ;
    rdfs:comment "pH lower than expected and/or anticipated." ;
    rdfs:subClassOf imdrf:A0302 .

imdrf:A030208 a owl:Class ;
    rdfs:label "Unexpected Color" ;
    ex:statusDescription "Term was added on 18 March 2020 as an additional level 3 term under \"Device Ingredient or Reagent Problem\"." ;
    rdfs:comment "Color of product is different from that expected." ;
    rdfs:subClassOf imdrf:A0302 .

imdrf:A0303 a owl:Class ;
    rdfs:label "Improper Chemical Reaction" ;
    rdfs:comment "Problem associated with an unexpected or incomplete chemical reaction or effect." ;
    rdfs:subClassOf imdrf:A03 .

imdrf:A040101 a owl:Class ;
    rdfs:label "Fracture" ;
    rdfs:comment "Problem associated with a partial or full-thickness crack in the device materials." ;
    rdfs:subClassOf imdrf:A0401 .

imdrf:A040102 a owl:Class ;
    rdfs:label "Loss of or Failure to Bond" ;
    ex:statusDescription "Definition modified for Release Number 2024. See no. 26 of Change Log" ;
    rdfs:comment "Problem associated with lack or loss of adherence between materials intended to be joined together by any bonding such as an adhesive, heat welding, etc." ;
    rdfs:subClassOf imdrf:A0401 .

imdrf:A040103 a owl:Class ;
    rdfs:label "Material Fragmentation" ;
    rdfs:comment "Problem associated with small pieces of the device breaking off unexpectedly." ;
    rdfs:subClassOf imdrf:A0401 .

imdrf:A040104 a owl:Class ;
    rdfs:label "Solder Joint Fracture" ;
    rdfs:comment "Problem associated with undesired damage or breakage in a solder joint of materials used in the device construction." ;
    rdfs:subClassOf imdrf:A0401 .

imdrf:A0402 a owl:Class ;
    rdfs:label "Burst Container or Vessel" ;
    rdfs:comment "Problem associated with the pressure inside a vessel or container rising to such a degree that the container ruptures." ;
    rdfs:subClassOf imdrf:A04 .

imdrf:A0403 a owl:Class ;
    rdfs:label "Explosion" ;
    rdfs:comment "Problem associated with the violent bursting due to the sudden expansion of air, gas or fluid." ;
    rdfs:subClassOf imdrf:A04 .

imdrf:A0404 a owl:Class ;
    rdfs:label "Crack" ;
    rdfs:comment "Problem associated with an undesired partial separation and/or a visible opening along the length or width in the materials that are used in the device construction." ;
    rdfs:subClassOf imdrf:A04 .

imdrf:A040501 a owl:Class ;
    rdfs:label "Calcified" ;
    rdfs:comment "Problem associated with buildup of calcium salts on the device." ;
    rdfs:subClassOf imdrf:A0405 .

imdrf:A040502 a owl:Class ;
    rdfs:label "Corroded" ;
    rdfs:comment "Problem associated with the chemical or electrochemical reaction between materials, usually a metal and its environment that produces a deterioration of the metal and its properties." ;
    rdfs:subClassOf imdrf:A0405 .

imdrf:A040503 a owl:Class ;
    rdfs:label "Material Erosion" ;
    rdfs:comment "Problem associated with a progressive loss of a material from a solid surface." ;
    rdfs:subClassOf imdrf:A0405 .

imdrf:A040504 a owl:Class ;
    rdfs:label "Pitted" ;
    rdfs:comment "Problem associated with the corrosion of a material's surface, confined to a point or small area that takes the form of cavities." ;
    rdfs:subClassOf imdrf:A0405 .

imdrf:A040505 a owl:Class ;
    rdfs:label "Flaked" ;
    rdfs:comment "Problem associated with the detachment of small pieces of the coating film of a material." ;
    rdfs:subClassOf imdrf:A0405 .

imdrf:A040506 a owl:Class ;
    rdfs:label "Peeled/Delaminated" ;
    rdfs:comment "Peeling or delamination of composite materials, including coatings, that occurs when layers are separated as a result of stress or impact and resulting in loss of mechanical toughness." ;
    rdfs:subClassOf imdrf:A0405 .

imdrf:A040507 a owl:Class ;
    rdfs:label "Naturally Worn" ;
    rdfs:comment "Problem associated with material damage to a surface, usually involving progressive loss or displacement of material, due to relative motion between that surface and a contacting substance or substances." ;
    rdfs:subClassOf imdrf:A0405 .

imdrf:A040508 a owl:Class ;
    rdfs:label "Unraveled Material" ;
    rdfs:comment "Problem due to the undesired unravelling of material (e.g. disentangled, unwound etc.)." ;
    rdfs:subClassOf imdrf:A0405 .

imdrf:A040601 a owl:Class ;
    rdfs:label "Deformation Due to Compressive Stress" ;
    rdfs:comment "Problem associated with an undesired bulge, bend, bow, kink, or wavy condition observed in the device material resulting from compressive stresses." ;
    rdfs:subClassOf imdrf:A0406 .

imdrf:A040602 a owl:Class ;
    rdfs:label "Dent in Material" ;
    rdfs:comment "Problem associated with a undesired change in shape, characterized by the presence of a slight hollow (dent) in the device surface." ;
    rdfs:subClassOf imdrf:A0406 .

imdrf:A040603 a owl:Class ;
    rdfs:label "Failure to Fold" ;
    rdfs:comment "Problem associated with an undesired material change in physical property, characterized by failure to fold." ;
    rdfs:subClassOf imdrf:A0406 .

imdrf:A040604 a owl:Class ;
    rdfs:label "Failure to Unfold or Unwrap" ;
    rdfs:comment "Problem associated with the comprising materials' deformation in that device fails to open its wrapping or open/extend in a certain manner i.e. balloon or lens." ;
    rdfs:subClassOf imdrf:A0406 .

imdrf:A040605 a owl:Class ;
    rdfs:label "Material Frayed" ;
    rdfs:comment "Problem associated with the comprising materials having damaged edges." ;
    rdfs:subClassOf imdrf:A0406 .

imdrf:A040606 a owl:Class ;
    rdfs:label "Material Invagination" ;
    rdfs:comment "Problem associated with an undesired material change in shape, characterized by the infolding of one part within another part of a structure." ;
    rdfs:subClassOf imdrf:A0406 .

imdrf:A040607 a owl:Class ;
    rdfs:label "Material Too Rigid or Stiff" ;
    ex:status "Modified (technical)" ;
    ex:statusDescription "Definition modified for Release Number 2025. See no. 44 of Change Request Log" ;
    rdfs:comment "Problem associated with undesired rigidity of device material (resisting deformation in response to an applied force)." ;
    rdfs:subClassOf imdrf:A0406 .

imdrf:A040608 a owl:Class ;
    rdfs:label "Material Too Soft/Flexible" ;
    rdfs:comment "Problem associated with any device material that results in the material's inability to maintain the desired shape or support function." ;
    rdfs:subClassOf imdrf:A0406 .

imdrf:A040609 a owl:Class ;
    rdfs:label "Material Twisted/Bent" ;
    rdfs:comment "Problem associated with deformations that lead to twisting or bending of the device." ;
    rdfs:subClassOf imdrf:A0406 .

imdrf:A040610 a owl:Class ;
    rdfs:label "Melted" ;
    rdfs:comment "Problem associated with a solid device being transformed into a molten or liquid state." ;
    rdfs:subClassOf imdrf:A0406 .

imdrf:A040611 a owl:Class ;
    rdfs:label "Stretched" ;
    rdfs:comment "Problem associated with an increase or elongation in a materials' dimension." ;
    rdfs:subClassOf imdrf:A0406 .

imdrf:A040612 a owl:Class ;
    rdfs:label "Thickening of Material" ;
    ex:statusDescription "Term was added on 18 March 2020 as an additional level 3 term under \"Material Deformation\"." ;
    rdfs:comment "Device is thickened due to deformation. Note: Not to be used for thickening of liquid." ;
    rdfs:subClassOf imdrf:A0406 .

imdrf:A0407 a owl:Class ;
    rdfs:label "Material Discolored" ;
    rdfs:comment "Problem associated with an undesired streak, pattern and/or a noticeable change in color from the rest of the materials used in the device construction." ;
    rdfs:subClassOf imdrf:A04 .

imdrf:A0408 a owl:Class ;
    rdfs:label "Material Disintegration" ;
    rdfs:comment "Problem associated with material breaking into small particles." ;
    rdfs:subClassOf imdrf:A04 .

imdrf:A0409 a owl:Class ;
    rdfs:label "Material Opacification" ;
    rdfs:comment "Problem associated with an undesirable opaqueness or cloudiness." ;
    rdfs:subClassOf imdrf:A04 .

imdrf:A041001 a owl:Class ;
    rdfs:label "Material Puncture/Hole" ;
    rdfs:comment "Device material(s) punctured leading to undesired holes/openings." ;
    rdfs:subClassOf imdrf:A0410 .

imdrf:A0411 a owl:Class ;
    rdfs:label "Material Protrusion/Extrusion" ;
    rdfs:comment "Problem associated with undesired physical appearance of device material, specifically when material extends beyond or above device surface." ;
    rdfs:subClassOf imdrf:A04 .

imdrf:A0412 a owl:Class ;
    rdfs:label "Material Rupture" ;
    rdfs:comment "Problem associated with perforations that lead to bursting of the device." ;
    rdfs:subClassOf imdrf:A04 .

imdrf:A0413 a owl:Class ;
    rdfs:label "Material Separation" ;
    rdfs:comment "Problem associated with an undesired disassociation or breaking apart of the device." ;
    rdfs:subClassOf imdrf:A04 .

imdrf:A0414 a owl:Class ;
    rdfs:label "Material Split, Cut or Torn" ;
    rdfs:comment "Problem associated with materials consisting the device are split, cut or torn due to external forces (e.g. wrenching or laceration) or internal forces (e.g. exceeding the tensile stress limits belonging to the materials used in the device construction)." ;
    rdfs:subClassOf imdrf:A04 .

imdrf:A0415 a owl:Class ;
    rdfs:label "Scratched Material" ;
    rdfs:comment "Problem associated with an undesirable shallow cut or narrow groove in the surface of the device materials." ;
    rdfs:subClassOf imdrf:A04 .

imdrf:A0416 a owl:Class ;
    rdfs:label "Failure to Degrade" ;
    ex:status "New" ;
    ex:statusDescription "Term added for Release Number 2025. See no. 87 of Change Request Log" ;
    rdfs:comment "Failure of a material to degrade, absorb, dissolve, etc. in an appropriate manner, when the material is expected to do so." ;
    rdfs:subClassOf imdrf:A04 .

imdrf:A0501 a owl:Class ;
    rdfs:label "Detachment of Device or Device Component" ;
    rdfs:comment "Problem associated with the separation of the device from its physical construct, integrity, or chassis." ;
    rdfs:subClassOf imdrf:A05 .

imdrf:A0502 a owl:Class ;
    rdfs:label "Device Damaged by Another Device" ;
    rdfs:comment "Problem associated with one device causing harm to another device." ;
    rdfs:subClassOf imdrf:A05 .

imdrf:A050301 a owl:Class ;
    rdfs:label "Failure to Eject" ;
    ex:statusDescription "Editorial change to the definition on 18 March 2020." ;
    rdfs:comment "Problem associated with the inability of the device to be ejected or discharged from its physical location." ;
    rdfs:subClassOf imdrf:A0503 .

imdrf:A050302 a owl:Class ;
    rdfs:label "Unintended Ejection" ;
    ex:statusDescription "Editorial change to the definition on 18 March 2020." ;
    rdfs:comment "Problem associated with unexpected ejection of the device from its physical location. This includes but is not limited to devices such as clip appliers, film cartridge, and staples." ;
    rdfs:subClassOf imdrf:A0503 .

imdrf:A050401 a owl:Class ;
    rdfs:label "Fluid/Blood Leak" ;
    ex:statusDescription "Term/Definition was modified on 27 January 2022 (Old term/definition: Fluid Leak: Escape (Release, Discharge) of fluid through an unintended location often accompanied by a loss of pressure and/or output). For details, see comment No. 15, 16, 17, 18 of the Change Log (Release Number 2022)." ;
    rdfs:comment "Escape (Release, Discharge) of fluid (including blood or bodily fluid) through an unintended location; often accompanied by a loss of pressure and/or output. This includes both external and internal fluid leak. This does not include fluidized powder leak." ;
    rdfs:subClassOf imdrf:A0504 .

imdrf:A050402 a owl:Class ;
    rdfs:label "Gas/Air Leak" ;
    ex:statusDescription "Term/Definition was modified on 27 January 2022 (Old term/definition: Gas Leak: Problem associated with the unintended escape of a gas from the container in which it is housed). For details, see comment No. 19, 20 of the Change Log (Release Number 2022)." ;
    rdfs:comment "Problem associated with the unintended escape of a gas/air from the container in which it is housed. This also includes both external and internal air/gas leak." ;
    rdfs:subClassOf imdrf:A0504 .

imdrf:A050403 a owl:Class ;
    rdfs:label "Gel Leak" ;
    rdfs:comment "Escape (Release, Discharge) of gel through an unintended location - as in leakage of ultrasound gel. Escape or release of gel from containment structures - as in gel filled implant leak." ;
    rdfs:subClassOf imdrf:A0504 .

imdrf:A050404 a owl:Class ;
    rdfs:label "Radiation Leak" ;
    rdfs:comment "Escape of radiation (energy in the form of waves or subatomic particles, especially those that cause ionization) through containment structures, leading to unintended exposure." ;
    rdfs:subClassOf imdrf:A0504 .

imdrf:A050405 a owl:Class ;
    rdfs:label "Perivalvular Leak" ;
    ex:statusDescription "Definition was modified on 31 January 2023 (Old definition: Problem associated with the escape of blood around a heart valve, particularly around its leaflets.). For details, see comment No. 7 of the Change Log (Release Number 2023)." ;
    rdfs:comment "Problem associated with the escape of blood around a heart valve, particularly around its leaflets. Also known as paravalvular leak." ;
    rdfs:subClassOf imdrf:A0504 .

imdrf:A050406 a owl:Class ;
    rdfs:label "Intravalvular regurgitation" ;
    ex:statusDescription """Term was added on 27 January 2022. For details, see comment No. 147, 175 of the Change Log (Release Number 2022).
Term and Definition modified for Release Number 2024. Previous term was Central Regurgitation See no. 47 of Change Log""" ;
    rdfs:comment "Problem associated with the escape or backward flow of blood through or across the valve.  Also known as transvalvular regurgitation" ;
    rdfs:subClassOf imdrf:A0504 .

imdrf:A050407 a owl:Class ;
    rdfs:label "Powder Leak" ;
    ex:statusDescription "Term was added on 27 January 2022. For details, see comment No. 21 of the Change Log (Release Number 2022)." ;
    rdfs:comment "Escape (release, discharge) of powder (including particulates) through an unintended location,  often accompanied by a loss of pressure and/or output." ;
    rdfs:subClassOf imdrf:A0504 .

imdrf:A050408 a owl:Class ;
    rdfs:label "Device Endoleak" ;
    ex:status "Modified (technical)" ;
    ex:statusDescription "Term was added on 31 January 2023. For details, see comment No. 33 of the Change Log (Release Number 2023). Term and Definition modified for Release Number 2025. Previous term was \"Endoleaks\". See no. 116 of Change Request Log." ;
    rdfs:comment "The observed device problem is persistent blood flow/pressure in the aneurysm sac following an endovascular aneurysm repair (EVAR) procedure.  Where other device problems lead to an endoleak the observed problems should be coded and E2121 selected as the E term." ;
    rdfs:subClassOf imdrf:A0504 .

imdrf:A050409 a owl:Class ;
    rdfs:label "Unspecified Valve Regurgitation" ;
    ex:statusDescription "Term added for Release Number 2024. See no. 46 of Change Log" ;
    rdfs:comment "Problem associated with the escape or backward flow of blood relative to a valve where it is not specified or not confirmed whether the leak is transvalvular/intravalvular or paravalvular/perivalvular." ;
    rdfs:subClassOf imdrf:A0504 .

imdrf:A050501 a owl:Class ;
    rdfs:label "Failure to Fire" ;
    rdfs:comment "Problem associated with failure of the device to discharge its load (e.g. surgical stapler failed to partially or completely deploy its staples)." ;
    rdfs:subClassOf imdrf:A0505 .

imdrf:A050502 a owl:Class ;
    rdfs:label "Misfire" ;
    rdfs:comment "Problem associated with a therapy or algorithm not being delivered or executed at the expected time." ;
    rdfs:subClassOf imdrf:A0505 .

imdrf:A0506 a owl:Class ;
    rdfs:label "Mechanical Jam" ;
    rdfs:comment "The motion of the device is prevented or restricted." ;
    rdfs:subClassOf imdrf:A05 .

imdrf:A050701 a owl:Class ;
    rdfs:label "Failure to Align" ;
    rdfs:comment "Problem associated with a circuit, equipment, or system whereby its functions fail to be properly synchronized or its relative positions properly oriented." ;
    rdfs:subClassOf imdrf:A0507 .

imdrf:A050702 a owl:Class ;
    rdfs:label "Failure to Cut" ;
    rdfs:comment "Inability of the device to make an incision, pierce or open as intended." ;
    rdfs:subClassOf imdrf:A0507 .

imdrf:A050703 a owl:Class ;
    rdfs:label "Failure to Cycle" ;
    rdfs:comment "Problem associated with the device failing to complete a series of processes or events." ;
    rdfs:subClassOf imdrf:A0507 .

imdrf:A050704 a owl:Class ;
    rdfs:label "Failure to Form Staple" ;
    rdfs:comment "Problem associated with the device failing to connect tissue with a stapling device due to the staples not forming correctly." ;
    rdfs:subClassOf imdrf:A0507 .

imdrf:A050705 a owl:Class ;
    rdfs:label "Failure to Seal" ;
    ex:statusDescription """Term was added on 27 January 2022. For details, see comment No. 198 of the Change Log (Release Number 2022).
Editorial change to reinstate missing definition for release number 2024.1""" ;
    rdfs:comment "Problem associated with the device failing to seal the intended vessel with the device intended to provide a seal (e.g. electrosurgical hemostasis)." ;
    rdfs:subClassOf imdrf:A0507 .

imdrf:A0508 a owl:Class ;
    rdfs:label "Noise, Audible" ;
    rdfs:comment "Problem associated with any unintended sound which emanates from the device (for example, squeaking from two parts rubbing together or buzzing sounds from electrical components)." ;
    rdfs:subClassOf imdrf:A05 .

imdrf:A050901 a owl:Class ;
    rdfs:label "Adhesive Too Strong" ;
    ex:statusDescription "Term was added on 27 January 2022. For details, see comment No. 215 of the Change Log (Release Number 2022)." ;
    rdfs:comment "Strength of an adhesive bond is too great; typically used when the adhesive is meant as a temporary hold but is acting in a more permanent manner." ;
    rdfs:subClassOf imdrf:A0509 .

imdrf:A0510 a owl:Class ;
    rdfs:label "Retraction Problem" ;
    rdfs:comment "Problem associated with drawing back the device to an intended location." ;
    rdfs:subClassOf imdrf:A05 .

imdrf:A051101 a owl:Class ;
    rdfs:label "Collapse" ;
    rdfs:comment "Problem associated with the buckling or crushing of material from external forces." ;
    rdfs:subClassOf imdrf:A0511 .

imdrf:A051102 a owl:Class ;
    rdfs:label "Sharp Edges" ;
    rdfs:comment "The device has undesirable sharp edges which can cause harm or damage." ;
    rdfs:subClassOf imdrf:A0511 .

imdrf:A051103 a owl:Class ;
    rdfs:label "Difficult to Fold, Unfold or Collapse" ;
    ex:statusDescription "Technical change to the term on 18 March 2020 to include difficulty in collapsing." ;
    rdfs:comment "Problem associated with the use of the device in terms of user experiencing difficulty to close or to spread out/extend length of the device, even if the operation is being performed according to labeled instructions for use." ;
    rdfs:subClassOf imdrf:A0511 .

imdrf:A051104 a owl:Class ;
    rdfs:label "Difficult to Open or Close" ;
    rdfs:comment "Problem associated with the use of the device in terms of user experiencing difficulty opening and closing the device, even if the operation is being performed according to labeled instructions for use." ;
    rdfs:subClassOf imdrf:A0511 .

imdrf:A051105 a owl:Class ;
    rdfs:label "Incomplete Coaptation" ;
    rdfs:comment "Problem associated with the heart valve leaflet not closing properly." ;
    rdfs:subClassOf imdrf:A0511 .

imdrf:A051201 a owl:Class ;
    rdfs:label "Device Dislodged or Dislocated" ;
    rdfs:comment "Problems associated with the device not remaining in an expected location." ;
    rdfs:subClassOf imdrf:A0512 .

imdrf:A051202 a owl:Class ;
    rdfs:label "Device Tipped Over" ;
    rdfs:comment "Problem associated with the inability of the device to stay in an upright position." ;
    rdfs:subClassOf imdrf:A0512 .

imdrf:A051203 a owl:Class ;
    rdfs:label "Device Fell" ;
    rdfs:comment "Problem associated with the device or a component unexpectedly being dropped or moving down from an intended place." ;
    rdfs:subClassOf imdrf:A0512 .

imdrf:A051204 a owl:Class ;
    rdfs:label "Device Slipped" ;
    rdfs:comment "Problem associated with the device moving or sliding from the intended position." ;
    rdfs:subClassOf imdrf:A0512 .

imdrf:A051205 a owl:Class ;
    rdfs:label "Unintended Collision" ;
    rdfs:comment "Problem associated with the device impacting with another object." ;
    rdfs:subClassOf imdrf:A0512 .

imdrf:A051206 a owl:Class ;
    rdfs:label "Unintended System Motion" ;
    rdfs:comment "Problem associated with any motion of the system or components that was not initiated by the user." ;
    rdfs:subClassOf imdrf:A0512 .

imdrf:A051207 a owl:Class ;
    rdfs:label "Unstable" ;
    rdfs:comment "Problem associated with the mechanical stability of the device." ;
    rdfs:subClassOf imdrf:A0512 .

imdrf:A051208 a owl:Class ;
    rdfs:label "Vibration" ;
    rdfs:comment "Problem associated with the undesirable mechanical oscillation." ;
    rdfs:subClassOf imdrf:A0512 .

imdrf:A0513 a owl:Class ;
    rdfs:label "Inadequate Lubrication" ;
    ex:statusDescription "Term was added on 18 March 2020 as an additional level 2 term under \"Mechanical Problem." ;
    rdfs:comment "The device shows inadequate lubrication." ;
    rdfs:subClassOf imdrf:A05 .

imdrf:A0514 a owl:Class ;
    rdfs:label "Damaged Thread" ;
    ex:statusDescription "Term was added on 31 January 2023. For details, see comment No. 5 of the Change Log (Release Number 2023)." ;
    rdfs:comment "Problems associated with threads that are damaged either prior to use due to bad threading or repeated re-use (possibly with other damaged components) or threads that became stripped or damaged while being used." ;
    rdfs:subClassOf imdrf:A05 .

imdrf:A0601 a owl:Class ;
    rdfs:label "Misfocusing" ;
    rdfs:comment "The problem relates to the poor focusing of the object or the focus is on the wrong object or in the wrong area." ;
    rdfs:subClassOf imdrf:A06 .

imdrf:A0602 a owl:Class ;
    rdfs:label "Optical Decentration" ;
    rdfs:comment "Problem associated with being off-center of optical lenses." ;
    rdfs:subClassOf imdrf:A06 .

imdrf:A0603 a owl:Class ;
    rdfs:label "Optical Discoloration" ;
    rdfs:comment "Problem associated with an undesired change of color." ;
    rdfs:subClassOf imdrf:A06 .

imdrf:A0604 a owl:Class ;
    rdfs:label "Optical Distortion" ;
    rdfs:comment "Problem associated with an optical defect in an image-forming system whereby the image is not the shape of an ideal image of the object." ;
    rdfs:subClassOf imdrf:A06 .

imdrf:A0605 a owl:Class ;
    rdfs:label "Optical Obstruction" ;
    rdfs:comment "Problem associated with the blocking of optical devices, e.g. visual pathways." ;
    rdfs:subClassOf imdrf:A06 .

imdrf:A070101 a owl:Class ;
    rdfs:label "Failure to Capture" ;
    rdfs:comment "Problem associated with the failure to achieve effective and consistent depolarization of the heart resulting from the electrical stimulus of the pacemaker." ;
    rdfs:subClassOf imdrf:A0701 .

imdrf:A070102 a owl:Class ;
    rdfs:label "High Capture Threshold" ;
    rdfs:comment "Problem with the amount of output energy needed to cause cardiac depolarization being higher than expected/desired." ;
    rdfs:subClassOf imdrf:A0701 .

imdrf:A070103 a owl:Class ;
    rdfs:label "Intermittent Capture" ;
    rdfs:comment "Problem associated with the ineffective and inconsistent depolarization of the heart." ;
    rdfs:subClassOf imdrf:A0701 .

imdrf:A070104 a owl:Class ;
    rdfs:label "Unstable Capture Threshold" ;
    rdfs:comment "Problem with the amount of output energy needed to cause cardiac depolarization being unstable." ;
    rdfs:subClassOf imdrf:A0701 .

imdrf:A0702 a owl:Class ;
    rdfs:label "Continuous Firing" ;
    rdfs:comment "Problem associated with the excessive production of electrical impulses over a period." ;
    rdfs:subClassOf imdrf:A07 .

imdrf:A070301 a owl:Class ;
    rdfs:label "Arcing at Paddles" ;
    rdfs:comment "Problem associated with electrical current flowing through a gap between paddles (conductive surfaces), typically resulting in a visible flash of light." ;
    rdfs:subClassOf imdrf:A0703 .

imdrf:A070302 a owl:Class ;
    rdfs:label "Arcing of Electrodes" ;
    rdfs:comment "Problem associated with electrical current flowing through a gap between electrodes (conductive surfaces), typically resulting in a visible flash of light." ;
    rdfs:subClassOf imdrf:A0703 .

imdrf:A0704 a owl:Class ;
    rdfs:label "Sparking" ;
    rdfs:comment "Problem associated with a flash of light related to an electrical discharge into a normally non conductive medium, such as air. Not associated with a discharge between two conductive surfaces." ;
    rdfs:subClassOf imdrf:A07 .

imdrf:A070501 a owl:Class ;
    rdfs:label "Battery Problem: High Impedance" ;
    rdfs:comment "Problem related to increased battery internal impedance." ;
    rdfs:subClassOf imdrf:A0705 .

imdrf:A070502 a owl:Class ;
    rdfs:label "Battery Problem: Low Impedance" ;
    rdfs:comment "Problem related to decreased battery internal impedance." ;
    rdfs:subClassOf imdrf:A0705 .

imdrf:A070503 a owl:Class ;
    rdfs:label "Failure to Run on Battery" ;
    rdfs:comment "Problem associated with the device failing to operate when not connected to a fixed power source." ;
    rdfs:subClassOf imdrf:A0705 .

imdrf:A070504 a owl:Class ;
    rdfs:label "Premature Discharge of Battery" ;
    rdfs:comment "Battery discharging earlier than expected." ;
    rdfs:subClassOf imdrf:A0705 .

imdrf:A070601 a owl:Class ;
    rdfs:label "Aborted Charge" ;
    rdfs:comment "Problem associated with the premature ending of the charging process (e.g. of a battery or other charge storage device)." ;
    rdfs:subClassOf imdrf:A0706 .

imdrf:A070602 a owl:Class ;
    rdfs:label "Delayed Charge Time" ;
    rdfs:comment "Problem associated with an unexpected amount of time required to charge the device (e.g. a delay in starting charging or a longer than expected charge time)." ;
    rdfs:subClassOf imdrf:A0706 .

imdrf:A070603 a owl:Class ;
    rdfs:label "Failure to Charge" ;
    rdfs:comment "Problem associated with inability to initiate the appropriate charging process (e.g. of a battery or other charge storage device)" ;
    rdfs:subClassOf imdrf:A0706 .

imdrf:A0707 a owl:Class ;
    rdfs:label "Failure to Discharge" ;
    rdfs:comment "Problem associated with the failure of a battery or other charge storage device to appropriately discharge as intended. Does not apply to defibrillation." ;
    rdfs:subClassOf imdrf:A07 .

imdrf:A070801 a owl:Class ;
    rdfs:label "Complete Loss of Power" ;
    rdfs:comment "Problem associated with the lack of power to run the device." ;
    rdfs:subClassOf imdrf:A0708 .

imdrf:A070802 a owl:Class ;
    rdfs:label "Intermittent Loss of Power" ;
    rdfs:comment "Problem associated with an intermittent disruption to the power to run the device." ;
    rdfs:subClassOf imdrf:A0708 .

imdrf:A070803 a owl:Class ;
    rdfs:label "Failure to Power Up" ;
    rdfs:comment "Problem associated with the inability of the device to turn on related to energy delivered to the device." ;
    rdfs:subClassOf imdrf:A0708 .

imdrf:A070804 a owl:Class ;
    rdfs:label "Unintended Power Up" ;
    rdfs:comment "Problem associated with the device turning on when not intended." ;
    rdfs:subClassOf imdrf:A0708 .

imdrf:A070901 a owl:Class ;
    rdfs:label "Decreased Sensitivity" ;
    rdfs:comment "Problem with the device being less sensitive to an input than intended or expected." ;
    rdfs:subClassOf imdrf:A0709 .

imdrf:A070902 a owl:Class ;
    rdfs:label "Increased Sensitivity" ;
    rdfs:comment "Problem with the device being more sensitive to an input than intended or expected." ;
    rdfs:subClassOf imdrf:A0709 .

imdrf:A070903 a owl:Class ;
    rdfs:label "Failure to Analyze Signal" ;
    rdfs:comment "Problem with the device not analyzing a signal." ;
    rdfs:subClassOf imdrf:A0709 .

imdrf:A070904 a owl:Class ;
    rdfs:label "Failure to Select Signal" ;
    rdfs:comment "Problem associated with the failure of the device to select the appropriate input signal." ;
    rdfs:subClassOf imdrf:A0709 .

imdrf:A070905 a owl:Class ;
    rdfs:label "High Sensing Threshold" ;
    rdfs:comment "Problem associated with the amount of input required by the device to detect a signal being higher than expected/desired." ;
    rdfs:subClassOf imdrf:A0709 .

imdrf:A070906 a owl:Class ;
    rdfs:label "Low Sensing Threshold" ;
    rdfs:comment "Problem associated with the amount of an input required by the device to detect a signal being lower than expected/desired." ;
    rdfs:subClassOf imdrf:A0709 .

imdrf:A070907 a owl:Class ;
    rdfs:label "Loss of Threshold" ;
    rdfs:comment "Problem associated with the loss of the minimum amount of energy, voltage, or current needed to consistently stimulate the heart muscle." ;
    rdfs:subClassOf imdrf:A0709 .

imdrf:A070908 a owl:Class ;
    rdfs:label "Failure to Sense" ;
    rdfs:comment "Problem associated with the failure of the device designed to respond to a physical stimulus (as temperature, illumination, motion) to transmit a resulting signal for interpretation or measurement." ;
    rdfs:subClassOf imdrf:A0709 .

imdrf:A070909 a owl:Class ;
    rdfs:label "Over-Sensing" ;
    rdfs:comment "Problem related to failure of the device to properly filter cardiac signals resulting in inappropriate device response." ;
    rdfs:subClassOf imdrf:A0709 .

imdrf:A070910 a owl:Class ;
    rdfs:label "Under-Sensing" ;
    rdfs:comment "Problem related to failure of the device to properly detect intrinsic cardiac activity and respond appropriately." ;
    rdfs:subClassOf imdrf:A0709 .

imdrf:A070911 a owl:Class ;
    rdfs:label "Sensing Intermittently" ;
    rdfs:comment "Problem with the device receiving an incoming signal on an intermittent basis when expected to be continuous." ;
    rdfs:subClassOf imdrf:A0709 .

imdrf:A070912 a owl:Class ;
    rdfs:label "Incorrect Interpretation of Signal" ;
    rdfs:comment "Problem with the device inappropriately analyzing a signal." ;
    rdfs:subClassOf imdrf:A0709 .

imdrf:A0710 a owl:Class ;
    rdfs:label "Failure to Conduct" ;
    rdfs:comment "Problem associated with the inability of the device to allow a current of electricity to pass or to conduct electricity continuously along an electrical path." ;
    rdfs:subClassOf imdrf:A07 .

imdrf:A071101 a owl:Class ;
    rdfs:label "Difficult to Interrogate" ;
    rdfs:comment "Problem associated with difficulty of a transponder system to trigger a response." ;
    rdfs:subClassOf imdrf:A0711 .

imdrf:A071102 a owl:Class ;
    rdfs:label "Failure to Interrogate" ;
    rdfs:comment "Problem associated with the device failure to appropriately respond to signals from a system designed to interrogate its status." ;
    rdfs:subClassOf imdrf:A0711 .

imdrf:A071201 a owl:Class ;
    rdfs:label "Failure to Convert Rhythm" ;
    rdfs:comment "Failure of the device therapy or set of therapies to terminate the harmful cardiac rhythm that the therapy is meant to terminate." ;
    rdfs:subClassOf imdrf:A0712 .

imdrf:A071202 a owl:Class ;
    rdfs:label "Inaccurate Synchronization" ;
    rdfs:comment "Problem associated with an error due to imperfect timing of two operations, e.g. signal transmission time." ;
    rdfs:subClassOf imdrf:A0712 .

imdrf:A071203 a owl:Class ;
    rdfs:label "Inappropriate Waveform" ;
    rdfs:comment "Failure of the device to generate a correctly-shaped pacing output, e.g., a waveform that is too wide." ;
    rdfs:subClassOf imdrf:A0712 .

imdrf:A071204 a owl:Class ;
    rdfs:label "No Pacing" ;
    rdfs:comment "Problem associated with the device ceasing to deliver paces." ;
    rdfs:subClassOf imdrf:A0712 .

imdrf:A071205 a owl:Class ;
    rdfs:label "Pacemaker Found in Back-Up Mode" ;
    ex:status "Retired" ;
    ex:statusDescription "Term was inactivated on 31 January 2023, with the addition of term A0723 Device in Backup-mode. For details, see comment No. 8 of the Change Log (Release Number 2023)." ;
    rdfs:comment "A device with a pacing function found in back-up Mode. This may be an appropriate fail-safe action (e.g. end of battery life), or be caused by device malfunction or due to operator error." ;
    rdfs:subClassOf imdrf:A0712 .

imdrf:A071206 a owl:Class ;
    rdfs:label "Pacing Asynchronously" ;
    rdfs:comment "Problem associated with a pacing transmission process such that between any two significant instants in the same group, there is always an integral number of unit intervals. Between two significant instants located in different groups, there are not always an integral number of unit intervals." ;
    rdfs:subClassOf imdrf:A0712 .

imdrf:A071207 a owl:Class ;
    rdfs:label "Pacing Inadequately" ;
    rdfs:comment "Pacing voltage or pulse width is less than desired." ;
    rdfs:subClassOf imdrf:A0712 .

imdrf:A071208 a owl:Class ;
    rdfs:label "Pacing Intermittently" ;
    rdfs:comment "Problem associated with the failure of pacing device for a limited period of time, following which the item recovers its ability to perform its required function without being subjected to any external corrective action. Note: such as failure is often recurrent." ;
    rdfs:subClassOf imdrf:A0712 .

imdrf:A071209 a owl:Class ;
    rdfs:label "Extracardiac stimulation" ;
    ex:status "Modified (technical)" ;
    ex:statusDescription "Term and Definition modified for Release Number 2025. Previous term was  Pocket Stimulation . See no. 5 of Change Request Log." ;
    rdfs:comment "Problem associated with undesired pacemaker induced stimulation of extracardiac (muscle) tissue (e.g. diaphragm, pectoral or intercostal muscle)" ;
    rdfs:subClassOf imdrf:A0712 .

imdrf:A071301 a owl:Class ;
    rdfs:label "Failure to Deliver Shock/Stimulation" ;
    ex:statusDescription "Technical change to the term on 18 March 2020 to include stimulation." ;
    rdfs:comment "Problem associated with the failure of the device to deliver electrical energy." ;
    rdfs:subClassOf imdrf:A0713 .

imdrf:A071302 a owl:Class ;
    rdfs:label "Inappropriate/Inadequate Shock/Stimulation" ;
    ex:statusDescription "Technical change to the term and definition on 18 March 2020 to include inadequate stimulation." ;
    rdfs:comment "A shock was delivered with incorrect energy level or at incorrect timing." ;
    rdfs:subClassOf imdrf:A0713 .

imdrf:A071303 a owl:Class ;
    rdfs:label "Intermittent Shock/Stimulation" ;
    ex:statusDescription "Technical change to the term and definition on 18 March 2020 to include stimulation." ;
    rdfs:comment "Problem associated with the failure to deliver electrical energy for a limited period of time, following which the item recovers its ability to perform its required function without being subjected to any external corrective action. Note: such a failure is often recurrent." ;
    rdfs:subClassOf imdrf:A0713 .

imdrf:A0714 a owl:Class ;
    rdfs:label "Unintended Electrical Shock" ;
    ex:statusDescription "Technical change to the definition on 18 March 2020 to differentiate this term with \"Defibrillation/Stimulation Problem\" (A0713) and lower level terms." ;
    rdfs:comment "The device delivers unintended electrical shock. Use this term for devices that are not intended to deliver shocks/stimulation." ;
    rdfs:subClassOf imdrf:A07 .

imdrf:A0715 a owl:Class ;
    rdfs:label "Grounding Malfunction" ;
    rdfs:comment "Problem associated with the inability to connect conductors of an electronic system for the purpose of controlling or impeding ground currents and voltages." ;
    rdfs:subClassOf imdrf:A07 .

imdrf:A0716 a owl:Class ;
    rdfs:label "Electrical Overstress" ;
    rdfs:comment "Problem associated with an electrical activity that exceeded the specified threshold limit of the internal integrated circuitry." ;
    rdfs:subClassOf imdrf:A07 .

imdrf:A0717 a owl:Class ;
    rdfs:label "Electrostatic Discharge" ;
    ex:status "Modified (editorial)" ;
    ex:statusDescription "Term modified for Release Number 2025. Previous term was \"Electro-Static Discharge\". See no. 139 of Change Request Log." ;
    rdfs:comment "Problem associated with the discharge of electricity between two bodies previously electrically charged." ;
    rdfs:subClassOf imdrf:A07 .

imdrf:A071801 a owl:Class ;
    rdfs:label "Device Remains Activated" ;
    rdfs:comment "Problem associated with the device continuing to be in an active state after deactivation was requested." ;
    rdfs:subClassOf imdrf:A0718 .

imdrf:A0719 a owl:Class ;
    rdfs:label "Unexpected Shutdown" ;
    rdfs:comment "Problem associated with the device unexpectedly powering down." ;
    rdfs:subClassOf imdrf:A07 .

imdrf:A072001 a owl:Class ;
    rdfs:label "Electromagnetic Interference" ;
    rdfs:comment "Problem associated with a measure of electromagnetic radiation from equipment." ;
    rdfs:subClassOf imdrf:A0720 .

imdrf:A072002 a owl:Class ;
    rdfs:label "Radiofrequency Interference (RFI)" ;
    rdfs:comment "Problem associated with the degradation of the reception of a wanted signal caused by RF disturbance." ;
    rdfs:subClassOf imdrf:A0720 .

imdrf:A072101 a owl:Class ;
    rdfs:label "Capacitative Coupling" ;
    rdfs:comment "Problem associated with the transfer of energy within an electrical network by means of the capacitance between circuit nodes. It occurs when energy is coupled from one circuit to another through an electric field." ;
    rdfs:subClassOf imdrf:A0721 .

imdrf:A072102 a owl:Class ;
    rdfs:label "Electrical Shorting" ;
    rdfs:comment "Problem associated with an electric current travelling along an accidental path (unintended path) in a circuit." ;
    rdfs:subClassOf imdrf:A0721 .

imdrf:A072103 a owl:Class ;
    rdfs:label "Intermittent Continuity" ;
    rdfs:comment "Problem associated with intermittent faults in electrical/electronic interconnections." ;
    rdfs:subClassOf imdrf:A0721 .

imdrf:A072201 a owl:Class ;
    rdfs:label "High impedance" ;
    rdfs:comment "Problem associated with higher than intended electrical impedance levels between device and patient connections." ;
    rdfs:subClassOf imdrf:A0722 .

imdrf:A072202 a owl:Class ;
    rdfs:label "Low impedance" ;
    rdfs:comment "Problem associated with lower than intended electrical impedance levels between device and patient connections." ;
    rdfs:subClassOf imdrf:A0722 .

imdrf:A072203 a owl:Class ;
    rdfs:label "Unstable Impedance" ;
    ex:status "New" ;
    ex:statusDescription "Term added for Release Number 2025. See no. 7 of Change Request Log" ;
    rdfs:comment "The impedance varies without being consistently too high or too low." ;
    rdfs:subClassOf imdrf:A0722 .

imdrf:A0723 a owl:Class ;
    rdfs:label "Unexpected Mode Switch" ;
    ex:status "Modified (technical)" ;
    ex:statusDescription """Term was added on 31 January 2023. For details, see comment No. 8 of the Change Log (Release Number 2023).
Term and Definition modified for Release Number 2025. Previous term was  Device in Backup-mode . See no. 4 of Change Request Log.""" ;
    rdfs:comment "A device switches mode unexpectedly e.g. back-up mode or electrocautery mode." ;
    rdfs:subClassOf imdrf:A07 .

imdrf:A0801 a owl:Class ;
    rdfs:label "Failure to Calibrate" ;
    rdfs:comment "Problem associated with the failure of the device to perform a self-calibration procedure or process designed to assure the accuracy and proper performance of the device." ;
    rdfs:subClassOf imdrf:A08 .

imdrf:A0802 a owl:Class ;
    rdfs:label "Failure to Recalibrate" ;
    rdfs:comment "Problem associated with the failure of the device which is unable to regain a standard level of accuracy when performing a calibration procedure or process designed to assure the accuracy and proper performance of the device." ;
    rdfs:subClassOf imdrf:A08 .

imdrf:A0803 a owl:Class ;
    rdfs:label "Imprecision" ;
    rdfs:comment "Problem associated with the device providing imprecise measurements when compared to a reference standard." ;
    rdfs:subClassOf imdrf:A08 .

imdrf:A0804 a owl:Class ;
    rdfs:label "Overcorrection" ;
    rdfs:comment "Problem associated with an adjustment that surpasses a set of criteria." ;
    rdfs:subClassOf imdrf:A08 .

imdrf:A0805 a owl:Class ;
    rdfs:label "Undercorrection" ;
    ex:statusDescription "Term was added on 18 March 2020 as an additional level 2 term under \"Calibration Problem\"." ;
    rdfs:comment "Problem associated with an adjustment that falls below a set of criteria." ;
    rdfs:subClassOf imdrf:A08 .

imdrf:A090101 a owl:Class ;
    rdfs:label "Inappropriate Audible Prompt/Feedback" ;
    rdfs:comment "Problem with audible messages which do not guide a device user to the correct action." ;
    rdfs:subClassOf imdrf:A0901 .

imdrf:A090102 a owl:Class ;
    rdfs:label "Inaudible or Unclear Audible Prompt/Feedback" ;
    rdfs:comment "Problem associated with audible prompts which cannot be heard clearly." ;
    rdfs:subClassOf imdrf:A0901 .

imdrf:A090103 a owl:Class ;
    rdfs:label "No Audible Prompt/Feedback" ;
    rdfs:comment "Problem associated with the device ceasing to provide audible prompts." ;
    rdfs:subClassOf imdrf:A0901 .

imdrf:A090201 a owl:Class ;
    rdfs:label "Device Displays Incorrect Message" ;
    rdfs:comment "Problem associated with providing incorrect display information." ;
    rdfs:subClassOf imdrf:A0902 .

imdrf:A090202 a owl:Class ;
    rdfs:label "Display Difficult to Read" ;
    rdfs:comment "Problem associated with legibility of the display, compromising for instance  the reading/interpretation of patient parameters or test results. Legibility problems can be due to color, size of font, display screen contrast or other factors." ;
    rdfs:subClassOf imdrf:A0902 .

imdrf:A090203 a owl:Class ;
    rdfs:label "Erratic or Intermittent Display" ;
    rdfs:comment "A device does not consistently display the same message, result, reading, or image. e.g. the display might flicker, switch between readings or messages, or go completely blank for brief periods of time." ;
    rdfs:subClassOf imdrf:A0902 .

imdrf:A090204 a owl:Class ;
    rdfs:label "Image Display Error/Artifact" ;
    rdfs:comment "Problem with image display leading to corrupted images or readouts/measurement indications." ;
    rdfs:subClassOf imdrf:A0902 .

imdrf:A090205 a owl:Class ;
    rdfs:label "Image Orientation Incorrect" ;
    rdfs:comment "Problem associated with an incorrect image orientation on the device display." ;
    rdfs:subClassOf imdrf:A0902 .

imdrf:A090206 a owl:Class ;
    rdfs:label "No Display/Image" ;
    rdfs:comment "Problem associated with the absence of display or image." ;
    rdfs:subClassOf imdrf:A0902 .

imdrf:A090207 a owl:Class ;
    rdfs:label "No Visual Prompts/Feedback" ;
    rdfs:comment "Problem associated with the device ceasing to provide visual feedback." ;
    rdfs:subClassOf imdrf:A0902 .

imdrf:A090208 a owl:Class ;
    rdfs:label "Poor Quality Image" ;
    rdfs:comment "Inadequate quality of an image or any visual representation displayed by the device, or output from the device." ;
    rdfs:subClassOf imdrf:A0902 .

imdrf:A090209 a owl:Class ;
    rdfs:label "Visual Prompts will not Clear" ;
    rdfs:comment "Problem with visual messages which continue to be displayed on/by the device after the appropriate action has been taken." ;
    rdfs:subClassOf imdrf:A0902 .

imdrf:A090301 a owl:Class ;
    rdfs:label "Inappropriate Tactile Prompt/Feedback" ;
    rdfs:comment "Problem with tactile feedback which does not guide a device user to the correct action." ;
    rdfs:subClassOf imdrf:A0903 .

imdrf:A090302 a owl:Class ;
    rdfs:label "No Tactile Prompts/Feedback" ;
    rdfs:comment "Problem associated with the device ceasing to provide tactile feedback." ;
    rdfs:subClassOf imdrf:A0903 .

imdrf:A090401 a owl:Class ;
    rdfs:label "Energy Spectrum Incorrect" ;
    rdfs:comment "Problem associated with the energy output from the device not being in the expected part of the spectrum." ;
    rdfs:subClassOf imdrf:A0904 .

imdrf:A090402 a owl:Class ;
    rdfs:label "Failure to Deliver Energy" ;
    rdfs:comment "Problem associated with the failure of the device to deliver any energy." ;
    rdfs:subClassOf imdrf:A0904 .

imdrf:A090403 a owl:Class ;
    rdfs:label "Intermittent Energy Output" ;
    rdfs:comment "Problem associated with the energy output from the device being inconsistent over time." ;
    rdfs:subClassOf imdrf:A0904 .

imdrf:A090404 a owl:Class ;
    rdfs:label "Output above Specifications" ;
    rdfs:comment "Device output is exceeding the documented specifications of the device." ;
    rdfs:subClassOf imdrf:A0904 .

imdrf:A090405 a owl:Class ;
    rdfs:label "Output below Specifications" ;
    rdfs:comment "Device output is below the documented specifications of the device." ;
    rdfs:subClassOf imdrf:A0904 .

imdrf:A090406 a owl:Class ;
    rdfs:label "Therapeutic or Diagnostic Output Failure" ;
    rdfs:comment "Problem associated with the failure of the device to deliver the output required for treatment or identification of a disease." ;
    rdfs:subClassOf imdrf:A0904 .

imdrf:A090407 a owl:Class ;
    rdfs:label "Therapy Delivered to Incorrect Body Area" ;
    rdfs:comment "Problem associated with the device causing unintended therapeutic action to an area of the body other than the intended area." ;
    rdfs:subClassOf imdrf:A0904 .

imdrf:A090501 a owl:Class ;
    rdfs:label "Radiation Output Failure" ;
    rdfs:comment "Problem associated with the absence of radiation output from radiological or diagnostic devices." ;
    rdfs:subClassOf imdrf:A0905 .

imdrf:A090502 a owl:Class ;
    rdfs:label "Radiation Overexposure" ;
    rdfs:comment "Problem associated with excessive radiation emitted from radiological or diagnostic devices." ;
    rdfs:subClassOf imdrf:A0905 .

imdrf:A090503 a owl:Class ;
    rdfs:label "Radiation Underexposure" ;
    rdfs:comment "Problem associated with too little radiation emitted from radiological or diagnostic devices." ;
    rdfs:subClassOf imdrf:A0905 .

imdrf:A090504 a owl:Class ;
    rdfs:label "Unexpected/Unintended Radiation Output" ;
    rdfs:comment "Device-emitted radiation when it was not supposed to. This applies to devices which are intended to emit radiation, and the radiation being emitted from the correct part of the device, but at an incorrect time. Use \"radiation leak\" if the device emits radiation which should never have been emitted, or from a location from which it should never be emitted." ;
    rdfs:subClassOf imdrf:A0905 .

imdrf:A0906 a owl:Class ;
    rdfs:label "Gas Output Problem" ;
    rdfs:comment "Problem associated with gas output." ;
    rdfs:subClassOf imdrf:A09 .

imdrf:A0907 a owl:Class ;
    rdfs:label "No Device Output" ;
    rdfs:comment "Problem associated with no measurement outcome, value or data obtained from the device." ;
    rdfs:subClassOf imdrf:A09 .

imdrf:A090801 a owl:Class ;
    rdfs:label "Signal Artifact/Noise" ;
    ex:statusDescription "Technical change to the term on 18 March 2020 to include signal noise." ;
    rdfs:comment "Problem associated with impurities or interference in a signal (e.g. ECG artifact)." ;
    rdfs:subClassOf imdrf:A0908 .

imdrf:A090802 a owl:Class ;
    rdfs:label "Failure to Obtain Sample" ;
    rdfs:comment "The device does not collect or transfer the sample." ;
    rdfs:subClassOf imdrf:A0908 .

imdrf:A090803 a owl:Class ;
    rdfs:label "False Negative Result" ;
    ex:statusDescription "Definition modified for Release Number 2024. See no. 122 of Change Log" ;
    rdfs:comment "Problem associated with the device incorrectly reporting that something has not been detected and may mislead the operator/user/HCP into not taking certain actions when action should be taken." ;
    rdfs:subClassOf imdrf:A0908 .

imdrf:A090804 a owl:Class ;
    rdfs:label "False Positive Result" ;
    ex:statusDescription "Definition modified for Release Number 2024. See no. 123 of Change Log" ;
    rdfs:comment "Problem associated with the device incorrectly reporting that something has been detected and may mislead the operatorr/user/HCP to take certain actions." ;
    rdfs:subClassOf imdrf:A0908 .

imdrf:A090805 a owl:Class ;
    rdfs:label "Incorrect Measurement" ;
    rdfs:comment "Measurement obtained from or provided by the device is obviously incorrect." ;
    rdfs:subClassOf imdrf:A0908 .

imdrf:A090806 a owl:Class ;
    rdfs:label "Non Reproducible Results" ;
    rdfs:comment "Device results cannot be reliably reproduced." ;
    rdfs:subClassOf imdrf:A0908 .

imdrf:A090807 a owl:Class ;
    rdfs:label "High Readings" ;
    rdfs:comment "Reading provided by the device is too high or higher than expected." ;
    rdfs:subClassOf imdrf:A0908 .

imdrf:A090808 a owl:Class ;
    rdfs:label "Low Readings" ;
    rdfs:comment "Reading provided by the device is too low or lower than expected." ;
    rdfs:subClassOf imdrf:A0908 .

imdrf:A090809 a owl:Class ;
    rdfs:label "High Test Results" ;
    rdfs:comment "Test results provided by the device are too high or higher than expected." ;
    rdfs:subClassOf imdrf:A0908 .

imdrf:A090810 a owl:Class ;
    rdfs:label "Low Test Results" ;
    rdfs:comment "Test results provided by the device are too low or lower than expected." ;
    rdfs:subClassOf imdrf:A0908 .

imdrf:A090811 a owl:Class ;
    rdfs:label "Unable to Obtain Readings" ;
    rdfs:comment "The device does not provide or display a valid reading." ;
    rdfs:subClassOf imdrf:A0908 .

imdrf:A090812 a owl:Class ;
    rdfs:label "Missing Test Results" ;
    rdfs:comment "Problem associated with the results of a test or measurement not appearing." ;
    rdfs:subClassOf imdrf:A0908 .

imdrf:A090813 a owl:Class ;
    rdfs:label "Imprecise or Erratic Results" ;
    ex:status "Modified (technical)" ;
    ex:statusDescription "Term was added on 18 March 2020 as an additional level 3 term to \"Incorrect, Inadequate or Imprecise Results or Readings\".  Term modified for Release Number 2025. Previous term was Erratic Results. See no. 46 of Change Request Log." ;
    rdfs:comment "Reports of erroneous/discrepant results which combine high/low and/or positive/negative results. This term is not to be selected where reports indicate consistently high or low or false positive or false negative results." ;
    rdfs:subClassOf imdrf:A0908 .

imdrf:A090814 a owl:Class ;
    rdfs:label "Poor Visibility" ;
    ex:statusDescription "Term was added on 27 January 2022. For details, see comment No. 146 of the Change Log (Release Number 2022)." ;
    rdfs:comment "Implanted device is difficult to detect on imaging modalities, e.g. insufficient visibility." ;
    rdfs:subClassOf imdrf:A0908 .

imdrf:A0909 a owl:Class ;
    rdfs:label "Unexpected Therapeutic Results" ;
    rdfs:comment "Problem associated with the use of the device for therapeutic purposes." ;
    rdfs:subClassOf imdrf:A09 .

imdrf:A1001 a owl:Class ;
    rdfs:label "Excessive Cooling" ;
    rdfs:comment "Problem associated with the device producing temperatures that are lower than specified." ;
    rdfs:subClassOf imdrf:A10 .

imdrf:A1002 a owl:Class ;
    rdfs:label "Excessive Heating" ;
    rdfs:comment "Problem associated with the device which have a warming or heating function, producing excessive heat." ;
    rdfs:subClassOf imdrf:A10 .

imdrf:A1003 a owl:Class ;
    rdfs:label "Insufficient Cooling" ;
    rdfs:comment "Problem associated with the device insufficiently cooled in device active (working) or/and non-active (nonworking) state." ;
    rdfs:subClassOf imdrf:A10 .

imdrf:A1004 a owl:Class ;
    rdfs:label "Insufficient Heating" ;
    rdfs:comment "Problem associated with the device or its components producing temperatures that are not as high as what is specified." ;
    rdfs:subClassOf imdrf:A10 .

imdrf:A1005 a owl:Class ;
    rdfs:label "Overheating of Device" ;
    rdfs:comment "Problem associated with the device producing high temperatures, such that its operation is compromised or harm is caused (e.g. overheating that produces melting of components or automatic shutdown)." ;
    rdfs:subClassOf imdrf:A10 .

imdrf:A1006 a owl:Class ;
    rdfs:label "Thermal Decomposition of Device" ;
    rdfs:comment "Problems associated with a discoloration or destruction as a result of thermal decomposition of the device." ;
    rdfs:subClassOf imdrf:A10 .

imdrf:A1007 a owl:Class ;
    rdfs:label "Fire" ;
    rdfs:comment "Problem associated with the combustion of the device with a steady flame." ;
    rdfs:subClassOf imdrf:A10 .

imdrf:A1008 a owl:Class ;
    rdfs:label "Flare or Flash" ;
    rdfs:comment "Problem associated with device-related burn with an unsteady flame." ;
    rdfs:subClassOf imdrf:A10 .

imdrf:A1009 a owl:Class ;
    rdfs:label "Smoking" ;
    rdfs:comment "Problem associated with a cloud of vapor or gas generated from the device, generally associated after a fire or a burn." ;
    rdfs:subClassOf imdrf:A10 .

imdrf:A1101 a owl:Class ;
    rdfs:label "Application Network Problem" ;
    rdfs:comment "Problem associated with the deviations from documented system specifications that affects overall system performance and/or the performance of an individual device connected to that system." ;
    rdfs:subClassOf imdrf:A11 .

imdrf:A110201 a owl:Class ;
    rdfs:label "Application Program Freezes or Fails to Launch" ;
    ex:status "Modified (technical)" ;
    ex:statusDescription """Definition was modified on 27 January 2022 to add in "/or" For details, see comment No. 27 of the Change Log (Release Number 2022).
Term and Definition modified for Release Number 2025. Previous term was  Application Program Freezes, Becomes Nonfunctional . See no. 6 of Change Request Log.""" ;
    rdfs:comment "Problem associated with an application program which freezes and/or fails to launch." ;
    rdfs:subClassOf imdrf:A1102 .

imdrf:A110202 a owl:Class ;
    rdfs:label "Application Program Problem: Dose Calculation Error" ;
    rdfs:comment "Problem associated with the written program code or application software used by the device to calculate specific measurements or quantities managed by the device." ;
    rdfs:subClassOf imdrf:A1102 .

imdrf:A110203 a owl:Class ;
    rdfs:label "Application Program Problem: Medication Error" ;
    rdfs:comment "Event in which the device software results in errors of medication preparation or administration." ;
    rdfs:subClassOf imdrf:A1102 .

imdrf:A110204 a owl:Class ;
    rdfs:label "Application Program Problem: Parameter Calculation Error" ;
    rdfs:comment "Problem associated with the written program code or application software used by the device to calculate parameters other than those related to dose or power." ;
    rdfs:subClassOf imdrf:A1102 .

imdrf:A110205 a owl:Class ;
    rdfs:label "Application Program Problem: Power Calculation Error" ;
    rdfs:comment "Problem associated with the written program code or application software used by the device for calculations related to device power." ;
    rdfs:subClassOf imdrf:A1102 .

imdrf:A110206 a owl:Class ;
    rdfs:label "Application Program Version or Upgrade Problem" ;
    rdfs:comment "Problem associated with installing updates to a software system that affects the device performance or communication with another device." ;
    rdfs:subClassOf imdrf:A1102 .

imdrf:A110207 a owl:Class ;
    rdfs:label "Problem with Software Installation" ;
    rdfs:comment "Problem associated with installing the device software in a manner that allows full functioning of the device. Source of installation could be manufacturer or user." ;
    rdfs:subClassOf imdrf:A1102 .

imdrf:A110208 a owl:Class ;
    rdfs:label "Unintended Application Program Shut Down" ;
    rdfs:comment "Problem associated with an unintended shut down by malfunction of the application program." ;
    rdfs:subClassOf imdrf:A1102 .

imdrf:A110301 a owl:Class ;
    rdfs:label "Delayed Program or Algorithm Execution" ;
    rdfs:comment "Problem associated with delayed execution relating to program or algorithm." ;
    rdfs:subClassOf imdrf:A1103 .

imdrf:A110302 a owl:Class ;
    rdfs:label "Intermittent Program or Algorithm Execution" ;
    rdfs:comment "Problem associated with intermittent execution relating to program or algorithm." ;
    rdfs:subClassOf imdrf:A1103 .

imdrf:A110303 a owl:Class ;
    rdfs:label "Program or Algorithm Execution Failure" ;
    rdfs:comment "Problem associated with the failure of a program or algorithm to execute. Sudden/unexpected interruption to a program's execution." ;
    rdfs:subClassOf imdrf:A1103 .

imdrf:A110401 a owl:Class ;
    rdfs:label "Operating System Becomes Nonfunctional" ;
    rdfs:comment "Problem associated with malfunction of the computer operating system as opposed to an application software problem." ;
    rdfs:subClassOf imdrf:A1104 .

imdrf:A110402 a owl:Class ;
    rdfs:label "Operating System Version or Upgrade Problem" ;
    rdfs:comment "Problem associated with replacing an older operating system to an up-to-date operating system." ;
    rdfs:subClassOf imdrf:A1104 .

imdrf:A110501 a owl:Class ;
    rdfs:label "Application Security Problem" ;
    rdfs:comment "Problem associated with the acquisition of computer programming codes that can replicate and spread from one computer system to another thereby leading to damaged software, hardware and data." ;
    rdfs:subClassOf imdrf:A1105 .

imdrf:A110502 a owl:Class ;
    rdfs:label "Unauthorized Access to Computer System" ;
    rdfs:comment "Problem associated with an access that was not permitted to the computer system that may lead to modification of program, corruption of data, or and break in network security. This concept is closely associated with computer integrity which is the degree to which a system or component prevents unauthorized access to, or modification of, computer programs or data." ;
    rdfs:subClassOf imdrf:A1105 .

imdrf:A110601 a owl:Class ;
    rdfs:label "Failure to Back-Up" ;
    rdfs:comment "Problem associated with the inability to backup or to retrieve a backed up version (corrupted file) of device data or system files." ;
    rdfs:subClassOf imdrf:A1106 .

imdrf:A110602 a owl:Class ;
    rdfs:label "Failure to Convert to Back-Up" ;
    rdfs:comment "Problem associated with a failure to transition from a primary system, component, file, procedure to a backup in response to a failure in the primary item." ;
    rdfs:subClassOf imdrf:A1106 .

imdrf:A110701 a owl:Class ;
    rdfs:label "Loss of Data" ;
    rdfs:comment "Event in which data is unintentionally permanently or temporarily lost, deleted, corrupted, or overwritten." ;
    rdfs:subClassOf imdrf:A1107 .

imdrf:A110702 a owl:Class ;
    rdfs:label "Patient Data Problem" ;
    rdfs:comment "Event in which data is accessed by the healthcare provider and either the wrong patient or the wrong data is retrieved despite correct inquiry procedures." ;
    rdfs:subClassOf imdrf:A1107 .

imdrf:A1108 a owl:Class ;
    rdfs:label "Date/Time-Related Software Problem" ;
    rdfs:comment "Problem associated with programming of calendar dates and/or time as a factor in the operation of the device." ;
    rdfs:subClassOf imdrf:A11 .

imdrf:A1201 a owl:Class ;
    rdfs:label "Blocked Connection" ;
    rdfs:comment "Problem associated with linking of the device whereby their functional units set up to provide means for a transfer of fluid, gas, or data is prevented or impeded." ;
    rdfs:subClassOf imdrf:A12 .

imdrf:A1202 a owl:Class ;
    rdfs:label "Decoupling" ;
    rdfs:comment "Problem associated with the device being unassociated in such a way that fluid, gas, power or signal information may not be transferred from one to another." ;
    rdfs:subClassOf imdrf:A12 .

imdrf:A1203 a owl:Class ;
    rdfs:label "Disconnection" ;
    rdfs:comment "Problem associated with the linking of the device having a sufficient open space to prevent gas, liquid or electrical current flow between connectors." ;
    rdfs:subClassOf imdrf:A12 .

imdrf:A1204 a owl:Class ;
    rdfs:label "Failure to Disconnect" ;
    rdfs:comment "Problem associated with the linking of the device whereby termination of the transfer of liquid, gas, electricity, or information cannot be accomplished, or linking components do not come apart, or disconnect, when expected." ;
    rdfs:subClassOf imdrf:A12 .

imdrf:A1205 a owl:Class ;
    rdfs:label "Loose or Intermittent Connection" ;
    rdfs:comment "Problem associated with the connection of the device being loose or intermittent." ;
    rdfs:subClassOf imdrf:A12 .

imdrf:A1206 a owl:Class ;
    rdfs:label "Misconnection" ;
    rdfs:comment "Problem associated with the connection of the device being improper or not in accordance with device specification, requirements or intended uses." ;
    rdfs:subClassOf imdrf:A12 .

imdrf:A1207 a owl:Class ;
    rdfs:label "Incomplete or Inadequate Connection" ;
    rdfs:comment "Problem associated with a partial linking of the device whereby device may appear to be connected however only a partial, intermittent or no transfer of liquid, gas, electricity, or information can be accomplished." ;
    rdfs:subClassOf imdrf:A12 .

imdrf:A1208 a owl:Class ;
    rdfs:label "Fitting Problem" ;
    rdfs:comment "Problem associated with the connection of the device whereby channels, switching systems, and other functional units set up to provide means for a transfer of liquid, gas, electricity, or information do not match or fit." ;
    rdfs:subClassOf imdrf:A12 .

imdrf:A1301 a owl:Class ;
    rdfs:label "Failure to Read Input Signal" ;
    rdfs:comment "Problem associated with a failure of the device to read a signal for interpretation or measurement." ;
    rdfs:subClassOf imdrf:A13 .

imdrf:A1302 a owl:Class ;
    rdfs:label "Failure to Transmit Record" ;
    rdfs:comment "Problem associated with a failure of the device to transmit a record for interpretation or measurement." ;
    rdfs:subClassOf imdrf:A13 .

imdrf:A1303 a owl:Class ;
    rdfs:label "Intermittent Communication Failure" ;
    rdfs:comment "Inconsistent or lack of intended communication of data among internal components or with other external devices." ;
    rdfs:subClassOf imdrf:A13 .

imdrf:A1304 a owl:Class ;
    rdfs:label "Telemetry Discrepancy" ;
    rdfs:comment "Problem associated with variability of the transmission of telemetry signals." ;
    rdfs:subClassOf imdrf:A13 .

imdrf:A1305 a owl:Class ;
    rdfs:label "Wireless Communication Problem" ;
    rdfs:comment "Problems with the RF wireless technology characteristics and performance (e.g., frequency, output power, range, reception), wireless quality of service, wireless coexistence, security of wireless signals and data, and electromagnetic compatibility." ;
    rdfs:subClassOf imdrf:A13 .

imdrf:A140101 a owl:Class ;
    rdfs:label "Failure to Deflate" ;
    ex:statusDescription "Term was added on 18 March 2020 to differentiate between a failure to deflate and an unintended deflation." ;
    rdfs:comment "Problem associated with the inability to deflate a device which is intended to deflate." ;
    rdfs:subClassOf imdrf:A1401 .

imdrf:A140102 a owl:Class ;
    rdfs:label "Unintended Deflation" ;
    ex:statusDescription "Term was added on 18 March 2020 to differentiate between a failure to deflate and an unintended deflation." ;
    rdfs:comment "Problem associated with the unintended deflation of a device which was not designed to deflate or not at that point in time or not to that extent." ;
    rdfs:subClassOf imdrf:A1401 .

imdrf:A1402 a owl:Class ;
    rdfs:label "Excess Flow or Over-Infusion" ;
    rdfs:comment "Problem associated with a delivery overdose of therapeutic agents, such as drugs or fluids being delivered into a device or a patient." ;
    rdfs:subClassOf imdrf:A14 .

imdrf:A140301 a owl:Class ;
    rdfs:label "Inability to Auto-Fill" ;
    rdfs:comment "Complete failure to fill as part of an automated process. For insufficient filling use \"Short Fill\". For excessive filling use \"Overfill\". For inconsistent filling use \"Volume Accuracy Problem\"." ;
    rdfs:subClassOf imdrf:A1403 .

imdrf:A140302 a owl:Class ;
    rdfs:label "Overfill" ;
    rdfs:comment "Excessive filling of a device. For complete failure to fill use \"inability to auto-fill\". For insufficient filling use \"Short Fill\". For inconsistent filling use \"Volume Accuracy Problem\"." ;
    rdfs:subClassOf imdrf:A1403 .

imdrf:A140303 a owl:Class ;
    rdfs:label "Short Fill" ;
    rdfs:comment "Insufficient filling of a device. For complete failure to fill use \"inability to auto-fill\". For insufficient filling use \"short fill\". For inconsistent filling use \"Volume Accuracy Problem\"." ;
    rdfs:subClassOf imdrf:A1403 .

imdrf:A140304 a owl:Class ;
    rdfs:label "Volume Accuracy Problem" ;
    rdfs:comment "Inconsistent filling of a device. This describes a problem which is observed to vary between overfilling and under filling, and may be intermittent. Use \"Overfill\" or \"Short Fill\" if problem is consistent." ;
    rdfs:subClassOf imdrf:A1403 .

imdrf:A140401 a owl:Class ;
    rdfs:label "Inadequate Filtration Process" ;
    rdfs:comment "Problem associated with the filter failing to remove items or substances which should have been removed." ;
    rdfs:subClassOf imdrf:A1404 .

imdrf:A140402 a owl:Class ;
    rdfs:label "Inadequate Ultra Filtration" ;
    rdfs:comment "Problem associated with the transfer of fluid between the blood and dialysate through the dialysis membrane due to a pressure gradient (trans-membrane pressure) existing between the blood and dialysate compartments." ;
    rdfs:subClassOf imdrf:A1404 .

imdrf:A140501 a owl:Class ;
    rdfs:label "Backflow" ;
    rdfs:comment "Continuous flow of fluid (e.g. liquid, gas) against the intended flow direction." ;
    rdfs:subClassOf imdrf:A1405 .

imdrf:A140502 a owl:Class ;
    rdfs:label "Free or Unrestricted Flow" ;
    rdfs:comment "Problem associated with uncontrolled flow of infusion of air, gas or fluids." ;
    rdfs:subClassOf imdrf:A1405 .

imdrf:A140503 a owl:Class ;
    rdfs:label "Gradient Increase" ;
    rdfs:comment "Problem associated with the increased rate of change in temperature, pressure, or other variables as a function of distance, time, etc." ;
    rdfs:subClassOf imdrf:A1405 .

imdrf:A140504 a owl:Class ;
    rdfs:label "Inaccurate Delivery" ;
    rdfs:comment "Delivery at endpoint not as intended; either too low or too high." ;
    rdfs:subClassOf imdrf:A1405 .

imdrf:A140505 a owl:Class ;
    rdfs:label "Inaccurate Flow Rate" ;
    rdfs:comment "Problem associated with fluctuations in the flow volume delivered per time, even if end volume is correct, and delivered in the correct total time." ;
    rdfs:subClassOf imdrf:A1405 .

imdrf:A140506 a owl:Class ;
    rdfs:label "Intermittent Infusion" ;
    rdfs:comment "Problem associated with the infusion not being stead- characterised by intermittent stoppages to the flow." ;
    rdfs:subClassOf imdrf:A1405 .

imdrf:A140507 a owl:Class ;
    rdfs:label "Reflux within Device" ;
    rdfs:comment "Problem associated with partial backflow, compromising the device's flow output." ;
    rdfs:subClassOf imdrf:A1405 .

imdrf:A140508 a owl:Class ;
    rdfs:label "Restricted Flow rate" ;
    rdfs:comment "Problem associated with flow rate. Flow volume delivered over time is not reaching intended flow rate." ;
    rdfs:subClassOf imdrf:A1405 .

imdrf:A140509 a owl:Class ;
    rdfs:label "Tidal Volume Fluctuations" ;
    rdfs:comment "Problem associated with the amount of gas that is inspired and expired during one respiratory cycle." ;
    rdfs:subClassOf imdrf:A1405 .

imdrf:A1406 a owl:Class ;
    rdfs:label "Inflation Problem" ;
    rdfs:comment "Problem associated with the inability of the device to expand or enlarge with the intended inflation agent (e.g. saline or air)." ;
    rdfs:subClassOf imdrf:A14 .

imdrf:A1407 a owl:Class ;
    rdfs:label "Insufficient Flow or Under Infusion" ;
    rdfs:comment "Problem associated with an insufficient dose of therapeutic agents, e.g., drugs or fluids being delivered into a patient under positive pressure." ;
    rdfs:subClassOf imdrf:A14 .

imdrf:A140801 a owl:Class ;
    rdfs:label "Failure to Deliver" ;
    rdfs:comment "Failure (=complete nonperformance) with regard to the intended function of delivery." ;
    rdfs:subClassOf imdrf:A1408 .

imdrf:A140802 a owl:Class ;
    rdfs:label "Failure to Infuse" ;
    rdfs:comment "Failure (=complete nonperformance) with regard to the intended function of infusion." ;
    rdfs:subClassOf imdrf:A1408 .

imdrf:A140803 a owl:Class ;
    rdfs:label "Inability to Irrigate" ;
    rdfs:comment "Failure (=complete nonperformance) with regard to the intended function of irrigation." ;
    rdfs:subClassOf imdrf:A1408 .

imdrf:A140901 a owl:Class ;
    rdfs:label "Complete Blockage" ;
    rdfs:comment "Problem related to an obstruction or blockage within the device component (e.g. tube, opening, pipe) that results in no flow." ;
    rdfs:subClassOf imdrf:A1409 .

imdrf:A140902 a owl:Class ;
    rdfs:label "Partial Blockage" ;
    rdfs:comment "Problem related to an obstruction or blockage within the device component (e.g. tube, opening, pipe) that results in a reduction of the flow rate." ;
    rdfs:subClassOf imdrf:A1409 .

imdrf:A1410 a owl:Class ;
    rdfs:label "Difficult to Flush" ;
    rdfs:comment "The device is difficult to flush, possibly indicating an obstruction within device." ;
    rdfs:subClassOf imdrf:A14 .

imdrf:A141101 a owl:Class ;
    rdfs:label "Decrease in Pressure" ;
    rdfs:comment "Unintended decrease in pressure, compromising the device's intended function." ;
    rdfs:subClassOf imdrf:A1411 .

imdrf:A141102 a owl:Class ;
    rdfs:label "Increase in Pressure" ;
    rdfs:comment "Unintended increase in pressure, compromising the device's intended function." ;
    rdfs:subClassOf imdrf:A1411 .

imdrf:A141103 a owl:Class ;
    rdfs:label "No Pressure" ;
    rdfs:comment "Unintended complete loss of pressure, compromising the device's intended function." ;
    rdfs:subClassOf imdrf:A1411 .

imdrf:A141201 a owl:Class ;
    rdfs:label "Decreased Pump Speed" ;
    rdfs:comment "Unintended decrease in pump speed and hence, probably, flow rate, compromising the intended function of the device." ;
    rdfs:subClassOf imdrf:A1412 .

imdrf:A141202 a owl:Class ;
    rdfs:label "Increased Pump Speed" ;
    rdfs:comment "Unintended increase in pump speed and hence, probably, flow rate, compromising the intended function of the device." ;
    rdfs:subClassOf imdrf:A1412 .

imdrf:A141203 a owl:Class ;
    rdfs:label "Failure to Pump" ;
    rdfs:comment "Problem associated with the device which fails to start pumping." ;
    rdfs:subClassOf imdrf:A1412 .

imdrf:A141204 a owl:Class ;
    rdfs:label "Pumping Stopped" ;
    rdfs:comment "Unexpected/unintended cessation of pump." ;
    rdfs:subClassOf imdrf:A1412 .

imdrf:A141301 a owl:Class ;
    rdfs:label "Decrease in Suction" ;
    ex:statusDescription "Technical change to the definition on 18 March 2020 to include removal of fluid or gas from a device." ;
    rdfs:comment "Problem associated with the removal of fluid or gas from a body cavity or device due to decreased suction." ;
    rdfs:subClassOf imdrf:A1413 .

imdrf:A141302 a owl:Class ;
    rdfs:label "Increase in Suction" ;
    ex:statusDescription "Technical change to the definition on 18 March 2020 to include removal of fluid or gas from a device." ;
    rdfs:comment "Problem associated with the removal of fluid or gas from a body cavity or device due to increased suction." ;
    rdfs:subClassOf imdrf:A1413 .

imdrf:A141303 a owl:Class ;
    rdfs:label "Suction Failure" ;
    rdfs:comment "Problem associated with the complete inability to provide suction." ;
    rdfs:subClassOf imdrf:A1413 .

imdrf:A141401 a owl:Class ;
    rdfs:label "Failure to Prime" ;
    rdfs:comment "Problem associated with the device failing to begin the priming process (i.e. the process of preparation of device for the delivery of fluids)." ;
    rdfs:subClassOf imdrf:A1414 .

imdrf:A141402 a owl:Class ;
    rdfs:label "Incomplete or Inadequate Priming" ;
    rdfs:comment "Problem associated with not adequately preparing the device." ;
    rdfs:subClassOf imdrf:A1414 .

imdrf:A1415 a owl:Class ;
    rdfs:label "Air/Gas in Device" ;
    ex:statusDescription "Term was added on 18 March 2020 as an additional level 2 term to \"Infusion or Flow Problem\"." ;
    rdfs:comment "Problem associated with air in the device (e.g. air in line)." ;
    rdfs:subClassOf imdrf:A14 .

imdrf:A150101 a owl:Class ;
    rdfs:label "Activation Failure" ;
    ex:statusDescription "Editorial change to the definition on 18 March 2020." ;
    rdfs:comment "Problem associated with the device failing to be activated including partial activation." ;
    rdfs:subClassOf imdrf:A1501 .

imdrf:A150102 a owl:Class ;
    rdfs:label "Difficult or Delayed Activation" ;
    rdfs:comment "Problem associated with delayed or difficult activation of the device." ;
    rdfs:subClassOf imdrf:A1501 .

imdrf:A150103 a owl:Class ;
    rdfs:label "Premature Activation" ;
    rdfs:comment "Problem associated with early and unexpected activation of the device." ;
    rdfs:subClassOf imdrf:A1501 .

imdrf:A150104 a owl:Class ;
    rdfs:label "Self-Activation or Keying" ;
    ex:status "Modified (technical)" ;
    ex:statusDescription "Definition modified for Release Number 2025. See no. 3 of Change Request Log." ;
    rdfs:comment "Problem associated with the unexpected or unintended activation of the device or a device function.  For Unintended Power Up use A070804" ;
    rdfs:subClassOf imdrf:A1501 .

imdrf:A150105 a owl:Class ;
    rdfs:label "Key or Button Unresponsive/not Working" ;
    ex:statusDescription "Term was added on 18 March 2020 as an additional level 3 term to \"Activation Problem\"." ;
    rdfs:comment "Problem associated with a device not responding to key or button inputs." ;
    rdfs:subClassOf imdrf:A1501 .

imdrf:A150106 a owl:Class ;
    rdfs:label "Unexpected Deactivation" ;
    ex:status "New" ;
    ex:statusDescription "Term added for Release Number 2025. See no. 8 of Change Request Log" ;
    rdfs:comment "Problem associated with a device deactivating during use." ;
    rdfs:subClassOf imdrf:A1501 .

imdrf:A150201 a owl:Class ;
    rdfs:label "Positioning Failure" ;
    rdfs:comment "Problem associated with the inability of the device to be positioned in a specified location." ;
    rdfs:subClassOf imdrf:A1502 .

imdrf:A150202 a owl:Class ;
    rdfs:label "Malposition of Device" ;
    rdfs:comment "Problem associated with the device being positioned in a location other than intended or specified." ;
    rdfs:subClassOf imdrf:A1502 .

imdrf:A150203 a owl:Class ;
    rdfs:label "Difficult or Delayed Positioning" ;
    rdfs:comment "Problem associated with users experiencing difficulty or delay to position the device to a specified location." ;
    rdfs:subClassOf imdrf:A1502 .

imdrf:A150204 a owl:Class ;
    rdfs:label "Failure to Advance" ;
    rdfs:comment "Problem associated with failure to move the device to an intended location." ;
    rdfs:subClassOf imdrf:A1502 .

imdrf:A150205 a owl:Class ;
    rdfs:label "Difficult to Advance" ;
    rdfs:comment "Problem associated with difficulty moving the device to an intended location (e.g. difficulty in advancing guide wire)." ;
    rdfs:subClassOf imdrf:A1502 .

imdrf:A150206 a owl:Class ;
    rdfs:label "Difficult to Insert" ;
    rdfs:comment "Problem associated with problems introducing or inserting the device, even if the user is operating the device in accordance with the instructions for use or labeling." ;
    rdfs:subClassOf imdrf:A1502 .

imdrf:A150207 a owl:Class ;
    rdfs:label "Difficult to Remove" ;
    ex:statusDescription "Editorial change to the definition on 18 March 2020." ;
    rdfs:comment "Problem associated with the user experiencing difficulty when taking out the device, even if the user is operating device in accordance with the instructions for use or labeling." ;
    rdfs:subClassOf imdrf:A1502 .

imdrf:A150208 a owl:Class ;
    rdfs:label "Entrapment of Device" ;
    rdfs:comment "Problem associated with the device caught within patient vasculature, tissue, or other device." ;
    rdfs:subClassOf imdrf:A1502 .

imdrf:A150301 a owl:Class ;
    rdfs:label "Separation Failure" ;
    rdfs:comment "Problem associated with the device or one of its components failing to detach or separate as intended." ;
    rdfs:subClassOf imdrf:A1503 .

imdrf:A150302 a owl:Class ;
    rdfs:label "Difficult or Delayed Separation" ;
    rdfs:comment "Problem associated with users experiencing difficulty or delay with detachment or separation of the device." ;
    rdfs:subClassOf imdrf:A1503 .

imdrf:A150303 a owl:Class ;
    rdfs:label "Premature Separation" ;
    rdfs:comment "Problem associated with an early and unexpected detachment or separation of the device from the system." ;
    rdfs:subClassOf imdrf:A1503 .

imdrf:A160101 a owl:Class ;
    rdfs:label "Alarm Not Visible" ;
    rdfs:comment "The device does not display an alarm message when required." ;
    rdfs:subClassOf imdrf:A1601 .

imdrf:A160102 a owl:Class ;
    rdfs:label "No Audible Alarm" ;
    rdfs:comment "The device fails to emit an audible alarm." ;
    rdfs:subClassOf imdrf:A1601 .

imdrf:A160103 a owl:Class ;
    rdfs:label "Low Audible Alarm" ;
    rdfs:comment "The audible device alarm cannot be heard clearly." ;
    rdfs:subClassOf imdrf:A1601 .

imdrf:A160104 a owl:Class ;
    rdfs:label "Delayed Alarm" ;
    rdfs:comment "The device alarm system operates with delay." ;
    rdfs:subClassOf imdrf:A1601 .

imdrf:A160105 a owl:Class ;
    rdfs:label "False Alarm" ;
    rdfs:comment "Problem associated with the device providing incorrect alarm warning or alert to user." ;
    rdfs:subClassOf imdrf:A1601 .

imdrf:A160106 a owl:Class ;
    rdfs:label "Defective Alarm" ;
    rdfs:comment "The device alarm does not operate as expected and/or in agreement with device's specifications." ;
    rdfs:subClassOf imdrf:A1601 .

imdrf:A160201 a owl:Class ;
    rdfs:label "Fail-Safe Did Not Operate" ;
    rdfs:comment "Problem associated with the device fail-safe mechanism, which did not function or function in a non effective way, compromising safe use of the device." ;
    rdfs:subClassOf imdrf:A1602 .

imdrf:A160202 a owl:Class ;
    rdfs:label "No Fail-Safe Mechanism" ;
    rdfs:comment "The device does not have a fail-safe mechanism, although such mechanism would be required for its appropriate and/or safe functioning." ;
    rdfs:subClassOf imdrf:A1602 .

imdrf:A1603 a owl:Class ;
    rdfs:label "Failure of Device to Self-Test" ;
    rdfs:comment "Problem associated with the device failing to perform an internal self-diagnostic process to ensure normal operation during or prior to use." ;
    rdfs:subClassOf imdrf:A16 .

imdrf:A1604 a owl:Class ;
    rdfs:label "Failure to Auto Stop" ;
    rdfs:comment "Problem associated with the inability of device to turn itself off when the device is not in an operable condition." ;
    rdfs:subClassOf imdrf:A16 .

imdrf:A160501 a owl:Class ;
    rdfs:label "Failure to Reset" ;
    rdfs:comment "Problem associated with the device failing to set a variable, register, or other storage location back to a prescribed state." ;
    rdfs:subClassOf imdrf:A1605 .

imdrf:A160502 a owl:Class ;
    rdfs:label "Failure to Zero" ;
    rdfs:comment "Problem associated with the device failing to set a variable, register, or other storage location back to zero." ;
    rdfs:subClassOf imdrf:A1605 .

imdrf:A160503 a owl:Class ;
    rdfs:label "Inappropriate or Unexpected Reset" ;
    rdfs:comment "Problem associated with the device setting a variable, register, or other storage location to an inappropriate or unexpected state." ;
    rdfs:subClassOf imdrf:A1605 .

imdrf:A160601 a owl:Class ;
    rdfs:label "Premature Elective Replacement Indicator" ;
    rdfs:comment "Problems with the early or unexpected activation of the elective replacement indicator." ;
    rdfs:subClassOf imdrf:A1606 .

imdrf:A160602 a owl:Class ;
    rdfs:label "Premature End-of-Life Indicator" ;
    rdfs:comment "Problem with the early or unexpected activation of the end-of-life indicator." ;
    rdfs:subClassOf imdrf:A1606 .

imdrf:A1607 a owl:Class ;
    rdfs:label "Shielding Failure" ;
    rdfs:comment "Problem associated with the device inability to act as a barrier for absorption of radiation energy in X-rays, gamma rays, etc." ;
    rdfs:subClassOf imdrf:A16 .

imdrf:A170101 a owl:Class ;
    rdfs:label "Accessory Incompatible" ;
    rdfs:comment "An accessory required for the intended purpose of the device appears incompatible with device, thus compromising the intended function of the device." ;
    rdfs:subClassOf imdrf:A1701 .

imdrf:A170102 a owl:Class ;
    rdfs:label "Component Incompatible" ;
    rdfs:comment "A component required for the proper functioning of the device is not compatible with other components or subassemblies of the device, thus compromising the intended function of the device." ;
    rdfs:subClassOf imdrf:A1701 .

imdrf:A1702 a owl:Class ;
    rdfs:label "Device-Device Incompatibility" ;
    rdfs:comment "Problem associated with the incompatibility of two or more devices while being operated in the same use environment thereby leading to a dysfunction of more than one device." ;
    rdfs:subClassOf imdrf:A17 .

imdrf:A1703 a owl:Class ;
    rdfs:label "Measurement System Incompatibility" ;
    rdfs:comment "Problem associated with the incompatibility of the measurement systems between and/or within device systems that are inherent to the individual device thereby leading to miscalculated or mismatched measurements from those devices, e.g., international metric system versus U.S. measurement system." ;
    rdfs:subClassOf imdrf:A17 .

imdrf:A1704 a owl:Class ;
    rdfs:label "Unintended Compatibility" ;
    rdfs:comment "Problem associated with the ability of two or more devices which are intended to be incompatible but are able to work or fit together." ;
    rdfs:subClassOf imdrf:A17 .

imdrf:A180101 a owl:Class ;
    rdfs:label "Biofilm coating in Device" ;
    rdfs:comment "Problem associated with the undesired introduction of a biofilm coating into or onto the device." ;
    rdfs:subClassOf imdrf:A1801 .

imdrf:A180102 a owl:Class ;
    rdfs:label "Contamination of Device Ingredient or Reagent" ;
    rdfs:comment "Problem associated with the undesired introduction of impurities either chemical or microbiological in nature, or of foreign matter into or onto the device ingredient or reagent." ;
    rdfs:subClassOf imdrf:A1801 .

imdrf:A180103 a owl:Class ;
    rdfs:label "Device Contamination with Body Fluid" ;
    rdfs:comment "Problem associated with the undesired presence of body fluid in/on the device, which are not part of the documented device specifications and requirements." ;
    rdfs:subClassOf imdrf:A1801 .

imdrf:A180104 a owl:Class ;
    rdfs:label "Device Contamination with Chemical or Other Material" ;
    rdfs:comment "Problem associated with contamination of the device with chemical substance or other non biologic material." ;
    rdfs:subClassOf imdrf:A1801 .

imdrf:A180105 a owl:Class ;
    rdfs:label "Microbial Contamination of Device" ;
    rdfs:comment "Problem associated with undesired microbial contamination of the device." ;
    rdfs:subClassOf imdrf:A1801 .

imdrf:A1802 a owl:Class ;
    rdfs:label "Device Contaminated During Manufacture or Shipping" ;
    ex:statusDescription "Technical change to the definition on 18 March 2020 to clarify that contamination occurred during manufacture or shipping." ;
    rdfs:comment "Problem associated with the presence of any unexpected foreign substance found on the surface or in the package materials, which may affect optimal performance for its intended use, and which occurred during manufacture or shipping." ;
    rdfs:subClassOf imdrf:A18 .

imdrf:A180301 a owl:Class ;
    rdfs:label "Failure to Clean Adequately" ;
    rdfs:comment "Problem associated with the failure of the device or operator to remove any visible soil, foreign material or organism deposits on the external surfaces, crevices, and joints of the device." ;
    rdfs:subClassOf imdrf:A1803 .

imdrf:A180302 a owl:Class ;
    rdfs:label "Failure to Disinfect" ;
    rdfs:comment "Failure to properly disinfect the device when reprocessing it." ;
    rdfs:subClassOf imdrf:A1803 .

imdrf:A180303 a owl:Class ;
    rdfs:label "Flushing Problem" ;
    rdfs:comment "Flushing process was not executed properly." ;
    rdfs:subClassOf imdrf:A1803 .

imdrf:A180304 a owl:Class ;
    rdfs:label "Problem with Removal of Enzymatic Cleaner" ;
    rdfs:comment "Enzymatic cleaner was not removed properly." ;
    rdfs:subClassOf imdrf:A1803 .

imdrf:A180305 a owl:Class ;
    rdfs:label "Problem with Sterilization" ;
    rdfs:comment "Device was not sterilized properly during reprocessing." ;
    rdfs:subClassOf imdrf:A1803 .

imdrf:A180306 a owl:Class ;
    rdfs:label "Residue After Decontamination" ;
    rdfs:comment "Problem associated with the decontamination process not adequately removing unwanted visible soil, foreign material, or organism deposits." ;
    rdfs:subClassOf imdrf:A1803 .

imdrf:A1804 a owl:Class ;
    rdfs:label "Device Contaminated at the User Facility" ;
    ex:statusDescription "Term was added on 18 March 2020 for coding of contamination at the user facility which was originally included in \"Contamination During Use\" (A1801)." ;
    rdfs:comment "Problem associated with the presence of any unexpected foreign substance found on the surface or in the package materials, which may affect optimal performance for its intended use, and which occurred at the user facility." ;
    rdfs:subClassOf imdrf:A18 .

imdrf:A1901 a owl:Class ;
    rdfs:label "Ambient Noise Problem" ;
    rdfs:comment "Problem associated with any undesired acoustic energy or vibration that tends to interfere with the operation of the device." ;
    rdfs:subClassOf imdrf:A19 .

imdrf:A1902 a owl:Class ;
    rdfs:label "Ambient Temperature Problem" ;
    rdfs:comment "Problem associated with compromised device performance at the ambient temperature or the storage at an inappropriate ambient temperature." ;
    rdfs:subClassOf imdrf:A19 .

imdrf:A1903 a owl:Class ;
    rdfs:label "Fumes or Vapors" ;
    rdfs:comment "Problem associated with the visibility, odor, or toxicity of an ambient vapor or gas." ;
    rdfs:subClassOf imdrf:A19 .

imdrf:A1904 a owl:Class ;
    rdfs:label "Fungus in Device Environment" ;
    rdfs:comment "Problem associated with the visibility of molds, mildews, yeasts, and/or mushrooms in the immediate environment in which the device is being used." ;
    rdfs:subClassOf imdrf:A19 .

imdrf:A190501 a owl:Class ;
    rdfs:label "Moisture Damage" ;
    rdfs:comment "Problem associated with damage inflicted upon the device from water vapor or water in the immediate environment in which the device is being used." ;
    rdfs:subClassOf imdrf:A1905 .

imdrf:A190601 a owl:Class ;
    rdfs:label "Fogging" ;
    rdfs:comment "Problem associated with the visibility of water vapor in the immediate atmosphere in which the device is being used." ;
    rdfs:subClassOf imdrf:A1906 .

imdrf:A1907 a owl:Class ;
    rdfs:label "Device Unsafe to Use in Environment" ;
    rdfs:comment "Problem associated with environmental condition that results in the unsafe use of the device. (e.g. electromagnetic fields, noise, vibration, microbiological contamination etc.)" ;
    rdfs:subClassOf imdrf:A19 .

imdrf:A1908 a owl:Class ;
    rdfs:label "Environmental Particulates" ;
    rdfs:comment "Problem associated with fine solids or liquid particles such as dust, smoke, fume, and/or mist suspended in the immediate atmosphere in which the device is being used." ;
    rdfs:subClassOf imdrf:A19 .

imdrf:A1909 a owl:Class ;
    rdfs:label "Medical Gas Supply Problem" ;
    rdfs:comment "Problem associated with the facility-supplied medical gases such as medical air, oxygen, nitrous oxide, and nitrogen." ;
    rdfs:subClassOf imdrf:A19 .

imdrf:A191001 a owl:Class ;
    rdfs:label "Emergency Power Failure" ;
    rdfs:comment "Problem associated with the failure of the facility's emergency power backup system(s) including generators and/or interruptible power systems (UPS)." ;
    rdfs:subClassOf imdrf:A1910 .

imdrf:A191002 a owl:Class ;
    rdfs:label "Loss of Power" ;
    rdfs:comment "Problem associated with the failure of primary power supplied by the facility." ;
    rdfs:subClassOf imdrf:A1910 .

imdrf:A191003 a owl:Class ;
    rdfs:label "Power Conditioning Problem" ;
    rdfs:comment "Problem associated with a momentary overpower/over voltage from the utility and electrical systems of user facilities; - Problem associated with inadequate power conditioning such as the presence of fluctuation, surges, spikes, dropouts, noise and other such undesirable transients." ;
    rdfs:subClassOf imdrf:A1910 .

imdrf:A2001 a owl:Class ;
    rdfs:label "Misassembled During Installation" ;
    rdfs:comment "Problem associated with the use of the device characterized by incorrect assembly of device components, parts or constituents." ;
    rdfs:subClassOf imdrf:A20 .

imdrf:A210101 a owl:Class ;
    rdfs:label "Expiration Date Error" ;
    rdfs:comment "Problem associated with errors in identification of expiration date." ;
    rdfs:subClassOf imdrf:A2101 .

imdrf:A210102 a owl:Class ;
    rdfs:label "Illegible Information" ;
    rdfs:comment "Problem associated with information unable to be read or deciphered." ;
    rdfs:subClassOf imdrf:A2101 .

imdrf:A210103 a owl:Class ;
    rdfs:label "Inaccurate Information" ;
    rdfs:comment "Problem associated with imprecise, inexact information." ;
    rdfs:subClassOf imdrf:A2101 .

imdrf:A210104 a owl:Class ;
    rdfs:label "Unclear Information" ;
    rdfs:comment "Problem associated with ambiguous, confused information." ;
    rdfs:subClassOf imdrf:A2101 .

imdrf:A210105 a owl:Class ;
    rdfs:label "Missing Information" ;
    rdfs:comment "Absence of information e.g. labeling, instruction for use." ;
    rdfs:subClassOf imdrf:A2101 .

imdrf:A210106 a owl:Class ;
    rdfs:label "Wrong Label" ;
    ex:statusDescription "Term was added on 27 January 2022. For details, see comment No. 2 of the Change Log (Release Number 2022)." ;
    rdfs:comment "Problem associated with an incorrect label being affixed to the device or packaging." ;
    rdfs:subClassOf imdrf:A2101 .

imdrf:A210107 a owl:Class ;
    rdfs:label "Device label look-alike" ;
    ex:statusDescription "Term added for Release Number 2024. See no. 117 of Change Log" ;
    rdfs:comment "Problem associated with medical device label that  looks similar to another product leading to confusion. The other product may be another device or a different product such as a medicine or cleaning agent.  Use A020505 for Device packaging look-alike." ;
    rdfs:subClassOf imdrf:A2101 .

imdrf:A2102 a owl:Class ;
    rdfs:label "Lack of Maintenance Documentation or Guidelines" ;
    rdfs:comment "Problem associated with user facility not receiving adequate service documentation, guidelines, or recommendations to perform preventative and corrective maintenance and performance assurance checks." ;
    rdfs:subClassOf imdrf:A21 .

imdrf:A2103 a owl:Class ;
    rdfs:label "Inadequate Instructions for Healthcare Professional" ;
    rdfs:comment "Problem associated with inaccuracies in any written, printed, or graphic matter that is affixed to the device or its packaging with any matter that accompanies the device including verbal instructions related to identification, technical description and use of device provided by the device manufacturers that is intended for healthcare professionals." ;
    rdfs:subClassOf imdrf:A21 .

imdrf:A2104 a owl:Class ;
    rdfs:label "Inadequate Instructions for Non-Healthcare Professional" ;
    rdfs:comment "Problem associated with users being unclear and not able to follow any written, printed, or graphic matter that is affixed to device or its packaging with any matter that accompanies the device including verbal instructions related to identification, technical description and use of the device provided by the device manufactures that vary from the standard of medical care in a given environment." ;
    rdfs:subClassOf imdrf:A21 .

imdrf:A2105 a owl:Class ;
    rdfs:label "Inadequate or Insufficient Training" ;
    rdfs:comment "Problem associated with facility not providing satisfactory initial and/or periodic user training covering operation of the device." ;
    rdfs:subClassOf imdrf:A21 .

imdrf:A2201 a owl:Class ;
    rdfs:label "Device Difficult to Setup or Prepare" ;
    ex:status "Modified (technical)" ;
    ex:statusDescription "Definition modified for Release Number 2025. See no. 45 of Change Request Log." ;
    rdfs:comment """Problem associated with the user experiencing difficulty in preparing the device for use, even if the operation is being performed according to labeled instructions for use.
This includes difficulty attaching or connecting parts together.""" ;
    rdfs:subClassOf imdrf:A22 .

imdrf:A2202 a owl:Class ;
    rdfs:label "Device Difficult to Program or Calibrate" ;
    rdfs:comment "The device is difficult to program, calibrate or set to desired state, even by appropriately trained user/operator." ;
    rdfs:subClassOf imdrf:A22 .

imdrf:A2203 a owl:Class ;
    rdfs:label "Device Difficult to Maintain" ;
    rdfs:comment "Problem associated with the user's ability to service the device according to the manufacturer specifications relating to the device routine maintenance, i.e., periodic inspection, failure detection, repair, and care of the device to sustain or restore acceptable operating conditions." ;
    rdfs:subClassOf imdrf:A22 .

imdrf:A2204 a owl:Class ;
    rdfs:label "Inadequate User Interface" ;
    rdfs:comment "Problem associated with the means by which the operator and the equipment communicate or interact." ;
    rdfs:subClassOf imdrf:A22 .

imdrf:A2205 a owl:Class ;
    rdfs:label "Device Provides Uninformative Message" ;
    ex:statusDescription "Term added for Release Number 2024. See no. 42 of Change Log" ;
    rdfs:comment """The device provides a message which is unhelpful or uninformative, such as an error code without further information about the meaning or appropriate action to take.
If the message does not make sense then use A2206 - Device Provides Unintelligible Message.""" ;
    rdfs:subClassOf imdrf:A22 .

imdrf:A2206 a owl:Class ;
    rdfs:label "Device Provides Unintelligible Message" ;
    ex:statusDescription "Term added for Release Number 2024. See no. 42 of Change Log" ;
    rdfs:comment """The device provides an unintelligible or incomprehensible message such as an apparently random string of characters.
If the message makes sense but is not helpful then use A2205 - Device Provides Uninformative Message.""" ;
    rdfs:subClassOf imdrf:A22 .

imdrf:A2301 a owl:Class ;
    rdfs:label "Device Handling Problem" ;
    rdfs:comment "Handling of the device not in accordance with specification, prior to use on the patient." ;
    rdfs:subClassOf imdrf:A23 .

imdrf:A2302 a owl:Class ;
    rdfs:label "Use of Incorrect Control/Treatment Settings" ;
    ex:statusDescription "Term/Definition was modified on 27 January 2022 (Old term/definition: Use of Incorrect Control Settings: Problem associated with the use of the device in terms of inappropriate or false control settings for the device's specified operation and/or intended use). For details, see comment No. 26 of the Change Log (Release Number 2022)." ;
    rdfs:comment "Problem associated with the use of the device in terms of inappropriate or incorrect control settings or incorrect treatment parameters for the device's specified operation and/or intended use." ;
    rdfs:subClassOf imdrf:A23 .

imdrf:A2303 a owl:Class ;
    rdfs:label "Improper or Incorrect Procedure or Method" ;
    rdfs:comment "Problem associated with the use of the device in terms of nonconforming to that device's intended use, specifications, procedure and process or service instructions and information provided by the device manufacturers." ;
    rdfs:subClassOf imdrf:A23 .

imdrf:A2304 a owl:Class ;
    rdfs:label "Off-Label Use" ;
    rdfs:comment "Problem associated with the device which has been used for an unapproved indication or for an unapproved intended use." ;
    rdfs:subClassOf imdrf:A23 .

imdrf:A230501 a owl:Class ;
    rdfs:label "Misassembly by Users" ;
    rdfs:comment "Problem associated with incorrect assembly of the device or constituents by the users." ;
    rdfs:subClassOf imdrf:A2305 .

imdrf:A230502 a owl:Class ;
    rdfs:label "Misassembly During Maintenance/Repair" ;
    rdfs:comment "Problem associated with incorrect assembly of the device or constituents during maintenance or repair." ;
    rdfs:subClassOf imdrf:A2305 .

imdrf:A24 a owl:Class ;
    rdfs:label "Adverse Event Without Identified Device or Use Problem" ;
    rdfs:comment "An adverse event (e.g. patient harm) appears to have occurred, but there does not appear to have been a problem with the device or the way it was used." .

imdrf:A2501 a owl:Class ;
    rdfs:label "Prophylactic removal due to corrective action" ;
    ex:statusDescription "Term was added on 31 January 2023. For details, see comment No. 30 of the Change Log (Release Number 2023)." ;
    rdfs:comment "Prophylactic removal of a device due to corrective action without malfunction or problem of the specific device involved" ;
    rdfs:subClassOf imdrf:A25 .

imdrf:A26 a owl:Class ;
    rdfs:label "Insufficient Device Problem Information" ;
    ex:status "Modified (editorial)" ;
    ex:statusDescription "Term modified for Release Number 2025. Previous term was Insufficient Information. See no. 120 of Change Request Log." ;
    rdfs:comment "An adverse event appears to have occurred but there is not yet enough information available to classify the device problem." .

imdrf:A27 a owl:Class ;
    rdfs:label "Appropriate Device Problem Term/Code Not Available" ;
    ex:status "Modified (editorial)" ;
    ex:statusDescription "Term modified for Release Number 2025. Previous term was \"Appropriate Term/Code Not Available\". See no. 107 of Change Request Log." ;
    rdfs:comment "The device problem is not adequately described by any other term. Note: this code must not be used unless there is no other feasible code. The preferred term should be documented when submitting an adverse event report. This information will be used to determine if a new term should be added to the code table." .

imdrf:B01 a owl:Class ;
    rdfs:label "Testing of Actual/Suspected Device" ;
    rdfs:comment "The investigation employed relevant empirical testing of the actual device suspected in the reported adverse event in order to establish their functional and other properties and to identify possible causes for the adverse event. Relevant testing would typically be based on test methods used for evaluating safety and performance as described in the latest relevant standards." .

imdrf:B02 a owl:Class ;
    rdfs:label "Testing of Device from Same Lot/Batch Retained by Manufacturer" ;
    rdfs:comment "The investigation employed relevant empirical testing of the device of the same lot or batch than that of the suspected device in the reported adverse event in order to support the identification of possible causes for the adverse event. Testing was performed using the device retained by the manufacturer (i.e. was not shipped). Relevant testing would typically be based on test methods used for evaluating safety and performance as described in the latest relevant standards." .

imdrf:B03 a owl:Class ;
    rdfs:label "Testing of Device from Same Lot/Batch Returned from User" ;
    rdfs:comment "The investigation employed relevant empirical testing of the device of the same lot or batch than that of the suspected device in the reported adverse event in order to support the identification of possible causes for the adverse event. The device was returned from the user. Relevant testing would typically be based on test methods used for evaluating safety and performance as described in the latest relevant standards." .

imdrf:B04 a owl:Class ;
    rdfs:label "Testing of Device from Other Lot/Batch Retained by Manufacturer" ;
    rdfs:comment "The investigation employed relevant empirical testing of the device of another lot or batch than that of the suspected device in the reported adverse event in order to support the identification of possible causes for the adverse event. This includes devices without a lot/batch designation. Testing was performed using the device retained by the manufacturer (i.e. was not shipped). Relevant testing would typically be based on test methods used for evaluating safety and performance as described in the latest relevant standards." .

imdrf:B05 a owl:Class ;
    rdfs:label "Testing of Device from Other Lot/Batch Returned From User" ;
    ex:statusDescription "Definition was modified on 27 January 2022. See comment No. 13 of the Change Log (Release Number 2022)." ;
    rdfs:comment "The investigation employed relevant empirical testing of the device of another lot or batch than that of the suspected device in the reported adverse event in order to support the identification of possible causes for the adverse event. This includes devices without a lot/batch designation. The device was returned from the user. Relevant testing would typically be based on test methods used for evaluating safety and performance as described in the technical file or in the latest relevant standards." .

imdrf:B06 a owl:Class ;
    rdfs:label "Testing of Model Variant" ;
    rdfs:comment "The investigation employed relevant empirical testing of a model variant of the device involved in the reported adverse event in order to support the identification of possible causes for the adverse event through plausibility reasoning. A model variant is not identical to the actual device, but shares relevant characteristics with the device involved. Relevant testing would typically be based on test methods used for evaluating safety and performance as described in the latest relevant standards." .

imdrf:B07 a owl:Class ;
    rdfs:label "Testing of Raw/Starting Materials" ;
    rdfs:comment "The investigation employed relevant empirical testing of the materials used in construction of the device involved in the reported adverse event in order to support the identification of possible causes for the adverse event. Relevant testing would typically be based on test methods used for evaluating safety and performance as described in the latest relevant standards." .

imdrf:B08 a owl:Class ;
    rdfs:label "Testing of Patient Sample or Reference Material Using Manufacturer's Device" ;
    ex:status "Retired" ;
    ex:statusDescription "Term retired for Release Number 2025. Use B26 Testing of Patient Sample Using Manufacturer's Device or B27 Testing of Reference Material Using Manufacturer's Device. See no. 9 and 10 of Change Log" ;
    rdfs:comment "The investigation employed relevant empirical testing of a patient sample or reference material using the device (usually an IVD) involved in the reported adverse event in order to support the identification of possible causes for the adverse event. Relevant testing would typically be based on test methods used for evaluating safety and performance as described in the latest relevant standards." .

imdrf:B09 a owl:Class ;
    rdfs:label "Testing of Patient Sample or Reference Material Using Reference Method" ;
    rdfs:comment "The investigation employed relevant empirical testing of a patient sample or reference material using an appropriate reference method to the device (usually an IVD) involved in the reported adverse event in order to support the identification of possible causes for the adverse event. Relevant testing would typically be based on test methods used for evaluating safety and performance as described in the latest relevant standards." .

imdrf:B10 a owl:Class ;
    rdfs:label "Testing of Patient Sample or Reference Material Using Competitor's Device" ;
    rdfs:comment "The investigation employed relevant empirical testing of a patient sample or reference material using a competitor's device that is comparable to the device (usually an IVD) involved in the reported adverse event in order to support the identification of possible causes for the adverse event. Relevant testing would typically be based on test methods used for evaluating safety and performance as described in the latest relevant standards." .

imdrf:B11 a owl:Class ;
    rdfs:label "Historical Data Analysis" ;
    rdfs:comment "The investigation involved the analysis of historical adverse events data of the actual device involved in the adverse event and/or of products from the same and/or different batches/lots." .

imdrf:B12 a owl:Class ;
    rdfs:label "Trend Analysis" ;
    rdfs:comment "The investigation involved trend analysis of adverse event of the actual device involved in the adverse event and/or of products from the same and/or different batches/lots. It should be noted that trend analysis typically is not considered sufficient as a stand-alone method, but should be used in conjunction with other investigation methods for providing for instance complementary information." .

imdrf:B13 a owl:Class ;
    rdfs:label "Communication/Interviews" ;
    rdfs:comment "The investigation involved communication/interviews (either interpersonal or through technical means, e.g. phone, e-mail) with persons close to the adverse event, e.g. healthcare professionals (doctors, nurses etc.), the affected patient(s) or other users including, where appropriate, relatives or others engaged in caring for the affected patient." .

imdrf:B14 a owl:Class ;
    rdfs:label "Analysis of Production Records" ;
    rdfs:comment "The investigation involved the analysis of relevant production records in view of supporting the identification of possible causes for the adverse event." .

imdrf:B15 a owl:Class ;
    rdfs:label "Analysis of Information Provided by User/Third Party" ;
    ex:statusDescription "Term/definition was modified on 31 January 2023 (Old term/definition: Analysis of Data Provided by User/Third Party: The investigation involved the analysis of relevant data provided by the user (e.g. healthcare professional, patient, clinical engineer) or a third party (e.g. testing facility) in view of supporting the identification of possible causes for the adverse event.). For details, refer to comment No. 41 of the Change Log (Release Number 2023)." ;
    rdfs:comment "The investigation involved the analysis of relevant information provided by the user (e.g. healthcare professional, patient, clinical engineer) or a third party (e.g. testing facility) in view of supporting the identification of possible causes for the adverse event. This does not include information recorded by the device." .

imdrf:B16 a owl:Class ;
    rdfs:label "Device Not Manufactured by Reporting Manufacturer" ;
    ex:statusDescription "Definition was modified on 31 January 2023 (Old definition: Further information was obtained which established that the manufacturer of the device involved was not the one to which it was initially attributed. Use in conjunction with C20 and D14.). For details, refer to comment No. 49 of the Change Log (Release Number 2023)." ;
    rdfs:comment "Further information was obtained which established that the manufacturer of the device involved was not the one to which it was initially attributed. This includes mistaken identity or falsified device. Use in conjunction with C20 and D13 or D14." .

imdrf:B17 a owl:Class ;
    rdfs:label "Device Not Returned" ;
    rdfs:comment "The actual device involved in the adverse event was not returned for testing despite requests by manufacturer." .

imdrf:B18 a owl:Class ;
    rdfs:label "Device Discarded" ;
    rdfs:comment "The actual device involved in the adverse event had been already discarded and thus irretrievably lost for testing." .

imdrf:B19 a owl:Class ;
    rdfs:label "Incomplete Device Returned" ;
    rdfs:comment "The device was returned incompletely, lacking parts, components or accessories that would be required for appropriate testing and analysis of root causes." .

imdrf:B20 a owl:Class ;
    rdfs:label "Device Not Accessible for Testing" ;
    rdfs:comment "The actual device involved in the adverse event is not readily accessible for testing (e.g. remains implanted in patient)." .

imdrf:B21 a owl:Class ;
    rdfs:label "Type of Investigation Not Yet Determined" ;
    rdfs:comment "Details to determine the type of investigation are not yet available, but are being sought. Do not use this code if the investigation is complete." .

imdrf:B22 a owl:Class ;
    rdfs:label "Insufficient Information Available" ;
    rdfs:comment "The information available relating to the reported event is not sufficient to identify either the manufacturer, the device, or other essential information. This term indicates that no further investigation is possible. Do not use this code if further information is being sought, instead use ''Type of investigation not yet determined''." .

imdrf:B23 a owl:Class ;
    rdfs:label "Specimen Requested But Not Provided" ;
    ex:statusDescription "Term was added on 21 January 2021. For details, refer to comment No. 22 of the Change Log." ;
    rdfs:comment "A patient specimen was required to adequately investigate the issue and was requested but not provided." .

imdrf:B24 a owl:Class ;
    rdfs:label "Event History Log Review" ;
    ex:statusDescription "Definition was modified on 31 January 2023 (Old definition: The investigation involved the analysis of the history log files retrieved from the device to support possible causes for the adverse event.). For details, refer to comment No. 41 of the Change Log (Release Number 2023)." ;
    rdfs:comment "The investigation involved the analysis of the history log files retrieved from the device to support possible causes for the adverse event, includes device interrogation." .

imdrf:B25 a owl:Class ;
    rdfs:label "Particulate Testing" ;
    ex:statusDescription "Term was added on 31 January 2023. For details, refer to comment No. 42 of the Change Log (Release Number 2023)." ;
    rdfs:comment "Analysis of particulate or foreign material returned from user for evaluation." .

imdrf:B26 a owl:Class ;
    rdfs:label "Testing of Patient Sample Using Manufacturer's Device" ;
    ex:status "New" ;
    ex:statusDescription "Term added for Release Number 2025. See no. 9 of Change Request Log" ;
    rdfs:comment "The investigation employed relevant empirical testing of a patient sample using the device (usually an IVD) involved in the reported adverse event or an identical device. Relevant testing would typically be based on test methods used for evaluating safety and performance as described in the latest relevant standards." .

imdrf:B27 a owl:Class ;
    rdfs:label "Testing of Reference Material Using Manufacturer's Device" ;
    ex:status "New" ;
    ex:statusDescription "Term added for Release Number 2025. See no. 10 of Change Request Log" ;
    rdfs:comment "The investigation employed relevant empirical testing of a reference material using the device (usually an IVD) involved in the reported adverse event or an identical device. Relevant testing would typically be based on test methods used for evaluating safety and performance as described in the latest relevant standards." .

imdrf:B28 a owl:Class ;
    rdfs:label "Device Lost in Transit" ;
    ex:status "New" ;
    ex:statusDescription "Term added for Release Number 2025. See no. 11 of Change Request Log" ;
    rdfs:comment "The actual device involved in the adverse event has been returned by the user but not received for testing." .

imdrf:B29 a owl:Class ;
    rdfs:label "Device Data not Available for Required Analysis" ;
    ex:status "New" ;
    ex:statusDescription "Term added for Release Number 2025. See no. 12 of Change Request Log" ;
    rdfs:comment "Device data such as software logs are not available for analysis by the manufacturer" .

imdrf:B30 a owl:Class ;
    rdfs:label "Analysis of Images" ;
    ex:status "New" ;
    ex:statusDescription "Term added for Release Number 2025. See no. 36 of Change Request Log" ;
    rdfs:comment "The investigation involved review of images of the device, and/or procedural or diagnostic images." .

imdrf:B31 a owl:Class ;
    rdfs:label "Labelling Review" ;
    ex:status "New" ;
    ex:statusDescription "Term added for Release Number 2025. See no. 85 of Change Request Log" ;
    rdfs:comment "A review of the reported information against the product labelling, including instructions for use was conducted to determine if the complaint resulted from inadequacies in the product labelling or a failure by the user to adhere to the labelling. Note: labelling review alone is not sufficient as an investigation for the incident." .

imdrf:B32 a owl:Class ;
    rdfs:label "Analysis of Service/Maintenance Records" ;
    ex:status "New" ;
    ex:statusDescription "Term added for Release Number 2025. See no. 89 of Change Request Log" ;
    rdfs:comment "The investigation involved the analysis of the service history or maintenance records for the device involved." .

imdrf:C0101 a owl:Class ;
    rdfs:label "Biocompatibility Problem Identified" ;
    rdfs:comment "The device causes cellular or tissue responses that elicit an undesirable local or systemic effect in the recipient or beneficiary of that therapy. (See ISO 10993)" ;
    rdfs:subClassOf imdrf:C01 .

imdrf:C010201 a owl:Class ;
    rdfs:label "Endotoxin Contamination" ;
    rdfs:comment "The undesirable presence of toxins associated with certain bacteria (e.g. gram negative bacteria)." ;
    rdfs:subClassOf imdrf:C0102 .

imdrf:C010202 a owl:Class ;
    rdfs:label "Microbial Contamination" ;
    rdfs:comment "The undesirable presence of microorganisms or microbes such as bacteria and fungi (yeasts and molds)." ;
    rdfs:subClassOf imdrf:C0102 .

imdrf:C0103 a owl:Class ;
    rdfs:label "Material or Material Leachate Pyrogenic Problem" ;
    rdfs:comment "The undesirable presence of pyrogens or fever-producing organisms caused by materials that permeate through the device." ;
    rdfs:subClassOf imdrf:C01 .

imdrf:C0104 a owl:Class ;
    rdfs:label "Cytotoxicity Problem Identified" ;
    rdfs:comment "The device was found to have an undesirable level of toxicity to living cells." ;
    rdfs:subClassOf imdrf:C01 .

imdrf:C010501 a owl:Class ;
    rdfs:label "Carcinogenic Problem" ;
    rdfs:comment "The device's ability to trigger development of cancer." ;
    rdfs:subClassOf imdrf:C0105 .

imdrf:C010502 a owl:Class ;
    rdfs:label "Mutagenic Problem" ;
    rdfs:comment "The device's ability to change genetic information (usually DNA) of an organism and thus increasing the frequency of mutations." ;
    rdfs:subClassOf imdrf:C0105 .

imdrf:C010601 a owl:Class ;
    rdfs:label "Agglutination Problem" ;
    rdfs:comment "The device affects the ability of the blood to clot which may be induced by chemical, mechanical, or thermal properties of the device." ;
    rdfs:subClassOf imdrf:C0106 .

imdrf:C010602 a owl:Class ;
    rdfs:label "Complement Activation Problem" ;
    rdfs:comment "The device affects the body's ability to activate the complement system of the immune system, thereby interfering with the ability to clear pathogens. This may be caused by an interaction of the device with chemicals or materials." ;
    rdfs:subClassOf imdrf:C0106 .

imdrf:C010603 a owl:Class ;
    rdfs:label "Platelet Activation Problem" ;
    rdfs:comment "The device affects the body's ability to activate platelet formation." ;
    rdfs:subClassOf imdrf:C0106 .

imdrf:C010604 a owl:Class ;
    rdfs:label "Problem due to Thrombosis Activation" ;
    rdfs:comment "The device causes the formation of blood clots in or along blood vessels resulting in disturbed or disrupted blood flow." ;
    rdfs:subClassOf imdrf:C0106 .

imdrf:C0107 a owl:Class ;
    rdfs:label "Unintended Presence of Allergens" ;
    rdfs:comment "Unintended or unexpected presence of allergens in the device. If the presence of the allergen is expected but not adequately labelled, then use \"Labelling Problem\"." ;
    rdfs:subClassOf imdrf:C01 .

imdrf:C0108 a owl:Class ;
    rdfs:label "Reproductive Toxicity Problem Identified" ;
    rdfs:comment "The device affects reproductive function, embryo development (teratogenicity), and prenatal and early postnatal development. (ISO 10993 part 3)" ;
    rdfs:subClassOf imdrf:C01 .

imdrf:C0109 a owl:Class ;
    rdfs:label "Undesirable Presence of Endogenous Materials" ;
    ex:statusDescription "Term was added on 31 January 2023. For details, see comment No. 61 and No. 64 of the Change Log (Release Number 2023)." ;
    rdfs:comment "Undesirable presence of endogenous substances, body fluids, cellular tissues, etc." ;
    rdfs:subClassOf imdrf:C01 .

imdrf:C0201 a owl:Class ;
    rdfs:label "Electrical/Electronic Component Problem Identified" ;
    rdfs:comment "The performance of an electrical or electronic component was found to be inadequate." ;
    rdfs:subClassOf imdrf:C02 .

imdrf:C0202 a owl:Class ;
    rdfs:label "Hardware Timing Problem Identified" ;
    rdfs:comment "Problems that results from improper sequential activation of components." ;
    rdfs:subClassOf imdrf:C02 .

imdrf:C0203 a owl:Class ;
    rdfs:label "Impedance Problem Identified" ;
    rdfs:comment "Problems due to insufficient or excessive resistance to current flow either by the device or circuit." ;
    rdfs:subClassOf imdrf:C02 .

imdrf:C0204 a owl:Class ;
    rdfs:label "Insulation Problem Identified" ;
    rdfs:comment "Problems due to inadequate or incorrect electrical insulation material." ;
    rdfs:subClassOf imdrf:C02 .

imdrf:C0205 a owl:Class ;
    rdfs:label "Open Circuit" ;
    rdfs:comment "Problem due to an electrical circuit that does not conduct current because a switch is open, a wire is broken, etc." ;
    rdfs:subClassOf imdrf:C02 .

imdrf:C0206 a owl:Class ;
    rdfs:label "Current Leakage Problem" ;
    rdfs:comment "Problems related to leakage currents which may cause electric shock. These currents usually flow through the protective ground conductor. In its absence, these currents could flow from the device to the ground via the human body." ;
    rdfs:subClassOf imdrf:C02 .

imdrf:C020701 a owl:Class ;
    rdfs:label "Energy Storage System Problem" ;
    rdfs:comment "Problems related to the energy storage system (e.g. the rechargeable battery, charging system, or capacitor) and includes problems such as premature power source depletion and battery explosions." ;
    rdfs:subClassOf imdrf:C0207 .

imdrf:C020702 a owl:Class ;
    rdfs:label "Loss of Power Identified" ;
    ex:status "Modified (editorial)" ;
    ex:statusDescription "Term modified for Release Number 2025. Previous term was \"Loss of Power\". See no. 126 of Change Request Log." ;
    rdfs:comment "A device that experienced problems due to a loss in the power supply." ;
    rdfs:subClassOf imdrf:C0207 .

imdrf:C020703 a owl:Class ;
    rdfs:label "Power Fluctuation" ;
    rdfs:comment "The device failed due to fluctuations within the power supply (e.g. transient power, power spike, power dip, or power sequencing)." ;
    rdfs:subClassOf imdrf:C0207 .

imdrf:C0208 a owl:Class ;
    rdfs:label "Short Circuit" ;
    rdfs:comment "Problems due to an unintentionally low-resistance connection between two points in an electric circuit, resulting in either excessive current flow that often causes damage or in a new shorter circuit that draws current away from the original pathways and components." ;
    rdfs:subClassOf imdrf:C02 .

imdrf:C0209 a owl:Class ;
    rdfs:label "Signal Loss" ;
    rdfs:comment "Problems due to the loss or weakening of an electrical signal or signals." ;
    rdfs:subClassOf imdrf:C02 .

imdrf:C0210 a owl:Class ;
    rdfs:label "Corrupted memory" ;
    ex:statusDescription "Term was added on 31 January 2023. For details, see comment No. 60 of the Change Log (Release Number 2023)." ;
    rdfs:comment "Malfunction that resulted from a device memory corruption, including bit flips or single event errors." ;
    rdfs:subClassOf imdrf:C02 .

imdrf:C0301 a owl:Class ;
    rdfs:label "Conducted Interference" ;
    rdfs:comment "Problems related to electromagnetic interference (EMI) by physical contact with conductors (e.g. wires, resistors, terminals) as opposed to radiated EMI which is caused by induction (without physical contact of the conductors)." ;
    rdfs:subClassOf imdrf:C03 .

imdrf:C0302 a owl:Class ;
    rdfs:label "Electrostatic Discharge Identified" ;
    ex:status "Modified (editorial)" ;
    ex:statusDescription "Term modified for Release Number 2025. Previous term was \"Electrostatic Discharge\". See no. 140 of Change Request Log." ;
    rdfs:comment "Problems due to sudden and momentary bursts of electrical current flowing between two objects at different electrical potentials." ;
    rdfs:subClassOf imdrf:C03 .

imdrf:C0303 a owl:Class ;
    rdfs:label "Inadequate Immunity" ;
    rdfs:comment "Problems related to immunity or capabilities to resist electromagnetic interference (EMI)." ;
    rdfs:subClassOf imdrf:C03 .

imdrf:C0304 a owl:Class ;
    rdfs:label "Unintended Emission" ;
    rdfs:comment "Problems due to unintended emission of electromagnetic energy by the device." ;
    rdfs:subClassOf imdrf:C03 .

imdrf:C0305 a owl:Class ;
    rdfs:label "Radiofrequency Interference (RFI) Identified" ;
    ex:status "Modified (editorial)" ;
    ex:statusDescription "Term modified for Release Number 2025. Previous term was \"Radiofrequency Interference (RFI)\". See no. 132 of Change Request Log." ;
    rdfs:comment "Problems due to radiofrequency interference. RFI is a disturbance that affects an electrical circuit due to either electromagnetic conduction or electromagnetic radiation emitted from an external source." ;
    rdfs:subClassOf imdrf:C03 .

imdrf:C040101 a owl:Class ;
    rdfs:label "Wired Communication Problem" ;
    rdfs:comment "Communications problems between devices within a wired system." ;
    rdfs:subClassOf imdrf:C0401 .

imdrf:C040102 a owl:Class ;
    rdfs:label "Wireless Communication Problem Identified" ;
    ex:status "Modified (editorial)" ;
    ex:statusDescription "Term modified for Release Number 2025. Previous term was \"Wireless Communication Problem\". See no. 138 of Change Request Log." ;
    rdfs:comment "Communications problems between devices within a wireless system." ;
    rdfs:subClassOf imdrf:C0401 .

imdrf:C040103 a owl:Class ;
    rdfs:label "Network Communication Problem" ;
    rdfs:comment "Communications problems between devices within a network system." ;
    rdfs:subClassOf imdrf:C0401 .

imdrf:C0402 a owl:Class ;
    rdfs:label "Incompatible Component/ Accessory" ;
    rdfs:comment "A device that malfunctions due to a component(s)/accessory that does not operate correctly and according to the device's specifications." ;
    rdfs:subClassOf imdrf:C04 .

imdrf:C0403 a owl:Class ;
    rdfs:label "Device Not Compatible With Another Device" ;
    rdfs:comment "A device that malfunctions due to being used in combination with, or in the presence of, another device." ;
    rdfs:subClassOf imdrf:C04 .

imdrf:C0404 a owl:Class ;
    rdfs:label "Unintended Compatibility Identified" ;
    ex:status "Modified (editorial)" ;
    ex:statusDescription "Term modified for Release Number 2025. Previous term was \"Unintended Compatibility\". See no. 136 of Change Request Log." ;
    rdfs:comment "The device was confirmed to be compatible with another device with which the device is intended to be incompatible." ;
    rdfs:subClassOf imdrf:C04 .

imdrf:C0501 a owl:Class ;
    rdfs:label "Inadequate Labelling and/or Instructions for Use" ;
    rdfs:comment "Inadequate information on the labels or in the instructions for use e.g. steps that are difficult to follow or that are missing." ;
    rdfs:subClassOf imdrf:C05 .

imdrf:C0502 a owl:Class ;
    rdfs:label "Incorrect Labeling and/or Instructions for Use" ;
    rdfs:comment "Missing, incorrect, or inappropriate information on the labels e.g. mislabeled contents or device labeling characteristics or package contents." ;
    rdfs:subClassOf imdrf:C05 .

imdrf:C0503 a owl:Class ;
    rdfs:label "Inadequate or Incorrect Instructions for Maintenance" ;
    rdfs:comment "Inadequate or incorrect information in the instructions for maintenance." ;
    rdfs:subClassOf imdrf:C05 .

imdrf:C0601 a owl:Class ;
    rdfs:label "Degradation Problem Identified" ;
    rdfs:comment "Problems that occur when the device becomes worn, weakened, corroded, or broken down due to processes such as aging, permeation, and corrosion." ;
    rdfs:subClassOf imdrf:C06 .

imdrf:C060201 a owl:Class ;
    rdfs:label "Improper Composition/ Concentration" ;
    rdfs:comment "Problems associated with the improper combination of materials or elements present in the device (e.g. improper composition of the materials of a capacitor)." ;
    rdfs:subClassOf imdrf:C0602 .

imdrf:C060202 a owl:Class ;
    rdfs:label "Improper Physical Structure" ;
    rdfs:comment "Problems related to the incorrect or inadequate arrangement of the parts, components, elements, or materials." ;
    rdfs:subClassOf imdrf:C0602 .

imdrf:C060203 a owl:Class ;
    rdfs:label "Molecular Structure Problem" ;
    rdfs:comment "Problems related to the presence of an inappropriate molecular geometry somewhere in the device (i.e. the spatial arrangement of atoms in a molecule and the chemical bonds that hold the atoms together)." ;
    rdfs:subClassOf imdrf:C0602 .

imdrf:C0603 a owl:Class ;
    rdfs:label "Inadequate Physicochemical Properties" ;
    rdfs:comment "Problems that occur due to the physicochemical properties." ;
    rdfs:subClassOf imdrf:C06 .

imdrf:C0604 a owl:Class ;
    rdfs:label "Incompatible Material" ;
    rdfs:comment "Problems that occur due to the incompatibility of materials that co-exist simultaneously as part of the device." ;
    rdfs:subClassOf imdrf:C06 .

imdrf:C0605 a owl:Class ;
    rdfs:label "Reactivity Problem Identified" ;
    rdfs:comment "Problems that occur due to the reactivity of materials (e.g. over-react or under-react)." ;
    rdfs:subClassOf imdrf:C06 .

imdrf:C0606 a owl:Class ;
    rdfs:label "Tolerance Stack-Up" ;
    rdfs:comment "Problems that result from a combination of specification variances of the components." ;
    rdfs:subClassOf imdrf:C06 .

imdrf:C0701 a owl:Class ;
    rdfs:label "Device Migration" ;
    rdfs:comment "A device that has moved from its original location due to external forces (e.g. stent or lead movement)." ;
    rdfs:subClassOf imdrf:C07 .

imdrf:C0702 a owl:Class ;
    rdfs:label "Friction Problem Identified" ;
    rdfs:comment "Problems caused by its surface coming in contact with another surface or fluid." ;
    rdfs:subClassOf imdrf:C07 .

imdrf:C0703 a owl:Class ;
    rdfs:label "Leakage/Seal" ;
    rdfs:comment "Problems caused by inadequate/broken seal within the device." ;
    rdfs:subClassOf imdrf:C07 .

imdrf:C0704 a owl:Class ;
    rdfs:label "Lubrication Problem Identified" ;
    rdfs:comment "Problems that occurred because of the presence of either too much or too little lubricant where required (e.g. connectors, leading to failure mechanisms such as corrosion)." ;
    rdfs:subClassOf imdrf:C07 .

imdrf:C0705 a owl:Class ;
    rdfs:label "Stiffness Problem Identified" ;
    rdfs:comment "Problems that occurred when its material is either too flexible/pliable or inflexible/rigid when in contact by an applied force." ;
    rdfs:subClassOf imdrf:C07 .

imdrf:C070601 a owl:Class ;
    rdfs:label "Deformation/Distortion Problem" ;
    ex:status "Modified (technical)" ;
    ex:statusDescription "Term and Definition modified for Release Number 2025. Previous term was \"Deformation Problem\". See no. 13 of Change Request Log." ;
    rdfs:comment "Problems caused by changes in the shape or size of the device due to an applied force. This can be a result of tensile forces (pulling), compressive forces, shear, bending, knotting, or torsion." ;
    rdfs:subClassOf imdrf:C0706 .

imdrf:C070602 a owl:Class ;
    rdfs:label "Fatigue Problem" ;
    rdfs:comment "Problems due to the weakening or breakdown of its material when subjected to stress or a series of repeated stresses." ;
    rdfs:subClassOf imdrf:C0706 .

imdrf:C070603 a owl:Class ;
    rdfs:label "Separation Problem" ;
    ex:status "Modified (technical)" ;
    ex:statusDescription "Term and Definition modified for Release Number 2025. Previous term was \"Fracture Problem\". See no. 15 of Change Request Log." ;
    rdfs:comment "Problems caused by the cut, tear, or fracture of a component, object, or material into two or more pieces including shear." ;
    rdfs:subClassOf imdrf:C0706 .

imdrf:C070604 a owl:Class ;
    rdfs:label "Mechanical Shock Problem" ;
    rdfs:comment "Problems caused by the sudden violent blow or collision to the whole device (e.g. by dropping)." ;
    rdfs:subClassOf imdrf:C0706 .

imdrf:C070605 a owl:Class ;
    rdfs:label "Vibration Problem" ;
    rdfs:comment "Problems caused by the constant rhythmic motion of the device, or something in the environment to which the device is exposed." ;
    rdfs:subClassOf imdrf:C0706 .

imdrf:C070606 a owl:Class ;
    rdfs:label "Wear Problem" ;
    rdfs:comment "Problems due to the premature or expected erosion of its material by use, deterioration, or change." ;
    rdfs:subClassOf imdrf:C0706 .

imdrf:C0707 a owl:Class ;
    rdfs:label "Incorrect Dimension" ;
    rdfs:comment "Problems caused by incorrect physical dimensions of the device or one of its parts" ;
    rdfs:subClassOf imdrf:C07 .

imdrf:C0708 a owl:Class ;
    rdfs:label "Blockage Identified" ;
    ex:statusDescription "Term was added on 31 January 2023. For details, see comment No. 45 of the Change Log (Release Number 2023)." ;
    rdfs:comment "Problems that occurred due to an obstruction or blockage." ;
    rdfs:subClassOf imdrf:C07 .

imdrf:C0801 a owl:Class ;
    rdfs:label "Optical Transmission Problem Identified" ;
    rdfs:comment "Problems with the device's ability to pass light energy." ;
    rdfs:subClassOf imdrf:C08 .

imdrf:C0802 a owl:Class ;
    rdfs:label "Light Source Problem Identified" ;
    rdfs:comment "Problems with the optical properties of a device such as diopter, glare, and irradiance or glistening." ;
    rdfs:subClassOf imdrf:C08 .

imdrf:C0901 a owl:Class ;
    rdfs:label "Gradient Induced Field Problem" ;
    rdfs:comment "Problems that result from the gradient-induced fields generated during radiologic procedures e.g. magnetic resonance imaging." ;
    rdfs:subClassOf imdrf:C09 .

imdrf:C0902 a owl:Class ;
    rdfs:label "Image Artifact" ;
    rdfs:comment "The unacceptable distortion of an image due to signal loss that may occur during a radiologic procedure such as magnetic resonance imaging." ;
    rdfs:subClassOf imdrf:C09 .

imdrf:C0903 a owl:Class ;
    rdfs:label "Magnetically-Induced Movement" ;
    rdfs:comment "Problems due to unintended or excessive movement created by the application of magnetic fields." ;
    rdfs:subClassOf imdrf:C09 .

imdrf:C0904 a owl:Class ;
    rdfs:label "Radiofrequency Induced Overheating" ;
    rdfs:comment "Problems due to unintended radiofrequency-induced temperature increase that can occur in the vicinity of the device." ;
    rdfs:subClassOf imdrf:C09 .

imdrf:C1001 a owl:Class ;
    rdfs:label "Configuration Issue" ;
    rdfs:comment "Problems due to change control or incorrect version, including regional requirements." ;
    rdfs:subClassOf imdrf:C10 .

imdrf:C100201 a owl:Class ;
    rdfs:label "Data Compression Error" ;
    rdfs:comment "Data was lost or corrupted during the operation of reducing storage space or communication bandwidth." ;
    rdfs:subClassOf imdrf:C1002 .

imdrf:C100202 a owl:Class ;
    rdfs:label "Incorrect Algorithm" ;
    rdfs:comment "The device software was found to implement an incorrect sequence of steps for a specific computation." ;
    rdfs:subClassOf imdrf:C1002 .

imdrf:C100203 a owl:Class ;
    rdfs:label "Incorrect Data Definition" ;
    rdfs:comment "The device software was found to contain errors in specifying or manipulating data items." ;
    rdfs:subClassOf imdrf:C1002 .

imdrf:C100204 a owl:Class ;
    rdfs:label "Interface Design Error" ;
    rdfs:comment "The device software was found to contain errors in the user interface (including usability problems) or the interfaces with other systems." ;
    rdfs:subClassOf imdrf:C1002 .

imdrf:C100205 a owl:Class ;
    rdfs:label "Non-Functional Defect" ;
    rdfs:comment "The device software contained software errors that did not impact its operation." ;
    rdfs:subClassOf imdrf:C1002 .

imdrf:C100206 a owl:Class ;
    rdfs:label "Software Timing Problem" ;
    rdfs:comment "Problems that results from the incorrect sequencing or activation of software modules." ;
    rdfs:subClassOf imdrf:C1002 .

imdrf:C1003 a owl:Class ;
    rdfs:label "Software Maintenance Problem Identified" ;
    rdfs:comment "The device software was not maintained/updated properly." ;
    rdfs:subClassOf imdrf:C10 .

imdrf:C1004 a owl:Class ;
    rdfs:label "Software Installation Problem Identified" ;
    rdfs:comment "The device software was not installed as per the specifications or failed to properly install." ;
    rdfs:subClassOf imdrf:C10 .

imdrf:C1005 a owl:Class ;
    rdfs:label "Software Requirement Error" ;
    rdfs:comment "The software requirements for the device are either incomplete, inadequate, or in conflict." ;
    rdfs:subClassOf imdrf:C10 .

imdrf:C1006 a owl:Class ;
    rdfs:label "Software Runtime Error" ;
    rdfs:comment "The device software failed during operation as a result of a coding error." ;
    rdfs:subClassOf imdrf:C10 .

imdrf:C1007 a owl:Class ;
    rdfs:label "Software Security Vulnerability" ;
    rdfs:comment "The device software failed to provide adequate authorization, access control, protection and accountability features." ;
    rdfs:subClassOf imdrf:C10 .

imdrf:C1008 a owl:Class ;
    rdfs:label "Erroneous Data Transfer" ;
    rdfs:comment "The device software fails to transfer the expected data within a system or to another device." ;
    rdfs:subClassOf imdrf:C10 .

imdrf:C1009 a owl:Class ;
    rdfs:label "Data Storage or Loss of Data" ;
    rdfs:comment "Storage of data was unsuccessful in total or in part." ;
    rdfs:subClassOf imdrf:C10 .

imdrf:C1010 a owl:Class ;
    rdfs:label "Artificial Intelligence Training/Validation Problem Identified" ;
    ex:statusDescription "Term was added on 27 January 2022. For details, see comment No. 11 of the Change Log (Release Number 2022)." ;
    rdfs:comment "Problem associated with the training and/or validation of artificial intelligence, including machine learning algorithms." ;
    rdfs:subClassOf imdrf:C10 .

imdrf:C1011 a owl:Class ;
    rdfs:label "Corrupt Software" ;
    ex:statusDescription "Term was added on 27 January 2022. For details, see comment No. 30 of the Change Log (Release Number 2022)." ;
    rdfs:comment "The device software becomes corrupted and results in device malfunction." ;
    rdfs:subClassOf imdrf:C10 .

imdrf:C1101 a owl:Class ;
    rdfs:label "Overheating Problem Identified" ;
    rdfs:comment "The device was found to become hotter than expected during operation. This applies to devices which are not intended to deliver heat. Use \"Excessive heating identified\" for devices which are intended to deliver heat during operation. Use \"Inadequate cooling identified\" if the overheating was related to a problem with a cooling system." ;
    rdfs:subClassOf imdrf:C11 .

imdrf:C1102 a owl:Class ;
    rdfs:label "Excessive Heating Identified" ;
    rdfs:comment "The device delivered more heat than intended or expected during operation. This applies to devices which are intended to deliver heat. Use \"Overheating problem identified\" for devices which are not intended to deliver heat during operation." ;
    rdfs:subClassOf imdrf:C11 .

imdrf:C1103 a owl:Class ;
    rdfs:label "Excessive Cooling Identified" ;
    rdfs:comment "The device cooled the patient or another device more than intended or expected during operation." ;
    rdfs:subClassOf imdrf:C11 .

imdrf:C1104 a owl:Class ;
    rdfs:label "Inadequate Cooling Identified" ;
    rdfs:comment "The device did not sufficiently cool the patient or another device during operation." ;
    rdfs:subClassOf imdrf:C11 .

imdrf:C1201 a owl:Class ;
    rdfs:label "Fail-safe Problem Identified" ;
    rdfs:comment "A system intended to prevent unsafe operation of the device did not operate correctly." ;
    rdfs:subClassOf imdrf:C12 .

imdrf:C1202 a owl:Class ;
    rdfs:label "Alarm System Problem Identified" ;
    rdfs:comment "A system intended to warn of a potentially unsafe condition did not operate correctly." ;
    rdfs:subClassOf imdrf:C12 .

imdrf:C1203 a owl:Class ;
    rdfs:label "Problem of Device to Self-Test" ;
    rdfs:comment "Malfunction of the device's self-test system." ;
    rdfs:subClassOf imdrf:C12 .

imdrf:C1204 a owl:Class ;
    rdfs:label "Problem to Auto Stop" ;
    rdfs:comment "An auto stop function of a device did not operate correctly." ;
    rdfs:subClassOf imdrf:C12 .

imdrf:C1205 a owl:Class ;
    rdfs:label "Premature Indicator Activation Identified" ;
    ex:status "Modified (editorial)" ;
    ex:statusDescription "Term modified for Release Number 2025. Previous term was \"Premature Indicator Activation\". See no. 130 of Change Request Log." ;
    rdfs:comment "A system intended to indicate the device status was triggered prematurely." ;
    rdfs:subClassOf imdrf:C12 .

imdrf:C1206 a owl:Class ;
    rdfs:label "Reset Problem Identified" ;
    ex:status "Modified (editorial)" ;
    ex:statusDescription "Term modified for Release Number 2025. Previous term was \"Reset Problem\". See no. 134 of Change Request Log." ;
    rdfs:comment "The device does not reset properly." ;
    rdfs:subClassOf imdrf:C12 .

imdrf:C1207 a owl:Class ;
    rdfs:label "Shielding Problem" ;
    rdfs:comment "Inadequate shielding of/by the device." ;
    rdfs:subClassOf imdrf:C12 .

imdrf:C1208 a owl:Class ;
    rdfs:label "Missing or Inadequate Safety Measures Identified" ;
    ex:status "Modified (editorial)" ;
    ex:statusDescription "Term modified for Release Number 2025. Previous term was \"Missing or Inadequate Safety Measures\". See no. 127 of Change Request Log." ;
    rdfs:comment "Safety measures are inadequately applied or missing." ;
    rdfs:subClassOf imdrf:C12 .

imdrf:C130101 a owl:Class ;
    rdfs:label "Device Incorrectly Cleaned During Reprocessing" ;
    rdfs:comment "The cleaning procedure is not followed correctly or used inappropriate cleaning materials." ;
    rdfs:subClassOf imdrf:C1301 .

imdrf:C130102 a owl:Class ;
    rdfs:label "Device Incorrectly Disinfected/Sterilised During Reprocessing" ;
    rdfs:comment "The disinfection/sterilization process was incorrect and/or the wrong products for disinfection/sterilization were used." ;
    rdfs:subClassOf imdrf:C1301 .

imdrf:C130103 a owl:Class ;
    rdfs:label "Device Incorrectly Assembled During Reprocessing" ;
    rdfs:comment "Incorrect assembly of the device following reprocessing." ;
    rdfs:subClassOf imdrf:C1301 .

imdrf:C1302 a owl:Class ;
    rdfs:label "Failure to Calibrate or Used Out of Calibration" ;
    ex:statusDescription "Term/definition was modified on 31 January 2023 (Old term/definition: Failure to Calibrate: A device that cannot calibrate (establish the relationship between a measuring device and the units of measure) to ensure accurate readings). For details, see comment No. 58 of the Change Log (Release Number 2023)." ;
    rdfs:comment "A device that cannot calibrate (establish the relationship between a measuring device and the units of measure) or is used out of calibration to ensure accurate readings." ;
    rdfs:subClassOf imdrf:C13 .

imdrf:C1303 a owl:Class ;
    rdfs:label "Device Difficult to Operate" ;
    rdfs:comment "Problems including set-up, operation, and disassembly of equipment. Not including reprocessing." ;
    rdfs:subClassOf imdrf:C13 .

imdrf:C1304 a owl:Class ;
    rdfs:label "Incorrect Interpretation of Results/Data" ;
    rdfs:comment "Problems resulting from the incorrect interpretation by the user of the results or data provided by the device." ;
    rdfs:subClassOf imdrf:C13 .

imdrf:C1401 a owl:Class ;
    rdfs:label "New or Unknown Interferent" ;
    rdfs:comment "New or unknown endogenous or exogenous interferent (sample) identified." ;
    rdfs:subClassOf imdrf:C14 .

imdrf:C1402 a owl:Class ;
    rdfs:label "Known Interferent" ;
    rdfs:comment "Known interferent in the sample identified." ;
    rdfs:subClassOf imdrf:C14 .

imdrf:C1403 a owl:Class ;
    rdfs:label "Problem Related to Variant/Mutant" ;
    ex:status "Modified (technical)" ;
    ex:statusDescription "Term and Definition modified for Release Number 2025. Previous term was \"Change in Target Marker/Variant/ Mutant\". See no. 56 of Change Request Log." ;
    rdfs:comment "Device performance affected by variant/mutant which is not covered in the labelling." ;
    rdfs:subClassOf imdrf:C14 .

imdrf:C1404 a owl:Class ;
    rdfs:label "Pre-analytical Handling Problem" ;
    rdfs:comment "Incorrect pre-analytical handling of patient's sample by the user." ;
    rdfs:subClassOf imdrf:C14 .

imdrf:C1501 a owl:Class ;
    rdfs:label "Environmental Temperature Problem Identified" ;
    rdfs:comment "Device performance was affected by the temperature, or changes in temperature, of the environment in which it was used." ;
    rdfs:subClassOf imdrf:C15 .

imdrf:C1502 a owl:Class ;
    rdfs:label "Contamination of Device by Foreign Material from Environment" ;
    ex:status "Modified (technical)" ;
    ex:statusDescription "Term and Definition modified for Release Number 2025. Previous term was \"Dust or Dirt Problem Identified\". See no. 14 of Change Request Log." ;
    rdfs:comment "A device that experienced problems due to ingress or coating of dust, dirt or other foreign material" ;
    rdfs:subClassOf imdrf:C15 .

imdrf:C1503 a owl:Class ;
    rdfs:label "Contamination of Environment by Device" ;
    rdfs:comment "Operation of the device results in contamination of the nearby environment e.g. dust, dirt, smoke, heat or biological material." ;
    rdfs:subClassOf imdrf:C15 .

imdrf:C1504 a owl:Class ;
    rdfs:label "Environmental Pressure Problem Identified" ;
    rdfs:comment "Device performance was affected by the pressure, or changes in pressure, of the environment in which it was used." ;
    rdfs:subClassOf imdrf:C15 .

imdrf:C1505 a owl:Class ;
    rdfs:label "Ambient Light Problem Identified" ;
    rdfs:comment "Device performance was affected by ambient light. This term applies to the direct effects of ambient light on the device, and to the user's ability to operate the device (e.g. to read device output)." ;
    rdfs:subClassOf imdrf:C15 .

imdrf:C1506 a owl:Class ;
    rdfs:label "Environmental Humidity Problem Identified" ;
    rdfs:comment "Device performance was affected by the humidity, or changes in humidity, of the environment in which it was used." ;
    rdfs:subClassOf imdrf:C15 .

imdrf:C1601 a owl:Class ;
    rdfs:label "Assembly Problem Identified" ;
    rdfs:comment "Problems that occurred because the device was assembled incorrectly." ;
    rdfs:subClassOf imdrf:C16 .

imdrf:C1602 a owl:Class ;
    rdfs:label "Sterilization Problem Identified" ;
    rdfs:comment "Problems that occurred during terminal sterilization by the manufacturer." ;
    rdfs:subClassOf imdrf:C16 .

imdrf:C1603 a owl:Class ;
    rdfs:label "Installation Problem Identified" ;
    rdfs:comment "A device that malfunctions because it was incorrectly installed, set-up, or configured (e.g. misconfiguration of an \"automatic\" defibrillator to \"semi-automatic\", thereby leading to failure)." ;
    rdfs:subClassOf imdrf:C16 .

imdrf:C1604 a owl:Class ;
    rdfs:label "Maintenance of Manufacturing Machinery" ;
    rdfs:comment "Problems caused by failure to maintain manufacturing equipment used to produce the device." ;
    rdfs:subClassOf imdrf:C16 .

imdrf:C160501 a owl:Class ;
    rdfs:label "Packaging Compromised" ;
    rdfs:comment "Problems that occurred because of a compromised packaging of the device (e.g. broken or incomplete seal)." ;
    rdfs:subClassOf imdrf:C1605 .

imdrf:C160502 a owl:Class ;
    rdfs:label "Packaging Materials Problem" ;
    rdfs:comment "Problems that occurred because of the composition or type of packaging materials was inappropriate for the device." ;
    rdfs:subClassOf imdrf:C1605 .

imdrf:C160503 a owl:Class ;
    rdfs:label "Packaging Contains Unintended Material" ;
    rdfs:comment "Problems that occurred because unintended material was packaged with the device." ;
    rdfs:subClassOf imdrf:C1605 .

imdrf:C160504 a owl:Class ;
    rdfs:label "Packaging Contains Incorrect or Incomplete Device" ;
    ex:statusDescription "Term/definition was modified on 31 January 2023 (Old term/definition: Packaging Contains Incorrect Device: Problems that occurred because the packaging contained an incorrect device.). For details, see comment No. 51 of the Change Log (Release Number 2023)." ;
    rdfs:comment "Problems that occurred because the packaging contained an incorrect or incomplete device (missing components)." ;
    rdfs:subClassOf imdrf:C1605 .

imdrf:C1701 a owl:Class ;
    rdfs:label "Misadjustment/misalignment identified" ;
    ex:statusDescription "Term added for Release Number 2024. See no. 49 of Change Log." ;
    rdfs:comment "Problems caused by incorrect adjustment of device components." ;
    rdfs:subClassOf imdrf:C17 .

imdrf:C1801 a owl:Class ;
    rdfs:label "Transport Problem Identified" ;
    rdfs:comment "Problems traced to how the device was transported e.g. temperature of shipping compartment or method of transportation." ;
    rdfs:subClassOf imdrf:C18 .

imdrf:C1802 a owl:Class ;
    rdfs:label "Storage Problem Identified" ;
    rdfs:comment "Problems that result from storing the device in an uncontrolled or improper environment (e.g. moisture sensitive devices stored in a humid environment)." ;
    rdfs:subClassOf imdrf:C18 .

imdrf:C19 a owl:Class ;
    rdfs:label "No Device Problem Found" ;
    ex:statusDescription "Definition of this term was clarified on 21 January 2021. For details, refer to comment No. 17 and 29 of the Change Log. (Old definition: \"The device either functioned as intended or a problem was not found.\")" ;
    rdfs:comment "Reported problem cannot be reproduced during investigation." .

imdrf:C20 a owl:Class ;
    rdfs:label "No Findings Available" ;
    rdfs:comment "Use when no investigation can be performed and therefore no results will be obtained." .

imdrf:C21 a owl:Class ;
    rdfs:label "Results Pending Completion of Investigation" ;
    rdfs:comment "Investigation is ongoing and results are not yet available. Do not use this code if the investigation is complete." .

imdrf:C22 a owl:Class ;
    rdfs:label "Appropriate Investigation Findings Term/Code Not Available" ;
    ex:status "Modified (editorial)" ;
    ex:statusDescription "Term modified for Release Number 2025. Previous term was \"Appropriate Term/Code Not Available\". See no. 108 of Change Request Log." ;
    rdfs:comment "Problems is not adequately described by any other term. Note: This code must not be used unless there is no other feasible code. The preferred term should be documented when submitting an adverse event report. This information will be used to determine if a new term should be added to the code table." .

imdrf:C2301 a owl:Class ;
    rdfs:label "Insufficient Sample Volume" ;
    ex:statusDescription "Term was added on 31 January 2023.  For details, see comment No. 53 of the Change Log (Release Number 2023)." ;
    rdfs:comment "Not having a sufficient volume of sample to perform a test." ;
    rdfs:subClassOf imdrf:C23 .

imdrf:C2302 a owl:Class ;
    rdfs:label "Use of Non-Validated Controls Identified" ;
    ex:statusDescription "Term was added on 31 January 2023.  For details, see comment No. 57 of the Change Log (Release Number 2023)." ;
    rdfs:comment "Problems that occur related to the use of non-validated controls." ;
    rdfs:subClassOf imdrf:C23 .

imdrf:C24 a owl:Class ;
    rdfs:label "Malfunction Observed Without Conclusive Finding" ;
    ex:statusDescription "Term was added on 31 January 2023.  For details, see comment No. 62 of the Change Log (Release Number 2023)." ;
    rdfs:comment "Malfunction was verified but no conclusive finding is available." .

imdrf:D0101 a owl:Class ;
    rdfs:label "Design Inadequate for Purpose" ;
    rdfs:comment "Problems traced to design/design features of the device that do not support or interfere with the intended purpose of the device." ;
    rdfs:subClassOf imdrf:D01 .

imdrf:D0102 a owl:Class ;
    rdfs:label "Human Factors Engineering - Device Difficult to Operate" ;
    rdfs:comment "Problems traced to inappropriate and/or inadequate assessment and engineering design of the device to accommodate how or where the device will be used." ;
    rdfs:subClassOf imdrf:D01 .

imdrf:D0103 a owl:Class ;
    rdfs:label "Human Factors Engineering - Device Difficult to Assemble" ;
    rdfs:comment "Problems traced to inadequate design of the component parts and/or assembly steps resulting in the device not being able to be assembled correctly." ;
    rdfs:subClassOf imdrf:D01 .

imdrf:D0104 a owl:Class ;
    rdfs:label "Human Factors Engineering - Device Difficult to Reprocess" ;
    rdfs:comment "Problems traced to inadequate design of the reprocessing steps and/or the device resulting in the device remaining unclean." ;
    rdfs:subClassOf imdrf:D01 .

imdrf:D0105 a owl:Class ;
    rdfs:label "Cause Traced to Missing or Inadequate Safety Measures" ;
    ex:status "Modified (editorial)" ;
    ex:statusDescription "Editorial change to term for Release Number 2025. See no. 128 of Change Log." ;
    rdfs:comment "Problems traced to inadequate design or complete lack of safety measures leading to device malfunction or unintended properties of the device including possible hazards for persons using the device." ;
    rdfs:subClassOf imdrf:D01 .

imdrf:D0106 a owl:Class ;
    rdfs:label "Design Change Validation Inadequate" ;
    rdfs:comment "Problems traced to inadequate or lack of validation of design changes of the device leading to malfunction or unintended properties of the device including possible hazards for persons using the device." ;
    rdfs:subClassOf imdrf:D01 .

imdrf:D0107 a owl:Class ;
    rdfs:label "Inadequate Cybersecurity" ;
    ex:statusDescription "New term/definition added on 21 January 2021. for details, refer to comment No. 26 of the Change Log." ;
    rdfs:comment "Problems traced to inadequate protection of computers, servers, mobile devices, electronic systems, networks, programs, and data from malicious attacks, damage, or unauthorized access." ;
    rdfs:subClassOf imdrf:D01 .

imdrf:D0108 a owl:Class ;
    rdfs:label "Inadequate Software Design." ;
    ex:statusDescription "New term/definition added on 21 January 2021. for details, refer to comment No. 27 of the Change Log." ;
    rdfs:comment "Cause traced to inadequate or inappropriate design of the software component of a medical device, or Software as a Medical Device." ;
    rdfs:subClassOf imdrf:D01 .

imdrf:D02 a owl:Class ;
    rdfs:label "Cause Traced to Component Failure" ;
    rdfs:comment "Expected or random component failure without any design or manufacturing issue." .

imdrf:D0301 a owl:Class ;
    rdfs:label "Manufacturing Deficiency" ;
    rdfs:comment "Problems traced to manufacturing process." ;
    rdfs:subClassOf imdrf:D03 .

imdrf:D0302 a owl:Class ;
    rdfs:label "Quality Control Deficiency" ;
    ex:statusDescription "Definition modified for Release Number 2024. See no. 55 of Change Log" ;
    rdfs:comment "Problems traced to the failure to maintain or establish techniques for controlling and verifying the product specifications identified by the manufacturer.  Includes inadequacy of components or raw materials supplied to the manufacturer." ;
    rdfs:subClassOf imdrf:D03 .

imdrf:D04 a owl:Class ;
    rdfs:label "Cause Traced to Transport/Storage" ;
    rdfs:comment "Problems traced to the inappropriate transport or storage of the device." .

imdrf:D05 a owl:Class ;
    rdfs:label "Cause Traced to Infrastructure" ;
    rdfs:comment "Problems traced to underlying framework, systems, and processes at the healthcare facility or other point of use (e.g. as building power supply, network, oxygen systems)." .

imdrf:D06 a owl:Class ;
    rdfs:label "Cause Traced to Environment" ;
    rdfs:comment "Problems caused by exposure to environmental conditions outside the expected range." .

imdrf:D07 a owl:Class ;
    rdfs:label "Cause Traced to Maintenance" ;
    rdfs:comment "Problems traced to improper routine or preventative maintenance." .

imdrf:D08 a owl:Class ;
    rdfs:label "Cause Traced to Training" ;
    rdfs:comment "Problems caused by inadequate training." .

imdrf:D09 a owl:Class ;
    rdfs:label "Cause Traced to Labeling" ;
    rdfs:comment "Problems that occur as the result of problems with the labeling (including package inserts, instruction manuals, instructions for use)." .

imdrf:D1001 a owl:Class ;
    rdfs:label "Adverse Event Related to Patient Anatomy and/or Condition" ;
    ex:status "Modified (technical)" ;
    ex:statusDescription "Term and Definition modified for Release Number 2025. Previous term was \"Adverse Event Related to Patient Condition\". See no. 53 of Change Request Log." ;
    rdfs:comment "The patient's condition, disease or anatomy is demonstrably responsible for the adverse event and use of the device has neither caused nor otherwise influenced the adverse event." ;
    rdfs:subClassOf imdrf:D10 .

imdrf:D1002 a owl:Class ;
    rdfs:label "Adverse Event Related to Procedure" ;
    rdfs:comment "The adverse event occurred during the procedure and the device had no influence on event." ;
    rdfs:subClassOf imdrf:D10 .

imdrf:D1003 a owl:Class ;
    rdfs:label "Adverse Event Related to Commutability" ;
    rdfs:comment "The adverse event occurred because the material being used to calibrate or assess IVD performance did not have similar properties to those of human samples, leading to inappropriate bias and erroneous results. Examples of materials include: reference materials, calibrators, proficiency testing samples." ;
    rdfs:subClassOf imdrf:D10 .

imdrf:D1101 a owl:Class ;
    rdfs:label "Failure To Follow Instructions" ;
    rdfs:comment "Problems traced to the user not following the manufacturer's instructions." ;
    rdfs:subClassOf imdrf:D11 .

imdrf:D1102 a owl:Class ;
    rdfs:label "Unintended Use Error Caused or Contributed to Event" ;
    rdfs:comment "The interaction between the user and device, or sample, caused or contributed to the error. This includes unintended inappropriate use of the device and incorrect sample preparation." ;
    rdfs:subClassOf imdrf:D11 .

imdrf:D1103 a owl:Class ;
    rdfs:label "Cause Traced to Intentional Off-Label, Unapproved, or Contraindicated Use" ;
    rdfs:comment "Problems traced to the intentional use of the device in an unapproved procedure, for an unapproved patient, or for which it is contraindicated, or not listed on the label." ;
    rdfs:subClassOf imdrf:D11 .

imdrf:D1104 a owl:Class ;
    rdfs:label "Shelf Life/Expiration Date Exceeded" ;
    rdfs:comment "A device that has exceeded the period of time/date recommended by the manufacturer for storing the device without a degradation in quality." ;
    rdfs:subClassOf imdrf:D11 .

imdrf:D1105 a owl:Class ;
    rdfs:label "End of Life Problem Identified" ;
    rdfs:comment "Problems traced to the device reaching the end of its useful life." ;
    rdfs:subClassOf imdrf:D11 .

imdrf:D1106 a owl:Class ;
    rdfs:label "Reuse of Single Use Device" ;
    rdfs:comment "Problems traced to the use of the device more than once when it is designed for only one use." ;
    rdfs:subClassOf imdrf:D11 .

imdrf:D1107 a owl:Class ;
    rdfs:label "Sabotage or Intentional Misuse" ;
    ex:statusDescription "Editorial change to the definition on 16 February 2021." ;
    rdfs:comment "Problems occurred because of willful damage or reckless misuse. This term indicates that there was an apparent intent to cause damage or injury." ;
    rdfs:subClassOf imdrf:D11 .

imdrf:D1108 a owl:Class ;
    rdfs:label "Reasonably Foreseeable Misuse" ;
    ex:statusDescription "Term was added on 27 January 2022. For details, see comment No. 10 of the Change Log (Release Number 2022)." ;
    rdfs:comment "Problems related to the use of a device in a way not intended in the instructions for use, but which may result from readily predictable human behavior." ;
    rdfs:subClassOf imdrf:D11 .

imdrf:D12 a owl:Class ;
    rdfs:label "Known Inherent Risk of Device" ;
    ex:statusDescription "The definition was modified on 21 January 2021 (addition of phrase \"and all reasonable mitigation steps have been taken.\"). For details, refer to comment No. 31 of the Change Log." ;
    rdfs:comment "Reported adverse event known and documented in the labeling and all reasonable mitigation steps have been taken (including both short or long term known complications or adverse reactions)." .

imdrf:D13 a owl:Class ;
    rdfs:label "Falsified Device" ;
    rdfs:comment "Devices that deliberately and/or fraudulently misrepresent their identity, composition or source." .

imdrf:D1401 a owl:Class ;
    rdfs:label "Unable to exclude device problem" ;
    ex:statusDescription "Term added for Release Number 2024. See no. 54 of Change Log" ;
    rdfs:comment "The investigation findings do not clearly confirm the presence or absence of the reported problem with the device." ;
    rdfs:subClassOf imdrf:D14 .

imdrf:D1402 a owl:Class ;
    rdfs:label "Device problem excluded" ;
    ex:statusDescription "Term added for Release Number 2024. See no. 54 of Change Log" ;
    rdfs:comment "The investigation findings clearly confirm that there was no problem with the device." ;
    rdfs:subClassOf imdrf:D14 .

imdrf:D1501 a owl:Class ;
    rdfs:label "Cause Linked to Device but Unable to Trace More Specifically" ;
    ex:statusDescription "New term/definition added on 21 January 2021. for details, refer to comment No. 30 of the Change Log." ;
    rdfs:comment "Problems traced to the device, but the investigation could not identify the actual root cause (e.g. Design, Manufacturing, Component)." ;
    rdfs:subClassOf imdrf:D15 .

imdrf:D16 a owl:Class ;
    rdfs:label "Conclusion Not Yet Available" ;
    rdfs:comment "A conclusion has yet to be established as the investigation is incomplete. Do not use this code if the investigation is complete." .

imdrf:D17 a owl:Class ;
    rdfs:label "Appropriate Investigation Conclusion Term/Code Not Available" ;
    ex:status "Modified (editorial)" ;
    ex:statusDescription "Editorial change to term for Release Number 2025. See no. 109 of Change Log." ;
    rdfs:comment "The concluded cause is not adequately described by any other term. Note: This code must not be used unless there is no other feasible code. The preferred term should be documented when submitting an adverse event report. This information will be used to determine if a new term should be added to the code table." .

imdrf:D18 a owl:Class ;
    rdfs:label "Cause Traced to Software Coding" ;
    ex:statusDescription "New term/definition added on 21 January 2021. for details, refer to comment No. 27 of the Change Log." ;
    rdfs:comment "Problems traced to an error, flaw or fault in a computer program or system that causes it to produce an incorrect or unexpected result, or to behave in unintended ways." .

imdrf:D19 a owl:Class ;
    rdfs:label "Cause Traced to Artificial Intelligence Training/Validation Process" ;
    ex:statusDescription "Term was added on 27 January 2022. For details, see comment No. 12 of the Change Log (Release Number 2022)." ;
    rdfs:comment "Problem traced to the process or dataset(s) used for training and/or validating artificial intelligence, including machine learning algorithms." .

imdrf:D20 a owl:Class ;
    rdfs:label "Cause Traced to Another Device" ;
    ex:statusDescription "Term was added on 31 January 2023. For details, see comment No. 75 of the Change Log (Release Number 2023)." ;
    rdfs:comment "Problem is traced to be caused by another device." .

imdrf:D21 a owl:Class ;
    rdfs:label "Cause Traced to Health Disparity" ;
    ex:statusDescription "Term was added on 31 January 2023. For details, see comment No. 142 of the Change Log (Release Number 2023)." ;
    rdfs:comment "Problems traced to device performing inadequately or inconsistently in people with certain equality characteristics (e.g. sex, racial or ethnic origin)." .

imdrf:E0101 a owl:Class ;
    rdfs:label "Balance Problems" ;
    ex:nonIMDRFCode "MedDRA:10049848:Balance disorder" ;
    rdfs:comment "A feeling of falling down which can occur whether the person is standing, sitting or lying down." ;
    rdfs:subClassOf imdrf:E01 .

imdrf:E010201 a owl:Class ;
    rdfs:label "Encephalocele" ;
    ex:nonIMDRFCode "MedDRA:10014617:Encephalocele" ;
    rdfs:comment "Hernia of brain substance and meninges through a congenital or traumatic opening of the skull." ;
    rdfs:subClassOf imdrf:E0102 .

imdrf:E0103 a owl:Class ;
    rdfs:label "Cerebral Edema" ;
    ex:nonIMDRFCode "MedDRA:10008107:Cerebral edema" ;
    rdfs:comment "A swelling in the brain caused by the presence of excessive fluid." ;
    rdfs:subClassOf imdrf:E01,
        imdrf:E2338 .

imdrf:E0104 a owl:Class ;
    rdfs:label "Cerebral Hyperperfusion Syndrome" ;
    ex:nonIMDRFCode "MedDRA:10064730:Cerebral hyperperfusion syndrome" ;
    rdfs:comment "Unexpected increase in cerebral blood flow after carotid endarterectomy (CEA) or carotid artery stenting (CAS)." ;
    rdfs:subClassOf imdrf:E01,
        imdrf:E05 .

imdrf:E0105 a owl:Class ;
    rdfs:label "Cerebral Ventriculomegaly" ;
    ex:nonIMDRFCode "MedDRA:10068352:Cerebral ventriculomegaly" ;
    ex:statusDescription "Term was modified on 21 January 2021 (old term: Cerebral Ventriculomeglia)." ;
    rdfs:comment "Abnormal enlargement of the cerebral ventricles." ;
    rdfs:subClassOf imdrf:E01 .

imdrf:E0106 a owl:Class ;
    rdfs:label "Cerebrospinal Fluid Leakage" ;
    ex:nonIMDRFCode "MedDRA:10008164:Cerebrospinal fluid leakage" ;
    ex:statusDescription "Definition modified for Release Number 2024. See no. 6 of Change Log" ;
    rdfs:comment "The loss of cerebrospinal fluid into the surrounding tissues or outside the body." ;
    rdfs:subClassOf imdrf:E01 .

imdrf:E010701 a owl:Class ;
    rdfs:label "Confusion/ Disorientation" ;
    ex:nonIMDRFCode "MedDRA:10010300:Confusion" ;
    rdfs:comment "A mental state characterized by a lack of clear and orderly thought and behavior." ;
    rdfs:subClassOf imdrf:E0107 .

imdrf:E010702 a owl:Class ;
    rdfs:label "Dementia" ;
    ex:nonIMDRFCode "MedDRA:10012267:Dementia" ;
    rdfs:comment "Loss of intellectual abilities interfering with an individual's social and occupational functions." ;
    rdfs:subClassOf imdrf:E0107 .

imdrf:E0108 a owl:Class ;
    rdfs:label "Concussion" ;
    ex:nonIMDRFCode "MedDRA:10010254:Concussion" ;
    rdfs:comment "Traumatic brain injury as a result of the action of a mechanical force on the head." ;
    rdfs:subClassOf imdrf:E01,
        imdrf:E20 .

imdrf:E010901 a owl:Class ;
    rdfs:label "Convulsion, Clonic" ;
    ex:nonIMDRFCode "MedDRA:10053398:Clonic convulsion" ;
    rdfs:comment "A convulsion marked by alternating contracting and relaxing of the muscles." ;
    rdfs:subClassOf imdrf:E0109 .

imdrf:E010902 a owl:Class ;
    rdfs:label "Convulsion, Tonic" ;
    ex:nonIMDRFCode "MedDRA:10043994:Tonic convulsion" ;
    rdfs:comment "A convulsion marked by prolonged contraction of the muscles." ;
    rdfs:subClassOf imdrf:E0109 .

imdrf:E010903 a owl:Class ;
    rdfs:label "Epilepsy" ;
    ex:nonIMDRFCode "MedDRA:10015037:Epilepsy" ;
    rdfs:comment "Epilepsy caused or apparently caused by device. Do not use when epilepsy is a pre-existing condition." ;
    rdfs:subClassOf imdrf:E0109 .

imdrf:E010904 a owl:Class ;
    rdfs:label "Status Epilepticus" ;
    ex:nonIMDRFCode "MedDRA:10041962:Status epilepticus" ;
    ex:statusDescription "Editorial change to the definition on 16 February 2021." ;
    rdfs:comment "A life-threatening condition characterised by a single prolonged seizure or a series of seizures without intervening full recovery of consciousness." ;
    rdfs:subClassOf imdrf:E0109 .

imdrf:E0110 a owl:Class ;
    rdfs:label "Hyporesponsive to stimuli" ;
    ex:nonIMDRFCode "MedDRA:10071552:Hyporesponsive to stimuli" ;
    ex:status "Modified (editorial)" ;
    ex:statusDescription "Term and Definition modified for Release Number 2025. Previous term was \"Decreased Sensitivity\". See no. 115 of Change Request Log." ;
    rdfs:comment "Decreased sensitivity affecting one or more senses" ;
    rdfs:subClassOf imdrf:E01 .

imdrf:E0111 a owl:Class ;
    rdfs:label "Hyperresponsive to stimuli" ;
    ex:nonIMDRFCode "MedDRA:10082489:Hyperresponsive to stimuli" ;
    ex:status "Modified (editorial)" ;
    ex:statusDescription "Term and Definition modified for Release Number 2025. Previous term was \"Increased Sensitivity\". See no. 119 of Change Request Log." ;
    rdfs:comment "Increased sensitivity affecting one or more senses" ;
    rdfs:subClassOf imdrf:E01 .

imdrf:E0112 a owl:Class ;
    rdfs:label "Dizziness" ;
    ex:nonIMDRFCode "MedDRA:10013573:Dizziness" ;
    rdfs:comment "A sensation of lightheadedness, unsteadiness, turning, spinning or rocking." ;
    rdfs:subClassOf imdrf:E01 .

imdrf:E011301 a owl:Class ;
    rdfs:label "Aphonia" ;
    ex:nonIMDRFCode "MedDRA:10002953:Aphonia" ;
    rdfs:comment "Inability to speak." ;
    rdfs:subClassOf imdrf:E0113 .

imdrf:E0114 a owl:Class ;
    rdfs:label "Encephalitis" ;
    ex:nonIMDRFCode "MedDRA:10014581:Encephalitis" ;
    rdfs:comment "An acute inflammatory process affecting the brain parenchyma." ;
    rdfs:subClassOf imdrf:E01,
        imdrf:E19 .

imdrf:E0115 a owl:Class ;
    rdfs:label "Encephalopathy" ;
    ex:nonIMDRFCode "MedDRA:10014625:Encephalopathy" ;
    ex:statusDescription "Editorial change to the definition on 16 February 2021." ;
    rdfs:comment "A functional and/or structural disorder of the brain that is acquired or congenital and characterised by mental and neurological symptoms." ;
    rdfs:subClassOf imdrf:E01 .

imdrf:E0116 a owl:Class ;
    rdfs:label "Headache" ;
    ex:nonIMDRFCode "MedDRA:10019211:Headache" ;
    rdfs:comment "Pain in various parts of the head, not confined to the area of distribution of any nerve." ;
    rdfs:subClassOf imdrf:E01,
        imdrf:E2330 .

imdrf:E0117 a owl:Class ;
    rdfs:label "Hydrocephalus" ;
    ex:nonIMDRFCode "MedDRA:10020508:Hydrocephalus" ;
    rdfs:comment "A disorder characterized by an abnormal increase of cerebrospinal fluid in the ventricles of the brain." ;
    rdfs:subClassOf imdrf:E01 .

imdrf:E0118 a owl:Class ;
    rdfs:label "Intracranial Hemorrhage" ;
    ex:nonIMDRFCode "MedDRA:10022763:Intracranial hemorrhage" ;
    rdfs:comment "Bleeding within the cranium." ;
    rdfs:subClassOf imdrf:E01 .

imdrf:E011901 a owl:Class ;
    rdfs:label "Coma" ;
    ex:nonIMDRFCode "MedDRA:10010071:Coma" ;
    rdfs:comment "A state of profound unconsciousness associated with markedly depressed cerebral activity." ;
    rdfs:subClassOf imdrf:E0119 .

imdrf:E011902 a owl:Class ;
    rdfs:label "Presyncope" ;
    ex:nonIMDRFCode "MedDRA:10036653:Presyncope" ;
    rdfs:comment "Extremely weak; threatened with syncope." ;
    rdfs:subClassOf imdrf:E0119 .

imdrf:E011903 a owl:Class ;
    rdfs:label "Syncope/Fainting" ;
    ex:nonIMDRFCode "MedDRA:10042772:Syncope" ;
    rdfs:comment "A spontaneous, transient, loss of consciousness caused by insufficient blood supply to the brain." ;
    rdfs:subClassOf imdrf:E0119 .

imdrf:E0120 a owl:Class ;
    rdfs:label "Memory Loss/Impairment" ;
    ex:nonIMDRFCode "MedDRA:10027176:Memory loss" ;
    rdfs:comment "Systematic and extensive loss or impairment of memory caused by organic or psychological factors. This may be temporary or permanent, and may involve old or recent memories." ;
    rdfs:subClassOf imdrf:E01 .

imdrf:E0121 a owl:Class ;
    rdfs:label "Meningitis" ;
    ex:nonIMDRFCode "MedDRA:10027199:Meningitis" ;
    rdfs:comment "A disorder characterized by acute inflammation of the meninges of the brain and/or spinal cord." ;
    rdfs:subClassOf imdrf:E01,
        imdrf:E19 .

imdrf:E012201 a owl:Class ;
    rdfs:label "Dyskinesia" ;
    ex:nonIMDRFCode "MedDRA:10013916:Dyskinesia" ;
    rdfs:comment "Difficulty moving; distortion or impairment of voluntary movement, as in tic, spasm, or myoclonus." ;
    rdfs:subClassOf imdrf:E0122 .

imdrf:E012202 a owl:Class ;
    rdfs:label "Paralysis" ;
    ex:nonIMDRFCode "MedDRA:10033799:Paralysis" ;
    rdfs:comment "Partial or complete loss of function of one or more muscles. It is usually caused by damage to the nervous system." ;
    rdfs:subClassOf imdrf:E0122 .

imdrf:E012203 a owl:Class ;
    rdfs:label "Paraplegia" ;
    ex:nonIMDRFCode "MedDRA:10033892:Paraplegia" ;
    rdfs:comment "Paralysis of the legs and lower part of the body." ;
    rdfs:subClassOf imdrf:E0122 .

imdrf:E012204 a owl:Class ;
    rdfs:label "Paresis" ;
    ex:nonIMDRFCode "MedDRA:10033985:Paresis" ;
    rdfs:comment "A slight or incomplete paralysis." ;
    rdfs:subClassOf imdrf:E0122 .

imdrf:E012205 a owl:Class ;
    rdfs:label "Quadriplegia" ;
    ex:nonIMDRFCode "MedDRA:10037714:Quadriplegia" ;
    rdfs:comment "Paralysis of all four limbs." ;
    rdfs:subClassOf imdrf:E0122 .

imdrf:E012206 a owl:Class ;
    rdfs:label "Shaking/Tremors" ;
    ex:nonIMDRFCode "MedDRA:10040528:Shaking" ;
    rdfs:comment "The shaking movement of the whole body or just a certain part of it, often caused by problems of the neurons responsible for muscle action." ;
    rdfs:subClassOf imdrf:E0122 .

imdrf:E012207 a owl:Class ;
    rdfs:label "Twitching" ;
    ex:nonIMDRFCode "MedDRA:10045198:Twitching" ;
    rdfs:comment "The occurrence of a single contraction or a series of contractions of a muscle." ;
    rdfs:subClassOf imdrf:E0122 .

imdrf:E012208 a owl:Class ;
    rdfs:label "Restless Legs Syndrome" ;
    ex:nonIMDRFCode "MedDRA:10058920:Restless legs syndrome" ;
    ex:statusDescription "Term was added on 27 January 2022. For details, see comment No. 85 of the Change Log (Release Number 2022)." ;
    rdfs:comment "A condition that is characterized by an irresistible urgency to move the legs to obtain relief from a strange and uncomfortable sensation in the legs." ;
    rdfs:subClassOf imdrf:E0122 .

imdrf:E012209 a owl:Class ;
    rdfs:label "Facial Paralysis" ;
    ex:nonIMDRFCode "MedDRA:10016062:Facial paralysis" ;
    ex:statusDescription "Term was added on 27 January 2022. For details, see comment No. 242 / 243 / 244 / 245 of the Change Log (Release Number 2022)." ;
    rdfs:comment "A partial or complete loss of function of one or more of the facial muscles resulting in paralysis of the facial regions. Includes both central and peripheral facial paralysis or palsy." ;
    rdfs:subClassOf imdrf:E0122 .

imdrf:E012301 a owl:Class ;
    rdfs:label "Optical Nerve Damage" ;
    ex:nonIMDRFCode "MedDRA:10030938:Optic nerve injury" ;
    rdfs:comment "Injury to optical nerve." ;
    rdfs:subClassOf imdrf:E0123 .

imdrf:E012401 a owl:Class ;
    rdfs:label "Spinal Cord Injury" ;
    ex:nonIMDRFCode "MedDRA:10041552:Spinal cord injury" ;
    rdfs:comment "Traumatic damage of the spinal cord." ;
    rdfs:subClassOf imdrf:E0124 .

imdrf:E0125 a owl:Class ;
    rdfs:label "Neuralgia" ;
    ex:nonIMDRFCode "MedDRA:10029223:Neuralgia" ;
    rdfs:comment "Intense painful sensation along a nerve or group of nerves." ;
    rdfs:subClassOf imdrf:E01 .

imdrf:E0126 a owl:Class ;
    rdfs:label "Neuropathy" ;
    ex:nonIMDRFCode "MedDRA:10029328:Neuropathy" ;
    rdfs:comment "A disorder affecting the cranial nerves or the peripheral nervous system. It manifests with pain, tingling, numbness, and muscle weakness." ;
    rdfs:subClassOf imdrf:E01 .

imdrf:E0127 a owl:Class ;
    rdfs:label "Numbness" ;
    ex:nonIMDRFCode "MedDRA:10029829:Numbness" ;
    rdfs:comment "The loss of the sensation of feeling in an area of the body." ;
    rdfs:subClassOf imdrf:E01 .

imdrf:E0128 a owl:Class ;
    rdfs:label "Peripheral Nervous Injury" ;
    ex:nonIMDRFCode "MedDRA:10034586:Peripheral nerve injury" ;
    rdfs:comment "Injury to the peripheral nervous system." ;
    rdfs:subClassOf imdrf:E01,
        imdrf:E20 .

imdrf:E0129 a owl:Class ;
    rdfs:label "Sensitivity of Teeth" ;
    ex:nonIMDRFCode "MedDRA:10040012:Sensitivity of teeth" ;
    rdfs:comment "Pain or discomfort caused by exposure of the dentin layer of tooth to thermal, tactile, or other stimuli." ;
    rdfs:subClassOf imdrf:E01 .

imdrf:E0130 a owl:Class ;
    rdfs:label "Sleep Dysfunction" ;
    ex:nonIMDRFCode "MedDRA:10040984:Sleep disorder" ;
    rdfs:comment "A change from the patient's baseline sleeping pattern, in the hours slept and/or an alteration/dysfunction in the stages of sleep." ;
    rdfs:subClassOf imdrf:E01 .

imdrf:E0131 a owl:Class ;
    rdfs:label "Speech Disorder" ;
    ex:nonIMDRFCode "MedDRA:10041466:Speech disorder" ;
    rdfs:comment "A term referring to disorders characterized by the disruption of normal speech. It includes stuttering, lisps, dysarthria and voice disorders." ;
    rdfs:subClassOf imdrf:E01 .

imdrf:E0132 a owl:Class ;
    rdfs:label "Spinal Arachnoiditis" ;
    ex:nonIMDRFCode "MedDRA:10068160:Spinal arachnoiditis" ;
    rdfs:comment "A chronic adhesive arachnoiditis in the spinal arachnoid, with root and spinal cord symptoms similar to those caused by pressure from a tumor." ;
    rdfs:subClassOf imdrf:E01 .

imdrf:E013301 a owl:Class ;
    rdfs:label "Hemorrhagic Stroke" ;
    ex:nonIMDRFCode "MedDRA:10048863:Hemorrhagic stroke" ;
    rdfs:comment "An acute neurological deficit caused by bleeding within the brain or between the brain and the skull." ;
    rdfs:subClassOf imdrf:E0133 .

imdrf:E013302 a owl:Class ;
    rdfs:label "Ischemia Stroke" ;
    ex:nonIMDRFCode "MedDRA:10055221:Ischemic stroke" ;
    rdfs:comment "An ischemic condition of the brain, producing a persistent focal neurological deficit in the area of distribution of the cerebral arteries." ;
    rdfs:subClassOf imdrf:E0133 .

imdrf:E013401 a owl:Class ;
    rdfs:label "Hyperesthesia" ;
    ex:nonIMDRFCode "MedDRA:10020622:Hyperesthesia" ;
    rdfs:comment "Increased sensitivity to tactile stimulation." ;
    rdfs:subClassOf imdrf:E0134 .

imdrf:E013402 a owl:Class ;
    rdfs:label "Hypoesthesia" ;
    ex:nonIMDRFCode "MedDRA:10020976:Hypoesthesia" ;
    rdfs:comment "Impairment of tactile sensitivity manifesting as partial loss of sensitivity to sensory stimuli." ;
    rdfs:subClassOf imdrf:E0134 .

imdrf:E013403 a owl:Class ;
    rdfs:label "Paresthesia" ;
    ex:nonIMDRFCode "MedDRA:10033987:Paresthesia" ;
    rdfs:comment "Abnormal touch sensations, such as burning or prickling, that occur without an outside stimulus." ;
    rdfs:subClassOf imdrf:E0134 .

imdrf:E013501 a owl:Class ;
    rdfs:label "Ageusia" ;
    ex:nonIMDRFCode "MedDRA:10001480:Ageusia" ;
    rdfs:comment "Inability to taste." ;
    rdfs:subClassOf imdrf:E0135 .

imdrf:E013502 a owl:Class ;
    rdfs:label "Dysgeusia" ;
    ex:nonIMDRFCode "MedDRA:10013911:Dysgeusia" ;
    rdfs:comment "Distortion of taste." ;
    rdfs:subClassOf imdrf:E0135 .

imdrf:E0136 a owl:Class ;
    rdfs:label "Tics/Tremor" ;
    ex:nonIMDRFCode "MedDRA:10066770:Motor tic" ;
    rdfs:comment "An involuntary, compulsive, repetitive stereotyped movement." ;
    rdfs:subClassOf imdrf:E01 .

imdrf:E0137 a owl:Class ;
    rdfs:label "Transient Ischemic Attack" ;
    ex:nonIMDRFCode "MedDRA:10072760:Transient ischemic attack" ;
    rdfs:comment "A brief attack (from a few minutes to an hour) of cerebral dysfunction of vascular origin, with no persistent neurological deficit." ;
    rdfs:subClassOf imdrf:E01 .

imdrf:E0138 a owl:Class ;
    rdfs:label "Undesired Nerve Stimulation" ;
    ex:nonIMDRFCode "MedDRA:10068145:Undesired device stimulation of nerve" ;
    ex:status "Retired" ;
    ex:statusDescription "Term retired for Release Number 2025. Use E2131 - Inappropriate Device Stimulation of Tissue. See no. 17 of Change Request Log" ;
    rdfs:comment "Unintended reaction in nerve system caused by electrical stimulation." ;
    rdfs:subClassOf imdrf:E01 .

imdrf:E0139 a owl:Class ;
    rdfs:label "Unspecified Nervous System Problem" ;
    ex:statusDescription "Term was added on 18 March 2020 for cases where the category of a health effect was reported but with no further details." ;
    rdfs:comment "The report describes a non-specific problem with the nervous system. Note: Please use \"Appropriate Term / Code Not Available\" if the report describes a specific injury but the relevant term does not exist." ;
    rdfs:subClassOf imdrf:E01 .

imdrf:E0140 a owl:Class ;
    rdfs:label "Intracranial Pressure Increased" ;
    ex:nonIMDRFCode "MedDRA:10022773:Intracranial pressure increased" ;
    ex:statusDescription "Term was added on 27 January 2022. For details, see comment No. 86 of the Change Log (Release Number 2022)." ;
    rdfs:comment "Pressure within the craniospinal compartment is increased." ;
    rdfs:subClassOf imdrf:E01 .

imdrf:E0141 a owl:Class ;
    rdfs:label "Pneumocephalus" ;
    ex:nonIMDRFCode "MedDRA:10048736:Pneumocephalus" ;
    ex:statusDescription "Term was added on 27 January 2022. For details, see comment No. 212 of the Change Log (Release Number 2022)." ;
    rdfs:comment "The presence of air or gas within the cranial cavity." ;
    rdfs:subClassOf imdrf:E01 .

imdrf:E0142 a owl:Class ;
    rdfs:label "Idiopathic Intracranial Hypertension" ;
    ex:nonIMDRFCode "MedDRA:10078904:Idiopathic intracranial hypertension" ;
    ex:statusDescription "Term was added on 27 January 2022. For details, see comment No. 219 of the Change Log (Release Number 2022)." ;
    rdfs:comment "A condition that mimics the presence of a tumour (Pseudotumour Cerebri) or hydrocephalus, caused by chronic  increase in intracranial pressure." ;
    rdfs:subClassOf imdrf:E01 .

imdrf:E014301 a owl:Class ;
    rdfs:label "Increased Level of Consciousness" ;
    ex:nonIMDRFCode "MedDRA:10021683:Increased state of alertness" ;
    ex:statusDescription "Term was added on 27 January 2022. For details, see comment No. 77 of the Change Log (Release Number 2022)." ;
    rdfs:comment "A neurological state characterised by increased ability to perceive and respond." ;
    rdfs:subClassOf imdrf:E0143 .

imdrf:E014302 a owl:Class ;
    rdfs:label "Decreased Level  of Consciousness" ;
    ex:nonIMDRFCode "MedDRA:10012373:Depressed level of consciousness" ;
    ex:statusDescription "Term was added on 27 January 2022. For details, see comment No. 77 of the Change Log (Release Number 2022)." ;
    rdfs:comment "A neurological state characterised by decreased ability to perceive and respond." ;
    rdfs:subClassOf imdrf:E0143 .

imdrf:E0144 a owl:Class ;
    rdfs:label "Dural Tear" ;
    ex:nonIMDRFCode "MedDRA:10063395:Dural Tear" ;
    ex:statusDescription "Term added for Release Number 2024. See no. 22 of Change Log" ;
    rdfs:comment "Injury to the dura mater, with or without damage to any other layer of the meninges." ;
    rdfs:subClassOf imdrf:E01,
        imdrf:E21 .

imdrf:E0201 a owl:Class ;
    rdfs:label "Bruxism" ;
    ex:nonIMDRFCode "MedDRA:10006514:Bruxism" ;
    rdfs:comment "Excessive clenching of the jaw and grinding of the teeth." ;
    rdfs:subClassOf imdrf:E02 .

imdrf:E020201 a owl:Class ;
    rdfs:label "Anxiety" ;
    ex:nonIMDRFCode "MedDRA:10002855:Anxiety" ;
    rdfs:comment "Apprehension or uneasiness which may be accompanied by restlessness, tension, tachycardia, and dyspnea." ;
    rdfs:subClassOf imdrf:E0202 .

imdrf:E020202 a owl:Class ;
    rdfs:label "Depression" ;
    ex:nonIMDRFCode "MedDRA:10012378:Depression" ;
    rdfs:comment "A condition marked by ongoing feelings of sadness, despair, loss of energy, diminished interest/pleasure and difficulty dealing with normal daily life." ;
    rdfs:subClassOf imdrf:E0202 .

imdrf:E020203 a owl:Class ;
    rdfs:label "Distress" ;
    ex:nonIMDRFCode "MedDRA:10049119:Emotional distress" ;
    rdfs:comment "A state of physiological or psychological stress that cannot be compensated for by normal adaptive measures." ;
    rdfs:subClassOf imdrf:E0202 .

imdrf:E020204 a owl:Class ;
    rdfs:label "Malaise" ;
    ex:nonIMDRFCode "MedDRA:10025482:Malaise" ;
    rdfs:comment "A feeling of general discomfort or uneasiness, an out-of-sorts feeling." ;
    rdfs:subClassOf imdrf:E0202 .

imdrf:E020205 a owl:Class ;
    rdfs:label "Irritability" ;
    ex:nonIMDRFCode "MedDRA:10022998:Irritability" ;
    rdfs:comment "A feeling of agitation. Tending to become frustrated or upset easily." ;
    rdfs:subClassOf imdrf:E0202 .

imdrf:E0203 a owl:Class ;
    rdfs:label "Hallucination" ;
    ex:nonIMDRFCode "MedDRA:10019063:Hallucination" ;
    rdfs:comment "A false sensory perception in the absence of an external stimulus." ;
    rdfs:subClassOf imdrf:E02 .

imdrf:E0204 a owl:Class ;
    rdfs:label "Lethargy" ;
    ex:nonIMDRFCode "MedDRA:10024264:Lethargy" ;
    rdfs:comment "Characterized by a lack of vitality or energy." ;
    rdfs:subClassOf imdrf:E02 .

imdrf:E0205 a owl:Class ;
    rdfs:label "Suicidal Ideation" ;
    ex:nonIMDRFCode "MedDRA:10042458:Suicidal ideation" ;
    rdfs:comment "Thoughts of taking one's own life." ;
    rdfs:subClassOf imdrf:E02 .

imdrf:E0206 a owl:Class ;
    rdfs:label "Unspecified Mental, Emotional or Behavioural Problem" ;
    ex:statusDescription "Term was added on 18 March 2020 for cases where the category of a health effect was reported but with no further details." ;
    rdfs:comment "The report describes a non-specific Mental, Emotional or Behavioural problem. Note: Please use \"Appropriate Term / Code Not Available\" if the report describes a specific problem but the relevant term does not exist." ;
    rdfs:subClassOf imdrf:E02 .

imdrf:E0207 a owl:Class ;
    rdfs:label "Delirium" ;
    ex:nonIMDRFCode "MedDRA:10012218:Delirium" ;
    ex:statusDescription "Term was added on 27 January 2022. For details, see comment No. 36 of the Change Log (Release Number 2022)." ;
    rdfs:comment "A usually reversible condition characterized by the acute and sudden development of confusion, illusions, movement changes, inattentiveness, agitation and hallucinations." ;
    rdfs:subClassOf imdrf:E02 .

imdrf:E0208 a owl:Class ;
    rdfs:label "Psychosis" ;
    ex:nonIMDRFCode "MedDRA:10037234:Psychosis" ;
    ex:statusDescription "Term was added on 27 January 2022. For details, see comment No. 37 of the Change Log (Release Number 2022)." ;
    rdfs:comment "A mental disorder characterized by personality change, impaired functioning and loss of touch with reality." ;
    rdfs:subClassOf imdrf:E02 .

imdrf:E0209 a owl:Class ;
    rdfs:label "Sleepiness/Drowsiness/Somnolence" ;
    ex:nonIMDRFCode "MedDRA:10041349:Somnolence" ;
    ex:statusDescription "Term was added on 31 January 2023. For details, see comment No. 77 of the Change Log (Release Number 2023)." ;
    rdfs:comment "The sensation of struggling to remain awake." ;
    rdfs:subClassOf imdrf:E02 .

imdrf:E030101 a owl:Class ;
    rdfs:label "Hemolytic Anemia" ;
    ex:nonIMDRFCode "MedDRA:10019493:Hemolytic anemia" ;
    rdfs:comment "Anemia resulting from the premature destruction of the peripheral blood red cells." ;
    rdfs:subClassOf imdrf:E0301 .

imdrf:E030201 a owl:Class ;
    rdfs:label "Disseminated Intravascular Coagulation (DIC)" ;
    ex:nonIMDRFCode "MedDRA:10013442:Disseminated intravascular coagulation" ;
    rdfs:comment "A pathological process where the blood starts to coagulate throughout the whole body. This depletes the body of its platelets and coagulation factors, and there is an increased risk of hemorrhage." ;
    rdfs:subClassOf imdrf:E0302 .

imdrf:E030202 a owl:Class ;
    rdfs:label "Thrombocytopenia" ;
    ex:nonIMDRFCode "MedDRA:10043554:Thrombocytopenia" ;
    rdfs:comment "Low blood platelet count." ;
    rdfs:subClassOf imdrf:E0302 .

imdrf:E0303 a owl:Class ;
    rdfs:label "Hemolysis" ;
    ex:nonIMDRFCode "MedDRA:10019491:Hemolysis" ;
    rdfs:comment "Disruption of the integrity of the erythrocyte membrane causing release of hemoglobin." ;
    rdfs:subClassOf imdrf:E03 .

imdrf:E0304 a owl:Class ;
    rdfs:label "Hypervolemia" ;
    ex:nonIMDRFCode "MedDRA:10020920:Hypervolemia" ;
    ex:statusDescription "Definition was modified on 21 January 2021 (Old definition: Too much fluid in the blood.). For details, see comment No. 2 of the Change Log." ;
    rdfs:comment "An abnormally high circulating blood volume." ;
    rdfs:subClassOf imdrf:E03 .

imdrf:E0305 a owl:Class ;
    rdfs:label "Hypovolemia" ;
    ex:nonIMDRFCode "MedDRA:10021139:Hypovolemia" ;
    rdfs:comment "An abnormally low circulating blood volume." ;
    rdfs:subClassOf imdrf:E03 .

imdrf:E0306 a owl:Class ;
    rdfs:label "Sepsis" ;
    ex:nonIMDRFCode "MedDRA:10040047:Sepsis" ;
    rdfs:comment "The presence of pathogenic microorganisms in the blood stream causing a rapidly progressing systemic reaction that may lead to shock. Symptoms include fever, chills, tachycardia, and increased respiratory rate. It is a medical emergency that requires urgent medical attention." ;
    rdfs:subClassOf imdrf:E03,
        imdrf:E19 .

imdrf:E0307 a owl:Class ;
    rdfs:label "Seroma" ;
    ex:nonIMDRFCode "MedDRA:10040102:Seroma" ;
    rdfs:comment "A tumor-like collection of serum in the tissues." ;
    rdfs:subClassOf imdrf:E03 .

imdrf:E0308 a owl:Class ;
    rdfs:label "Swollen Lymph Nodes/Glands" ;
    ex:nonIMDRFCode "MedDRA:10067201:Swollen lymph nodes" ;
    rdfs:comment "The presence of an enlarged lymph node." ;
    rdfs:subClassOf imdrf:E03 .

imdrf:E0309 a owl:Class ;
    rdfs:label "Low White Blood Cell Count" ;
    ex:nonIMDRFCode "MedDRA:10051617:White blood cell count low" ;
    ex:statusDescription "Definition was modified on 27 January 2022 (Old definition:The white blood cell count is below the normal range.). MedDRA mapping also updated from White blood cell count decreased (10047942) to White blood cell count low (10051617). For details, see comment No. 73 of the Change Log (Release Number 2022)." ;
    rdfs:comment "The white blood cell count is below the normal range, including neutropenia." ;
    rdfs:subClassOf imdrf:E03 .

imdrf:E0310 a owl:Class ;
    rdfs:label "Unspecified Blood or Lymphatic problem" ;
    ex:statusDescription "Term was added on 18 March 2020 for cases where the category of a health effect was reported but with no further details." ;
    rdfs:comment "The report describes a non-specific problem with the blood or lymphatic system. Note: Please use \"Appropriate Term / Code Not Available\" if the report describes a specific problem but the relevant term does not exist." ;
    rdfs:subClassOf imdrf:E03 .

imdrf:E0311 a owl:Class ;
    rdfs:label "High White Blood Cell Count" ;
    ex:nonIMDRFCode "MedDRA:10051771:White blood cell count high" ;
    ex:statusDescription "Term was added on 27 January 2022. For details, see comment No. 79 of the Change Log (Release Number 2022)." ;
    rdfs:comment "The white blood cell count is above the normal range." ;
    rdfs:subClassOf imdrf:E03 .

imdrf:E0312 a owl:Class ;
    rdfs:label "Transfusion Reaction" ;
    ex:nonIMDRFCode "MedDRA:10044359:Transfusion reaction" ;
    ex:statusDescription "Term was added on 27 January 2022. For details, see comment No. 202 of the Change Log (Release Number 2022)." ;
    rdfs:comment "Adverse events associated with the transfusion of whole blood or one of its components, most commonly a hemolytic reaction to cross-typed blood." ;
    rdfs:subClassOf imdrf:E03 .

imdrf:E0313 a owl:Class ;
    rdfs:label "Blood Protein Abnormal" ;
    ex:statusDescription "Term was added on 27 January 2022. For details, see comment No. 108 / 111 of the Change Log (Release Number 2022)." ;
    rdfs:comment "One or more of the blood protein levels being higher or lower than normal (e.g. Albumin, C-reactive Protein)." ;
    rdfs:subClassOf imdrf:E03 .

imdrf:E0401 a owl:Class ;
    rdfs:label "Autoimmune Disorder" ;
    ex:nonIMDRFCode "MedDRA:10061664:Autoimmune disorder" ;
    rdfs:comment "A disorder resulting from loss of function or tissue destruction of an organ or multiple organs, arising from humoral or cellular immune responses of the individual to his own tissue constituents." ;
    rdfs:subClassOf imdrf:E04 .

imdrf:E040201 a owl:Class ;
    rdfs:label "Anaphylactic Shock" ;
    ex:nonIMDRFCode "MedDRA:10002199:Anaphylactic shock" ;
    rdfs:comment "Progression of anaphylaxis into systemic shock, which is characterized by significant reduction in tissue perfusion which leads to hypoxia and hypotension, and can lead to death if untreated." ;
    rdfs:subClassOf imdrf:E0402,
        imdrf:E2336 .

imdrf:E040202 a owl:Class ;
    rdfs:label "Anaphylactoid / Anaphylaxis" ;
    ex:nonIMDRFCode "MedDRA:10002218:Anaphylaxis" ;
    ex:statusDescription "Definition was modified on 31 January 2023 (Old definition: Resembling anaphylaxis.) MedDRA mapping also updated from Anaphylactoid reaction (10002216) to Anaphylaxis (10002218). For details, see comment No. 78 of the Change Log (Release Number 2023).",
        "Definition was modified on 31 January 2023 (Old definition: Resembling anaphylaxis.). MedDRA mapping also updated from Anaphylactoid reaction (10002216) to Anaphylaxis (10002218). For details, see comment No. 85 of the Change Log (Release Number 2023)." ;
    rdfs:comment "Acute immune response that occurs from exposure to an allergen. For conditions which have progressed to systemic shock, use E040201 - Anaphylactic Shock." ;
    rdfs:subClassOf imdrf:E0402,
        imdrf:E23 .

imdrf:E040203 a owl:Class ;
    rdfs:label "Local Reaction" ;
    ex:nonIMDRFCode "MedDRA:10024769:Local reaction" ;
    rdfs:comment "A regionally-limited response to an antigen, which may include inflammation, induration, erythema, pruritus or pain." ;
    rdfs:subClassOf imdrf:E0402 .

imdrf:E0403 a owl:Class ;
    rdfs:label "Immunodeficiency" ;
    ex:nonIMDRFCode "MedDRA:10061598:Immunodeficiency" ;
    rdfs:comment "A deficiency of immune response or a disorder characterized by deficient immune response." ;
    rdfs:subClassOf imdrf:E04 .

imdrf:E0404 a owl:Class ;
    rdfs:label "Positive antinuclear antibodies (ANA)" ;
    ex:nonIMDRFCode "MedDRA:10060055:Antinuclear antibody positive" ;
    rdfs:comment "Indicates that antibodies directed against nuclear antigens have been detected. Almost invariably found in systemic lupus erythematosus and are frequently found in rheumatoid arthritis, scleroderma, Sjogren's Syndrome and mixed connective tissue disease." ;
    rdfs:subClassOf imdrf:E04 .

imdrf:E0405 a owl:Class ;
    rdfs:label "Unspecified Immune System Problem" ;
    ex:statusDescription "Term was added on 18 March 2020 for cases where the category of a health effect was reported but with no further details." ;
    rdfs:comment "The report describes a non-specific problem with the immune system. Note: Please use \"Appropriate Term / Code Not Available\" if the report describes a specific problem but the relevant term does not exist." ;
    rdfs:subClassOf imdrf:E04 .

imdrf:E050101 a owl:Class ;
    rdfs:label "Ruptured Aneurysm" ;
    ex:nonIMDRFCode "MedDRA:10048380:Aneurysm ruptured" ;
    rdfs:comment "An aneurysm that has burst, resulting in hemorrhage into adjacent tissues." ;
    rdfs:subClassOf imdrf:E0501 .

imdrf:E050102 a owl:Class ;
    rdfs:label "Aneurysm expansion" ;
    ex:nonIMDRFCode "MedDRA:10069506:Aneurysm enlargement" ;
    ex:statusDescription "Term was added on 27 January 2022. For details, see comment No. 185 of the Change Log (Release Number 2022)." ;
    rdfs:comment "Expansion of aneurysm." ;
    rdfs:subClassOf imdrf:E0501 .

imdrf:E0502 a owl:Class ;
    rdfs:label "Arteriosclerosis/ Atherosclerosis" ;
    ex:nonIMDRFCode "MedDRA:10003210:Arteriosclerosis" ;
    rdfs:comment "A vascular disorder characterized by thickening and hardening of the walls of the arteries. Build-up of fatty material and calcium deposition in the arterial wall resulting in partial or complete occlusion of the arterial lumen." ;
    rdfs:subClassOf imdrf:E05 .

imdrf:E050301 a owl:Class ;
    rdfs:label "Air Embolism" ;
    ex:nonIMDRFCode "MedDRA:10001526:Air embolism" ;
    rdfs:comment "The presence of bubbles of air in the vascular system; occurrence is related to the entry of air into the venous circulation following trauma or surgery." ;
    rdfs:subClassOf imdrf:E0503 .

imdrf:E050302 a owl:Class ;
    rdfs:label "Foreign Body Embolism" ;
    ex:nonIMDRFCode "MedDRA:10075247:Foreign body embolism" ;
    rdfs:comment "Type of embolism when lumen of vessel or ductus is occluded by part of device." ;
    rdfs:subClassOf imdrf:E0503 .

imdrf:E050303 a owl:Class ;
    rdfs:label "Pulmonary Embolism" ;
    ex:nonIMDRFCode "MedDRA:10037377:Pulmonary embolism" ;
    rdfs:comment "The obstruction of the pulmonary artery or one of its branches by an embolus, sometimes associated with infarction of the lung." ;
    rdfs:subClassOf imdrf:E0503,
        imdrf:E07 .

imdrf:E050304 a owl:Class ;
    rdfs:label "Thromboembolism" ;
    ex:nonIMDRFCode "MedDRA:10043566:Thromboembolism" ;
    rdfs:comment "Occlusion of the lumen of a vessel by a thrombus that has migrated from a distal site via the blood stream." ;
    rdfs:subClassOf imdrf:E0503 .

imdrf:E050305 a owl:Class ;
    rdfs:label "Fat embolism" ;
    ex:nonIMDRFCode "MedDRA:10016246:Fat embolism" ;
    ex:statusDescription "Term added for Release Number 2024. See no. 57 of Change Log" ;
    rdfs:comment "The blockage of a blood vessel by fat particles in the circulation." ;
    rdfs:subClassOf imdrf:E0503 .

imdrf:E0504 a owl:Class ;
    rdfs:label "Extravasation" ;
    ex:nonIMDRFCode "MedDRA:10015866:Extravasation" ;
    rdfs:comment "The leakage of body fluid or cells from the vascular system to the surrounding tissues. This process occurs either by force or as a result of a pathologic reaction (e.g., inflammation)." ;
    rdfs:subClassOf imdrf:E05 .

imdrf:E0505 a owl:Class ;
    rdfs:label "Hematoma" ;
    ex:nonIMDRFCode "MedDRA:10019428:Hematoma" ;
    rdfs:comment "A localized collection of blood, usually clotted, in an organ, space, or tissue, due to a break in the wall of a blood vessel." ;
    rdfs:subClassOf imdrf:E05 .

imdrf:E050601 a owl:Class ;
    rdfs:label "Ecchymosis" ;
    ex:nonIMDRFCode "MedDRA:10014080:Ecchymosis" ;
    rdfs:comment "A flat discoloration of the skin or a mucous membrane, larger in area than a petechia, caused by the extravasation of blood. Discolouration under the skin caused by a bleed underneath. Typically a bruise." ;
    rdfs:subClassOf imdrf:E0506 .

imdrf:E050602 a owl:Class ;
    rdfs:label "Exsanguination" ;
    ex:nonIMDRFCode "MedDRA:10015719:Exsanguination" ;
    rdfs:comment "Extensive loss of blood due to internal or external hemorrhage." ;
    rdfs:subClassOf imdrf:E0506 .

imdrf:E0507 a owl:Class ;
    rdfs:label "High Pulmonary Arterial Wedge Pressure" ;
    ex:nonIMDRFCode "MedDRA:10037328:Pulmonary arterial wedge pressure high" ;
    rdfs:comment "The measurement of the mean left atrial pressure, as measured by a catheter introduced into the distal pulmonary artery, is high." ;
    rdfs:subClassOf imdrf:E05,
        imdrf:E22 .

imdrf:E0508 a owl:Class ;
    rdfs:label "Low Pulmonary Arterial Wedge Pressure" ;
    ex:nonIMDRFCode "MedDRA:10037330:Pulmonary arterial wedge pressure low" ;
    ex:statusDescription "Definition was modified on 21 January 2021 (Old definition: The measurement of the mean left pulmonary atrial pressure, as measured by a catheter introduced into the distal pulmonary artery, is low.). For details, see comment No. 3 of the Change Log." ;
    rdfs:comment "The measurement of the mean left atrial pressure, as measured by a catheter introduced into the distal pulmonary artery, is low." ;
    rdfs:subClassOf imdrf:E05,
        imdrf:E22 .

imdrf:E0509 a owl:Class ;
    rdfs:label "Ischemia" ;
    ex:nonIMDRFCode "MedDRA:10054438:Ischemia" ;
    rdfs:comment "Lack of oxygen in tissues, commonly due to impaired blood supply to an area of the body, resulting in impairment of tissue oxygenation." ;
    rdfs:subClassOf imdrf:E05 .

imdrf:E0510 a owl:Class ;
    rdfs:label "Neovascularization" ;
    ex:nonIMDRFCode "MedDRA:10029114:Neovascularization" ;
    rdfs:comment "The formation of new blood vessels." ;
    rdfs:subClassOf imdrf:E05 .

imdrf:E051101 a owl:Class ;
    rdfs:label "Great Vessel Perforation" ;
    ex:nonIMDRFCode "MedDRA:10080896:Perforation of great vessels" ;
    rdfs:comment "Damage to the venae cavae, pulmonary artery, pulmonary veins or aorta resulting from a full thickness disruption in the integrity of the vessel wall." ;
    rdfs:subClassOf imdrf:E0511,
        imdrf:E2114 .

imdrf:E0512 a owl:Class ;
    rdfs:label "Vasculitis" ;
    ex:nonIMDRFCode "MedDRA:10047115:Vasculitis" ;
    ex:statusDescription "Term and Definition and MedDRA map modified for Release Number 2024. Previous term was Phlebitis. Previous MedDRA map was 10034879:Phlebitis. See no. 19 of Change Log." ;
    rdfs:comment "Inflammation of any one of the blood vessels, including the ARTERIES; VEINS; and rest of the vasculature system in the body." ;
    rdfs:subClassOf imdrf:E05 .

imdrf:E0513 a owl:Class ;
    rdfs:label "Pseudoaneurysm" ;
    ex:nonIMDRFCode "MedDRA:10048977:Pseudoaneurysm" ;
    rdfs:comment "The creation of hematoma outside the arterial wall following bleeding due to puncture of the arterial wall. Pseudoaneurysms can also occur in the heart chambers following myocardial infarction with rupture of the wall of the ventricle." ;
    rdfs:subClassOf imdrf:E05 .

imdrf:E0514 a owl:Class ;
    rdfs:label "Thrombosis/Thrombus" ;
    ex:nonIMDRFCode "MedDRA:10043607:Thrombosis" ;
    rdfs:comment "The formation of a blood clot in the lumen of a vessel or heart chamber." ;
    rdfs:subClassOf imdrf:E05 .

imdrf:E051501 a owl:Class ;
    rdfs:label "Aortic dissection" ;
    ex:nonIMDRFCode "MedDRA:10002895:Aortic dissection" ;
    ex:statusDescription "Term added for Release Number 2024. See no. 83 of Change Log" ;
    rdfs:comment "Spontaneous or induced tear within the wall of the aorta" ;
    rdfs:subClassOf imdrf:E0515 .

imdrf:E0516 a owl:Class ;
    rdfs:label "Vasoconstriction" ;
    ex:nonIMDRFCode "MedDRA:10047139:Vasoconstriction" ;
    rdfs:comment "Vasoconstriction involves narrowing of a blood vessel lumen due to smooth muscle contraction in the vessel wall and leads to decreased blood flow." ;
    rdfs:subClassOf imdrf:E05 .

imdrf:E0517 a owl:Class ;
    rdfs:label "Vasodilatation" ;
    ex:nonIMDRFCode "MedDRA:10047141:Vasodilatation" ;
    rdfs:comment "Widening of a blood vessel lumen due to smooth muscle relaxation in the vessel wall and leads to increased blood flow." ;
    rdfs:subClassOf imdrf:E05 .

imdrf:E0518 a owl:Class ;
    rdfs:label "Unspecified Vascular Problem" ;
    ex:statusDescription "Term was added on 18 March 2020 for cases where the category of a health effect was reported but with no further details." ;
    rdfs:comment "The report describes a non-specific problem with the vascular system. Note: Please use \"Appropriate Term / Code Not Available\" if the report describes a specific problem but the relevant term does not exist." ;
    rdfs:subClassOf imdrf:E05 .

imdrf:E0519 a owl:Class ;
    rdfs:label "Reduced Blood Flow" ;
    ex:nonIMDRFCode "MedDRA:10054880:Vascular insufficiency" ;
    ex:statusDescription "Term was added on 27 January 2022. For details, see comment No. 190 of the Change Log (Release Number 2022)." ;
    rdfs:comment "Inadequate blood flow to a particular area of the body." ;
    rdfs:subClassOf imdrf:E05 .

imdrf:E0520 a owl:Class ;
    rdfs:label "Reperfusion Injury" ;
    ex:nonIMDRFCode "MedDRA:10063837:Reperfusion injury" ;
    ex:statusDescription "Term was added on 31 January 2023. For details, see comment No. 125 of the Change Log (Release Number 2023)." ;
    rdfs:comment "Tissue damage caused when blood supply returns to tissue after a period of ischemia or lack of oxygen. The restoration of circulation results in inflammation and oxidative damage." ;
    rdfs:subClassOf imdrf:E05 .

imdrf:E0521 a owl:Class ;
    rdfs:label "Coronary obstruction/occlusion" ;
    ex:nonIMDRFCode "MedDRA:10011103:Coronary occlusion" ;
    ex:statusDescription "Term added for Release Number 2024. See no. 82 of Change Log" ;
    rdfs:comment "Partial or total occlusion or obstruction of the coronary ostia or artery." ;
    rdfs:subClassOf imdrf:E05,
        imdrf:E06 .

imdrf:E0522 a owl:Class ;
    rdfs:label "Vasospasm" ;
    ex:nonIMDRFCode "MedDRA:10047163:Vasospasm" ;
    ex:status "New" ;
    ex:statusDescription "Term added for Release Number 2025. See no. 35 of Change Log" ;
    rdfs:comment "Contraction of muscular walls of blood vessels" ;
    rdfs:subClassOf imdrf:E05 .

imdrf:E0523 a owl:Class ;
    rdfs:label "False Lumen Perfusion" ;
    ex:nonIMDRFCode "MedDRA:10074841:Continued perfusion of a false lumen" ;
    ex:status "New" ;
    ex:statusDescription "Term added for Release Number 2025. See no. 66 of Change Log" ;
    rdfs:comment "Persistent blood flow in the false lumen of a dissection following an endovascular aortic repair (EVAR) procedure." ;
    rdfs:subClassOf imdrf:E05 .

imdrf:E060101 a owl:Class ;
    rdfs:label "Asystole" ;
    ex:nonIMDRFCode "MedDRA:10003586:Asystole" ;
    rdfs:comment "An electrocardiographic finding showing a state of cardiac standstill with no cardiac output and no ventricular depolarization." ;
    rdfs:subClassOf imdrf:E0601 .

imdrf:E060102 a owl:Class ;
    rdfs:label "Atrial Fibrillation" ;
    ex:nonIMDRFCode "MedDRA:10003658:Atrial fibrillation" ;
    rdfs:comment "Irregular heart rhythm, usually associated with a rapid rate, that is caused by abnormal electrical activity within the atrial." ;
    rdfs:subClassOf imdrf:E0601 .

imdrf:E060103 a owl:Class ;
    rdfs:label "Atrial Flutter" ;
    ex:nonIMDRFCode "MedDRA:10003662:Atrial flutter" ;
    rdfs:comment "A rapid heart rate, associated with a regular rhythm, that is caused by abnormal electrical activity within the atria." ;
    rdfs:subClassOf imdrf:E0601 .

imdrf:E060104 a owl:Class ;
    rdfs:label "Bradycardia" ;
    ex:nonIMDRFCode "MedDRA:10006093:Bradycardia" ;
    rdfs:comment "An abnormally slow heart rate. Thresholds for different age, gender, and patient populations exist." ;
    rdfs:subClassOf imdrf:E0601 .

imdrf:E060105 a owl:Class ;
    rdfs:label "Ectopic Heartbeat" ;
    ex:nonIMDRFCode "MedDRA:10014159:Ectopic heartbeats" ;
    rdfs:comment "A cardiac beat originating from an abnormal site. These changes lead to extra or dropped heartbeats." ;
    rdfs:subClassOf imdrf:E0601 .

imdrf:E060106 a owl:Class ;
    rdfs:label "Heart Block" ;
    ex:nonIMDRFCode "MedDRA:10019252:Heart block" ;
    rdfs:comment "An interference with the normal conduction of electrical impulses that control activity of the heart muscle." ;
    rdfs:subClassOf imdrf:E0601 .

imdrf:E060107 a owl:Class ;
    rdfs:label "Idioventricular Rhythm" ;
    ex:nonIMDRFCode "MedDRA:10039111:Rhythm idioventricular" ;
    rdfs:comment "An electrocardiographic finding of three or more consecutive complexes of ventricular origin. The QRS complexes are wide and have an abnormal morphology. (CDISC)" ;
    rdfs:subClassOf imdrf:E0601 .

imdrf:E060108 a owl:Class ;
    rdfs:label "Irregular Pulse" ;
    ex:nonIMDRFCode "MedDRA:10022994:Irregular pulse" ;
    rdfs:comment "A pulse that beats at irregular intervals." ;
    rdfs:subClassOf imdrf:E0601 .

imdrf:E060109 a owl:Class ;
    rdfs:label "Tachycardia" ;
    ex:nonIMDRFCode "MedDRA:10043071:Tachycardia" ;
    rdfs:comment "Abnormally high heart rate. Thresholds for different age, gender, and patient populations exist." ;
    rdfs:subClassOf imdrf:E0601 .

imdrf:E060110 a owl:Class ;
    rdfs:label "Ventricular Fibrillation" ;
    ex:nonIMDRFCode "MedDRA:10047290:Ventricular fibrillation" ;
    rdfs:comment "Arrhythmia characterized by chaotic contractions of the ventricular muscle." ;
    rdfs:subClassOf imdrf:E0601 .

imdrf:E0602 a owl:Class ;
    rdfs:label "Cardiac Arrest" ;
    ex:nonIMDRFCode "MedDRA:10007515:Cardiac arrest" ;
    rdfs:comment "The sudden cessation of productive cardiac activity in an individual who becomes unresponsive, without normal breathing and no signs of circulation." ;
    rdfs:subClassOf imdrf:E06 .

imdrf:E0603 a owl:Class ;
    rdfs:label "Cardiac Enzyme Elevation" ;
    ex:nonIMDRFCode "MedDRA:10007548:Cardiac enzymes increased" ;
    rdfs:comment "Increase from the normal levels of cardiac enzymes." ;
    rdfs:subClassOf imdrf:E06,
        imdrf:E22 .

imdrf:E0604 a owl:Class ;
    rdfs:label "Cardiac Perforation" ;
    ex:nonIMDRFCode "MedDRA:10058039:Cardiac perforation" ;
    rdfs:comment "The presence of an acquired hole in the heart." ;
    rdfs:subClassOf imdrf:E06,
        imdrf:E2114 .

imdrf:E0605 a owl:Class ;
    rdfs:label "Cardiac Tamponade" ;
    ex:nonIMDRFCode "MedDRA:10007610:Cardiac tamponade" ;
    rdfs:comment "Acute compression of the heart caused by increased intrapericardial pressure due to the accumulation of blood or fluid in the pericardium from rupture of the heart or great vessels, penetrating trauma, or progressive effusion." ;
    rdfs:subClassOf imdrf:E06 .

imdrf:E0606 a owl:Class ;
    rdfs:label "Cardiomyopathy" ;
    ex:nonIMDRFCode "MedDRA:10007636:Cardiomyopathy" ;
    rdfs:comment "A disease of the heart muscle." ;
    rdfs:subClassOf imdrf:E06 .

imdrf:E0607 a owl:Class ;
    rdfs:label "Cardiovascular Dysfunction/Insufficiency" ;
    ex:nonIMDRFCode "MedDRA:10065929:Cardiovascular insufficiency" ;
    ex:statusDescription """Term and definition was modified on 31 January 2023 (Old term/definition: Cardiovascular Insufficiency: Circulatory insufficiency due to a decrease in the force of the cardiac contractions and / or the tone of the vascular walls.). For details, see comment No. 81 of the Change Log (Release Number 2023).
Error in secondary CodeHierarchy corrected for Release No. 2024""" ;
    rdfs:comment "Circulatory dysfunction/insufficiency due to a decrease in the force of the cardiac contractions and / or the tone of the vascular walls. Includes diastolic and systolic dysfunction." ;
    rdfs:subClassOf imdrf:E05,
        imdrf:E06 .

imdrf:E0608 a owl:Class ;
    rdfs:label "Cusp Tear" ;
    ex:nonIMDRFCode "MedDRA:10068167:Cusp tear" ;
    rdfs:comment "A tear located on a leaflet of a heart valve that prevents its complete closing, which can result in valvular dysfunction." ;
    rdfs:subClassOf imdrf:E06 .

imdrf:E0609 a owl:Class ;
    rdfs:label "Diminished Pulse Pressure" ;
    ex:nonIMDRFCode "MedDRA:10037480:Pulse pressure decreased" ;
    rdfs:comment "Weak or absent palpable pulse due to decreased arterial pulse pressure." ;
    rdfs:subClassOf imdrf:E06 .

imdrf:E0610 a owl:Class ;
    rdfs:label "Endocarditis" ;
    ex:nonIMDRFCode "MedDRA:10014665:Endocarditis" ;
    rdfs:comment "Inflammation of the endocardium." ;
    rdfs:subClassOf imdrf:E06,
        imdrf:E19 .

imdrf:E0611 a owl:Class ;
    rdfs:label "Heart Failure/Congestive Heart Failure" ;
    ex:nonIMDRFCode "MedDRA:10019279:Heart failure" ;
    rdfs:comment "Inability of the heart to pump blood adequately to fill tissue metabolic requirements or the ability to do so only at an elevated filling pressure." ;
    rdfs:subClassOf imdrf:E06 .

imdrf:E061201 a owl:Class ;
    rdfs:label "Angina" ;
    ex:nonIMDRFCode "MedDRA:10002383:Angina pectoris" ;
    rdfs:comment "Chest pain resulting from inadequate oxygen delivery for the needs of the myocardium." ;
    rdfs:subClassOf imdrf:E0612 .

imdrf:E061202 a owl:Class ;
    rdfs:label "Myocardial Infarction" ;
    ex:nonIMDRFCode "MedDRA:10028596:Myocardial infarction" ;
    rdfs:comment "A condition which occurs when blood flow decreases or stops to a part of the heart, causing damage to the heart muscle." ;
    rdfs:subClassOf imdrf:E0612 .

imdrf:E0613 a owl:Class ;
    rdfs:label "Low Cardiac Output" ;
    ex:nonIMDRFCode "MedDRA:10007595:Cardiac output decreased" ;
    rdfs:comment "A below normal volume of blood pumped from the right or left ventricle of the heart per unit time." ;
    rdfs:subClassOf imdrf:E06 .

imdrf:E0614 a owl:Class ;
    rdfs:label "Mitral Perforation" ;
    ex:nonIMDRFCode "MedDRA:10068138:Mitral perforation" ;
    rdfs:comment "A rupture in the mitral valve tissue due to traumatic or pathologic processes." ;
    rdfs:subClassOf imdrf:E06,
        imdrf:E2114 .

imdrf:E0615 a owl:Class ;
    rdfs:label "Myocardial Contusion" ;
    ex:nonIMDRFCode "MedDRA:10068147:Myocardial contusion" ;
    rdfs:comment "A bruise to the heart." ;
    rdfs:subClassOf imdrf:E06,
        imdrf:E2002 .

imdrf:E0616 a owl:Class ;
    rdfs:label "Myocardial Hypertrophy" ;
    ex:nonIMDRFCode "MedDRA:10072733:Myocardial hypertrophy" ;
    rdfs:comment "Thickening of the myocardium often due to chronic pressure overload." ;
    rdfs:subClassOf imdrf:E06 .

imdrf:E0617 a owl:Class ;
    rdfs:label "Myocarditis" ;
    ex:nonIMDRFCode "MedDRA:10028606:Myocarditis" ;
    rdfs:comment "Inflammation of the muscle tissue of the heart." ;
    rdfs:subClassOf imdrf:E06 .

imdrf:E0618 a owl:Class ;
    rdfs:label "Non specific EKG/ECG Changes" ;
    ex:nonIMDRFCode "MedDRA:10061116:Electrocardiogram change" ;
    rdfs:comment "An electrocardiographic finding of a change in cardiac electrical activity." ;
    rdfs:subClassOf imdrf:E06 .

imdrf:E0619 a owl:Class ;
    rdfs:label "Pericardial Effusion" ;
    ex:nonIMDRFCode "MedDRA:10034474:Pericardial effusion" ;
    ex:statusDescription "Error in MedDRA mapping corrected for Release No. 2024" ;
    rdfs:comment "Fluid collection within the pericardial sac, usually due to inflammation." ;
    rdfs:subClassOf imdrf:E06 .

imdrf:E0620 a owl:Class ;
    rdfs:label "Pericarditis" ;
    ex:nonIMDRFCode "MedDRA:10034484:Pericarditis" ;
    rdfs:comment "Inflammation of the pericardium." ;
    rdfs:subClassOf imdrf:E06 .

imdrf:E062101 a owl:Class ;
    rdfs:label "Aortic Valve Insufficiency/ Regurgitation" ;
    ex:nonIMDRFCode "MedDRA:10052839:Aortic valve insufficiency" ;
    rdfs:comment "Incomplete closure or damage to a valve leaflet of the aortic valve, resulting in aortic valve backflow." ;
    rdfs:subClassOf imdrf:E0621 .

imdrf:E062102 a owl:Class ;
    rdfs:label "Mitral Valve Insufficiency/ Regurgitation" ;
    ex:nonIMDRFCode "MedDRA:10074862:Mitral valve insufficiency" ;
    rdfs:comment "Incomplete closure or damage to a valve leaflet of the mitral valve, resulting in mitral valve backflow." ;
    rdfs:subClassOf imdrf:E0621 .

imdrf:E062103 a owl:Class ;
    rdfs:label "Pulmonary Valve Insufficiency/ Regurgitation" ;
    ex:nonIMDRFCode "MedDRA:10052842:Pulmonary valve insufficiency" ;
    rdfs:comment "Incomplete closure or damage to a valve leaflet of the pulmonary valve, resulting in pulmonary valve backflow." ;
    rdfs:subClassOf imdrf:E0621 .

imdrf:E062104 a owl:Class ;
    rdfs:label "Tricuspid Valve Insufficiency/ Regurgitation" ;
    ex:nonIMDRFCode "MedDRA:10044635:Tricuspid insufficiency" ;
    rdfs:comment "Incomplete closure or damage to a valve leaflet of the tricuspid valve, resulting in tricuspid valve backflow." ;
    rdfs:subClassOf imdrf:E0621 .

imdrf:E062201 a owl:Class ;
    rdfs:label "Aortic Valve Stenosis" ;
    ex:nonIMDRFCode "MedDRA:10002918:Aortic valve stenosis" ;
    rdfs:comment "Obstruction of flow across a aortic heart valve due to immobility reduced elasticity of the leaflets and/or a restricted orifice." ;
    rdfs:subClassOf imdrf:E0622 .

imdrf:E062202 a owl:Class ;
    rdfs:label "Mitral Valve Stenosis" ;
    ex:nonIMDRFCode "MedDRA:10027733:Mitral valve stenosis" ;
    rdfs:comment "Obstruction of flow across a mitral heart valve due to immobility reduced elasticity of the leaflets and/or a restricted orifice." ;
    rdfs:subClassOf imdrf:E0622 .

imdrf:E062203 a owl:Class ;
    rdfs:label "Pulmonary Valve Stenosis" ;
    ex:nonIMDRFCode "MedDRA:10037450:Pulmonary valve stenosis" ;
    rdfs:comment "Obstruction of flow across a pulmonary heart valve due to immobility reduced elasticity of the leaflets and/or a restricted orifice." ;
    rdfs:subClassOf imdrf:E0622 .

imdrf:E062204 a owl:Class ;
    rdfs:label "Tricuspid Valve Stenosis" ;
    ex:nonIMDRFCode "MedDRA:10044642:Tricuspid valve stenosis" ;
    rdfs:comment "Obstruction of flow across a tricuspid heart valve due to immobility reduced elasticity of the leaflets and/or a restricted orifice." ;
    rdfs:subClassOf imdrf:E0622 .

imdrf:E0623 a owl:Class ;
    rdfs:label "Unspecified Heart Problem" ;
    ex:statusDescription "Term was added on 18 March 2020 for cases where the category of a health effect was reported but with no further details." ;
    rdfs:comment "The report describes a non-specific problem with the heart. Note: Please use \"Appropriate Term / Code Not Available\" if the report describes a specific problem but the relevant term does not exist." ;
    rdfs:subClassOf imdrf:E06 .

imdrf:E0624 a owl:Class ;
    rdfs:label "Intraoperative Cardiac Valve Injury" ;
    ex:nonIMDRFCode "MedDRA:10088741:Intraoperative cardiac valve injury" ;
    ex:status "Modified (technical)" ;
    ex:statusDescription "Term was added on 31 January 2023. For details, see comment No. 80 / 114 of the Change Log (Release Number 2023). Definition modified for Release Number 2025. See no. 62 of Change Request Log" ;
    rdfs:comment "An intraoperative event that results in damage to, or abnormal function of, a heart valve. E.g. a tear in the leaflet or the chordae tendinae." ;
    rdfs:subClassOf imdrf:E06,
        imdrf:E21 .

imdrf:E0625 a owl:Class ;
    rdfs:label "Cardiac Septal Defect Residual Shunt" ;
    ex:nonIMDRFCode "MedDRA:10069121:Cardiac septal defect residual shunt" ;
    ex:statusDescription "Term was added on 31 January 2023. For details, see comment No. 82 of the Change Log (Release Number 2023)." ;
    rdfs:comment "Irregular blood flow in the heart after surgical correction of a septal defect." ;
    rdfs:subClassOf imdrf:E06 .

imdrf:E0626 a owl:Class ;
    rdfs:label "Transvalvular Pressure Gradient Increased" ;
    ex:nonIMDRFCode "MedDRA:10079128:Transvalvular pressure gradient increased" ;
    ex:statusDescription "Term was added on 31 January 2023. For details, see comment No. 112 of the Change Log (Release Number 2023)." ;
    rdfs:comment "Increased pressure across the heart valve" ;
    rdfs:subClassOf imdrf:E06 .

imdrf:E0627 a owl:Class ;
    rdfs:label "Intraoperative Cardiac Injury" ;
    ex:nonIMDRFCode "MedDRA:10065843:Intraoperative cardiac injury" ;
    ex:status "Modified (technical)" ;
    ex:statusDescription "Term was added on 31 January 2023. For details, see comment No. 118 of the Change Log (Release Number 2023). Definition modified for Release Number 2025. See no. 62 of Change Request Log" ;
    rdfs:comment "An intraoperative event that results in damage to, or abnormal function of, the heart. For valvular injury, use E0624 - Intraoperative Cardiac Valve Injury" ;
    rdfs:subClassOf imdrf:E06 .

imdrf:E0628 a owl:Class ;
    rdfs:label "Pneumopericardium" ;
    ex:nonIMDRFCode "MedDRA:10048731:Pneumopericardium" ;
    ex:status "New" ;
    ex:statusDescription "Term added for Release Number 2025. See no. 32 of Change Request Log" ;
    rdfs:comment "A collection of air or gas in the pericardial cavity." ;
    rdfs:subClassOf imdrf:E06 .

imdrf:E0629 a owl:Class ;
    rdfs:label "Palpitations" ;
    ex:nonIMDRFCode "MedDRA:10033557:Palpitations" ;
    ex:status "New" ;
    ex:statusDescription "Term added for Release Number 2025. See no. 60 of Change Request Log" ;
    rdfs:comment "The feeling of having a fast-beating, fluttering or pounding heart." ;
    rdfs:subClassOf imdrf:E06 .

imdrf:E0701 a owl:Class ;
    rdfs:label "Adult Respiratory Distress Syndrome" ;
    ex:nonIMDRFCode "MedDRA:10001409:Adult respiratory distress syndrome" ;
    rdfs:comment "Progressive and life-threatening pulmonary distress in the absence of an underlying pulmonary condition, usually following major trauma or surgery. Cases of neonatal respiratory distress syndrome are not included in this definition." ;
    rdfs:subClassOf imdrf:E07 .

imdrf:E0702 a owl:Class ;
    rdfs:label "Airway Obstruction" ;
    ex:nonIMDRFCode "MedDRA:10001539:Airways obstruction" ;
    rdfs:comment "Blockage of air flow in the respiratory tract." ;
    rdfs:subClassOf imdrf:E07 .

imdrf:E0703 a owl:Class ;
    rdfs:label "Apnea" ;
    ex:nonIMDRFCode "MedDRA:10002972:Apnea" ;
    rdfs:comment "Transient cessation of respiration." ;
    rdfs:subClassOf imdrf:E07 .

imdrf:E0704 a owl:Class ;
    rdfs:label "Aspiration/Inhalation" ;
    ex:nonIMDRFCode "MedDRA:10003504:Aspiration" ;
    rdfs:comment "The entry of foreign material past the trachea, and into the lower respiratory tract." ;
    rdfs:subClassOf imdrf:E07 .

imdrf:E0705 a owl:Class ;
    rdfs:label "Aspiration Pneumonitis" ;
    ex:nonIMDRFCode "MedDRA:10003526:Aspiration pneumonitis" ;
    rdfs:comment "Inflammation of the lungs due to the inhalation of solid or liquid material." ;
    rdfs:subClassOf imdrf:E07 .

imdrf:E0706 a owl:Class ;
    rdfs:label "Asthma" ;
    ex:nonIMDRFCode "MedDRA:10003553:Asthma" ;
    rdfs:comment "A chronic respiratory disease manifested as difficulty breathing due to the narrowing of bronchial passageways." ;
    rdfs:subClassOf imdrf:E07 .

imdrf:E0707 a owl:Class ;
    rdfs:label "Bronchial Hemorrhage" ;
    ex:nonIMDRFCode "MedDRA:10065757:Bronchial hemorrhage" ;
    rdfs:comment "Bleeding from the bronchial wall and/or lung parenchyma." ;
    rdfs:subClassOf imdrf:E05,
        imdrf:E07 .

imdrf:E0708 a owl:Class ;
    rdfs:label "Bronchitis" ;
    ex:nonIMDRFCode "MedDRA:10006451:Bronchitis" ;
    rdfs:comment "An acute or chronic inflammatory process affecting the bronchi." ;
    rdfs:subClassOf imdrf:E07 .

imdrf:E0709 a owl:Class ;
    rdfs:label "Bronchospasm" ;
    ex:nonIMDRFCode "MedDRA:10006482:Bronchospasm" ;
    rdfs:comment "Sudden contraction of the smooth muscles of the bronchial wall." ;
    rdfs:subClassOf imdrf:E07 .

imdrf:E0710 a owl:Class ;
    rdfs:label "Choking" ;
    ex:nonIMDRFCode "MedDRA:10008589:Choking" ;
    ex:statusDescription "Editorial change to the definition on 16 February 2021." ;
    rdfs:comment "Interference with respiration by obstruction of the larynx or trachea." ;
    rdfs:subClassOf imdrf:E07,
        imdrf:E20 .

imdrf:E071101 a owl:Class ;
    rdfs:label "Pulmonary Emphysema" ;
    ex:nonIMDRFCode "MedDRA:10014563:Emphysema pulmonary" ;
    rdfs:comment "A condition characterized by increase beyond normal in the size of air spaces distal to the terminal bronchioles, either from dilatation of the alveoli or from destruction of their walls." ;
    rdfs:subClassOf imdrf:E0711 .

imdrf:E0712 a owl:Class ;
    rdfs:label "Cough" ;
    ex:nonIMDRFCode "MedDRA:10011224:Cough" ;
    rdfs:comment "A sudden, often repetitive, spasmodic contraction of the thoracic cavity, resulting in violent release of air from the lungs, and usually accompanied by a distinctive sound." ;
    rdfs:subClassOf imdrf:E07 .

imdrf:E0713 a owl:Class ;
    rdfs:label "Decreased Peak Expiratory Flow rate" ;
    ex:nonIMDRFCode "MedDRA:10034195:Peak expiratory flow rate decreased" ;
    rdfs:comment "Decrease in the maximum flow rate generated during a forceful exhalation, starting from full lung inflation." ;
    rdfs:subClassOf imdrf:E07,
        imdrf:E22 .

imdrf:E0714 a owl:Class ;
    rdfs:label "Increased Peak Expiratory Flow rate" ;
    ex:nonIMDRFCode "MedDRA:10034196:Peak expiratory flow rate increased" ;
    rdfs:comment "An increase of the greatest rate of flow that can be achieved during forced expiration beginning with the lungs fully inflated." ;
    rdfs:subClassOf imdrf:E07,
        imdrf:E22 .

imdrf:E0715 a owl:Class ;
    rdfs:label "Decreased Respiratory Rate" ;
    ex:nonIMDRFCode "MedDRA:10038710:Respiratory rate decreased" ;
    rdfs:comment "Abnormal decrease of rate of breathing." ;
    rdfs:subClassOf imdrf:E07,
        imdrf:E22 .

imdrf:E0716 a owl:Class ;
    rdfs:label "Increased Respiratory Rate" ;
    ex:nonIMDRFCode "MedDRA:10038712:Respiratory rate increased" ;
    rdfs:comment "Abnormal increase of rate of breathing." ;
    rdfs:subClassOf imdrf:E07,
        imdrf:E22 .

imdrf:E0717 a owl:Class ;
    rdfs:label "Dyspnea" ;
    ex:nonIMDRFCode "MedDRA:10013963:Dyspnea" ;
    rdfs:comment "An uncomfortable sensation of difficulty breathing. It may present as an acute or chronic sign of an underlying respiratory or heart disorder." ;
    rdfs:subClassOf imdrf:E07 .

imdrf:E0718 a owl:Class ;
    rdfs:label "Epistaxis" ;
    ex:nonIMDRFCode "MedDRA:10015090:Epistaxis" ;
    rdfs:comment "Nose bleed." ;
    rdfs:subClassOf imdrf:E07 .

imdrf:E0719 a owl:Class ;
    rdfs:label "Forced Expiratory Volume Decreased" ;
    ex:nonIMDRFCode "MedDRA:10016987:Forced expiratory volume decreased" ;
    rdfs:comment "A decrease in the fraction of the forced vital capacity that is exhaled in a specific number of seconds." ;
    rdfs:subClassOf imdrf:E07,
        imdrf:E22 .

imdrf:E0720 a owl:Class ;
    rdfs:label "Forced Expiratory Volume Increased" ;
    ex:nonIMDRFCode "MedDRA:10016989:Forced expiratory volume increased" ;
    rdfs:comment "An increase in the fraction of the forced vital capacity that is exhaled in a specific number of seconds." ;
    rdfs:subClassOf imdrf:E07,
        imdrf:E22 .

imdrf:E0721 a owl:Class ;
    rdfs:label "Hemoptysis" ;
    ex:nonIMDRFCode "MedDRA:10019523:Hemoptysis" ;
    rdfs:comment "Coughing up blood from the respiratory tract." ;
    rdfs:subClassOf imdrf:E07 .

imdrf:E0722 a owl:Class ;
    rdfs:label "Hemothorax" ;
    ex:nonIMDRFCode "MedDRA:10019614:Hemothorax" ;
    rdfs:comment "A collection of blood in the pleural cavity." ;
    rdfs:subClassOf imdrf:E07 .

imdrf:E0723 a owl:Class ;
    rdfs:label "Hiccups" ;
    ex:nonIMDRFCode "MedDRA:10020039:Hiccups" ;
    rdfs:comment "An involuntary contraction of the diaphragm against closed vocal cords, producing the hic sound." ;
    rdfs:subClassOf imdrf:E07 .

imdrf:E0724 a owl:Class ;
    rdfs:label "Hyperventilation" ;
    ex:nonIMDRFCode "MedDRA:10020910:Hyperventilation" ;
    rdfs:comment "Abnormally prolonged, rapid, and deep breathing." ;
    rdfs:subClassOf imdrf:E07 .

imdrf:E0725 a owl:Class ;
    rdfs:label "Hypoventilation" ;
    ex:nonIMDRFCode "MedDRA:10021133:Hypoventilation" ;
    rdfs:comment "A state in which there is a reduced amount of air entering the pulmonary alveoli." ;
    rdfs:subClassOf imdrf:E07 .

imdrf:E0726 a owl:Class ;
    rdfs:label "Hypoxia" ;
    ex:nonIMDRFCode "MedDRA:10021143:Hypoxia" ;
    rdfs:comment "A deficiency in the amount of oxygen reaching the tissues." ;
    rdfs:subClassOf imdrf:E07 .

imdrf:E0727 a owl:Class ;
    rdfs:label "Mediastinal Shift" ;
    ex:nonIMDRFCode "MedDRA:10066239:Mediastinal shift" ;
    rdfs:comment "Displacement of structures in the thoracic cavity in one direction due to increased pleural pressure on the contralateral side." ;
    rdfs:subClassOf imdrf:E07 .

imdrf:E0728 a owl:Class ;
    rdfs:label "Nasal Obstruction" ;
    ex:nonIMDRFCode "MedDRA:10028748:Nasal obstruction" ;
    rdfs:comment "Blockage of the nasal passages." ;
    rdfs:subClassOf imdrf:E07 .

imdrf:E0729 a owl:Class ;
    rdfs:label "Overinflation of Lung" ;
    ex:nonIMDRFCode "MedDRA:10059487:Lung hyperinflation" ;
    rdfs:comment "Abnormal permanent enlargement of the lung air spaces distal to terminal bronchiole not resulted from wall destruction, e.g. due to loss of opposite lung." ;
    rdfs:subClassOf imdrf:E07 .

imdrf:E0730 a owl:Class ;
    rdfs:label "Pharyngitis" ;
    ex:nonIMDRFCode "MedDRA:10034835:Pharyngitis" ;
    rdfs:comment "Inflammation of the throat most often caused by viral and bacterial infections." ;
    rdfs:subClassOf imdrf:E07 .

imdrf:E0731 a owl:Class ;
    rdfs:label "Pleural Effusion" ;
    ex:nonIMDRFCode "MedDRA:10035598:Pleural effusion" ;
    rdfs:comment "Increased amounts of fluid within the pleural cavity. Symptoms include shortness of breath, cough, and chest pain." ;
    rdfs:subClassOf imdrf:E07 .

imdrf:E0732 a owl:Class ;
    rdfs:label "Pleural Empyema" ;
    ex:nonIMDRFCode "MedDRA:10090758:Pleural empyema" ;
    ex:status "Modified (editorial)" ;
    ex:statusDescription "MedDRA map modified for release No. 2025.  Previous MedDRA map was 10037381:Pulmonary empyema" ;
    rdfs:comment "An accumulation of pus in the pleural space" ;
    rdfs:subClassOf imdrf:E07 .

imdrf:E073301 a owl:Class ;
    rdfs:label "Bronchopneumonia" ;
    ex:nonIMDRFCode "MedDRA:10006469:Bronchopneumonia" ;
    rdfs:comment "Acute inflammation of the walls of the terminal bronchioles." ;
    rdfs:subClassOf imdrf:E0733 .

imdrf:E0734 a owl:Class ;
    rdfs:label "Pneumothorax" ;
    ex:nonIMDRFCode "MedDRA:10035759:Pneumothorax" ;
    rdfs:comment "Abnormal presence of air in the pleural cavity." ;
    rdfs:subClassOf imdrf:E07 .

imdrf:E0735 a owl:Class ;
    rdfs:label "Pulmonary Dysfunction" ;
    ex:nonIMDRFCode "MedDRA:10037386:Pulmonary function impairment" ;
    rdfs:comment "Impaired or abnormal functioning of the pulmonary system causing multiple pulmonary issues." ;
    rdfs:subClassOf imdrf:E07 .

imdrf:E0736 a owl:Class ;
    rdfs:label "Pulmonary Edema" ;
    ex:nonIMDRFCode "MedDRA:10037375:Pulmonary edema" ;
    rdfs:comment "Accumulation of fluid in the lung tissues causing disturbance of the gas exchange that may lead to respiratory failure." ;
    rdfs:subClassOf imdrf:E07,
        imdrf:E2338 .

imdrf:E0737 a owl:Class ;
    rdfs:label "Pulmonary Hypertension" ;
    ex:nonIMDRFCode "MedDRA:10037400:Pulmonary hypertension" ;
    rdfs:comment "Increased pressure within the pulmonary circulation due to lung or heart disorder." ;
    rdfs:subClassOf imdrf:E07 .

imdrf:E0738 a owl:Class ;
    rdfs:label "Pulmonary Infarction" ;
    ex:nonIMDRFCode "MedDRA:10037410:Pulmonary infarction" ;
    rdfs:comment "Localized necrosis of lung tissue caused by obstruction of the arterial blood supply, most often due to pulmonary embolism." ;
    rdfs:subClassOf imdrf:E07 .

imdrf:E0739 a owl:Class ;
    rdfs:label "Respiratory Acidosis" ;
    ex:nonIMDRFCode "MedDRA:10038661:Respiratory acidosis" ;
    rdfs:comment "A condition in which the blood pH is less than normal, secondary to impaired gas exchange." ;
    rdfs:subClassOf imdrf:E07,
        imdrf:E12 .

imdrf:E0740 a owl:Class ;
    rdfs:label "Respiratory Alkalosis" ;
    ex:nonIMDRFCode "MedDRA:10038664:Respiratory alkalosis" ;
    rdfs:comment "A condition in which the blood pH is greater than normal, secondary to impaired gas exchange." ;
    rdfs:subClassOf imdrf:E07,
        imdrf:E12 .

imdrf:E0741 a owl:Class ;
    rdfs:label "Respiratory Arrest" ;
    ex:nonIMDRFCode "MedDRA:10038669:Respiratory arrest" ;
    rdfs:comment "Cessation of breathing function." ;
    rdfs:subClassOf imdrf:E07 .

imdrf:E0742 a owl:Class ;
    rdfs:label "Respiratory Failure" ;
    ex:nonIMDRFCode "MedDRA:10038695:Respiratory failure" ;
    rdfs:comment "The significant impairment of gas exchange within the lungs resulting in hypoxia, hypercarbia, or both, to the extent that organ tissue perfusion is severely compromised." ;
    rdfs:subClassOf imdrf:E07 .

imdrf:E0743 a owl:Class ;
    rdfs:label "Respiratory Insufficiency" ;
    ex:nonIMDRFCode "MedDRA:10038701:Respiratory insufficiency" ;
    rdfs:comment "Impairment of gas exchange within the lungs secondary to a disease process, neoplasm, or trauma, possibly resulting in hypoxia, hypercarbia, or both." ;
    rdfs:subClassOf imdrf:E07 .

imdrf:E0744 a owl:Class ;
    rdfs:label "Respiratory Tract Infection" ;
    ex:nonIMDRFCode "MedDRA:10062352:Respiratory tract infection" ;
    rdfs:comment "An infectious disease affecting the respiratory tract." ;
    rdfs:subClassOf imdrf:E07,
        imdrf:E19 .

imdrf:E0745 a owl:Class ;
    rdfs:label "Sinus Perforation" ;
    ex:nonIMDRFCode "MedDRA:10040748:Sinus perforation" ;
    rdfs:comment "A rupture in the sinus tissue due to traumatic or pathologic processes." ;
    rdfs:subClassOf imdrf:E07,
        imdrf:E2114 .

imdrf:E0746 a owl:Class ;
    rdfs:label "Sneezing" ;
    ex:nonIMDRFCode "MedDRA:10041232:Sneezing" ;
    rdfs:comment "A symptom consisting of the involuntary expulsion of air from the nose." ;
    rdfs:subClassOf imdrf:E07 .

imdrf:E0747 a owl:Class ;
    rdfs:label "Sore Throat" ;
    ex:nonIMDRFCode "MedDRA:10041367:Sore throat" ;
    rdfs:comment "Any kind of inflammatory process of the tonsils, pharynx, or/and larynx characterized by pain in swallowing." ;
    rdfs:subClassOf imdrf:E07 .

imdrf:E0748 a owl:Class ;
    rdfs:label "Stacking Breaths" ;
    ex:nonIMDRFCode "MedDRA:10068523:Breath stacking" ;
    rdfs:comment "Condition where there are a greater number of inhalations relative to the number of exhalations." ;
    rdfs:subClassOf imdrf:E07 .

imdrf:E0749 a owl:Class ;
    rdfs:label "Strangulation" ;
    ex:nonIMDRFCode "MedDRA:10042169:Strangulation" ;
    ex:statusDescription "Editorial change to the definition on 16 February 2021." ;
    rdfs:comment "Interference with respiration by compression of the larynx, laryngopharynx or trachea, as well as of the carotid arteria or jugular veins." ;
    rdfs:subClassOf imdrf:E07,
        imdrf:E20 .

imdrf:E0750 a owl:Class ;
    rdfs:label "Ventilator Dependent" ;
    ex:nonIMDRFCode "MedDRA:10080927:Dependence on ventilator" ;
    rdfs:comment "A condition that requires mechanical life support due to inability to breath effectively to maintain normal levels of oxygen and carbon dioxide in the body." ;
    rdfs:subClassOf imdrf:E07 .

imdrf:E0751 a owl:Class ;
    rdfs:label "Wheezing" ;
    ex:nonIMDRFCode "MedDRA:10047924:Wheezing" ;
    ex:statusDescription "Definition modified for Release Number 2024. See no. 60 of Change Log" ;
    rdfs:comment "A symptom and finding during physical examination, characterized by high-pitched, whistling sound during breathing. It results from narrowing or obstruction of the respiratory airways.  Also known as stridor." ;
    rdfs:subClassOf imdrf:E07 .

imdrf:E0752 a owl:Class ;
    rdfs:label "Unspecified Respiratory Problem" ;
    ex:statusDescription "Term was added on 18 March 2020 for cases where the category of a health effect was reported but with no further details." ;
    rdfs:comment "The report describes a non-specific problem with the respiratory system. Note: Please use \"Appropriate Term / Code Not Available\" if the report describes a specific problem but the relevant term does not exist." ;
    rdfs:subClassOf imdrf:E07 .

imdrf:E0753 a owl:Class ;
    rdfs:label "Upper Respiratory Tract Injury" ;
    ex:status "Retired" ;
    ex:statusDescription "Term was added on 27 January 2022. For details, see comment No. 103 of the Change Log (Release Number 2022). Term retired for Release Number 2025. For mechanical injury use E0759 Mechanical Respiratory Tract Injury. For chemical injuries or exposure use E170401 - Caustic/Chemical Burns or E2003 - Chemical Exposure. See no. 86 of Change Request Log" ;
    rdfs:comment "Mechanical or chemical injuries to the upper airways, including trachea, pharynx and larynx." ;
    rdfs:subClassOf imdrf:E07 .

imdrf:E0754 a owl:Class ;
    rdfs:label "Upper Respiratory Tract Irritation" ;
    ex:nonIMDRFCode "MedDRA:10070841:Upper respiratory tract irritation" ;
    ex:statusDescription "Term added for Release Number 2024. See no. 1 of Change Log" ;
    rdfs:comment "Irritation and swelling of the upper airways" ;
    rdfs:subClassOf imdrf:E07 .

imdrf:E0755 a owl:Class ;
    rdfs:label "Snoring" ;
    ex:nonIMDRFCode "MedDRA:10041235:Snoring" ;
    ex:statusDescription "Term added for Release Number 2024. See no. 2 of Change Log" ;
    rdfs:comment "A particular type of noisy sound made by air passage across relaxed tissues during sleep." ;
    rdfs:subClassOf imdrf:E07 .

imdrf:E0756 a owl:Class ;
    rdfs:label "Nasal congestion" ;
    ex:nonIMDRFCode "MedDRA:10028735:Nasal congestion" ;
    ex:statusDescription "Term added for Release Number 2024. See no. 21 of Change Log" ;
    rdfs:comment "The blockage of the nasal passage due to mucosal edema. It is usually the result of a viral infection or an allergic reaction." ;
    rdfs:subClassOf imdrf:E07 .

imdrf:E0757 a owl:Class ;
    rdfs:label "Breathing-related sleep disorder" ;
    ex:nonIMDRFCode "MedDRA:10006344:Breathing-related sleep disorder" ;
    ex:statusDescription "Term added for Release Number 2024. See no. 61 of Change Log" ;
    rdfs:comment "Clinical spectrum with frequent episodes of either complete or partial obstruction of the upper airway during sleep. Includes sleep apnea. Also known as Sleep disordered breathing (SDB)." ;
    rdfs:subClassOf imdrf:E07 .

imdrf:E0758 a owl:Class ;
    rdfs:label "Rhinitis" ;
    ex:nonIMDRFCode "MedDRA:10039083:Rhinitis" ;
    ex:statusDescription "Term added for Release Number 2024. See no. 62 of Change Log" ;
    rdfs:comment "Pattern of symptoms as a result of nasal inflammation and/or dysfunction of the nasal mucosa. There are various subtypes, such as allergic, infectious and non-allergic (e.g. atrophic) rhinitis." ;
    rdfs:subClassOf imdrf:E07 .

imdrf:E0759 a owl:Class ;
    rdfs:label "Mechanical Respiratory Tract Injury" ;
    ex:nonIMDRFCode "MedDRA:10081319:Respiratory tract procedural complication" ;
    ex:status "New" ;
    ex:statusDescription "Term added for Release Number 2025. See no. 86 of Change Request Log" ;
    rdfs:comment "Mechanical injuries to the upper and/or lower airways. For chemical injuries or exposure use E170401 - Caustic/Chemical Burns or E2003 - Chemical Exposure" ;
    rdfs:subClassOf imdrf:E07 .

imdrf:E0760 a owl:Class ;
    rdfs:label "Atelectasis" ;
    ex:nonIMDRFCode "MedDRA:10003598:Atelectasis" ;
    ex:status "New" ;
    ex:statusDescription "Term added for Release Number 2025. See no. 88 of Change Request Log" ;
    rdfs:comment "Incomplete expansion of a lung or a portion of a lung; or portion of the lung collapses or becomes airless, often due to a blockage in the airway." ;
    rdfs:subClassOf imdrf:E07 .

imdrf:E0761 a owl:Class ;
    rdfs:label "Nasal Dryness" ;
    ex:nonIMDRFCode "MedDRA:10028740:Nasal dryness" ;
    ex:status "New" ;
    ex:statusDescription "Term added for Release Number 2025. See no. 101 of Change Request Log" ;
    rdfs:comment "Lack of moisture in the nasal mucosa" ;
    rdfs:subClassOf imdrf:E07 .

imdrf:E0801 a owl:Class ;
    rdfs:label "Capsular Bag Tear" ;
    ex:nonIMDRFCode "MedDRA:10063941:Posterior capsule tear" ;
    rdfs:comment "A tear in the capsular bag housing the lens." ;
    rdfs:subClassOf imdrf:E08 .

imdrf:E0802 a owl:Class ;
    rdfs:label "Cataract" ;
    ex:nonIMDRFCode "MedDRA:10007739:Cataract" ;
    rdfs:comment "Partial or complete opacity of the crystalline lens of one or both eyes that decreases visual acuity and eventually results in blindness. Some cataracts appear in infancy or in childhood, but most develop in older individuals. (Sternberg Diagnostic Surgical Pathology, 3rd ed.)" ;
    rdfs:subClassOf imdrf:E08 .

imdrf:E0803 a owl:Class ;
    rdfs:label "Chemosis" ;
    ex:nonIMDRFCode "MedDRA:10008435:Chemosis" ;
    rdfs:comment "Edema of the mucous membrane of the eyeball and eyelid lining." ;
    rdfs:subClassOf imdrf:E08,
        imdrf:E19 .

imdrf:E0804 a owl:Class ;
    rdfs:label "Conjunctivitis" ;
    ex:nonIMDRFCode "MedDRA:10010741:Conjunctivitis" ;
    rdfs:comment "Inflammation of the conjunctiva of the eye." ;
    rdfs:subClassOf imdrf:E08 .

imdrf:E0805 a owl:Class ;
    rdfs:label "Corneal Clouding/Hazing" ;
    ex:nonIMDRFCode "MedDRA:10052116:Corneal clouding" ;
    rdfs:comment "Clouding of the middle area of the cornea, usually as a result of scarring due to infection, injury, or inflammation." ;
    rdfs:subClassOf imdrf:E08 .

imdrf:E0806 a owl:Class ;
    rdfs:label "Corneal Decompensation" ;
    ex:nonIMDRFCode "MedDRA:10052117:Corneal decompensation" ;
    rdfs:comment "Inability to maintain corneal integrity; or corneal edema resulting from failure of the corneal endothelium to maintain detumescence." ;
    rdfs:subClassOf imdrf:E08 .

imdrf:E080701 a owl:Class ;
    rdfs:label "Corneal Stromal Edema" ;
    ex:nonIMDRFCode "MedDRA:10054772:Corneal stromal edema" ;
    rdfs:comment "Fluid from the aqueous humor enters the corneal stroma and causes swelling." ;
    rdfs:subClassOf imdrf:E0807,
        imdrf:E2338 .

imdrf:E080702 a owl:Class ;
    rdfs:label "Microcystic Edema" ;
    ex:nonIMDRFCode "MedDRA:10068529:Corneal microcystic edema" ;
    rdfs:comment "Corneal edema of inflammatory origin associated with contact lens wear and morphologically characterized by presence of epithelial microcysts." ;
    rdfs:subClassOf imdrf:E0807,
        imdrf:E2338 .

imdrf:E0808 a owl:Class ;
    rdfs:label "Corneal Epithelial Microcysts" ;
    ex:nonIMDRFCode "MedDRA:10068144:Corneal epithelial microcysts" ;
    rdfs:comment "Very small, round vesicles containing fluid and cellular debris observed on the surface of the cornea under slit lamp examination in some types of corneal dystrophy and in wearers of extended wear lenses." ;
    rdfs:subClassOf imdrf:E08 .

imdrf:E0809 a owl:Class ;
    rdfs:label "Corneal Infiltrates" ;
    ex:nonIMDRFCode "MedDRA:10011022:Corneal infiltrates" ;
    rdfs:comment "Discrete, small lesions present in the cornea as a result of corneal inflammation and, in some cases, after soft contact lens wear especially extended-wear lenses." ;
    rdfs:subClassOf imdrf:E08 .

imdrf:E0810 a owl:Class ;
    rdfs:label "Corneal Pannus" ;
    ex:nonIMDRFCode "MedDRA:10033682:Pannus (corneal)" ;
    rdfs:comment "Superficial vascularization of the cornea with infiltration of granulation tissue." ;
    rdfs:subClassOf imdrf:E08 .

imdrf:E0811 a owl:Class ;
    rdfs:label "Corneal Perforation" ;
    ex:nonIMDRFCode "MedDRA:10011039:Corneal perforation" ;
    rdfs:comment "A rupture in the corneal tissue due to traumatic or pathologic processes." ;
    rdfs:subClassOf imdrf:E08,
        imdrf:E2114 .

imdrf:E0812 a owl:Class ;
    rdfs:label "Corneal Scar" ;
    ex:nonIMDRFCode "MedDRA:10011044:Corneal scar" ;
    rdfs:comment "Replacement of corneal tissue with scar tissue as a result of injury to the deeper layers of the cornea." ;
    rdfs:subClassOf imdrf:E08 .

imdrf:E0813 a owl:Class ;
    rdfs:label "Corneal Touch" ;
    ex:nonIMDRFCode "MedDRA:10011055:Corneal touch" ;
    rdfs:comment "Complications of intraocular lens surgery; usually refers to intraocular lens contact with cornea, can be intermittent or chronic." ;
    rdfs:subClassOf imdrf:E08 .

imdrf:E0814 a owl:Class ;
    rdfs:label "Corneal Ulcer" ;
    ex:nonIMDRFCode "MedDRA:10048492:Corneal ulcer" ;
    rdfs:comment "Area of epithelial tissue loss from corneal surface; associated with inflammatory cells in the cornea and anterior chamber." ;
    rdfs:subClassOf imdrf:E08 .

imdrf:E0815 a owl:Class ;
    rdfs:label "Dry Eye(s)" ;
    ex:nonIMDRFCode "MedDRA:10013774:Dry eye" ;
    rdfs:comment "A syndrome characterized by dryness of the cornea and conjunctiva. It is usually caused by a deficiency in tear production. Symptoms include a feeling of burning eyes and a possible foreign body presence in the eye." ;
    rdfs:subClassOf imdrf:E08 .

imdrf:E0816 a owl:Class ;
    rdfs:label "Endophthalmitis" ;
    ex:nonIMDRFCode "MedDRA:10014801:Endophthalmitis" ;
    rdfs:comment "Inflammation of the intraocular fluids or tissues usually with microbial organisms." ;
    rdfs:subClassOf imdrf:E08,
        imdrf:E19 .

imdrf:E0817 a owl:Class ;
    rdfs:label "Excessive Tear Production" ;
    ex:nonIMDRFCode "MedDRA:10015591:Excess tears" ;
    rdfs:comment "Profuse lacrimation." ;
    rdfs:subClassOf imdrf:E08 .

imdrf:E081801 a owl:Class ;
    rdfs:label "Intraocular Infection" ;
    ex:nonIMDRFCode "MedDRA:10054762:Eye infection intraocular" ;
    rdfs:comment "Infection within the eye." ;
    rdfs:subClassOf imdrf:E0818 .

imdrf:E081901 a owl:Class ;
    rdfs:label "Corneal Abrasion" ;
    ex:nonIMDRFCode "MedDRA:10010984:Corneal abrasion" ;
    rdfs:comment "Injury to the epithelium of the cornea." ;
    rdfs:subClassOf imdrf:E0819 .

imdrf:E081902 a owl:Class ;
    rdfs:label "Eye Burn" ;
    ex:nonIMDRFCode "MedDRA:10015911:Eye burns" ;
    rdfs:comment "Burn injury, including chemical burn, to any part of the eye." ;
    rdfs:subClassOf imdrf:E0819 .

imdrf:E081903 a owl:Class ;
    rdfs:label "Retinal Detachment" ;
    ex:nonIMDRFCode "MedDRA:10038848:Retinal detachment" ;
    rdfs:comment "Separation of the inner retina layers from the underlying pigment epithelium." ;
    rdfs:subClassOf imdrf:E0819 .

imdrf:E081904 a owl:Class ;
    rdfs:label "Retinal Injury" ;
    ex:nonIMDRFCode "MedDRA:10057430:Retinal injury" ;
    rdfs:comment "Damage to the retina due to toxicity, exposure to bright lights, or trauma." ;
    rdfs:subClassOf imdrf:E0819 .

imdrf:E081905 a owl:Class ;
    rdfs:label "Retinal Tear" ;
    ex:nonIMDRFCode "MedDRA:10038897:Retinal tear" ;
    rdfs:comment "A usually small tearing of the retina occurring when the vitreous separates from the retina. It may lead to retinal detachment." ;
    rdfs:subClassOf imdrf:E0819 .

imdrf:E081906 a owl:Class ;
    rdfs:label "Vitreous Detachment" ;
    ex:nonIMDRFCode "MedDRA:10047650:Vitreous detachment" ;
    rdfs:comment "Detachment of the vitreous humor from the retina." ;
    rdfs:subClassOf imdrf:E0819,
        imdrf:E21 .

imdrf:E0820 a owl:Class ;
    rdfs:label "Eye Pain" ;
    ex:nonIMDRFCode "MedDRA:10015958:Eye pain" ;
    rdfs:comment "Painful sensation in the eye." ;
    rdfs:subClassOf imdrf:E08,
        imdrf:E2330 .

imdrf:E0821 a owl:Class ;
    rdfs:label "Foreign Body Sensation in Eye" ;
    ex:nonIMDRFCode "MedDRA:10051116:Foreign body sensation in eyes" ;
    rdfs:comment "Feeling of grittiness or having something in the eye; frequently caused by a foreign body." ;
    rdfs:subClassOf imdrf:E08 .

imdrf:E0822 a owl:Class ;
    rdfs:label "Glaucoma" ;
    ex:nonIMDRFCode "MedDRA:10018304:Glaucoma" ;
    rdfs:comment "Increased pressure in the eyeball due to obstruction of the outflow of aqueous humor." ;
    rdfs:subClassOf imdrf:E08 .

imdrf:E0823 a owl:Class ;
    rdfs:label "Halo" ;
    ex:nonIMDRFCode "MedDRA:10019099:Halo vision" ;
    rdfs:comment "Hazy ring around bright lights seen by some patients with refractive error or optical defects, e.g. cataracts, or corneal swelling." ;
    rdfs:subClassOf imdrf:E08 .

imdrf:E0824 a owl:Class ;
    rdfs:label "Hyphema" ;
    ex:nonIMDRFCode "MedDRA:10020924:Hyphema" ;
    ex:statusDescription "Definition was modified on 31 January 2023 to remove \"bloodshot\". For details, see comment No. 139 of the Change Log (Release Number 2023)." ;
    rdfs:comment "Hemorrhage within the anterior chamber of the eye." ;
    rdfs:subClassOf imdrf:E08 .

imdrf:E0825 a owl:Class ;
    rdfs:label "Hypopyon" ;
    ex:nonIMDRFCode "MedDRA:10021086:Hypopyon" ;
    rdfs:comment "An accumulation of pus in the anterior chamber of the eye." ;
    rdfs:subClassOf imdrf:E08 .

imdrf:E0826 a owl:Class ;
    rdfs:label "Intraocular Pressure Decreased" ;
    ex:nonIMDRFCode "MedDRA:10022804:Intraocular pressure decreased" ;
    rdfs:comment "Decrease of pressure of the intraocular fluid in the eye." ;
    rdfs:subClassOf imdrf:E08 .

imdrf:E0827 a owl:Class ;
    rdfs:label "Intraocular Pressure Increased" ;
    ex:nonIMDRFCode "MedDRA:10022806:Intraocular pressure increased" ;
    ex:statusDescription "Definition was modified on 31 January 2023 (Old definition: Increase of pressure of the intraocular fluid in the eye.). For details, see comment No. 108 of the Change Log (Release Number 2023)." ;
    rdfs:comment "Increase of pressure of the intraocular fluid in the eye, also known as ocular hypertension." ;
    rdfs:subClassOf imdrf:E08 .

imdrf:E0828 a owl:Class ;
    rdfs:label "Iritis" ;
    ex:nonIMDRFCode "MedDRA:10022955:Iritis" ;
    rdfs:comment "Inflammation of the iris." ;
    rdfs:subClassOf imdrf:E08 .

imdrf:E082901 a owl:Class ;
    rdfs:label "Infective Keratitis" ;
    ex:nonIMDRFCode "MedDRA:10076672:Infective keratitis" ;
    ex:statusDescription "Term/Definition was modified on 27 January 2022 (Old term/definition: Acanthamoeba Keratitis: Keratitis due to infection by acanthamoeba.) MedDRA mapping also updated from Acanthameba keratitis(10074137) to Infective keratitis(10076672). For details, see comment No. 252 of the Change Log (Release Number 2022)." ;
    rdfs:comment "Keratitis due to infection, including infection by acanthamoeba." ;
    rdfs:subClassOf imdrf:E0829 .

imdrf:E0830 a owl:Class ;
    rdfs:label "Macular Edema" ;
    ex:nonIMDRFCode "MedDRA:10054467:Macular edema" ;
    rdfs:comment "Accumulation of intraretinal fluid and protein in the macula, which may result in swelling and decreased central vision." ;
    rdfs:subClassOf imdrf:E08,
        imdrf:E2338 .

imdrf:E0831 a owl:Class ;
    rdfs:label "Overwear Syndrome" ;
    ex:nonIMDRFCode "MedDRA:10080905:Overwear syndrome" ;
    rdfs:comment "Ocular pain which may be very intense, accompanied by corneal epithelium damage, conjunctival injection, lacrimation, blepharospasm, photophobia and hazy vision following corneal edema caused by overwear of contact lenses, principally the PMMA type." ;
    rdfs:subClassOf imdrf:E08 .

imdrf:E0832 a owl:Class ;
    rdfs:label "Pupillary Block" ;
    ex:nonIMDRFCode "MedDRA:10037520:Pupillary block" ;
    rdfs:comment "An obstruction of the pupil." ;
    rdfs:subClassOf imdrf:E08 .

imdrf:E0833 a owl:Class ;
    rdfs:label "Red Eye(s)" ;
    ex:nonIMDRFCode "MedDRA:10038189:Red eye" ;
    rdfs:comment "Lay term applied to any condition with dilation of conjunctival or ciliary blood vessels; innumerable causes." ;
    rdfs:subClassOf imdrf:E08 .

imdrf:E0834 a owl:Class ;
    rdfs:label "Retinal Degeneration" ;
    ex:nonIMDRFCode "MedDRA:10038845:Retinal degeneration" ;
    rdfs:comment "Degeneration of the retina." ;
    rdfs:subClassOf imdrf:E08 .

imdrf:E0835 a owl:Class ;
    rdfs:label "Toxic Anterior Segment Syndrome (TASS)" ;
    ex:nonIMDRFCode "MedDRA:10066366:Toxic anterior segment syndrome" ;
    ex:statusDescription "Editorial change to the definition on 16 February 2021." ;
    rdfs:comment "An acute postoperative inflammatory reaction in which a noninfectious substance enters the anterior segment and induces toxic damage to the intraocular tissues." ;
    rdfs:subClassOf imdrf:E08 .

imdrf:E0836 a owl:Class ;
    rdfs:label "UGH (Uveitis Glaucoma Hyphema) Syndrome" ;
    ex:nonIMDRFCode "MedDRA:10068156:Uveitis-glaucoma-hyphema syndrome" ;
    rdfs:comment "Clinical triad of uveitis, glaucoma, and hyphema (UGH), especially associated with the insertion of an anterior chamber intraocular lens (IOL)." ;
    rdfs:subClassOf imdrf:E08 .

imdrf:E0837 a owl:Class ;
    rdfs:label "Uveitis" ;
    ex:nonIMDRFCode "MedDRA:10046851:Uveitis" ;
    rdfs:comment "Inflammation of the uvea." ;
    rdfs:subClassOf imdrf:E08 .

imdrf:E083801 a owl:Class ;
    rdfs:label "Flashers" ;
    ex:nonIMDRFCode "MedDRA:10047569:Visual flashes" ;
    rdfs:comment "The perception of sudden or brief bursts of light." ;
    rdfs:subClassOf imdrf:E0838 .

imdrf:E083802 a owl:Class ;
    rdfs:label "Phosphene Visualization" ;
    ex:nonIMDRFCode "MedDRA:10034936:Phosphenes" ;
    rdfs:comment "An objective visual sensation that appears with the eyes closed and in the absence of visual light." ;
    rdfs:subClassOf imdrf:E0838,
        imdrf:E23 .

imdrf:E083803 a owl:Class ;
    rdfs:label "Vitreous Floaters" ;
    ex:nonIMDRFCode "MedDRA:10047654:Vitreous floaters" ;
    rdfs:comment "Spots or stringy shapes in vision, often caused by deposits, aggregates, or cell fragments in the vitreous humor or lens." ;
    rdfs:subClassOf imdrf:E0838 .

imdrf:E083804 a owl:Class ;
    rdfs:label "Photophobia" ;
    ex:nonIMDRFCode "MedDRA:10034960:Photophobia" ;
    ex:statusDescription "Term was added on 27 January 2022. For details, see comment No. 251 of the Change Log (Release Number 2022)." ;
    rdfs:comment "Increased sensitivity of the eyes to light causing discomfort or pain." ;
    rdfs:subClassOf imdrf:E0838 .

imdrf:E083901 a owl:Class ;
    rdfs:label "Blurred Vision" ;
    ex:nonIMDRFCode "MedDRA:10005886:Blurred vision" ;
    rdfs:comment "The loss of visual acuity (sharpness of vision)." ;
    rdfs:subClassOf imdrf:E0839 .

imdrf:E083902 a owl:Class ;
    rdfs:label "Loss of Vision" ;
    ex:nonIMDRFCode "MedDRA:10024881:Loss of vision" ;
    rdfs:comment "Severely reduced visual acuity that cannot be corrected, or total loss of vision." ;
    rdfs:subClassOf imdrf:E0839 .

imdrf:E083903 a owl:Class ;
    rdfs:label "Diplopia/Double Vision" ;
    ex:nonIMDRFCode "MedDRA:10013036:Diplopia" ;
    ex:statusDescription "Term was added on 27 January 2022. For details, see comment No. 130 of the Change Log (Release Number 2022)." ;
    rdfs:comment "Perception of multiple images from one object." ;
    rdfs:subClassOf imdrf:E0839 .

imdrf:E0840 a owl:Class ;
    rdfs:label "Vitreous Hemorrhage" ;
    ex:nonIMDRFCode "MedDRA:10047656:Vitreous hemorrhage" ;
    rdfs:comment "Blood extravasation in the vitreous humor." ;
    rdfs:subClassOf imdrf:E08 .

imdrf:E0841 a owl:Class ;
    rdfs:label "Vitreous Loss" ;
    ex:nonIMDRFCode "MedDRA:10063942:Vitreous loss" ;
    rdfs:comment "loss or prolapse of vitreous gel." ;
    rdfs:subClassOf imdrf:E08 .

imdrf:E0842 a owl:Class ;
    rdfs:label "Vitritis" ;
    ex:nonIMDRFCode "MedDRA:10047663:Vitritis" ;
    rdfs:comment "Inflammatory intraocular reaction with clouding and cells in vitreous; often accompanies inflammation of ciliary body, iris, choroid, or retina." ;
    rdfs:subClassOf imdrf:E08 .

imdrf:E0843 a owl:Class ;
    rdfs:label "Zonular Dehiscence" ;
    ex:nonIMDRFCode "MedDRA:10068351:Ciliary zonular dehiscence" ;
    ex:statusDescription "Editorial change to the definition on 16 February 2021." ;
    rdfs:comment "Rupture of the fibrous strands connecting the ciliary body with the crystalline lens of the eye (usually at the time of cataract surgery)." ;
    rdfs:subClassOf imdrf:E08 .

imdrf:E0844 a owl:Class ;
    rdfs:label "Unspecified Eye / Vision Problem" ;
    ex:statusDescription "Term was added on 18 March 2020 for cases where the category of a health effect was reported but with no further details." ;
    rdfs:comment "The report describes a non-specific problem with the eye(s) or vision. Note: Please use \"Appropriate Term / Code Not Available\" if the report describes a specific problem but the relevant term does not exist." ;
    rdfs:subClassOf imdrf:E08 .

imdrf:E0845 a owl:Class ;
    rdfs:label "Eye Irritation" ;
    ex:nonIMDRFCode "MedDRA:10015946:Eye irritation" ;
    ex:status "Modified (technical)" ;
    ex:statusDescription "Definition was modified on 31 January 2023 to add \"abnormal\". For details, see comment No. 103 of the Change Log (Release Number 2023). Definition modified for Release Number 2025. See no. 102 of Change Request Log" ;
    rdfs:comment "A generic term used to describe abnormal sensations that bother the eyes like dryness, itchiness, burning, grittiness and excessive blinking." ;
    rdfs:subClassOf imdrf:E08 .

imdrf:E0846 a owl:Class ;
    rdfs:label "Corneal Thinning" ;
    ex:nonIMDRFCode "MedDRA:10054760:Corneal thinning" ;
    ex:statusDescription "Term was added on 27 January 2022. For details, see comment No. 126 of the Change Log (Release Number 2022)." ;
    rdfs:comment "Progressive deformation of the corneal structure, characterized by thinning of the cornea." ;
    rdfs:subClassOf imdrf:E08 .

imdrf:E0847 a owl:Class ;
    rdfs:label "Pigment Dispersion Syndrome" ;
    ex:nonIMDRFCode "MedDRA:10052134:Pigment dispersion syndrome" ;
    ex:statusDescription "Term was added on 27 January 2022. For details, see comment No. 127 of the Change Log (Release Number 2022)." ;
    rdfs:comment "Condition where iris pigment is released into the anterior chamber and deposited in the trabecular meshwork, due to a procedure or device implantation." ;
    rdfs:subClassOf imdrf:E08,
        imdrf:E21 .

imdrf:E0848 a owl:Class ;
    rdfs:label "Corneal Endothelial Cell Loss" ;
    ex:nonIMDRFCode "MedDRA:10071681:Corneal endothelial cell loss" ;
    ex:statusDescription "Term was added on 27 January 2022. For details, see comment No. 129 of the Change Log (Release Number 2022)." ;
    rdfs:comment "Decrease in corneal endothelial cell density." ;
    rdfs:subClassOf imdrf:E08,
        imdrf:E21 .

imdrf:E0849 a owl:Class ;
    rdfs:label "Posterior Capsule Opacification" ;
    ex:nonIMDRFCode "MedDRA:10036346:Posterior capsule opacification" ;
    ex:statusDescription "Term was added on 27 January 2022. For details, see comment No. 131 of the Change Log (Release Number 2022)." ;
    rdfs:comment "Remnant lens epithelial cell proliferation and migration to the posterior capsule." ;
    rdfs:subClassOf imdrf:E08,
        imdrf:E21 .

imdrf:E0850 a owl:Class ;
    rdfs:label "Conjunctival Hemorrhage" ;
    ex:nonIMDRFCode "MedDRA:10010720:Conjunctival hemorrhage" ;
    ex:statusDescription "Term was added on 27 January 2022. For details, see comment No. 136 of the Change Log (Release Number 2022)." ;
    rdfs:comment "Blood extravasation in the conjunctiva." ;
    rdfs:subClassOf imdrf:E05,
        imdrf:E08 .

imdrf:E0851 a owl:Class ;
    rdfs:label "Retinal Hemorrhage" ;
    ex:nonIMDRFCode "MedDRA:10038870:Retinal hemorrhage" ;
    ex:statusDescription "Term was added on 27 January 2022. For details, see comment No. 137 of the Change Log (Release Number 2022)." ;
    rdfs:comment "Blood extravasation in the retina." ;
    rdfs:subClassOf imdrf:E05,
        imdrf:E08 .

imdrf:E0852 a owl:Class ;
    rdfs:label "Choroidal Hemorrhage" ;
    ex:nonIMDRFCode "MedDRA:10055239:Choroidal hemorrhage" ;
    ex:statusDescription "Term was added on 27 January 2022. For details, see comment No. 138 of the Change Log (Release Number 2022)." ;
    rdfs:comment "Blood extravasation in the choroid." ;
    rdfs:subClassOf imdrf:E05,
        imdrf:E08 .

imdrf:E0853 a owl:Class ;
    rdfs:label "Optic Nerve Sheath Hemorrhage" ;
    ex:nonIMDRFCode "MedDRA:10054519:Optic nerve sheath hemorrhage" ;
    ex:statusDescription "Term was added on 27 January 2022. For details, see comment No. 139 of the Change Log (Release Number 2022)." ;
    rdfs:comment "Blood extravasation in the Optic Nerve Sheath." ;
    rdfs:subClassOf imdrf:E05,
        imdrf:E08 .

imdrf:E0854 a owl:Class ;
    rdfs:label "Mydriasis" ;
    ex:nonIMDRFCode "MedDRA:10028521:Mydriasis" ;
    ex:statusDescription "Term was added on 31 January 2023. For details, see comment No. 107 of the Change Log (Release Number 2023)." ;
    rdfs:comment "Dilated pupils" ;
    rdfs:subClassOf imdrf:E08 .

imdrf:E0855 a owl:Class ;
    rdfs:label "Anterior Capsule Opacification" ;
    ex:nonIMDRFCode "MedDRA:10088740:Anterior capsule opacification" ;
    ex:statusDescription "Term was added on 31 January 2023. For details, see comment No. 119 / 121 of the Change Log (Release Number 2023)." ;
    rdfs:comment "Remnant lens epithelial cell proliferation of the anterior capsule." ;
    rdfs:subClassOf imdrf:E08 .

imdrf:E0856 a owl:Class ;
    rdfs:label "Pupillary Disorder" ;
    ex:nonIMDRFCode "MedDRA:10037521:Pupillary disorder" ;
    ex:statusDescription "Term was added on 31 January 2023. For details, see comment No. 120 of the Change Log (Release Number 2023)." ;
    rdfs:comment "Condition which affects the structures or function of the pupil of the eye." ;
    rdfs:subClassOf imdrf:E08 .

imdrf:E0857 a owl:Class ;
    rdfs:label "Corneal Warpage" ;
    ex:nonIMDRFCode "MedDRA:10075404:Corneal warpage" ;
    ex:statusDescription "Term was added on 31 January 2023. For details, see comment No. 129 of the Change Log (Release Number 2023)." ;
    rdfs:comment "A change in the shape of the corneal surface presenting as abnormal radial symmetry." ;
    rdfs:subClassOf imdrf:E08 .

imdrf:E0858 a owl:Class ;
    rdfs:label "Choroidal detachment" ;
    ex:nonIMDRFCode "MedDRA:10008783:Choroidal detachment" ;
    ex:statusDescription "Term added for Release Number 2024. See no. 7 of Change Log" ;
    rdfs:comment "A detachment of the choroid from the underlying sclera often due to the accumulation of fluid (blood for hemorrhagic, other fluids for serous detachment) in the suprachoroidal space" ;
    rdfs:subClassOf imdrf:E08 .

imdrf:E0859 a owl:Class ;
    rdfs:label "Choroidal effusion" ;
    ex:nonIMDRFCode "MedDRA:10063970:Choroidal effusion" ;
    ex:statusDescription "Term added for Release Number 2024. See no. 8 of Change Log" ;
    rdfs:comment "Fluid accumulation in the suprachoroidal space, can lead to detachment" ;
    rdfs:subClassOf imdrf:E08 .

imdrf:E0860 a owl:Class ;
    rdfs:label "Eye Strain/Fatigue" ;
    ex:nonIMDRFCode "MedDRA:10049755:Eye Strain" ;
    ex:status "New" ;
    ex:statusDescription "Term added for Release Number 2025. See no. 100 of Change Request Log" ;
    rdfs:comment "A feeling of general eye weakness/fatigue. (e.g. asthenopia)." ;
    rdfs:subClassOf imdrf:E08 .

imdrf:E0901 a owl:Class ;
    rdfs:label "Acoustic Shock" ;
    ex:nonIMDRFCode "MedDRA:10068150:Acoustic shock" ;
    rdfs:comment "Neurophysiological and psychological symptoms caused by sudden and unexpected loud noise." ;
    rdfs:subClassOf imdrf:E01,
        imdrf:E09 .

imdrf:E0902 a owl:Class ;
    rdfs:label "Acoustic Trauma" ;
    ex:nonIMDRFCode "MedDRA:10000528:Acoustic trauma" ;
    rdfs:comment "Injury to the hearing mechanisms within the inner ear, caused by excessively loud noise." ;
    rdfs:subClassOf imdrf:E09 .

imdrf:E090301 a owl:Class ;
    rdfs:label "Partial Hearing Loss" ;
    ex:nonIMDRFCode "MedDRA:10050564:Partial hearing loss" ;
    rdfs:comment "A condition in which a person partially loses the ability to hear sounds in one or both ears." ;
    rdfs:subClassOf imdrf:E0903 .

imdrf:E090302 a owl:Class ;
    rdfs:label "Total Hearing Loss" ;
    ex:nonIMDRFCode "MedDRA:10074290:Complete hearing loss" ;
    rdfs:comment "A condition in which a person completely loses the hearing in one or both ears." ;
    rdfs:subClassOf imdrf:E0903 .

imdrf:E0904 a owl:Class ;
    rdfs:label "Tinnitus" ;
    ex:nonIMDRFCode "MedDRA:10043882:Tinnitus" ;
    rdfs:comment "A noise in the ears, such as ringing, buzzing, roaring or clicking in the absence of auditory stimulation." ;
    rdfs:subClassOf imdrf:E01,
        imdrf:E09 .

imdrf:E0905 a owl:Class ;
    rdfs:label "Vertigo" ;
    ex:nonIMDRFCode "MedDRA:10047340:Vertigo" ;
    rdfs:comment "A feeling of movement, a sensation as if the external world were revolving around the person or as if they were revolving in space (subjective vertigo). Vertigo is medically distinct from dizziness, lightheadedness, and unsteadiness." ;
    rdfs:subClassOf imdrf:E09 .

imdrf:E0906 a owl:Class ;
    rdfs:label "Unspecified Ear or Labyrinth Problem" ;
    ex:statusDescription "Term was added on 18 March 2020 for cases where the category of a health effect was reported but with no further details." ;
    rdfs:comment "The report describes a non-specific problem with the ear or labyrinth. Note: Please use \"Appropriate Term / Code Not Available\" if the report describes a specific problem but the relevant term does not exist." ;
    rdfs:subClassOf imdrf:E09 .

imdrf:E0907 a owl:Class ;
    rdfs:label "Ear Pain" ;
    ex:nonIMDRFCode "MedDRA:10014020:Ear pain" ;
    ex:statusDescription "Term was added on 27 January 2022. For details, see comment No. 234 / 235 of the Change Log (Release Number 2022)." ;
    rdfs:comment "Earache or ear pain." ;
    rdfs:subClassOf imdrf:E09,
        imdrf:E2330 .

imdrf:E090801 a owl:Class ;
    rdfs:label "Infectious Otitis Externa" ;
    ex:nonIMDRFCode "MedDRA:10033072:Otitis externa" ;
    ex:statusDescription "Editorial change to the term on 31 January 2023." ;
    rdfs:comment "An infectious process involving the outer ear and ear canal." ;
    rdfs:subClassOf imdrf:E0908 .

imdrf:E090802 a owl:Class ;
    rdfs:label "Infectious Otitis Media" ;
    ex:nonIMDRFCode "MedDRA:10033078:Otitis media" ;
    ex:statusDescription "Editorial change to the term on 31 January 2023." ;
    rdfs:comment "An infectious process involving the middle ear, includes acute otitis media, chronic otitis media, chronic suppurative otitis media, otitis media with effusion (OME), etc." ;
    rdfs:subClassOf imdrf:E0908 .

imdrf:E0909 a owl:Class ;
    rdfs:label "Middle Ear Inflammation" ;
    ex:nonIMDRFCode "MedDRA:10065838:Middle ear inflammation" ;
    ex:statusDescription "Term was added on 27 January 2022. For details, see comment No. 232 of the Change Log (Release Number 2022)." ;
    rdfs:comment "Inflammation (swelling and redness) to the middle ear." ;
    rdfs:subClassOf imdrf:E09 .

imdrf:E0910 a owl:Class ;
    rdfs:label "Labyrinthitis" ;
    ex:nonIMDRFCode "MedDRA:10023567:Labyrinthitis" ;
    ex:statusDescription "Term was added on 27 January 2022. For details, see comment No. 233 of the Change Log (Release Number 2022)." ;
    rdfs:comment "An inflammation of the labyrinth in the inner ear that causes dizziness and reduced or distorted hearing." ;
    rdfs:subClassOf imdrf:E09,
        imdrf:E19 .

imdrf:E0911 a owl:Class ;
    rdfs:label "Cholesteatoma" ;
    ex:nonIMDRFCode "MedDRA:10008642:Cholesteatoma" ;
    ex:status "New" ;
    ex:statusDescription "Term added for Release Number 2025. See no. 16 of Change Request Log" ;
    rdfs:comment "An abnormal growth of skin cells in the middle ear, with or without infection.  May be invasive and can erode neighboring structures including bone." ;
    rdfs:subClassOf imdrf:E09 .

imdrf:E0912 a owl:Class ;
    rdfs:label "Ear injury" ;
    ex:nonIMDRFCode "MedDRA:10057446:Ear injury" ;
    ex:status "New" ;
    ex:statusDescription "Term added for Release Number 2025. See no. 76 of Change Request Log" ;
    rdfs:comment "Injury to the outer, middle or inner ear." ;
    rdfs:subClassOf imdrf:E09,
        imdrf:E20 .

imdrf:E0913 a owl:Class ;
    rdfs:label "Cerumen impaction" ;
    ex:nonIMDRFCode "MedDRA:10050337:Cerumen impaction" ;
    ex:status "New" ;
    ex:statusDescription "Term added for Release Number 2025. See no. 105 of Change Request Log" ;
    rdfs:comment "A buildup and/or blockage of earwax in the ear canal." ;
    rdfs:subClassOf imdrf:E09 .

imdrf:E1001 a owl:Class ;
    rdfs:label "Abdominal Distention" ;
    ex:nonIMDRFCode "MedDRA:10000060:Abdominal distension" ;
    rdfs:comment "The condition of the abdomen being enlarged or swollen from internal pressure." ;
    rdfs:subClassOf imdrf:E10 .

imdrf:E1002 a owl:Class ;
    rdfs:label "Abdominal Pain" ;
    ex:nonIMDRFCode "MedDRA:10000081:Abdominal pain" ;
    rdfs:comment "Painful sensation in the abdominal region." ;
    rdfs:subClassOf imdrf:E10,
        imdrf:E2330 .

imdrf:E1003 a owl:Class ;
    rdfs:label "Achalasia" ;
    ex:nonIMDRFCode "MedDRA:10000420:Achalasia" ;
    rdfs:comment "Failure of the smooth muscle fibers of the gastrointestinal tract to relax at any one point of junction of one part with another." ;
    rdfs:subClassOf imdrf:E10 .

imdrf:E1004 a owl:Class ;
    rdfs:label "Ascites" ;
    ex:nonIMDRFCode "MedDRA:10003445:Ascites" ;
    rdfs:comment "Accumulation of fluid in the peritoneal cavity. The fluid may be serous, hemorrhagic, or the result of tumor metastasis to the peritoneum." ;
    rdfs:subClassOf imdrf:E10 .

imdrf:E1005 a owl:Class ;
    rdfs:label "Bowel Burn" ;
    ex:nonIMDRFCode "MedDRA:10082501:Intestinal burn" ;
    rdfs:comment "A thermal injury to the bowels." ;
    rdfs:subClassOf imdrf:E10,
        imdrf:E1704 .

imdrf:E1006 a owl:Class ;
    rdfs:label "Bowel Perforation" ;
    ex:nonIMDRFCode "MedDRA:10006056:Bowel perforation" ;
    rdfs:comment "A rupture in the wall of the small or large intestine due to traumatic or pathologic processes." ;
    rdfs:subClassOf imdrf:E10,
        imdrf:E2114 .

imdrf:E1007 a owl:Class ;
    rdfs:label "Constipation" ;
    ex:nonIMDRFCode "MedDRA:10010774:Constipation" ;
    rdfs:comment "Irregular and infrequent or difficult evacuation of the bowels." ;
    rdfs:subClassOf imdrf:E10 .

imdrf:E1008 a owl:Class ;
    rdfs:label "Diarrhea" ;
    ex:nonIMDRFCode "MedDRA:10012727:Diarrhea" ;
    rdfs:comment "Frequent, watery bowel movements." ;
    rdfs:subClassOf imdrf:E10 .

imdrf:E1009 a owl:Class ;
    rdfs:label "Dysphagia/ Odynophagia" ;
    ex:nonIMDRFCode "MedDRA:10013950:Dysphagia" ;
    rdfs:comment "A symptom referring to difficult and or painful swallowing." ;
    rdfs:subClassOf imdrf:E10 .

imdrf:E1010 a owl:Class ;
    rdfs:label "Eructate" ;
    ex:nonIMDRFCode "MedDRA:10015137:Eructation" ;
    rdfs:comment "To belch, the casting of upwind from the stomach." ;
    rdfs:subClassOf imdrf:E10 .

imdrf:E1011 a owl:Class ;
    rdfs:label "Flatus" ;
    ex:nonIMDRFCode "MedDRA:10016769:Flatus" ;
    rdfs:comment "Gas or air in the gastrointestinal tract." ;
    rdfs:subClassOf imdrf:E10 .

imdrf:E1012 a owl:Class ;
    rdfs:label "Gastritis" ;
    ex:nonIMDRFCode "MedDRA:10017853:Gastritis" ;
    rdfs:comment "Inflammation of the stomach." ;
    rdfs:subClassOf imdrf:E10 .

imdrf:E1013 a owl:Class ;
    rdfs:label "Gastroesophageal Burn" ;
    ex:nonIMDRFCode "MedDRA:10082500:Gastroesophageal burn" ;
    rdfs:comment "Thermal, chemical or radiation injury to stomach or esophagus." ;
    rdfs:subClassOf imdrf:E10,
        imdrf:E1704 .

imdrf:E1014 a owl:Class ;
    rdfs:label "Gastrointestinal Hemorrhage" ;
    ex:nonIMDRFCode "MedDRA:10017960:Gastrointestinal hemorrhage" ;
    rdfs:comment "Bleeding originating from any part of the gastrointestinal tract." ;
    rdfs:subClassOf imdrf:E10 .

imdrf:E1015 a owl:Class ;
    rdfs:label "Gastrointestinal Regurgitation" ;
    ex:nonIMDRFCode "MedDRA:10067171:Regurgitation" ;
    rdfs:comment "Flow in the opposite direction from normal, as the casting up of undigested food or gas from the stomach, or the backward flowing of blood into the heart, or between the chambers of the heart when a valve is incompetent." ;
    rdfs:subClassOf imdrf:E10 .

imdrf:E1016 a owl:Class ;
    rdfs:label "Hematemesis" ;
    ex:nonIMDRFCode "MedDRA:10019418:Hematemesis" ;
    rdfs:comment "Vomiting blood." ;
    rdfs:subClassOf imdrf:E10 .

imdrf:E1017 a owl:Class ;
    rdfs:label "Intra-Abdominal Hemorrhage" ;
    ex:nonIMDRFCode "MedDRA:10055291:Intra-abdominal hemorrhage" ;
    rdfs:comment "Bleeding within the abdominal cavity." ;
    rdfs:subClassOf imdrf:E10 .

imdrf:E1018 a owl:Class ;
    rdfs:label "Laceration(s) of Esophagus" ;
    ex:nonIMDRFCode "MedDRA:10068164:Esophageal laceration" ;
    rdfs:comment "A torn, ragged, mangled wound, or an accidental cut of esophagus." ;
    rdfs:subClassOf imdrf:E10 .

imdrf:E1019 a owl:Class ;
    rdfs:label "Melena" ;
    ex:nonIMDRFCode "MedDRA:10027162:Melena" ;
    rdfs:comment "Abnormally dark tarry feces containing blood, usually from gastrointestinal bleeding." ;
    rdfs:subClassOf imdrf:E10 .

imdrf:E1020 a owl:Class ;
    rdfs:label "Nausea" ;
    ex:nonIMDRFCode "MedDRA:10028813:Nausea" ;
    rdfs:comment "Upper abdominal discomfort associated with an urge to vomit." ;
    rdfs:subClassOf imdrf:E10 .

imdrf:E1021 a owl:Class ;
    rdfs:label "Pancreatitis" ;
    ex:nonIMDRFCode "MedDRA:10033645:Pancreatitis" ;
    rdfs:comment "Inflammation of the pancreas." ;
    rdfs:subClassOf imdrf:E10,
        imdrf:E19 .

imdrf:E1022 a owl:Class ;
    rdfs:label "Perforation of Esophagus" ;
    ex:nonIMDRFCode "MedDRA:10034419:Perforation of esophagus" ;
    rdfs:comment "The presence of a hole or other type of opening in the esophageal wall through which the contents of the esophagus can pass into the mediastinum." ;
    rdfs:subClassOf imdrf:E10,
        imdrf:E2114 .

imdrf:E1023 a owl:Class ;
    rdfs:label "Peritoneal Laceration(s)" ;
    ex:nonIMDRFCode "MedDRA:10068140:Peritoneal laceration" ;
    rdfs:comment "A cut or tear of the peritoneum." ;
    rdfs:subClassOf imdrf:E10,
        imdrf:E20 .

imdrf:E1024 a owl:Class ;
    rdfs:label "Peritonitis" ;
    ex:nonIMDRFCode "MedDRA:10034674:Peritonitis" ;
    rdfs:comment "Inflammation of the peritoneum due to infection by bacteria or fungi." ;
    rdfs:subClassOf imdrf:E10,
        imdrf:E19 .

imdrf:E1025 a owl:Class ;
    rdfs:label "Heartburn/Indigestion" ;
    ex:nonIMDRFCode "MedDRA:10013946:Dyspepsia" ;
    ex:statusDescription "Term/Definition was modified on 27 January 2022 (Old term/definition: Pyrosis/Heartburn: Abdominal discomfort with retrosternal pain usually associated with gastroesophageal reflux.) MedDRA mapping also updated from Heartburn(10019326) to Dyspepsia(10013946). For details, see comment No. 110 of the Change Log (Release Number 2022)." ;
    rdfs:comment "Abdominal discomfort with retrosternal pain usually associated with gastroesophageal reflux, pyrosis or dyspepsia." ;
    rdfs:subClassOf imdrf:E10 .

imdrf:E1026 a owl:Class ;
    rdfs:label "Rectal Anastomotic Leakage" ;
    ex:nonIMDRFCode "MedDRA:10065894:Rectal anastomotic leak" ;
    ex:status "Retired" ;
    ex:statusDescription "Term retired for Release Number 2024. Use E2108 - Failure to Anastomose. See no. 81 of Change Log" ;
    rdfs:comment "Leakage due to breakdown of a rectal anastomosis." ;
    rdfs:subClassOf imdrf:E10,
        imdrf:E21 .

imdrf:E1027 a owl:Class ;
    rdfs:label "Retroperitoneal Hemorrhage" ;
    ex:nonIMDRFCode "MedDRA:10038981:Retroperitoneal hemorrhage" ;
    rdfs:comment "Bleeding originating in the retroperitoneal area." ;
    rdfs:subClassOf imdrf:E10 .

imdrf:E102801 a owl:Class ;
    rdfs:label "Dry Mouth" ;
    ex:nonIMDRFCode "MedDRA:10013781:Dry mouth" ;
    rdfs:comment "The condition of not having enough saliva to keep the mouth moist." ;
    rdfs:subClassOf imdrf:E1028 .

imdrf:E102802 a owl:Class ;
    rdfs:label "Salivary Hypersecretion" ;
    ex:nonIMDRFCode "MedDRA:10039424:Salivary hypersecretion" ;
    rdfs:comment "Excessive saliva production." ;
    rdfs:subClassOf imdrf:E1028 .

imdrf:E1029 a owl:Class ;
    rdfs:label "Stenosis of the esophagus" ;
    ex:nonIMDRFCode "MedDRA:10041978:Stenosis esophageal" ;
    rdfs:comment "Narrowing or tightening of the esophagus" ;
    rdfs:subClassOf imdrf:E10 .

imdrf:E1030 a owl:Class ;
    rdfs:label "Stomach Ulceration" ;
    ex:nonIMDRFCode "MedDRA:10042116:Stomach ulcer" ;
    rdfs:comment "The formation of sores or a break in the wall of the stomach." ;
    rdfs:subClassOf imdrf:E10 .

imdrf:E103101 a owl:Class ;
    rdfs:label "Glossitis" ;
    ex:nonIMDRFCode "MedDRA:10018386:Glossitis" ;
    rdfs:comment "Inflammation of the tongue." ;
    rdfs:subClassOf imdrf:E1031 .

imdrf:E1032 a owl:Class ;
    rdfs:label "Vomiting" ;
    ex:nonIMDRFCode "MedDRA:10047700:Vomiting" ;
    rdfs:comment "Forceful ejection of the contents of the stomach through the mouth." ;
    rdfs:subClassOf imdrf:E10 .

imdrf:E1033 a owl:Class ;
    rdfs:label "Unspecified Gastrointestinal Problem" ;
    ex:statusDescription "Term was added on 18 March 2020 for cases where the category of a health effect was reported but with no further details." ;
    rdfs:comment "The report describes a non-specific problem with the gastrointestinal system. Note: Please use \"Appropriate Term / Code Not Available\" if the report describes a specific problem but the relevant term does not exist." ;
    rdfs:subClassOf imdrf:E10 .

imdrf:E1034 a owl:Class ;
    rdfs:label "Fecal Urgency" ;
    ex:nonIMDRFCode "MedDRA:10012114:Defecation urgency" ;
    ex:statusDescription "Term was added on 27 January 2022. For details, see comment No. 7 of the Change Log (Release Number 2022)." ;
    rdfs:comment "A continual or recurrent inclination to evacuate the bowels." ;
    rdfs:subClassOf imdrf:E10 .

imdrf:E1035 a owl:Class ;
    rdfs:label "Pneumoperitoneum" ;
    ex:nonIMDRFCode "MedDRA:10048299:Pneumoperitoneum" ;
    ex:statusDescription "Term was added on 27 January 2022. For details, see comment No. 205 of the Change Log (Release Number 2022)." ;
    rdfs:comment "Free air within the peritoneal cavity." ;
    rdfs:subClassOf imdrf:E10 .

imdrf:E1036 a owl:Class ;
    rdfs:label "Colitis" ;
    ex:nonIMDRFCode "MedDRA:10009887:Colitis" ;
    ex:statusDescription "Term added for Release Number 2024. See no. 102 of Change Log" ;
    rdfs:comment "Inflammation of the large intestine" ;
    rdfs:subClassOf imdrf:E10 .

imdrf:E1101 a owl:Class ;
    rdfs:label "Biliary Cirrhosis" ;
    ex:nonIMDRFCode "MedDRA:10004659:Biliary cirrhosis" ;
    ex:statusDescription "Definition was modified on 21 January 2021 (Old definition: Biliary Cirrhosis/Cirrhosis of the liver caused either by destruction of the intrahepatic bile ducts (primary biliary cirrhosis) or blockage of the extrahepatic bile ducts (secondary biliary cirrhosis).). For details, refer to comment No. 5 of the Change Log." ;
    rdfs:comment "Cirrhosis of the liver caused either by destruction of the intrahepatic bile ducts (primary biliary cholangitis) or blockage of the extrahepatic bile ducts (secondary biliary cholangitis)." ;
    rdfs:subClassOf imdrf:E11 .

imdrf:E1102 a owl:Class ;
    rdfs:label "Hepatitis" ;
    ex:nonIMDRFCode "MedDRA:10056522:Hepatic infection" ;
    rdfs:comment "Inflammation of the liver; usually from a viral infection, but sometimes from toxic agents." ;
    rdfs:subClassOf imdrf:E11,
        imdrf:E19 .

imdrf:E1103 a owl:Class ;
    rdfs:label "Hyperbilirubinemia" ;
    ex:nonIMDRFCode "MedDRA:10020582:Hyperbilirubinemia" ;
    rdfs:comment "Abnormally high level of bilirubin in the blood. Excess bilirubin is associated with jaundice." ;
    rdfs:subClassOf imdrf:E11 .

imdrf:E1104 a owl:Class ;
    rdfs:label "Liver Damage/Dysfunction" ;
    ex:nonIMDRFCode "MedDRA:10019831:Hepatocellular damage" ;
    rdfs:comment "Non traumatic damage to the liver parenchyma resulting in hepatic insufficiency." ;
    rdfs:subClassOf imdrf:E11 .

imdrf:E1105 a owl:Class ;
    rdfs:label "Liver Failure" ;
    ex:nonIMDRFCode "MedDRA:10024678:Liver failure" ;
    rdfs:comment "Sustained, and severe damage to the liver with significant loss of function." ;
    rdfs:subClassOf imdrf:E11 .

imdrf:E1106 a owl:Class ;
    rdfs:label "Liver Laceration(s)" ;
    ex:nonIMDRFCode "MedDRA:10068143:Liver laceration" ;
    rdfs:comment "A cut or tear in the liver." ;
    rdfs:subClassOf imdrf:E11 .

imdrf:E1107 a owl:Class ;
    rdfs:label "Unspecified Hepatic or Biliary Problem" ;
    ex:statusDescription "Term was added on 18 March 2020 for cases where the category of a health effect was reported but with no further details." ;
    rdfs:comment "The report describes a non-specific problem with the liver or biliary system. Note: Please use \"Appropriate Term / Code Not Available\" if the report describes a specific problem but the relevant term does not exist." ;
    rdfs:subClassOf imdrf:E11 .

imdrf:E1108 a owl:Class ;
    rdfs:label "Biliary Leak" ;
    ex:nonIMDRFCode "MedDRA:10057586:Post procedural bile leak" ;
    ex:statusDescription "Term was added on 27 January 2022. For details, see comment No. 5 of the Change Log (Release Number 2022)." ;
    rdfs:comment "Sudden unexpected leakage of bile from the liver or soft tissue." ;
    rdfs:subClassOf imdrf:E11,
        imdrf:E21 .

imdrf:E1109 a owl:Class ;
    rdfs:label "Cholangitis" ;
    ex:nonIMDRFCode "MedDRA:10008604:Cholangitis" ;
    ex:statusDescription "Term was added on 27 January 2022. For details, see comment No. 6 of the Change Log (Release Number 2022)." ;
    rdfs:comment "Inflammation of the bile duct." ;
    rdfs:subClassOf imdrf:E11,
        imdrf:E21 .

imdrf:E1201 a owl:Class ;
    rdfs:label "Dehydration" ;
    ex:nonIMDRFCode "MedDRA:10012174:Dehydration" ;
    rdfs:comment "A condition resulting from the excessive loss of fluid from the body." ;
    rdfs:subClassOf imdrf:E12 .

imdrf:E120201 a owl:Class ;
    rdfs:label "Hypernatremia" ;
    ex:nonIMDRFCode "MedDRA:10020680:Hypernatremia" ;
    rdfs:comment "Higher than normal levels of sodium in the circulating blood." ;
    rdfs:subClassOf imdrf:E1202 .

imdrf:E120202 a owl:Class ;
    rdfs:label "Hyponatremia" ;
    ex:nonIMDRFCode "MedDRA:10021038:Hyponatremia" ;
    rdfs:comment "Lower than normal levels of sodium in the circulating blood." ;
    rdfs:subClassOf imdrf:E1202 .

imdrf:E120203 a owl:Class ;
    rdfs:label "Hypercalcemia" ;
    ex:nonIMDRFCode "MedDRA:10020587:Hypercalcemia" ;
    ex:statusDescription "Term was added on 27 January 2022. For details, see comment No. 38 / 90 of the Change Log (Release Number 2022)." ;
    rdfs:comment "Higher than normal levels of calcium in the circulating blood." ;
    rdfs:subClassOf imdrf:E1202 .

imdrf:E120204 a owl:Class ;
    rdfs:label "Hypocalcemia" ;
    ex:nonIMDRFCode "MedDRA:10020949:Hypocalcemia" ;
    ex:statusDescription "Term was added on 27 January 2022. For details, see comment No. 39 / 91 of the Change Log (Release Number 2022)." ;
    rdfs:comment "Lower than normal levels of calcium in the circulating blood." ;
    rdfs:subClassOf imdrf:E1202 .

imdrf:E120205 a owl:Class ;
    rdfs:label "Hyperkalemia" ;
    ex:nonIMDRFCode "MedDRA:10020647:Hyperkalemia" ;
    ex:statusDescription "Term was added on 27 January 2022. For details, see comment No. 63 of the Change Log (Release Number 2022)." ;
    rdfs:comment "Higher than normal levels of potassium in the circulating blood." ;
    rdfs:subClassOf imdrf:E1202 .

imdrf:E120206 a owl:Class ;
    rdfs:label "Hypokalemia" ;
    ex:nonIMDRFCode "MedDRA:10021018:Hypokalemia" ;
    ex:statusDescription "Term was added on 27 January 2022. For details, see comment No. 64 of the Change Log (Release Number 2022)." ;
    rdfs:comment "Lower than normal levels of potassium in the circulating blood." ;
    rdfs:subClassOf imdrf:E1202 .

imdrf:E120207 a owl:Class ;
    rdfs:label "Blood Bicarbonate Increased" ;
    ex:nonIMDRFCode "MedDRA:10005360:Blood bicarbonate increased" ;
    ex:statusDescription "Term was added on 27 January 2022. For details, see comment No. 88 of the Change Log (Release Number 2022)." ;
    rdfs:comment "Higher than normal levels of bicarbonate in the blood." ;
    rdfs:subClassOf imdrf:E1202 .

imdrf:E120208 a owl:Class ;
    rdfs:label "Blood Bicarbonate Decreased" ;
    ex:nonIMDRFCode "MedDRA:10005359:Blood bicarbonate decreased" ;
    ex:statusDescription "Term was added on 27 January 2022. For details, see comment No. 89 of the Change Log (Release Number 2022)." ;
    rdfs:comment "Lower than normal levels of bicarbonate in the blood." ;
    rdfs:subClassOf imdrf:E1202 .

imdrf:E120209 a owl:Class ;
    rdfs:label "Hyperphosphatemia" ;
    ex:nonIMDRFCode "MedDRA:10020712:Hyperphosphatemia" ;
    ex:statusDescription "Term was added on 27 January 2022. For details, see comment No. 61 of the Change Log (Release Number 2022)." ;
    rdfs:comment "Higher than normal levels of phosphate in the circulating blood." ;
    rdfs:subClassOf imdrf:E1202 .

imdrf:E1203 a owl:Class ;
    rdfs:label "Feeding Problem" ;
    ex:nonIMDRFCode "MedDRA:10061148:Feeding disorder" ;
    rdfs:comment "Interruption or disruption of the intake of food/nutrition." ;
    rdfs:subClassOf imdrf:E12 .

imdrf:E1204 a owl:Class ;
    rdfs:label "Hot Flashes/Flushes" ;
    ex:nonIMDRFCode "MedDRA:10020407:Hot flashes" ;
    rdfs:comment "A temporary and/or sudden feeling of intense body warmth, flushing, sometimes accompanied by sweating." ;
    rdfs:subClassOf imdrf:E12 .

imdrf:E120501 a owl:Class ;
    rdfs:label "Elevated ketones/Diabetic Ketoacidosis" ;
    ex:nonIMDRFCode "MedDRA:10057594:Blood ketone body increased" ;
    ex:status "Modified (editorial)" ;
    ex:statusDescription "Editorial change on 31 January 2023 to align E120501 term. (Old term: Diabetic Ketoacidosis). MedDRA mapping is updated from Diabetic ketoacidosis (10012671) to Blood ketone body increased (10057594). For details, see comment No. 85 / 86 of the Change Log (Release Number 2023). Minor change to Term and Status Description to correct inconsistencies between primary and secondary location for Release No. 2025" ;
    rdfs:comment "Elevated ketones, including metabolic acidosis produced by accumulation of ketone bodies resulting from uncontrolled diabetes mellitus." ;
    rdfs:subClassOf imdrf:E1205 .

imdrf:E1206 a owl:Class ;
    rdfs:label "Hypoglycemia" ;
    ex:nonIMDRFCode "MedDRA:10021005:Hypoglycemia" ;
    rdfs:comment "Abnormally low level of glucose in the blood." ;
    rdfs:subClassOf imdrf:E12,
        imdrf:E22 .

imdrf:E1207 a owl:Class ;
    rdfs:label "Polydipsia" ;
    ex:nonIMDRFCode "MedDRA:10036067:Polydipsia" ;
    rdfs:comment "Extreme thirst accompanied by chronic excessive intake of water." ;
    rdfs:subClassOf imdrf:E12 .

imdrf:E1208 a owl:Class ;
    rdfs:label "Weight Changes" ;
    ex:nonIMDRFCode "MedDRA:10049040:Weight fluctuation" ;
    rdfs:comment "Repetitive loss and regain of body weight." ;
    rdfs:subClassOf imdrf:E12 .

imdrf:E1209 a owl:Class ;
    rdfs:label "Hormonal Imbalance" ;
    ex:nonIMDRFCode "MedDRA:10020381:Hormonal imbalance" ;
    ex:statusDescription "Editorial change on 27 January 2022 to the MedDRA mapping to include the MedDRA term.",
        "Term was added on 18 March 2020 as an additional level 2 term for \"Endocrine, Metabolism and Nutrition\"." ;
    rdfs:comment "An imbalance of one or more hormones in the body" ;
    rdfs:subClassOf imdrf:E12,
        imdrf:E22 .

imdrf:E1210 a owl:Class ;
    rdfs:label "Premature Menopause" ;
    ex:nonIMDRFCode "MedDRA:10036601:Premature menopause" ;
    ex:statusDescription "Term was added on 18 March 2020 as an additional level 2 term for \"Endocrine, Metabolism and Nutrition\"." ;
    rdfs:comment "Menopause occurring spontaneously before 40 years of age" ;
    rdfs:subClassOf imdrf:E12,
        imdrf:E14 .

imdrf:E1211 a owl:Class ;
    rdfs:label "Vitamin Deficiency" ;
    ex:nonIMDRFCode "MedDRA:10047628:Vitamin deficiency" ;
    ex:statusDescription "Term was added on 18 March 2020 as an additional level 2 term for \"Endocrine, Metabolism and Nutrition\"." ;
    rdfs:comment "Low levels of one or more vitamins in the body." ;
    rdfs:subClassOf imdrf:E12 .

imdrf:E1212 a owl:Class ;
    rdfs:label "Hypothyroidism" ;
    ex:nonIMDRFCode "MedDRA:10021114:Hypothyroidism" ;
    ex:statusDescription "Term was added on 31 January 2023. For details, see comment No. 87 of the Change Log (Release Number 2023)." ;
    rdfs:comment "Abnormally low levels of thyroid hormone" ;
    rdfs:subClassOf imdrf:E12 .

imdrf:E1213 a owl:Class ;
    rdfs:label "MetabolicAcidosis" ;
    ex:nonIMDRFCode "MedDRA:10027417:Metabolicacidosis" ;
    ex:status "New" ;
    ex:statusDescription "Term added for Release Number 2025. See no. 33 of Change Request Log" ;
    rdfs:comment "An increase in the hydrogen ion concentration in the systemic circulation that results in an abnormally low serum bicarbonate level." ;
    rdfs:subClassOf imdrf:E12 .

imdrf:E1214 a owl:Class ;
    rdfs:label "Hyperthyroidism" ;
    ex:nonIMDRFCode "MedDRA:10020850:Hyperthyroidism" ;
    ex:status "New" ;
    ex:statusDescription "Term added for Release Number 2025. See no. 73 of Change Request Log" ;
    rdfs:comment "Abnormally high levels of thyroid hormone" ;
    rdfs:subClassOf imdrf:E12 .

imdrf:E1215 a owl:Class ;
    rdfs:label "MetabolicAlkalosis" ;
    ex:nonIMDRFCode "MedDRA:10027423:Metabolicalkalosis" ;
    ex:status "New" ;
    ex:statusDescription "Term added for Release Number 2025. See no. 34 of Change Request Log" ;
    rdfs:comment "A disorder characterized by abnormally high alkalinity (low hydrogen-ion concentration) of the blood and other body tissues." ;
    rdfs:subClassOf imdrf:E12 .

imdrf:E1301 a owl:Class ;
    rdfs:label "Dysuria" ;
    ex:nonIMDRFCode "MedDRA:10013990:Dysuria" ;
    rdfs:comment "Difficult or painful urination." ;
    rdfs:subClassOf imdrf:E13 .

imdrf:E1302 a owl:Class ;
    rdfs:label "Hematuria" ;
    ex:nonIMDRFCode "MedDRA:10019450:Hematuria" ;
    rdfs:comment "Blood in the urine." ;
    rdfs:subClassOf imdrf:E13 .

imdrf:E1303 a owl:Class ;
    rdfs:label "Increased Intra-Peritoneal Volume (IIPV)" ;
    ex:nonIMDRFCode "MedDRA:10082492:Increased intraperitoneal volume" ;
    rdfs:comment "Abnormal build up of fluid in the abdomen." ;
    rdfs:subClassOf imdrf:E10,
        imdrf:E13 .

imdrf:E1304 a owl:Class ;
    rdfs:label "Micturition Urgency" ;
    ex:nonIMDRFCode "MedDRA:10027566:Micturition urgency" ;
    rdfs:comment "A sudden compelling urge to urinate." ;
    rdfs:subClassOf imdrf:E13 .

imdrf:E130501 a owl:Class ;
    rdfs:label "Renal Failure" ;
    ex:nonIMDRFCode "MedDRA:10038435:Renal failure" ;
    rdfs:comment "An acute or chronic condition that is characterized by the inability of the kidneys to adequately filter the blood resulting in uremia and electrolyte imbalances." ;
    rdfs:subClassOf imdrf:E1305 .

imdrf:E1306 a owl:Class ;
    rdfs:label "Uremia" ;
    ex:nonIMDRFCode "MedDRA:10046369:Uremia" ;
    rdfs:comment "Abnormally high concentration of non-protein nitrogen in the blood." ;
    rdfs:subClassOf imdrf:E12,
        imdrf:E13 .

imdrf:E1307 a owl:Class ;
    rdfs:label "Urethral Stenosis/Stricture" ;
    ex:nonIMDRFCode "MedDRA:10065584:Urethral stenosis" ;
    rdfs:comment "Narrowing of any part of the urethra. With or without affecting the flow of urine." ;
    rdfs:subClassOf imdrf:E13 .

imdrf:E1308 a owl:Class ;
    rdfs:label "Urinary Frequency / Polyuria" ;
    ex:nonIMDRFCode "MedDRA:10036142:Polyuria" ;
    ex:statusDescription "Term/Definition was modified on 31 January 2023 (Old term/definition: Urinary Frequency: Urination at short intervals; it may result from increased urine formation, decreased bladder capacity, or lower urinary tract irritation.) MedDRA mapping also updated from Urinary frequency (10046539) to Polyuria (10036142). For details, see comment No. 88 of the Change Log (Release Number 2023)." ;
    rdfs:comment "Urination at short intervals or at higher volumes; it may result from increased urine formation, decreased bladder capacity, or lower urinary tract irritation." ;
    rdfs:subClassOf imdrf:E13 .

imdrf:E1309 a owl:Class ;
    rdfs:label "Urinary Retention" ;
    ex:nonIMDRFCode "MedDRA:10046555:Urinary retention" ;
    rdfs:comment "Accumulation of urine within the bladder because of the inability to urinate." ;
    rdfs:subClassOf imdrf:E13 .

imdrf:E131001 a owl:Class ;
    rdfs:label "Kidney Infection" ;
    ex:nonIMDRFCode "MedDRA:10023424:Kidney infection" ;
    rdfs:comment "An inflammatory process affecting the kidney." ;
    rdfs:subClassOf imdrf:E1310 .

imdrf:E1311 a owl:Class ;
    rdfs:label "Unspecified Kidney or Urinary Problem" ;
    ex:statusDescription "Term was added on 18 March 2020 for cases where the category of a health effect was reported but with no further details." ;
    rdfs:comment "The report describes a non-specific problem with the kidneys or urinary system. Note: Please use \"Appropriate Term / Code Not Available\" if the report describes a specific problem but the relevant term does not exist." ;
    rdfs:subClassOf imdrf:E13 .

imdrf:E1312 a owl:Class ;
    rdfs:label "Urolithiasis" ;
    ex:nonIMDRFCode "MedDRA:10046707:Urolithiasis" ;
    ex:statusDescription "Term was added on 31 January 2023. For details, see comment No. 89 of the Change Log (Release Number 2023)." ;
    rdfs:comment "A condition arising from the formation of renal calculi (e.g. kidney stones, bladder stones, urinary tract stones)." ;
    rdfs:subClassOf imdrf:E13 .

imdrf:E1313 a owl:Class ;
    rdfs:label "Interstitial Cystitis" ;
    ex:nonIMDRFCode "MedDRA:10011796:Cystitis interstitial" ;
    ex:statusDescription "Term was added on 31 January 2023. For details, see comment No. 90 of the Change Log (Release Number 2023)." ;
    rdfs:comment "A chronic bladder condition resulting in recurring discomfort or pain in the bladder or surrounding pelvic region. Also known as Bladder Pain Syndrome (BPS)." ;
    rdfs:subClassOf imdrf:E13 .

imdrf:E1314 a owl:Class ;
    rdfs:label "Bladder Wall Thickening" ;
    ex:nonIMDRFCode "MedDRA:10079064:Bladder wall thickening" ;
    ex:statusDescription "Term was added on 31 January 2023. For details, see comment No. 91 of the Change Log (Release Number 2023)." ;
    rdfs:comment "Thickening of the bladder walls, including Bladder Trabeculation." ;
    rdfs:subClassOf imdrf:E13 .

imdrf:E1315 a owl:Class ;
    rdfs:label "Hydronephrosis" ;
    ex:nonIMDRFCode "MedDRA:10020524:Hydronephrosis" ;
    ex:statusDescription "Term added for Release Number 2024. See no. 5 of Change Log" ;
    rdfs:comment "A condition of excess urine accumulation in kidney(s) that causes swelling of kidneys." ;
    rdfs:subClassOf imdrf:E13 .

imdrf:E1316 a owl:Class ;
    rdfs:label "Bladder Dysfunction" ;
    ex:nonIMDRFCode "MedDRA:10069632:Bladder Dysfunction" ;
    ex:statusDescription "Term added for Release Number 2024. See no. 14 of Change Log" ;
    rdfs:comment "Impaired or abnormal functioning of the bladder, including sphincters." ;
    rdfs:subClassOf imdrf:E13 .

imdrf:E1317 a owl:Class ;
    rdfs:label "Kidney injury" ;
    ex:nonIMDRFCode "MedDRA:10070510:Traumatic renal injury" ;
    ex:statusDescription "Term added for Release Number 2024. See no. 15 of Change Log" ;
    rdfs:comment "Traumatic damage to the kidney(s)." ;
    rdfs:subClassOf imdrf:E13 .

imdrf:E1401 a owl:Class ;
    rdfs:label "Abnormal Vaginal Discharge" ;
    ex:nonIMDRFCode "MedDRA:10057094:Vaginal discharge abnormality" ;
    rdfs:comment "Secretions from the vagina with a smell, colour, or texture which is different from normal." ;
    rdfs:subClassOf imdrf:E14 .

imdrf:E1402 a owl:Class ;
    rdfs:label "Breast Discomfort/Pain" ;
    ex:nonIMDRFCode "MedDRA:10006298:Breast pain" ;
    rdfs:comment "Having pain, tenderness or discomfort in the breast." ;
    rdfs:subClassOf imdrf:E14 .

imdrf:E1403 a owl:Class ;
    rdfs:label "Breast Mass" ;
    ex:nonIMDRFCode "MedDRA:10006272:Breast mass" ;
    rdfs:comment "Abnormality in the breast parenchyma, identified either by palpation or imaging. These abnormalities include calcifications, breast tissue distortion, presence of areas of density, and presence of benign or malignant tumors." ;
    rdfs:subClassOf imdrf:E14 .

imdrf:E1404 a owl:Class ;
    rdfs:label "Cervical Changes" ;
    ex:nonIMDRFCode "MedDRA:10008351:Cervix disorder" ;
    rdfs:comment "Changes such as abnormal, pathological, benign, malignant, etc." ;
    rdfs:subClassOf imdrf:E14,
        imdrf:E22 .

imdrf:E1405 a owl:Class ;
    rdfs:label "Dyspareunia" ;
    ex:nonIMDRFCode "MedDRA:10013941:Dyspareunia" ;
    rdfs:comment "Painful or difficult coitus." ;
    rdfs:subClassOf imdrf:E14 .

imdrf:E1406 a owl:Class ;
    rdfs:label "Fallopian Tube Perforation" ;
    ex:nonIMDRFCode "MedDRA:10065790:Fallopian tube perforation" ;
    rdfs:comment "A rupture in the fallopian tube due to traumatic or pathologic processes." ;
    rdfs:subClassOf imdrf:E14,
        imdrf:E2114 .

imdrf:E140701 a owl:Class ;
    rdfs:label "Intermenstrual Bleeding" ;
    ex:nonIMDRFCode "MedDRA:10022559:Intermenstrual bleeding" ;
    rdfs:comment "Uterine bleeding that occurs during a time not associated with the normal menstrual period." ;
    rdfs:subClassOf imdrf:E1407 .

imdrf:E140702 a owl:Class ;
    rdfs:label "Menorrhagia" ;
    ex:nonIMDRFCode "MedDRA:10027313:Menorrhagia" ;
    rdfs:comment "Heavy or large blood loss during menses." ;
    rdfs:subClassOf imdrf:E1407 .

imdrf:E1408 a owl:Class ;
    rdfs:label "Menstrual Irregularities" ;
    ex:nonIMDRFCode "MedDRA:10027333:Menstrual irregularity" ;
    rdfs:comment "Deviations from the normal process; e.g. delayed, difficult, profuse, scanty, unusual bleeding, etc." ;
    rdfs:subClassOf imdrf:E14 .

imdrf:E1409 a owl:Class ;
    rdfs:label "Nipple Sensation Changes" ;
    ex:nonIMDRFCode "MedDRA:10082498:Nipple sensation changes" ;
    ex:statusDescription "Editorial change to the definition on 16 February 2021." ;
    rdfs:comment "Excessive sensitivity or changes in sensitivity in the nipple(s)" ;
    rdfs:subClassOf imdrf:E14 .

imdrf:E1410 a owl:Class ;
    rdfs:label "Nipple Ulceration" ;
    ex:nonIMDRFCode "MedDRA:10029424:Nipple ulceration" ;
    rdfs:comment "Ulcer that develops in the nipple." ;
    rdfs:subClassOf imdrf:E14 .

imdrf:E1411 a owl:Class ;
    rdfs:label "Pelvic Inflammatory Disease" ;
    ex:nonIMDRFCode "MedDRA:10034254:Pelvic inflammatory disease" ;
    rdfs:comment "Any pelvic infection involving the upper female genital tract beyond the cervix." ;
    rdfs:subClassOf imdrf:E14 .

imdrf:E1412 a owl:Class ;
    rdfs:label "Rectovaginal Fistula" ;
    ex:nonIMDRFCode "MedDRA:10051097:Rectovaginal fistula" ;
    ex:statusDescription "Editorial change to the definition on 16 February 2021." ;
    rdfs:comment "Abnormal connection between rectum and vagina." ;
    rdfs:subClassOf imdrf:E14 .

imdrf:E141301 a owl:Class ;
    rdfs:label "Erectile Dysfunction" ;
    ex:nonIMDRFCode "MedDRA:10061461:Erectile dysfunction" ;
    rdfs:comment "Persistent or recurrent inability to achieve or to maintain an erection during sexual activity." ;
    rdfs:subClassOf imdrf:E1413 .

imdrf:E1414 a owl:Class ;
    rdfs:label "Toxic Shock Syndrome" ;
    ex:nonIMDRFCode "MedDRA:10044248:Toxic shock syndrome" ;
    rdfs:comment "A rare acute life-threatening systemic bacterial noncontagious illness caused by staphylococcal exotoxins." ;
    rdfs:subClassOf imdrf:E14,
        imdrf:E19 .

imdrf:E1415 a owl:Class ;
    rdfs:label "Uterine Perforation" ;
    ex:nonIMDRFCode "MedDRA:10046810:Uterine perforation" ;
    rdfs:comment "A rupture in the uterus due to traumatic or pathologic processes." ;
    rdfs:subClassOf imdrf:E14,
        imdrf:E2114 .

imdrf:E1416 a owl:Class ;
    rdfs:label "Vesicovaginal Fistula" ;
    ex:nonIMDRFCode "MedDRA:10069086:Vesicovaginal fistula" ;
    rdfs:comment "Abnormal connection between vagina and bladder." ;
    rdfs:subClassOf imdrf:E14 .

imdrf:E1417 a owl:Class ;
    rdfs:label "Unspecified Reproductive System or Breast Problem" ;
    ex:statusDescription "Term was added on 18 March 2020 for cases where the category of a health effect was reported but with no further details." ;
    rdfs:comment "The report describes a non-specific problem with the breasts or reproductive system. Note: Please use \"Appropriate Term / Code Not Available\" if the report describes a specific problem but the relevant term does not exist." ;
    rdfs:subClassOf imdrf:E14 .

imdrf:E1418 a owl:Class ;
    rdfs:label "Breast Feeding Problem" ;
    ex:statusDescription "Term was added on 27 January 2022. For details, see comment No. 158 / 160 of the Change Log (Release Number 2022)." ;
    rdfs:comment "Issues related to the ability to breastfeed." ;
    rdfs:subClassOf imdrf:E14 .

imdrf:E1419 a owl:Class ;
    rdfs:label "Vaginal Dryness" ;
    ex:nonIMDRFCode "MedDRA:10046904:Vaginal dryness" ;
    ex:statusDescription "Term was added on 31 January 2023. For details, see comment No. 92 of the Change Log (Release Number 2023)." ;
    rdfs:comment "An uncomfortable feeling of itching and burning in the vaginal opening resulting from inadequate vaginal lubrication." ;
    rdfs:subClassOf imdrf:E14 .

imdrf:E1420 a owl:Class ;
    rdfs:label "Pelvic Pain" ;
    ex:nonIMDRFCode "MedDRA:10034263:Pelvic pain" ;
    ex:statusDescription "Term was added on 31 January 2023. For details, see comment No. 93 of the Change Log (Release Number 2023)." ;
    rdfs:comment "Pain in the pelvic area" ;
    rdfs:subClassOf imdrf:E14,
        imdrf:E23 .

imdrf:E150101 a owl:Class ;
    rdfs:label "Complete Induced Abortion" ;
    ex:nonIMDRFCode "MedDRA:10060928:Abortion induced complete" ;
    rdfs:comment "Expulsion of all the products of conception following medical or surgical pregnancy termination." ;
    rdfs:subClassOf imdrf:E1501 .

imdrf:E150102 a owl:Class ;
    rdfs:label "Incomplete Induced Abortion" ;
    ex:nonIMDRFCode "MedDRA:10053984:Abortion induced incomplete" ;
    rdfs:comment "The uterus is not entirely emptied of products of conception following medical or surgical pregnancy termination." ;
    rdfs:subClassOf imdrf:E1501 .

imdrf:E150103 a owl:Class ;
    rdfs:label "Induced Abortion" ;
    ex:nonIMDRFCode "MedDRA:10021716:Induced abortion" ;
    rdfs:comment "Abortion brought on intentionally." ;
    rdfs:subClassOf imdrf:E1501 .

imdrf:E150104 a owl:Class ;
    rdfs:label "Missed Abortion" ;
    ex:nonIMDRFCode "MedDRA:10027704:Missed abortion" ;
    rdfs:comment "Retention in uterus of an abortus." ;
    rdfs:subClassOf imdrf:E1501 .

imdrf:E150105 a owl:Class ;
    rdfs:label "Spontaneous Abortion" ;
    ex:nonIMDRFCode "MedDRA:10041687:Spontaneous abortion" ;
    rdfs:comment "Spontaneous expulsion of a human fetus before it is viable." ;
    rdfs:subClassOf imdrf:E1501 .

imdrf:E1502 a owl:Class ;
    rdfs:label "Amnionitis" ;
    ex:nonIMDRFCode "MedDRA:10051242:Amnionitis" ;
    rdfs:comment "Inflammation of the amnion." ;
    rdfs:subClassOf imdrf:E15 .

imdrf:E1503 a owl:Class ;
    rdfs:label "Cephalohematoma" ;
    ex:nonIMDRFCode "MedDRA:10060531:Cephalohematoma" ;
    rdfs:comment "A subperiosteal hemorrhage limited to the surface of one cranial bone, a usually benign condition seen in the newborn as a result of bone trauma." ;
    rdfs:subClassOf imdrf:E15 .

imdrf:E1504 a owl:Class ;
    rdfs:label "Chorioamnionitis" ;
    ex:nonIMDRFCode "MedDRA:10008755:Chorioamnionitis" ;
    rdfs:comment "An infection involving chorion, amnion and amniotic fluid; generally, there is also involve placental villi and from decidua." ;
    rdfs:subClassOf imdrf:E15,
        imdrf:E19 .

imdrf:E1505 a owl:Class ;
    rdfs:label "Congenital Defect/Deformity" ;
    ex:nonIMDRFCode "MedDRA:10048305:Birth defects" ;
    rdfs:comment "Any abnormality either hereditary or due an influence that happen during the pregnancy until the moment of birth." ;
    rdfs:subClassOf imdrf:E15,
        imdrf:E16 .

imdrf:E1506 a owl:Class ;
    rdfs:label "Ectopic Pregnancy" ;
    ex:nonIMDRFCode "MedDRA:10014166:Ectopic pregnancy" ;
    rdfs:comment "Pregnancy condition that happens when there is a developing fetus or embryo outside the uterus." ;
    rdfs:subClassOf imdrf:E14,
        imdrf:E15 .

imdrf:E1507 a owl:Class ;
    rdfs:label "Fetal Distress" ;
    ex:nonIMDRFCode "MedDRA:10016486:Fetal distress" ;
    rdfs:comment "Signs or symptoms which may be indicative of distress to a fetus, which may include repetitive variable decelerations, fetal tachycardia or bradycardia, late decelerations, or low biophysical profile." ;
    rdfs:subClassOf imdrf:E06,
        imdrf:E15 .

imdrf:E1508 a owl:Class ;
    rdfs:label "Hypoxia in Utero" ;
    ex:nonIMDRFCode "MedDRA:10022748:Intra-uterine hypoxia" ;
    rdfs:comment "Caused by conditions such as inadequate placental function (often abruptio placentae), preeclamptic toxicity, prolapse of the umbilical cord, or complications from anesthetic administration." ;
    rdfs:subClassOf imdrf:E15 .

imdrf:E1509 a owl:Class ;
    rdfs:label "Incompetent Cervix" ;
    ex:nonIMDRFCode "MedDRA:10021632:Incompetent cervix" ;
    rdfs:comment "Cervix that is abnormally prone to dilate without contractions in the second trimester of pregnancy, resulting in premature expulsion of the fetus." ;
    rdfs:subClassOf imdrf:E14,
        imdrf:E15 .

imdrf:E1510 a owl:Class ;
    rdfs:label "Low Apgar Score" ;
    ex:nonIMDRFCode "MedDRA:10002944:Apgar score low" ;
    rdfs:comment "Any Apgar score less than seven. This may be the initial or a subsequent apgar score." ;
    rdfs:subClassOf imdrf:E15,
        imdrf:E22 .

imdrf:E1511 a owl:Class ;
    rdfs:label "Neonatal Deformities" ;
    ex:nonIMDRFCode "MedDRA:10082494:Neonatal deformity" ;
    rdfs:comment "Anatomic abnormality manifested during the neonatal period of physical or mechanical origin." ;
    rdfs:subClassOf imdrf:E15,
        imdrf:E16 .

imdrf:E151201 a owl:Class ;
    rdfs:label "Complete Neonatal Hearing Loss" ;
    ex:nonIMDRFCode "MedDRA:10082499:Complete neonatal hearing loss" ;
    rdfs:comment "Complete loss of the ability to detect or understand sounds present in an infant within its first month after birth." ;
    rdfs:subClassOf imdrf:E1512 .

imdrf:E151202 a owl:Class ;
    rdfs:label "Partial Neonatal Hearing loss" ;
    ex:nonIMDRFCode "MedDRA:10082496:Partial neonatal hearing loss" ;
    rdfs:comment "Partial loss of the ability to detect or understand sounds present in an infant within its first month after birth." ;
    rdfs:subClassOf imdrf:E1512 .

imdrf:E1513 a owl:Class ;
    rdfs:label "Perinatal Brain Injury" ;
    ex:nonIMDRFCode "MedDRA:10056392:Perinatal brain damage" ;
    rdfs:comment "Injury to the brain of a newborn infant occurring around the time of birth." ;
    rdfs:subClassOf imdrf:E01,
        imdrf:E15 .

imdrf:E1514 a owl:Class ;
    rdfs:label "Pregnancy with a Contraceptive Device" ;
    ex:nonIMDRFCode "MedDRA:10063130:Pregnancy with contraceptive device" ;
    rdfs:comment "The woman became pregnant despite using a contraceptive device." ;
    rdfs:subClassOf imdrf:E15 .

imdrf:E1515 a owl:Class ;
    rdfs:label "Premature Labor" ;
    ex:nonIMDRFCode "MedDRA:10036599:Premature labor" ;
    rdfs:comment "Delivery of a viable infant before the normal end of gestation." ;
    rdfs:subClassOf imdrf:E15 .

imdrf:E1516 a owl:Class ;
    rdfs:label "Respiratory Distress Syndrome of Newborns" ;
    ex:nonIMDRFCode "MedDRA:10038692:Respiratory distress syndrome in newborn" ;
    rdfs:comment "A condition of the newborn marked by dyspnea with cyanosis." ;
    rdfs:subClassOf imdrf:E07,
        imdrf:E15 .

imdrf:E1517 a owl:Class ;
    rdfs:label "Teratogenic Effects" ;
    ex:nonIMDRFCode "MedDRA:10043275:Teratogenicity" ;
    rdfs:comment "Appearance of anomalies and/or developmental defects due to exposure to an agent that can disturb the development of an embryo or fetus." ;
    rdfs:subClassOf imdrf:E15 .

imdrf:E1518 a owl:Class ;
    rdfs:label "Toxins In Children" ;
    ex:nonIMDRFCode "MedDRA:10053487:Exposure to toxic agent" ;
    rdfs:comment "Children affected by toxins may be due to silicone breast implants and their effects on unborn children and from breastfeeding." ;
    rdfs:subClassOf imdrf:E15 .

imdrf:E1519 a owl:Class ;
    rdfs:label "Vaginal Mucosa Damage" ;
    ex:nonIMDRFCode "MedDRA:10080926:Vaginal mucosal damage" ;
    rdfs:comment "Injury to vaginal mucosa." ;
    rdfs:subClassOf imdrf:E14,
        imdrf:E15 .

imdrf:E1520 a owl:Class ;
    rdfs:label "Infertility" ;
    ex:nonIMDRFCode "MedDRA:10021926:Infertility" ;
    ex:statusDescription "Term was added on 27 January 2022. For details, see comment No. 159 / 206 of the Change Log (Release Number 2022)." ;
    rdfs:comment "Inability to conceive for at least one year after trying and having unprotected sex. Causes of female infertility include endometriosis, fallopian tubes obstruction, and polycystic ovary syndrome. Causes of male infertility include abnormal sperm production or function, blockage of the epididymis, blockage of the ejaculatory ducts and hypospadias." ;
    rdfs:subClassOf imdrf:E15 .

imdrf:E1601 a owl:Class ;
    rdfs:label "Arthralgia" ;
    ex:nonIMDRFCode "MedDRA:10003239:Arthralgia" ;
    rdfs:comment "Pain in a joint." ;
    rdfs:subClassOf imdrf:E16 .

imdrf:E160201 a owl:Class ;
    rdfs:label "Rheumatoid Arthritis" ;
    ex:nonIMDRFCode "MedDRA:10039073:Rheumatoid arthritis" ;
    rdfs:comment "A chronic systemic disease, primarily of the joints, marked by inflammatory changes in the synovial membranes and articular structures, widespread fibrinoid degeneration of the collagen fibers in mesenchymal tissues, and by atrophy and rarefaction of bony structures." ;
    rdfs:subClassOf imdrf:E1602 .

imdrf:E160301 a owl:Class ;
    rdfs:label "Hip Fracture" ;
    ex:nonIMDRFCode "MedDRA:10020100:Hip fracture" ;
    rdfs:comment "Traumatic or pathological injury to the hip in which the continuity of either the femoral head, femoral neck, intertrochanteric or subtrochanteric regions is broken." ;
    rdfs:subClassOf imdrf:E1603 .

imdrf:E160302 a owl:Class ;
    rdfs:label "Limb Fracture" ;
    ex:nonIMDRFCode "MedDRA:10074551:Limb fracture" ;
    rdfs:comment "A traumatic break in one or more of the bones in a limb." ;
    rdfs:subClassOf imdrf:E1603 .

imdrf:E160303 a owl:Class ;
    rdfs:label "Multiple Fractures" ;
    ex:nonIMDRFCode "MedDRA:10028200:Multiple fractures" ;
    rdfs:comment "Two or more simultaneous traumatic breaks in one or more bones." ;
    rdfs:subClassOf imdrf:E1603 .

imdrf:E160304 a owl:Class ;
    rdfs:label "Skull Fracture" ;
    ex:nonIMDRFCode "MedDRA:10061365:Skull fracture" ;
    rdfs:comment "A traumatic or pathologic injury to the bones of the skull in which the continuity of the bones of the skull is broken." ;
    rdfs:subClassOf imdrf:E1603 .

imdrf:E160305 a owl:Class ;
    rdfs:label "Vertebral Fracture" ;
    ex:nonIMDRFCode "MedDRA:10047333:Vertebral fracture" ;
    rdfs:comment "Traumatic or pathological injury to the spine in which the continuity of a vertebral bone is broken." ;
    rdfs:subClassOf imdrf:E1603 .

imdrf:E1604 a owl:Class ;
    rdfs:label "Connective Tissue Disease" ;
    ex:nonIMDRFCode "MedDRA:10061087:Connective tissue disorder" ;
    rdfs:comment "A non-neoplastic or neoplastic disorder that affects the connective tissue." ;
    rdfs:subClassOf imdrf:E16 .

imdrf:E160501 a owl:Class ;
    rdfs:label "Abdominal Cramps" ;
    ex:nonIMDRFCode "MedDRA:10000057:Abdominal cramps" ;
    rdfs:comment "An involuntary muscular contraction involving a muscle of the abdomen or of a hollow organ within the abdomen." ;
    rdfs:subClassOf imdrf:E1605 .

imdrf:E1606 a owl:Class ;
    rdfs:label "Damage to Ligament(s)" ;
    ex:nonIMDRFCode "MedDRA:10061223:Ligament injury" ;
    rdfs:comment "An injury to any of the fibrous bands of tissue that comprise an articulation (joint)." ;
    rdfs:subClassOf imdrf:E16,
        imdrf:E20 .

imdrf:E1607 a owl:Class ;
    rdfs:label "Difficulty Chewing" ;
    ex:nonIMDRFCode "MedDRA:10067464:Chewing difficulty" ;
    rdfs:comment "Problem with mastication due to pain, discomfort or loss of mobility in the jaw." ;
    rdfs:subClassOf imdrf:E10,
        imdrf:E16 .

imdrf:E1608 a owl:Class ;
    rdfs:label "Fasciitis" ;
    ex:nonIMDRFCode "MedDRA:10016228:Fasciitis" ;
    rdfs:comment "Inflammation of fascia." ;
    rdfs:subClassOf imdrf:E16 .

imdrf:E1609 a owl:Class ;
    rdfs:label "Fibromyositis" ;
    ex:nonIMDRFCode "MedDRA:10063041:Fibromyositis" ;
    rdfs:comment "Inflammation and fibrous degeneration of a muscle." ;
    rdfs:subClassOf imdrf:E16,
        imdrf:E19 .

imdrf:E1610 a owl:Class ;
    rdfs:label "Head Injury" ;
    ex:nonIMDRFCode "MedDRA:10019196:Head injury" ;
    rdfs:comment "A traumatic injury to the head." ;
    rdfs:subClassOf imdrf:E16,
        imdrf:E20 .

imdrf:E1611 a owl:Class ;
    rdfs:label "Hyperextension" ;
    ex:nonIMDRFCode "MedDRA:10062310:Joint hyperextension" ;
    rdfs:comment "Forceful extension of a joint beyond its normal limits." ;
    rdfs:subClassOf imdrf:E16 .

imdrf:E161201 a owl:Class ;
    rdfs:label "Aseptic loosening" ;
    ex:nonIMDRFCode "MedDRA:10090445:Aseptic joint prosthesis loosening" ;
    ex:statusDescription "Term added for Release Number 2024. See no. 69 of Change Log" ;
    rdfs:comment "Failure of the fixation of a prosthetic component in the absence of infection." ;
    rdfs:subClassOf imdrf:E1612 .

imdrf:E161202 a owl:Class ;
    rdfs:label "Septic loosening" ;
    ex:nonIMDRFCode "MedDRA:10090446:Septic joint prosthesis loosening" ;
    ex:statusDescription "Term added for Release Number 2024. See no. 70 of Change Log" ;
    rdfs:comment "Failure of the fixation of a prosthetic component in the presence of infection." ;
    rdfs:subClassOf imdrf:E1612 .

imdrf:E1613 a owl:Class ;
    rdfs:label "Intervertebral Disc Compression or Protrusion" ;
    ex:nonIMDRFCode "MedDRA:10055039:Intervertebral disc compression" ;
    rdfs:comment "Degenerative, pathological or traumatic changes in the cartilaginous tissue of the spine leading to unwanted compression or protrusion of the disc." ;
    rdfs:subClassOf imdrf:E16 .

imdrf:E161401 a owl:Class ;
    rdfs:label "Subluxation" ;
    ex:nonIMDRFCode "MedDRA:10042402:Subluxation" ;
    rdfs:comment "Partial dislocation of the bones in a joint." ;
    rdfs:subClassOf imdrf:E1614 .

imdrf:E1615 a owl:Class ;
    rdfs:label "Joint Laxity" ;
    ex:nonIMDRFCode "MedDRA:10070874:Joint laxity" ;
    rdfs:comment "Looseness or instability of a joint." ;
    rdfs:subClassOf imdrf:E16 .

imdrf:E161601 a owl:Class ;
    rdfs:label "Ankylosis" ;
    ex:nonIMDRFCode "MedDRA:10002559:Ankylosis" ;
    rdfs:comment "Immobility of the joint due to the formation of bone, cartilaginous or fibrous tissues around the joints." ;
    rdfs:subClassOf imdrf:E1616 .

imdrf:E161602 a owl:Class ;
    rdfs:label "Joint Contracture" ;
    ex:nonIMDRFCode "MedDRA:10023201:Joint contracture" ;
    rdfs:comment "Permanent restriction of a joint, usually resulting from prolonged spasticity in a muscle area." ;
    rdfs:subClassOf imdrf:E1616 .

imdrf:E161603 a owl:Class ;
    rdfs:label "Muscular Rigidity" ;
    ex:nonIMDRFCode "MedDRA:10028330:Muscle rigidity" ;
    rdfs:comment "An involuntary, persistent state of firm, tense muscles with marked resistance to passive movement." ;
    rdfs:subClassOf imdrf:E1616 .

imdrf:E161604 a owl:Class ;
    rdfs:label "Arthrofibrosis" ;
    ex:nonIMDRFCode "MedDRA:10058029:Arthrofibrosis" ;
    ex:statusDescription "Term added for Release Number 2024. See no. 71 of Change Log" ;
    rdfs:comment "Fibrotic joint disorder characterized by excessive collagen production and adhesions that result in restricted joint motion and pain." ;
    rdfs:subClassOf imdrf:E1616 .

imdrf:E161605 a owl:Class ;
    rdfs:label "Joint locking" ;
    ex:nonIMDRFCode "MedDRA:10061258:Joint lock" ;
    ex:statusDescription "Term added for Release Number 2024. See no. 72 of Change Log" ;
    rdfs:comment """Joint is blocked or becomes stuck.
For Pseudo-locking use E1616 - Loss of Range of Motion.""" ;
    rdfs:subClassOf imdrf:E1616 .

imdrf:E1617 a owl:Class ;
    rdfs:label "Malunion of Bone" ;
    ex:nonIMDRFCode "MedDRA:10026729:Malunion of fracture" ;
    rdfs:comment "Faulty healing of bone, resulting in improper anatomical alignment." ;
    rdfs:subClassOf imdrf:E16 .

imdrf:E1618 a owl:Class ;
    rdfs:label "Metal Related Pathology" ;
    ex:nonIMDRFCode "MedDRA:10081986:Periprosthetic metallosis" ;
    ex:statusDescription "Definition was modified on 27 January 2022 (Old definition: Aseptic fibrosis or local necrosis secondary to metal corrosion and release of wear debris. It's also known as Metallosis.). For details, see comment No. 114 / 203 of the Change Log (Release Number 2022)." ;
    rdfs:comment "Also known as Metallosis. Includes trunnionosis, aseptic fibrosis or local necrosis secondary to metal corrosion and release of wear debris." ;
    rdfs:subClassOf imdrf:E16 .

imdrf:E1619 a owl:Class ;
    rdfs:label "Muscle Hypotonia" ;
    ex:nonIMDRFCode "MedDRA:10081180:Muscle hypotonia" ;
    rdfs:comment "Abnormally low level of muscle tone." ;
    rdfs:subClassOf imdrf:E16 .

imdrf:E1620 a owl:Class ;
    rdfs:label "Muscle/Tendon Damage" ;
    ex:nonIMDRFCode "MedDRA:10028314:Muscle injury" ;
    rdfs:comment "Any injury to muscle or tendon tissue including strains." ;
    rdfs:subClassOf imdrf:E16 .

imdrf:E1621 a owl:Class ;
    rdfs:label "Muscle Weakness/Atrophy" ;
    ex:nonIMDRFCode "MedDRA:10028350:Muscle weakness" ;
    ex:statusDescription "Term/Definition was modified on 27 January 2022 (Old term/definition: Muscle Weakness: A reduction in the strength of one or more muscles.) For details, see comment No. 120 of the Change Log (Release Number 2022)." ;
    rdfs:comment "A reduction in the strength and/or mass of one or more muscles." ;
    rdfs:subClassOf imdrf:E01,
        imdrf:E16 .

imdrf:E1622 a owl:Class ;
    rdfs:label "Myalgia" ;
    ex:nonIMDRFCode "MedDRA:10028411:Myalgia" ;
    rdfs:comment "Pain sensation originating from a muscle or group of muscles." ;
    rdfs:subClassOf imdrf:E16,
        imdrf:E2330 .

imdrf:E1623 a owl:Class ;
    rdfs:label "Neck Pain" ;
    ex:nonIMDRFCode "MedDRA:10028836:Neck pain" ;
    rdfs:comment "Pain in the neck area." ;
    rdfs:subClassOf imdrf:E16,
        imdrf:E2330 .

imdrf:E1624 a owl:Class ;
    rdfs:label "Neck Stiffness" ;
    ex:nonIMDRFCode "MedDRA:10028843:Neck stiffness" ;
    rdfs:comment "Limited mobility of the neck, usually accompanied by pain." ;
    rdfs:subClassOf imdrf:E16 .

imdrf:E1625 a owl:Class ;
    rdfs:label "Nonunion/Delayed-union Bone Fracture" ;
    ex:nonIMDRFCode "MedDRA:10017081:Fracture delayed union" ;
    ex:statusDescription "Term/Definition was modified on 27 January 2022 (Old term/definition: Nonunion Bone Fracture: Broken bone that doesn't heal.) MedDRA mapping also updated from Nonunion of fracture(10029746) to Fracture delayed union(10017081). For details, see comment No. 117 of the Change Log (Release Number 2022)." ;
    rdfs:comment "Broken bone that doesn't heal or is delayed in healing." ;
    rdfs:subClassOf imdrf:E16 .

imdrf:E1626 a owl:Class ;
    rdfs:label "Extraskeletal ossification" ;
    ex:nonIMDRFCode "MedDRA:10049811:Extraskeletal ossification" ;
    ex:statusDescription "Term and Definition and MedDRA map modified for Release Number 2024. Previous term was Ossification. Previous MedDRA map was 10065453:Ectopic ossification. See no. 73 of Change Log." ;
    rdfs:comment "The formation of bone or of a bony substance outside the normal skeleton. Includes ectopic or heterotopic ossification, myositis ossificans." ;
    rdfs:subClassOf imdrf:E16 .

imdrf:E1627 a owl:Class ;
    rdfs:label "Osteolysis" ;
    ex:nonIMDRFCode "MedDRA:10031248:Osteolysis" ;
    rdfs:comment "Dissolution of bone; applied especially to the removal or loss of the calcium of bone." ;
    rdfs:subClassOf imdrf:E16 .

imdrf:E1628 a owl:Class ;
    rdfs:label "Osteomyelitis" ;
    ex:nonIMDRFCode "MedDRA:10031252:Osteomyelitis" ;
    rdfs:comment "Infection of bone or bone marrow." ;
    rdfs:subClassOf imdrf:E16,
        imdrf:E19 .

imdrf:E1629 a owl:Class ;
    rdfs:label "Osteopenia/ Osteoporosis" ;
    ex:nonIMDRFCode "MedDRA:10049088:Osteopenia" ;
    rdfs:comment "Decreased calcification or density of bone tissue." ;
    rdfs:subClassOf imdrf:E16 .

imdrf:E1630 a owl:Class ;
    rdfs:label "Polymyositis" ;
    ex:nonIMDRFCode "MedDRA:10036102:Polymyositis" ;
    rdfs:comment "An idiopathic inflammatory disorder affecting the muscles. It presents with symmetrical proximal muscle weakness and elevated skeletal muscle enzymes." ;
    rdfs:subClassOf imdrf:E16 .

imdrf:E1631 a owl:Class ;
    rdfs:label "Spinal Column Injury" ;
    ex:nonIMDRFCode "MedDRA:10069689:Spinal column injury" ;
    rdfs:comment "Damage to the bones of the spine." ;
    rdfs:subClassOf imdrf:E16,
        imdrf:E20 .

imdrf:E1632 a owl:Class ;
    rdfs:label "Synovitis" ;
    ex:nonIMDRFCode "MedDRA:10042868:Synovitis" ;
    rdfs:comment "Inflammation of a synovial membrane." ;
    rdfs:subClassOf imdrf:E16,
        imdrf:E19 .

imdrf:E1633 a owl:Class ;
    rdfs:label "Tooth Fracture" ;
    ex:nonIMDRFCode "MedDRA:10062544:Tooth fracture" ;
    rdfs:comment "Breakage of any portion of the tooth." ;
    rdfs:subClassOf imdrf:E16,
        imdrf:E20 .

imdrf:E1634 a owl:Class ;
    rdfs:label "Unequal Limb Length" ;
    ex:nonIMDRFCode "MedDRA:10065738:Unequal limb length" ;
    rdfs:comment "Discrepancy between the lengths of the lower or upper extremities." ;
    rdfs:subClassOf imdrf:E16 .

imdrf:E1635 a owl:Class ;
    rdfs:label "Unspecified Musculoskeletal problem" ;
    ex:statusDescription "Term was added on 18 March 2020 for cases where the category of a health effect was reported but with no further details." ;
    rdfs:comment "The report describes a non-specific problem with the musculoskeletal system. Note: Please use \"Appropriate Term / Code Not Available\" if the report describes a specific problem but the relevant term does not exist." ;
    rdfs:subClassOf imdrf:E16 .

imdrf:E1636 a owl:Class ;
    rdfs:label "Tooth Loss" ;
    ex:nonIMDRFCode "MedDRA:10044044:Tooth loss" ;
    ex:statusDescription "Term was added on 27 January 2022. For details, see comment No. 218 of the Change Log (Release Number 2022)." ;
    rdfs:comment "One or more teeth lost/dislodged from the mouth." ;
    rdfs:subClassOf imdrf:E16 .

imdrf:E1637 a owl:Class ;
    rdfs:label "Bursitis" ;
    ex:nonIMDRFCode "MedDRA:10006811:Bursitis" ;
    ex:statusDescription "Term was added on 27 January 2022. For details, see comment No. 112 of the Change Log (Release Number 2022)." ;
    rdfs:comment "Inflammation of the fluid-filled pad (bursa)." ;
    rdfs:subClassOf imdrf:E16 .

imdrf:E1638 a owl:Class ;
    rdfs:label "Cartilage damage" ;
    ex:nonIMDRFCode "MedDRA:10007705:Cartilage damage" ;
    ex:statusDescription "Term was added on 27 January 2022. For details, see comment No. 113 of the Change Log (Release Number 2022)." ;
    rdfs:comment "Damage of cartilage." ;
    rdfs:subClassOf imdrf:E16 .

imdrf:E1639 a owl:Class ;
    rdfs:label "Joint Impingement" ;
    ex:nonIMDRFCode "MedDRA:10087218:Joint impingement" ;
    ex:statusDescription "Term was added on 27 January 2022. For details, see comment No. 119 of the Change Log (Release Number 2022)." ;
    rdfs:comment "Impingement relating to joints. Can be e.g. implant-on-bone, implant-on-soft tissue, or implant-on-implant impingement." ;
    rdfs:subClassOf imdrf:E16 .

imdrf:E1640 a owl:Class ;
    rdfs:label "Mastoiditis" ;
    ex:nonIMDRFCode "MedDRA:10026900:Mastoiditis" ;
    ex:statusDescription "Term was added on 27 January 2022. For details, see comment No. 241 of the Change Log (Release Number 2022)." ;
    rdfs:comment "An infection of the bony air cells in the mastoid bone." ;
    rdfs:subClassOf imdrf:E16,
        imdrf:E19 .

imdrf:E1641 a owl:Class ;
    rdfs:label "Limb Pain" ;
    ex:nonIMDRFCode "MedDRA:10033447:Pain in limb" ;
    ex:statusDescription "Term was added on 27 January 2022. For details, see comment No. 57 / 187 of the Change Log (Release Number 2022)." ;
    rdfs:comment "Pain in the arms and/or legs." ;
    rdfs:subClassOf imdrf:E16 .

imdrf:E1642 a owl:Class ;
    rdfs:label "Spinal deformity" ;
    ex:nonIMDRFCode "MedDRA:10058907:Spinal deformity" ;
    ex:statusDescription "Term added for Release Number 2024. See no. 18 of Change Log" ;
    rdfs:comment "Abnormal curvature and/or alignment of the spine." ;
    rdfs:subClassOf imdrf:E16 .

imdrf:E1643 a owl:Class ;
    rdfs:label "Tendinopathy" ;
    ex:nonIMDRFCode "MedDRA:10080130:Tendinopathy" ;
    ex:statusDescription "Term added for Release Number 2024. See no. 68 of Change Log" ;
    rdfs:comment "Overuse tendon injuries characterized by a combination of pain, diffuse or localized swelling, and impaired performance. Problems include tendonitis/tendinitis and tendinosis, as well as tendon tears and inflammation of membranes around a tendon" ;
    rdfs:subClassOf imdrf:E16 .

imdrf:E1644 a owl:Class ;
    rdfs:label "Compartment syndrome" ;
    ex:nonIMDRFCode "MedDRA:10010121:Compartment syndrome" ;
    ex:statusDescription "Term added for Release Number 2024. See no. 74 of Change Log" ;
    rdfs:comment "Condition in which a closed muscle compartment's pressure increases to such an extent that the circulation is diminished, e.g. due to decrease in a compartment volume or an increase in the contents of a compartment, or both." ;
    rdfs:subClassOf imdrf:E05,
        imdrf:E16 .

imdrf:E1645 a owl:Class ;
    rdfs:label "Hemarthrosis" ;
    ex:nonIMDRFCode "MedDRA:10019409:Hemarthrosis" ;
    ex:statusDescription "Term added for Release Number 2024. See no. 75 of Change Log" ;
    rdfs:comment "Bleeding into the joints" ;
    rdfs:subClassOf imdrf:E05,
        imdrf:E16 .

imdrf:E1646 a owl:Class ;
    rdfs:label "Bone Notching" ;
    ex:nonIMDRFCode "MedDRA:10057328:Bone Injury" ;
    ex:statusDescription "Term added for Release Number 2024. See no. 76 of Change Log" ;
    rdfs:comment "An indentation made at the edge of the bone without bone breakage." ;
    rdfs:subClassOf imdrf:E16,
        imdrf:E21 .

imdrf:E1647 a owl:Class ;
    rdfs:label "Exostosis (bone)" ;
    ex:nonIMDRFCode "MedDRA:10015688:Exostosis" ;
    ex:statusDescription "Term added for Release Number 2024. See no. 77 of Change Log" ;
    rdfs:comment "Benign hypertrophy that projects outward from the surface of bone, often containing a cartilaginous component, such as bone spurs/osteophytes." ;
    rdfs:subClassOf imdrf:E16 .

imdrf:E1648 a owl:Class ;
    rdfs:label "Acetabular protrusion" ;
    ex:nonIMDRFCode "MedDRA:10090179:Acetabular protrusion" ;
    ex:status "Modified (editorial)" ;
    ex:statusDescription "Term added for Release Number 2024. See no. 90 of Change Log. MedDRA map modified for release No. 2025.  Previous MedDRA map was 10045982:Unspecified intrapelvic protrusion of acetabulum" ;
    rdfs:comment "Acetabular defect with a shift of the femoral head through the pelvic bone." ;
    rdfs:subClassOf imdrf:E16 .

imdrf:E1649 a owl:Class ;
    rdfs:label "Crepitus" ;
    ex:nonIMDRFCode "MedDRA:10051374:Joint crepitation" ;
    ex:statusDescription "Term added for Release Number 2024. See no. 91 of Change Log" ;
    rdfs:comment "Grating sound or sensation produced by friction between e.g. bone, cartilage, fractured parts of a bone." ;
    rdfs:subClassOf imdrf:E16 .

imdrf:E1650 a owl:Class ;
    rdfs:label "Arthropathy" ;
    ex:nonIMDRFCode "MedDRA:10003285:Arthropathy" ;
    ex:statusDescription "Term added for Release Number 2024. See no. 103 of Change Log" ;
    rdfs:comment """Diseases and disorders of a joint (e.g. Rotator cuff arthropathy, cuff tear arthropathy (CTA)) 
More specific codes and terms should be used where they exist e.g. E1602 - Arthritis""" ;
    rdfs:subClassOf imdrf:E16 .

imdrf:E1651 a owl:Class ;
    rdfs:label "Back pain" ;
    ex:nonIMDRFCode "MedDRA:10003988:Back pain" ;
    ex:statusDescription "Term added for Release Number 2024. See no. 107 of Change Log" ;
    rdfs:comment "Pain in any part of the back." ;
    rdfs:subClassOf imdrf:E16,
        imdrf:E2330 .

imdrf:E1652 a owl:Class ;
    rdfs:label "Loose body in joint" ;
    ex:nonIMDRFCode "MedDRA:10024829:Loose body in joint" ;
    ex:status "New" ;
    ex:statusDescription "Term added for Release Number 2025. See no. 69 of Change Log" ;
    rdfs:comment "Presence of fibrous, bony, cartilaginous or osseocartilaginous fragments in a synovial joint." ;
    rdfs:subClassOf imdrf:E16 .

imdrf:E1701 a owl:Class ;
    rdfs:label "Abrasion" ;
    ex:nonIMDRFCode "MedDRA:10080919:Abrasion" ;
    rdfs:comment "Superficial damage to the skin caused by rubbing or scraping." ;
    rdfs:subClassOf imdrf:E17,
        imdrf:E20 .

imdrf:E1702 a owl:Class ;
    rdfs:label "Angioedema" ;
    ex:nonIMDRFCode "MedDRA:10002424:Angioedema" ;
    rdfs:comment "Rapid swelling of the deep layers of the skin due to transient vascular leakage of serous fluid." ;
    rdfs:subClassOf imdrf:E17,
        imdrf:E2338 .

imdrf:E1703 a owl:Class ;
    rdfs:label "Blister" ;
    ex:nonIMDRFCode "MedDRA:10005191:Blister" ;
    rdfs:comment "A collection of fluid underneath the top layer of skin." ;
    rdfs:subClassOf imdrf:E17 .

imdrf:E170401 a owl:Class ;
    rdfs:label "Caustic/Chemical Burns" ;
    ex:nonIMDRFCode "MedDRA:10008420:Chemical burn" ;
    rdfs:comment "A burn caused by exposure to chemical substances." ;
    rdfs:subClassOf imdrf:E1704 .

imdrf:E170402 a owl:Class ;
    rdfs:label "Cryogenic Burn" ;
    ex:nonIMDRFCode "MedDRA:10081985:Cold burn" ;
    rdfs:comment "Local tissue damage due to exposure to extreme cold." ;
    rdfs:subClassOf imdrf:E1704 .

imdrf:E170403 a owl:Class ;
    rdfs:label "Radiation Burn" ;
    ex:nonIMDRFCode "MedDRA:10063640:Radiation burn" ;
    rdfs:comment "A burn caused by exposure to x-ray, radium, sunlight, ionizing radiation or any other type of radiant energy." ;
    rdfs:subClassOf imdrf:E1704 .

imdrf:E170404 a owl:Class ;
    rdfs:label "Superficial (First Degree) Burn" ;
    ex:nonIMDRFCode "MedDRA:10016700:First degree burns" ;
    rdfs:comment "A burn that affects the epidermis only, causing erythema without blistering." ;
    rdfs:subClassOf imdrf:E1704 .

imdrf:E170405 a owl:Class ;
    rdfs:label "Partial thickness (Second Degree) Burn" ;
    ex:nonIMDRFCode "MedDRA:10039798:Second degree burns" ;
    rdfs:comment "A burn that affects the epidermis and the dermis." ;
    rdfs:subClassOf imdrf:E1704 .

imdrf:E170406 a owl:Class ;
    rdfs:label "Full thickness (Third Degree) Burn" ;
    ex:nonIMDRFCode "MedDRA:10043441:Third degree burns" ;
    rdfs:comment "A burn to the skin that extends into deeper layers and underlying tissues." ;
    rdfs:subClassOf imdrf:E1704 .

imdrf:E170501 a owl:Class ;
    rdfs:label "Skin Burning Sensation" ;
    ex:nonIMDRFCode "MedDRA:10054786:Skin burning sensation" ;
    rdfs:comment "A sensation of dermal stinging or heat, not necessarily accompanied by redness or physical signs of skin irritation." ;
    rdfs:subClassOf imdrf:E1705 .

imdrf:E1706 a owl:Class ;
    rdfs:label "Cancer Cells Dissemination" ;
    ex:nonIMDRFCode "MedDRA:10082075:Iatrogenic metastasis" ;
    rdfs:comment "Spreading benign or malignant tissue during medical procedures." ;
    rdfs:subClassOf imdrf:E17 .

imdrf:E1707 a owl:Class ;
    rdfs:label "Impaired Healing" ;
    ex:nonIMDRFCode "MedDRA:10021519:Impaired healing" ;
    ex:statusDescription "Term moved and Definition modified for Release Number 2024. See no. 84 of Change Log. Please be aware that the code does not represent the current hierarchy." ;
    rdfs:comment "Improper repair of any body tissue due to factors affecting one or more of the phases of wound healing. Includes impaired healing of any body tissue." ;
    rdfs:subClassOf imdrf:E23 .

imdrf:E1708 a owl:Class ;
    rdfs:label "Itching Sensation" ;
    ex:nonIMDRFCode "MedDRA:10023084:Itching" ;
    rdfs:comment "An irritating feeling that produces the desire to scratch." ;
    rdfs:subClassOf imdrf:E17 .

imdrf:E1709 a owl:Class ;
    rdfs:label "Jaundice" ;
    ex:nonIMDRFCode "MedDRA:10023126:Jaundice" ;
    rdfs:comment "Yellow pigmentation of the skin, mucous membranes, and the eyes due to hyperbilirubinemia." ;
    rdfs:subClassOf imdrf:E17 .

imdrf:E1710 a owl:Class ;
    rdfs:label "Localized Skin Lesion" ;
    ex:nonIMDRFCode "MedDRA:10040882:Skin lesion" ;
    rdfs:comment "A pathologic process that affects the skin and is confined to a specific area." ;
    rdfs:subClassOf imdrf:E17 .

imdrf:E1711 a owl:Class ;
    rdfs:label "Peeling" ;
    ex:nonIMDRFCode "MedDRA:10034218:Peeling" ;
    rdfs:comment "A peeling off or loss of epidermis, as in sunburn, postscarlatinal peeling, or toxic epidermal necrolysis." ;
    rdfs:subClassOf imdrf:E17 .

imdrf:E1712 a owl:Class ;
    rdfs:label "Phototoxicity" ;
    ex:nonIMDRFCode "MedDRA:10034977:Phototoxicity" ;
    rdfs:comment "A nonimmunologic, chemically induced type of photosensitivity." ;
    rdfs:subClassOf imdrf:E17 .

imdrf:E1713 a owl:Class ;
    rdfs:label "Pocket Erosion" ;
    ex:nonIMDRFCode "MedDRA:10035771:Pocket erosion" ;
    rdfs:comment "Erosion of patient's tissue pocket which houses a device." ;
    rdfs:subClassOf imdrf:E17,
        imdrf:E2006 .

imdrf:E1714 a owl:Class ;
    rdfs:label "Rash" ;
    ex:nonIMDRFCode "MedDRA:10037844:Rash" ;
    rdfs:comment "An eruption in the skin which effects its appearance and/or texture." ;
    rdfs:subClassOf imdrf:E17 .

imdrf:E171501 a owl:Class ;
    rdfs:label "Abnormal scarring" ;
    ex:nonIMDRFCode "MedDRA:10080564:Abnormal scarring" ;
    ex:statusDescription "Term added for Release Number 2024. See no. 108 and 109 of Change Log" ;
    rdfs:comment "Excessive or unusual scarring related to impaired wound healing (e.g. Keloid or Hypertrophic scar)" ;
    rdfs:subClassOf imdrf:E1715 .

imdrf:E171601 a owl:Class ;
    rdfs:label "Erythema" ;
    ex:nonIMDRFCode "MedDRA:10015150:Erythema" ;
    rdfs:comment "Red discoloration of the skin." ;
    rdfs:subClassOf imdrf:E1716 .

imdrf:E171602 a owl:Class ;
    rdfs:label "Hyperpigmentation" ;
    ex:nonIMDRFCode "MedDRA:10040865:Skin hyperpigmentation" ;
    ex:statusDescription "Term was added on 27 January 2022. For details, see comment No. 105 of the Change Log (Release Number 2022)." ;
    rdfs:comment "Darkening of the skin due to excessive melanin deposition." ;
    rdfs:subClassOf imdrf:E1716 .

imdrf:E171603 a owl:Class ;
    rdfs:label "Hypopigmentation" ;
    ex:nonIMDRFCode "MedDRA:10040868:Skin hypopigmentation" ;
    ex:statusDescription "Term was added on 27 January 2022. For details, see comment No. 106 of the Change Log (Release Number 2022)." ;
    rdfs:comment "Abnormal lightening of skin due to decreased melanin production or deposition." ;
    rdfs:subClassOf imdrf:E1716 .

imdrf:E1717 a owl:Class ;
    rdfs:label "Skin Disorders" ;
    ex:nonIMDRFCode "MedDRA:10040831:Skin disorder" ;
    rdfs:comment "Affecting the skin." ;
    rdfs:subClassOf imdrf:E17 .

imdrf:E1718 a owl:Class ;
    rdfs:label "Skin Erosion" ;
    ex:nonIMDRFCode "MedDRA:10040840:Skin erosion" ;
    rdfs:comment "A gradual breakdown or very shallow ulceration of the skin which involves only the epidermis and heals without scarring." ;
    rdfs:subClassOf imdrf:E17,
        imdrf:E2006 .

imdrf:E1719 a owl:Class ;
    rdfs:label "Skin Infection" ;
    ex:nonIMDRFCode "MedDRA:10040872:Skin infection" ;
    rdfs:comment "An inflammatory process affecting the skin, caused by bacteria, viruses, parasites, or fungi." ;
    rdfs:subClassOf imdrf:E17,
        imdrf:E19 .

imdrf:E172001 a owl:Class ;
    rdfs:label "Abscess" ;
    ex:nonIMDRFCode "MedDRA:10000269:Abscess" ;
    rdfs:comment "An inflammatory process characterized by the accumulation of pus within a newly formed tissue cavity." ;
    rdfs:subClassOf imdrf:E1720,
        imdrf:E19 .

imdrf:E172002 a owl:Class ;
    rdfs:label "Cellulitis" ;
    ex:nonIMDRFCode "MedDRA:10007882:Cellulitis" ;
    rdfs:comment "Inflammation of the dermis and subcutaneous tissues caused by a bacterial infection." ;
    rdfs:subClassOf imdrf:E1720,
        imdrf:E19 .

imdrf:E172003 a owl:Class ;
    rdfs:label "Contact Dermatitis" ;
    ex:nonIMDRFCode "MedDRA:10056540:Dermatitis irritant contact" ;
    rdfs:comment "An inflammatory skin condition caused by direct contact between the skin and either an irritating substance or an allergen." ;
    rdfs:subClassOf imdrf:E1720 .

imdrf:E172004 a owl:Class ;
    rdfs:label "Eczema" ;
    ex:nonIMDRFCode "MedDRA:10014184:Eczema" ;
    rdfs:comment "A form of dermatitis characterized by red, itchy, scaly, or crusty patches that can be chronic or intermittent." ;
    rdfs:subClassOf imdrf:E1720 .

imdrf:E172005 a owl:Class ;
    rdfs:label "Radiodermatitis" ;
    ex:nonIMDRFCode "MedDRA:10061103:Dermatitis radiation" ;
    rdfs:comment "A cutaneous inflammatory reaction occurring as a result of exposure to biologically effective levels of ionizing radiation." ;
    rdfs:subClassOf imdrf:E1720 .

imdrf:E172006 a owl:Class ;
    rdfs:label "Urticaria" ;
    ex:nonIMDRFCode "MedDRA:10046735:Urticaria" ;
    rdfs:comment "A transient, itchy skin eruption characterized by wheals with pale interiors and red margins." ;
    rdfs:subClassOf imdrf:E1720 .

imdrf:E172007 a owl:Class ;
    rdfs:label "Wheal(s)" ;
    ex:nonIMDRFCode "MedDRA:10047918:Wheals" ;
    rdfs:comment "A smooth, slightly elevated area on the body surface, which is redder or paler than the surrounding skin." ;
    rdfs:subClassOf imdrf:E1720 .

imdrf:E1721 a owl:Class ;
    rdfs:label "Skin Tears" ;
    ex:nonIMDRFCode "MedDRA:10048704:Skin tear" ;
    rdfs:comment "A break in skin tissue caused by friction or shearing." ;
    rdfs:subClassOf imdrf:E17 .

imdrf:E1722 a owl:Class ;
    rdfs:label "Subcutaneous Nodule" ;
    ex:nonIMDRFCode "MedDRA:10042348:Subcutaneous nodule" ;
    rdfs:comment "A small palpable abnormal mass in the subcutaneous tissues." ;
    rdfs:subClassOf imdrf:E17 .

imdrf:E1723 a owl:Class ;
    rdfs:label "Wrinkling" ;
    ex:nonIMDRFCode "MedDRA:10048043:Wrinkling" ;
    rdfs:comment "A folding, ridge or creasing of the skin." ;
    rdfs:subClassOf imdrf:E17 .

imdrf:E1724 a owl:Class ;
    rdfs:label "Dry Skin" ;
    ex:nonIMDRFCode "MedDRA:10013786:Dry skin" ;
    ex:statusDescription "Term was added on 27 January 2022. For details, see comment No. 101 of the Change Log (Release Number 2022)." ;
    rdfs:comment "Skin that has become dry in texture and flaky." ;
    rdfs:subClassOf imdrf:E17 .

imdrf:E1725 a owl:Class ;
    rdfs:label "Injection Site Pooling" ;
    ex:nonIMDRFCode "MedDRA:10053425:Injection site swelling" ;
    ex:statusDescription "Term was added on 27 January 2022. For details, see comment No. 200 / 201 of the Change Log (Release Number 2022)." ;
    rdfs:comment "Liquid or a pocket of air trapped under the skin, typically due to injection problems. Does not include inflammation." ;
    rdfs:subClassOf imdrf:E17 .

imdrf:E1726 a owl:Class ;
    rdfs:label "Skin Maceration" ;
    ex:nonIMDRFCode "MedDRA:10048625:Skin maceration" ;
    ex:statusDescription "Term was added on 27 January 2022. For details, see comment No. 104 of the Change Log (Release Number 2022)." ;
    rdfs:comment "Softening of tissue by the action of a liquid. Occurs at the wound site/surrounding areas due to excessive moisture from exudate or products applied." ;
    rdfs:subClassOf imdrf:E17 .

imdrf:E1727 a owl:Class ;
    rdfs:label "Wound Odor" ;
    ex:nonIMDRFCode "MedDRA:10069389:Wound odor" ;
    ex:statusDescription "Term was added on 31 January 2023. For details, see comment No. 94 of the Change Log (Release Number 2023)." ;
    rdfs:comment "Malodor of the wound or skin not otherwise explained. Can include odors due to necrosis, bioburden or other barriers to wound healing." ;
    rdfs:subClassOf imdrf:E17 .

imdrf:E1728 a owl:Class ;
    rdfs:label "Nail disorder" ;
    ex:nonIMDRFCode "MedDRA:10028694:Nail disorder" ;
    ex:statusDescription "Term added for Release Number 2024. See no. 12 of Change Log" ;
    rdfs:comment "Abnormality of the nail, such as problems with the color, shape, texture, or thickness of the fingernails or toenails." ;
    rdfs:subClassOf imdrf:E17 .

imdrf:E1729 a owl:Class ;
    rdfs:label "Unspecified Skin and Subcutaneous Tissue Problem" ;
    ex:status "New" ;
    ex:statusDescription "Term added for Release Number 2025. See no. 74 of Change Log" ;
    rdfs:comment "The report describes a non-specific problem with the skin or subcutaneous tissue. Note: Please use \"Appropriate Term / Code Not Available\" if the report describes a specific problem but the relevant term does not exist." ;
    rdfs:subClassOf imdrf:E17 .

imdrf:E180101 a owl:Class ;
    rdfs:label "Breast Cancer" ;
    ex:nonIMDRFCode "MedDRA:10006187:Breast cancer" ;
    rdfs:comment "A malignant neoplasm that develops or arises in breast tissue." ;
    rdfs:subClassOf imdrf:E1801 .

imdrf:E180102 a owl:Class ;
    rdfs:label "Breast Implant Associated Anaplastic Large Cell Lymphoma (BIA ALCL)" ;
    ex:nonIMDRFCode "MedDRA:10082495:Breast implant-associated anaplastic large cell lymphoma" ;
    ex:statusDescription "Definition was modified on 27 January 2022 (Old definition: A peripheral (mature) T-cell lymphoma, consisting of usually large anaplastic, CD30 positive cells. The majority of cases are positive for the anaplastic large cell lymphoma (ALK) protein.). For details, see comment No. 9 of the Change Log (Release Number 2022)." ;
    rdfs:comment "A non-Hodgkin lymphoma which is associated with breast implants, and consists of large anaplastic cells. The WHO diagnostic criteria for BIA-ALCL includes positive expression of CD30 (CD30+) and negativity for anaplastic lymphoma kinase (ALK-)." ;
    rdfs:subClassOf imdrf:E1801 .

imdrf:E180103 a owl:Class ;
    rdfs:label "Leiomyosarcoma" ;
    ex:nonIMDRFCode "MedDRA:10024189:Leiomyosarcoma" ;
    rdfs:comment "A malignant tumor of smooth muscle cells that can arise almost anywhere in the body but is most common in the uterus, abdomen, or pelvis." ;
    rdfs:subClassOf imdrf:E1801 .

imdrf:E180104 a owl:Class ;
    rdfs:label "Lymphoma" ;
    ex:nonIMDRFCode "MedDRA:10025310:Lymphoma" ;
    rdfs:comment "A malignant (clonal) proliferation of B- lymphocytes or T- lymphocytes which involves the lymph nodes, bone marrow and/or extranodal sites. This category includes Non-Hodgkin lymphomas and Hodgkin lymphomas." ;
    rdfs:subClassOf imdrf:E1801 .

imdrf:E1802 a owl:Class ;
    rdfs:label "Cyst(s)" ;
    ex:nonIMDRFCode "MedDRA:10011732:Cyst" ;
    rdfs:comment "A sac-like closed membranous structure that may be empty or contain fluid or amorphous material." ;
    rdfs:subClassOf imdrf:E18 .

imdrf:E1803 a owl:Class ;
    rdfs:label "Nodule" ;
    ex:nonIMDRFCode "MedDRA:10054107:Nodule" ;
    rdfs:comment "A small lump, swelling or collection of tissue." ;
    rdfs:subClassOf imdrf:E18 .

imdrf:E1804 a owl:Class ;
    rdfs:label "Solid Tumour" ;
    ex:nonIMDRFCode "MedDRA:10065252:Solid tumor" ;
    rdfs:comment "Abnormal mass of tissue that usually does not contain cysts or liquid areas. Solid tumours may be benign (not cancerous), or malignant (cancerous). Different types of solid tumours are named for the type of cells that form them. If tumours are associated with those under the term cancer, these terms should be used." ;
    rdfs:subClassOf imdrf:E18 .

imdrf:E1805 a owl:Class ;
    rdfs:label "Non-malignant Neoplasm" ;
    ex:nonIMDRFCode "MedDRA:10060999:Benign neoplasm" ;
    ex:statusDescription "Term was added on 27 January 2022. For details, see comment No. 109 of the Change Log (Release Number 2022)." ;
    rdfs:comment "A new and abnormal growth of tissue in a part of the body which is not indicative of malignant disorder. Can include benign tumors." ;
    rdfs:subClassOf imdrf:E18 .

imdrf:E190101 a owl:Class ;
    rdfs:label "Drug Resistant Bacterial Infection" ;
    ex:nonIMDRFCode "MedDRA:10004052:Bacterial resistance" ;
    rdfs:comment "An infection that is resistant to antibiotics and antimicrobials, for example, MRSA or VRE." ;
    rdfs:subClassOf imdrf:E1901 .

imdrf:E190102 a owl:Class ;
    rdfs:label "Pyogenic Infection" ;
    ex:nonIMDRFCode "MedDRA:10021861:Infection pyogenic" ;
    rdfs:comment "An infection caused by pus-producing organisms." ;
    rdfs:subClassOf imdrf:E1901 .

imdrf:E190103 a owl:Class ;
    rdfs:label "Toxemia" ;
    ex:nonIMDRFCode "MedDRA:10059857:Toxemia" ;
    rdfs:comment "The condition resulting from the spread of bacterial products (toxins) by the bloodstream." ;
    rdfs:subClassOf imdrf:E15,
        imdrf:E1901 .

imdrf:E1902 a owl:Class ;
    rdfs:label "Fungal Infection" ;
    ex:nonIMDRFCode "MedDRA:10017533:Fungal infection" ;
    rdfs:comment "An infection caused by a fungus." ;
    rdfs:subClassOf imdrf:E19 .

imdrf:E1903 a owl:Class ;
    rdfs:label "Sexually Transmitted Infection" ;
    ex:nonIMDRFCode "MedDRA:10068720:Sexually transmitted infection" ;
    rdfs:comment "A disease acquired predominantly through sexual contact." ;
    rdfs:subClassOf imdrf:E19 .

imdrf:E1904 a owl:Class ;
    rdfs:label "Subclinical Infection" ;
    ex:nonIMDRFCode "MedDRA:10068163:Subclinical infection" ;
    ex:statusDescription "The definition was changed on 21 January 2021 (Old definition: Infection associated with no detectable symptoms but caused by microorganisms capable of producing easily recognizable diseases.). For details, refer to comment No. 8 of the Change Log)." ;
    rdfs:comment "Infection associated with no detectable signs or symptoms but caused by microorganisms capable of producing easily recognizable diseases." ;
    rdfs:subClassOf imdrf:E19 .

imdrf:E1905 a owl:Class ;
    rdfs:label "Transmissible Spongiform Encephalopathy(TSE)" ;
    ex:nonIMDRFCode "MedDRA:10080750:Transmissible spongiform encephalopathy" ;
    ex:statusDescription "Editorial change to the definition on 16 February 2021." ;
    rdfs:comment "A group of rare degenerative brain disorders associated with prions for example Creutzfeldt-Jakob disease (CJD) or Bovine Spongiform Encephalopathy (BSE)." ;
    rdfs:subClassOf imdrf:E19 .

imdrf:E1906 a owl:Class ;
    rdfs:label "Unspecified Infection" ;
    ex:nonIMDRFCode "MedDRA:10021789:Infection" ;
    ex:statusDescription "Editorial change to the definition on 18 March 2020 for consistency with other \"Unspecified ____\" definitions." ;
    rdfs:comment "The report describes a non-specific or unidentified infection. Note: Please use the appropriate term if the report describes a specific infection. i.e. Bacterial Infection E1901, Fungal Infection E1902, Viral Infection E1907, or a relevant Level 3 term where more detail is available." ;
    rdfs:subClassOf imdrf:E19 .

imdrf:E190701 a owl:Class ;
    rdfs:label "Cytomegalovirus (CMV) Infection" ;
    ex:nonIMDRFCode "MedDRA:10011831:Cytomegalovirus infection" ;
    rdfs:comment "A genus of the family herpesviridae, subfamily betaherpesvirinae, infecting the salivary glands, liver, spleen, lungs, eyes, and other organs, in which they produce characteristically enlarged cells with intranuclear inclusions." ;
    rdfs:subClassOf imdrf:E1907 .

imdrf:E2001 a owl:Class ;
    rdfs:label "Bone Shedding Debris" ;
    ex:nonIMDRFCode "MedDRA:10006011:Bone shedding debris" ;
    rdfs:comment "Shedding of accumulated bone fragments." ;
    rdfs:subClassOf imdrf:E20 .

imdrf:E2003 a owl:Class ;
    rdfs:label "Chemical Exposure" ;
    ex:nonIMDRFCode "MedDRA:10068154:Chemical exposure" ;
    rdfs:comment "Contact with a chemical substance through touch, inhalation, or ingestion." ;
    rdfs:subClassOf imdrf:E20 .

imdrf:E2004 a owl:Class ;
    rdfs:label "Crushing Injury" ;
    ex:nonIMDRFCode "MedDRA:10061097:Crush injury" ;
    rdfs:comment "Traumatic compression of the body or a part of the body." ;
    rdfs:subClassOf imdrf:E20 .

imdrf:E2005 a owl:Class ;
    rdfs:label "Easy Bruising" ;
    ex:nonIMDRFCode "MedDRA:10076258:Tendency to bruise easily" ;
    rdfs:comment "Appearance of bruises spontaneously or following minimal contact." ;
    rdfs:subClassOf imdrf:E17,
        imdrf:E20 .

imdrf:E2007 a owl:Class ;
    rdfs:label "Fall" ;
    ex:nonIMDRFCode "MedDRA:10016173:Fall" ;
    rdfs:comment "A sudden movement downward, usually resulting in injury." ;
    rdfs:subClassOf imdrf:E20 .

imdrf:E200801 a owl:Class ;
    rdfs:label "Device Embedded In Tissue or Plaque" ;
    ex:nonIMDRFCode "MedDRA:10074498:Embedded device" ;
    rdfs:comment "Device and/or fragments of device are embedded in patient's tissue and/or plaque." ;
    rdfs:subClassOf imdrf:E2008 .

imdrf:E2009 a owl:Class ;
    rdfs:label "Laceration(s)" ;
    ex:nonIMDRFCode "MedDRA:10023572:Laceration" ;
    rdfs:comment "A cut or tear in any tissue." ;
    rdfs:subClassOf imdrf:E20 .

imdrf:E2010 a owl:Class ;
    rdfs:label "Needle Stick/Puncture" ;
    ex:nonIMDRFCode "MedDRA:10028895:Needle stick/puncture" ;
    rdfs:comment "A penetrating stab wound from a needle (or other sharp object) that may result in exposure to blood or other body fluids." ;
    rdfs:subClassOf imdrf:E20 .

imdrf:E2011 a owl:Class ;
    rdfs:label "Physical Entrapment" ;
    ex:nonIMDRFCode "MedDRA:10082491:Patient entrapped in device" ;
    rdfs:comment "Patient becomes entangled or trapped in a device." ;
    rdfs:subClassOf imdrf:E20 .

imdrf:E2012 a owl:Class ;
    rdfs:label "Wound Infection" ;
    ex:nonIMDRFCode "MedDRA:10048038:Wound Infection" ;
    ex:statusDescription "Term/Definition was modified on 31 January 2023 (Old term/definition: Post Traumatic Wound Infection: Infection of a wound following trauma. This does not include post surgical wound infection.) MedDRA mapping also updated from Post-traumatic wound infection (10036317) to Wound Infection (10048038). For details, see comment No. 95 of the Change Log (Release Number 2023)." ;
    rdfs:comment "Infection of a wound. This does not include post surgical wound infection." ;
    rdfs:subClassOf imdrf:E19,
        imdrf:E20 .

imdrf:E2013 a owl:Class ;
    rdfs:label "Rupture" ;
    ex:nonIMDRFCode "MedDRA:10080972:Tissue rupture" ;
    rdfs:comment "Forcible tearing or disruption of tissue." ;
    rdfs:subClassOf imdrf:E20 .

imdrf:E201401 a owl:Class ;
    rdfs:label "Pressure Sore/Ulcer" ;
    ex:nonIMDRFCode "MedDRA:10011985:Decubitus ulcer" ;
    ex:status "Modified (technical)" ;
    ex:statusDescription "Term and Definition and MedDRA map modified for Release Number 2025. Previous term was \"Pressure Sores\". Previous MedDRA map was 10036651:Pressure sore. See no. 70 of Change RequestLog." ;
    rdfs:comment "Damage to tissue due as a result of external pressure." ;
    rdfs:subClassOf imdrf:E2014 .

imdrf:E2015 a owl:Class ;
    rdfs:label "Unspecified Tissue Injury" ;
    ex:nonIMDRFCode "MedDRA:10080903:Tissue injury" ;
    ex:statusDescription "Editorial change to the definition on 18 March 2020 for consistency with other \"Unspecified ____\" definitions." ;
    rdfs:comment "The report describes a non-specific injury to the skin or subcutaneous tissue. Note: Please use \"Appropriate Term / Code Not Available\" if the report describes a specific injury but the relevant term does not exist." ;
    rdfs:subClassOf imdrf:E20 .

imdrf:E2016 a owl:Class ;
    rdfs:label "Perineal injury" ;
    ex:nonIMDRFCode "MedDRA:10073329:Perineal injury" ;
    ex:statusDescription "Term added for Release Number 2024. See no. 17 of Change Log" ;
    rdfs:comment "Traumatic damage and/or injury to the perineum." ;
    rdfs:subClassOf imdrf:E20 .

imdrf:E2101 a owl:Class ;
    rdfs:label "Adhesion(s)" ;
    ex:nonIMDRFCode "MedDRA:10059837:Adhesion" ;
    rdfs:comment "A fibrous band of tissue that connects normally separate body regions." ;
    rdfs:subClassOf imdrf:E21,
        imdrf:E2313 .

imdrf:E2102 a owl:Class ;
    rdfs:label "Awareness during Anaesthesia" ;
    ex:nonIMDRFCode "MedDRA:10054330:Awareness during anesthesia" ;
    rdfs:comment "A state of consciousness that permits the formation of explicit and implicit memories while under general anesthesia." ;
    rdfs:subClassOf imdrf:E21 .

imdrf:E2103 a owl:Class ;
    rdfs:label "Device Overstimulation of Tissue" ;
    ex:nonIMDRFCode "MedDRA:10068141:Device overstimulation of tissue" ;
    ex:statusDescription "Editorial change on 27 January 2022 to the MedDRA mapping to correct the MedDRA code." ;
    rdfs:comment "A level of stimulation that is greater than the intended level." ;
    rdfs:subClassOf imdrf:E21 .

imdrf:E210401 a owl:Class ;
    rdfs:label "Shock from Patient Lead(s)" ;
    ex:nonIMDRFCode "MedDRA:10075322:Device inappropriate shock delivery" ;
    rdfs:comment "Unintended electric shock from patient leads. This includes an electric shock to a healthcare professional or a patient receiving a shock to an incorrect area of their body." ;
    rdfs:subClassOf imdrf:E2104 .

imdrf:E2105 a owl:Class ;
    rdfs:label "Exposure to Body Fluids" ;
    ex:nonIMDRFCode "MedDRA:10068528:Exposure to device contaminated with body fluid" ;
    rdfs:comment "Exposed to or contacted with blood or body fluids of another person." ;
    rdfs:subClassOf imdrf:E20,
        imdrf:E21 .

imdrf:E2106 a owl:Class ;
    rdfs:label "External Prosthetic Device Pain" ;
    ex:nonIMDRFCode "MedDRA:10059057:Medical device pain" ;
    ex:statusDescription "Definition was modified on 21 January 2021 to correct a typo in \"artificial\" (Old definition: Pain that is associated with an external ariticial replacement device.)" ;
    rdfs:comment "Pain that is associated with an external artificial replacement device." ;
    rdfs:subClassOf imdrf:E21,
        imdrf:E2330 .

imdrf:E2107 a owl:Class ;
    rdfs:label "Failure of Implant" ;
    ex:nonIMDRFCode "MedDRA:10016153:Failure of implant" ;
    ex:status "Retired" ;
    ex:statusDescription "Term retired for Release Number 2025. When there are no overt clinical signs and symptoms use E2403 - No Clinical Signs, Symptoms or Conditions, otherwise the appropriate E codes should be selected. See no. 61 of Change Request Log" ;
    rdfs:comment "Malfunction of a medical implant." ;
    rdfs:subClassOf imdrf:E21 .

imdrf:E2108 a owl:Class ;
    rdfs:label "Failure to Anastomose" ;
    ex:nonIMDRFCode "MedDRA:10016164:Failure to anastomose" ;
    ex:statusDescription "Definition modified for Release Number 2024. See no. 81 of Change Log" ;
    rdfs:comment "Failure of a surgically-induced connection between tubular structures in the body. Includes Anastomotic Leakage" ;
    rdfs:subClassOf imdrf:E21 .

imdrf:E2109 a owl:Class ;
    rdfs:label "Implant Pain" ;
    ex:nonIMDRFCode "MedDRA:10063782:Implant site pain" ;
    rdfs:comment "Pain localized to the site of the implanted device." ;
    rdfs:subClassOf imdrf:E21,
        imdrf:E2330 .

imdrf:E2110 a owl:Class ;
    rdfs:label "Inadequate Pain Relief" ;
    ex:nonIMDRFCode "MedDRA:10079788:Inadequate pain relief" ;
    rdfs:comment "Continuing discomfort due to a lack or failure of a medical approach to treat pain." ;
    rdfs:subClassOf imdrf:E21,
        imdrf:E2330 .

imdrf:E2111 a owl:Class ;
    rdfs:label "Injection Site Reaction" ;
    ex:nonIMDRFCode "MedDRA:10022095:Injection site reaction" ;
    rdfs:comment "An intense reaction (usually immunologic) developing at the site of injection" ;
    rdfs:subClassOf imdrf:E21 .

imdrf:E2112 a owl:Class ;
    rdfs:label "Intraoperative Pain" ;
    ex:nonIMDRFCode "MedDRA:10064882:Procedural pain" ;
    rdfs:comment "Pain occurring during a surgical operation." ;
    rdfs:subClassOf imdrf:E21,
        imdrf:E2330 .

imdrf:E2113 a owl:Class ;
    rdfs:label "Oversedation" ;
    ex:nonIMDRFCode "MedDRA:10033305:Oversedation" ;
    rdfs:comment "A level of sedation that is greater than the intended level." ;
    rdfs:subClassOf imdrf:E21 .

imdrf:E211401 a owl:Class ;
    rdfs:label "Internal Organ Perforation" ;
    ex:nonIMDRFCode "MedDRA:10080922:Perforation of organ" ;
    rdfs:comment "A rupture in the organ(s) due to traumatic or pathologic processes." ;
    rdfs:subClassOf imdrf:E2114 .

imdrf:E2115 a owl:Class ;
    rdfs:label "Post Operative Wound Infection" ;
    ex:nonIMDRFCode "MedDRA:10036410:Postoperative wound infection" ;
    rdfs:comment "Infection of a surgical skin incision." ;
    rdfs:subClassOf imdrf:E19,
        imdrf:E21 .

imdrf:E2116 a owl:Class ;
    rdfs:label "Radiation Sickness Syndrome" ;
    ex:nonIMDRFCode "MedDRA:10068142:Radiation sickness syndrome" ;
    rdfs:comment "The complex of symptoms characterizing the disease known as radiation injury, resulting from excessive exposure of the whole body (or large part) to ionizing radiation." ;
    rdfs:subClassOf imdrf:E20,
        imdrf:E21 .

imdrf:E2117 a owl:Class ;
    rdfs:label "Twiddlers Syndrome" ;
    ex:nonIMDRFCode "MedDRA:10045184:Twiddler's syndrome" ;
    rdfs:comment "Dislodgement, breakdown, or other malfunction of an artificial cardiac pacemaker, chemotherapy port, drip infusion valve, or similar implanted diagnostic or therapeutic device as a result of unconscious or habitual manipulation by the patient." ;
    rdfs:subClassOf imdrf:E21 .

imdrf:E2118 a owl:Class ;
    rdfs:label "Unintended Extubation" ;
    ex:nonIMDRFCode "MedDRA:10066823:Unintended endotracheal extubation" ;
    rdfs:comment "The removal of a previously inserted tube from a hollow organ or passageway, often from the airway." ;
    rdfs:subClassOf imdrf:E21 .

imdrf:E2119 a owl:Class ;
    rdfs:label "Unintended Radiation Exposure" ;
    ex:nonIMDRFCode "MedDRA:10063155:Radiation exposure" ;
    ex:statusDescription "Editorial change to the definition on 16 February 2021." ;
    rdfs:comment "The unintentional exposure to radiation of a person, or a part of a persons body. This might include exposure of a healthcare professional, or the exposure of the wrong part of the body of a patient who was intended to receive therapeutic or diagnostic radiation. This includes both ionizing and non ionizing radiation." ;
    rdfs:subClassOf imdrf:E21 .

imdrf:E2120 a owl:Class ;
    rdfs:label "Bone Cement Implantation Syndrome" ;
    ex:nonIMDRFCode "MedDRA:10085596:Bone cement implantation syndrome" ;
    ex:statusDescription "Term was added on 21 January 2021. For details, refer to comment No. 33 of the Change Log." ;
    rdfs:comment "A rare and potentially fatal perioperative complication of cemented bone surgery, characterised by hypotension, hypoxia, cardiac dysrhythmias, and in severe cases cardiac arrest." ;
    rdfs:subClassOf imdrf:E21 .

imdrf:E2121 a owl:Class ;
    rdfs:label "Clinical Endoleak" ;
    ex:nonIMDRFCode "MedDRA:10063824:Endoleak" ;
    ex:status "Modified (technical)" ;
    ex:statusDescription "Term was added on 27 January 2022. For details, see comment No. 181 / 207 of the Change Log (Release Number 2022). Term and Definition modified for Release Number 2025. Previous term was \"Endoleaks\". See no. 117 of Change Request Log." ;
    rdfs:comment "The observed patient condition is persistent blood flow/pressure in the aneurysm sac following an endovascular aneurysm repair (EVAR) procedure.  Where other patient signs and symptoms indicate the presence of an endoleak those signs and symptoms should be coded." ;
    rdfs:subClassOf imdrf:E05,
        imdrf:E21 .

imdrf:E2122 a owl:Class ;
    rdfs:label "Sinusitis" ;
    ex:nonIMDRFCode "MedDRA:10040753:Sinusitis" ;
    ex:statusDescription "Term was added on 27 January 2022. For details, see comment No. 240 of the Change Log (Release Number 2022)." ;
    rdfs:comment "Inflammation (swelling and redness) of the paranasal sinuses, associated or related to implantation procedures or devices." ;
    rdfs:subClassOf imdrf:E19,
        imdrf:E21 .

imdrf:E2123 a owl:Class ;
    rdfs:label "Medical device site infection" ;
    ex:nonIMDRFCode "MedDRA:10075580:Medical device site infection" ;
    ex:statusDescription """Term was added on 27 January 2022. For details, see comment No. 122 of the Change Log (Release Number 2022).
Term and Definition and MedDRA map modified for Release Number 2024. Previous term was Peri-prosthetic Joint Infection. Previous MedDRA map was 10076118:Medical device site joint infection. See no. 10 of Change Log.""" ;
    rdfs:comment "Infection local to an implanted or invasive medical device." ;
    rdfs:subClassOf imdrf:E19,
        imdrf:E21 .

imdrf:E2124 a owl:Class ;
    rdfs:label "Unintended Loss of Vascular Access" ;
    ex:nonIMDRFCode "MedDRA:10070944:Vascular access failure" ;
    ex:statusDescription "Term was added on 31 January 2023. For details, see comment No. 97 of the Change Log (Release Number 2023)." ;
    rdfs:comment "The accidental removal of a previously inserted line from a blood vessel." ;
    rdfs:subClassOf imdrf:E21 .

imdrf:E2125 a owl:Class ;
    rdfs:label "Complex regional pain syndrome" ;
    ex:nonIMDRFCode "MedDRA:10064332:Complex regional pain syndrome" ;
    ex:statusDescription "Term added for Release Number 2024. See no. 56 of Change Log" ;
    rdfs:comment "Condition where a person experiences persistent severe and debilitating pain, involving an extremity or other body region, hyperesthesia, and localized autonomic dysfunction following injury to soft tissue or nerve" ;
    rdfs:subClassOf imdrf:E01,
        imdrf:E21 .

imdrf:E2126 a owl:Class ;
    rdfs:label "Loss of fracture reduction" ;
    ex:nonIMDRFCode "MedDRA:10069723:Loss of anatomical alignment after fracture reduction" ;
    ex:statusDescription "Term added for Release Number 2024. See no. 65 of Change Log" ;
    rdfs:comment "Loss of anatomical alignment after fracture reduction." ;
    rdfs:subClassOf imdrf:E16,
        imdrf:E21 .

imdrf:E2127 a owl:Class ;
    rdfs:label "Periprosthetic fracture" ;
    ex:nonIMDRFCode "MedDRA:10069135:Periprosthetic fracture" ;
    ex:statusDescription "Term added for Release Number 2024. See no. 67 of Change Log" ;
    rdfs:comment "Fractures around joint replacement prosthetics or implants. These can occur intraoperatively or postoperatively." ;
    rdfs:subClassOf imdrf:E16,
        imdrf:E21 .

imdrf:E2128 a owl:Class ;
    rdfs:label "Implant site sclerosis" ;
    ex:nonIMDRFCode "MedDRA:10063876:Implant site sclerosis" ;
    ex:statusDescription "Term added for Release Number 2024. See no. 94 of Change Log" ;
    rdfs:comment "Pathological process consisting of hardening/thickening of tissue or structures." ;
    rdfs:subClassOf imdrf:E21 .

imdrf:E2129 a owl:Class ;
    rdfs:label "Peritoneal effluent abnormal" ;
    ex:nonIMDRFCode "MedDRA:10069638:Peritoneal effluent abnormal" ;
    ex:statusDescription "Term added for Release Number 2024. See no. 99 of Change Log" ;
    rdfs:comment "A change in the appearance or other characteristics of peritoneal dialysis effluent (e.g. cloudy or discolored)." ;
    rdfs:subClassOf imdrf:E21 .

imdrf:E2130 a owl:Class ;
    rdfs:label "Graft failure" ;
    ex:nonIMDRFCode "MedDRA:10069030:Graft failure" ;
    ex:statusDescription "Term added for Release Number 2024. See no. 104 of Change Log" ;
    rdfs:comment "Failure of a transplanted graft." ;
    rdfs:subClassOf imdrf:E21 .

imdrf:E2131 a owl:Class ;
    rdfs:label "Inappropriate Device Stimulation of Tissue" ;
    ex:nonIMDRFCode "MedDRA:10064414:Inappropriate device stimulation of tissue" ;
    ex:status "New" ;
    ex:statusDescription "Term added for Release Number 2025. See no. 17 of Change Request Log" ;
    rdfs:comment "Unintended reaction in a tissue (e.g. nerve, muscle) caused by electrical stimulation" ;
    rdfs:subClassOf imdrf:E21 .

imdrf:E2132 a owl:Class ;
    rdfs:label "Medical Device Site Inflammation" ;
    ex:nonIMDRFCode "MedDRA:10075581:Medical device site Inflammation" ;
    ex:status "New" ;
    ex:statusDescription "Term added for Release Number 2025. See no. 68 of Change Request Log" ;
    rdfs:comment "Inflammation local to an implanted or invasive medical device." ;
    rdfs:subClassOf imdrf:E21 .

imdrf:E2201 a owl:Class ;
    rdfs:label "Abnormal Blood Gases" ;
    ex:nonIMDRFCode "MedDRA:10005539:Blood gases abnormal" ;
    rdfs:comment "Abnormal Blood Gas Measurements." ;
    rdfs:subClassOf imdrf:E22 .

imdrf:E2202 a owl:Class ;
    rdfs:label "High Oxygen Saturation" ;
    ex:nonIMDRFCode "MedDRA:10033319:Oxygen saturation high" ;
    rdfs:comment "A high level of the degree to which oxygen is bound to hemoglobin given as a percentage calculated by dividing the maximum oxygen capacity into the actual oxygen content and multiplying by 100. Oxygen saturation usually is measured using pulse oximetry." ;
    rdfs:subClassOf imdrf:E07,
        imdrf:E22 .

imdrf:E2203 a owl:Class ;
    rdfs:label "Low Oxygen Saturation" ;
    ex:nonIMDRFCode "MedDRA:10033321:Oxygen saturation low" ;
    rdfs:comment "A low level of the degree to which oxygen is bound to hemoglobin given as a percentage calculated by dividing the maximum oxygen capacity into the actual oxygen content and multiplying by 100. Oxygen saturation usually is measured using pulse oximetry." ;
    rdfs:subClassOf imdrf:E07,
        imdrf:E22 .

imdrf:E2204 a owl:Class ;
    rdfs:label "Lactate Dehydrogenase Increased" ;
    ex:nonIMDRFCode "MedDRA:10023654:Lactate dehydrogenase increased" ;
    rdfs:comment "A laboratory test result indicating an increase in the lactate dehydrogenase concentration of a biological sample." ;
    rdfs:subClassOf imdrf:E22 .

imdrf:E2205 a owl:Class ;
    rdfs:label "Bacteremia" ;
    ex:nonIMDRFCode "MedDRA:10003999:Bacteremia" ;
    ex:statusDescription "Term was added on 27 January 2022. For details, see comment No. 49 of the Change Log (Release Number 2022)." ;
    rdfs:comment "Condition that relates to the presence of viable bacteria in the bloodstream, whether associated with active disease or not." ;
    rdfs:subClassOf imdrf:E19,
        imdrf:E22 .

imdrf:E2206 a owl:Class ;
    rdfs:label "High metal ion levels" ;
    ex:nonIMDRFCode "MedDRA:10086050:Heavy metal increased" ;
    ex:statusDescription "Term was added on 27 January 2022. For details, see comment No. 114 / 154 / 204 of the Change Log (Release Number 2022)." ;
    rdfs:comment "High blood or serum levels of ions which are attributed to one or more medical devices used, such as but not limited to Co, Cr, Ti, Ni, Mo." ;
    rdfs:subClassOf imdrf:E22 .

imdrf:E2207 a owl:Class ;
    rdfs:label "Radiolucent Lines" ;
    ex:statusDescription "Term was added on 27 January 2022. For details, see comment No. 123 of the Change Log (Release Number 2022)." ;
    rdfs:comment "Radiolucencies observed on x-ray." ;
    rdfs:subClassOf imdrf:E22 .

imdrf:E230101 a owl:Class ;
    rdfs:label "Fever" ;
    ex:nonIMDRFCode "MedDRA:10016558:Fever" ;
    rdfs:comment "Elevation of body temperature above normal due to the bodies own responses." ;
    rdfs:subClassOf imdrf:E2301 .

imdrf:E230102 a owl:Class ;
    rdfs:label "Hyperthermia" ;
    ex:nonIMDRFCode "MedDRA:10020843:Hyperthermia" ;
    rdfs:comment "An abnormally high body temperature. Not fever." ;
    rdfs:subClassOf imdrf:E2301 .

imdrf:E230103 a owl:Class ;
    rdfs:label "Hypothermia" ;
    ex:nonIMDRFCode "MedDRA:10021113:Hypothermia" ;
    rdfs:comment "Abnormally low body temperature." ;
    rdfs:subClassOf imdrf:E2301 .

imdrf:E2302 a owl:Class ;
    rdfs:label "Ambulation or Postural Difficulties" ;
    ex:nonIMDRFCode "MedDRA:10047810:Walking difficulty" ;
    ex:statusDescription "Term/Definition was modified on 31 January 2023 (Old term/definition: Ambulation Difficulties: Any persistent problem with walking or gait.) For details, see comment No. 98 of the Change Log (Release Number 2023)." ;
    rdfs:comment "Any persistent problem with walking, gait or maintaining posture (sitting, standing)." ;
    rdfs:subClassOf imdrf:E16,
        imdrf:E23 .

imdrf:E2303 a owl:Class ;
    rdfs:label "Capsular Contracture" ;
    ex:nonIMDRFCode "MedDRA:10080895:Capsular contracture associated with implant" ;
    rdfs:comment "The tightening of scar tissue that forms around the implant." ;
    rdfs:subClassOf imdrf:E23 .

imdrf:E2304 a owl:Class ;
    rdfs:label "Chills" ;
    ex:nonIMDRFCode "MedDRA:10008531:Chills" ;
    rdfs:comment "Shivering or moderate tremors of the body often accompanied by a cold sensation." ;
    rdfs:subClassOf imdrf:E23 .

imdrf:E2305 a owl:Class ;
    rdfs:label "Cyanosis" ;
    ex:nonIMDRFCode "MedDRA:10011703:Cyanosis" ;
    rdfs:comment "A bluish or purplish discoloration of the skin and mucous membranes resulting from a reduced amount of oxygenated hemoglobin in the blood." ;
    rdfs:subClassOf imdrf:E23 .

imdrf:E2306 a owl:Class ;
    rdfs:label "Decreased Appetite" ;
    ex:nonIMDRFCode "MedDRA:10061428:Decreased appetite" ;
    rdfs:comment "Lack of desire for food." ;
    rdfs:subClassOf imdrf:E12,
        imdrf:E23 .

imdrf:E2307 a owl:Class ;
    rdfs:label "Increased Appetite" ;
    ex:nonIMDRFCode "MedDRA:10021654:Increased appetite" ;
    rdfs:comment "Intense desire for food." ;
    rdfs:subClassOf imdrf:E12,
        imdrf:E23 .

imdrf:E2308 a owl:Class ;
    rdfs:label "Deformity/ Disfigurement" ;
    ex:nonIMDRFCode "MedDRA:10061619:Deformity" ;
    rdfs:comment "An alteration of appearance, shape, size or alignment." ;
    rdfs:subClassOf imdrf:E23 .

imdrf:E230901 a owl:Class ;
    rdfs:label "Calcium Deposits/Calcification" ;
    ex:nonIMDRFCode "MedDRA:10006958:Calcium deposits" ;
    rdfs:comment "Deposition of calcium salt in the tissues." ;
    rdfs:subClassOf imdrf:E2309 .

imdrf:E2310 a owl:Class ;
    rdfs:label "Diaphoresis" ;
    ex:nonIMDRFCode "MedDRA:10012703:Diaphoresis" ;
    rdfs:comment "Profuse sweating." ;
    rdfs:subClassOf imdrf:E23 .

imdrf:E2311 a owl:Class ;
    rdfs:label "Discomfort" ;
    ex:nonIMDRFCode "MedDRA:10013082:Discomfort" ;
    rdfs:comment "A feeling of mental or physical uneasiness, pain, or distress." ;
    rdfs:subClassOf imdrf:E23 .

imdrf:E231201 a owl:Class ;
    rdfs:label "Extreme Exhaustion" ;
    ex:nonIMDRFCode "MedDRA:10015667:Exhaustion" ;
    ex:statusDescription "Editorial change to the definition on 16 February 2021." ;
    rdfs:comment "Extreme fatigue; the inability to respond to stimuli." ;
    rdfs:subClassOf imdrf:E2312 .

imdrf:E2314 a owl:Class ;
    rdfs:label "Fistula" ;
    ex:nonIMDRFCode "MedDRA:10016717:Fistula" ;
    rdfs:comment "Abnormal epithelial-lined communication between two anatomical structures." ;
    rdfs:subClassOf imdrf:E23 .

imdrf:E231501 a owl:Class ;
    rdfs:label "Purulent Discharge" ;
    ex:nonIMDRFCode "MedDRA:10037569:Purulent discharge" ;
    ex:statusDescription "Editorial change to the definition on 16 February 2021." ;
    rdfs:comment "A flow or draining of pus or exudate from an orifice or wound." ;
    rdfs:subClassOf imdrf:E2315 .

imdrf:E2316 a owl:Class ;
    rdfs:label "Foreign Body Reaction" ;
    ex:nonIMDRFCode "MedDRA:10068159:Foreign body reaction" ;
    rdfs:comment "An inflammatory reaction evoked by the presence of an exogenous material in the tissues." ;
    rdfs:subClassOf imdrf:E23 .

imdrf:E2317 a owl:Class ;
    rdfs:label "Granuloma" ;
    ex:nonIMDRFCode "MedDRA:10018691:Granuloma" ;
    rdfs:comment "An inflammatory reaction usually caused by infectious organisms, foreign bodies, or cholesterol deposits. It is characterized by the presence of epithelioid histiocytes and chronic inflammation." ;
    rdfs:subClassOf imdrf:E1720,
        imdrf:E23 .

imdrf:E2318 a owl:Class ;
    rdfs:label "Hair Loss" ;
    ex:nonIMDRFCode "MedDRA:10019045:Hair loss" ;
    rdfs:comment "Loss of hair usually from the scalp that may result in bald spots or spread to the entire scalp or epidermis." ;
    rdfs:subClassOf imdrf:E23 .

imdrf:E2319 a owl:Class ;
    rdfs:label "Hernia" ;
    ex:nonIMDRFCode "MedDRA:10019909:Hernia" ;
    rdfs:comment "The protrusion of part of an organ or fibroadipose tissue through an opening or weakened area." ;
    rdfs:subClassOf imdrf:E23 .

imdrf:E2320 a owl:Class ;
    rdfs:label "High Blood Pressure/ Hypertension" ;
    ex:nonIMDRFCode "MedDRA:10020772:Hypertension" ;
    rdfs:comment "Blood pressure that is abnormally high." ;
    rdfs:subClassOf imdrf:E23 .

imdrf:E2321 a owl:Class ;
    rdfs:label "Low Blood Pressure/ Hypotension" ;
    ex:nonIMDRFCode "MedDRA:10021097:Hypotension" ;
    rdfs:comment "Blood pressure that is abnormally low." ;
    rdfs:subClassOf imdrf:E23 .

imdrf:E2322 a owl:Class ;
    rdfs:label "Hyperemia" ;
    ex:nonIMDRFCode "MedDRA:10020619:Hyperemia" ;
    ex:statusDescription "Definition was modified on 31 January 2023 to add \"bloodshot\". For details, see comment No. 132 of the Change Log (Release Number 2023)." ;
    rdfs:comment "The presence of an increased amount of blood in a part or organ; engorgement or bloodshot" ;
    rdfs:subClassOf imdrf:E23 .

imdrf:E2323 a owl:Class ;
    rdfs:label "Hyperplasia" ;
    ex:nonIMDRFCode "MedDRA:10020718:Hyperplasia" ;
    rdfs:comment "An abnormal increase in the number of cells in an organ or a tissue with consequent enlargement." ;
    rdfs:subClassOf imdrf:E23 .

imdrf:E232401 a owl:Class ;
    rdfs:label "Fecal Incontinence" ;
    ex:nonIMDRFCode "MedDRA:10016296:Fecal incontinence" ;
    ex:statusDescription """Editorial change to add Gastrointestinal System as Secondary Category. For details, see comment No. 99 of the Change Log (Release Number 2023).
Code hierarchy adjusted for secondary category to prevent primary parent term appearing in three places. Release No. 2024""" ;
    rdfs:comment "Inability to control voluntary passage of feces from the body." ;
    rdfs:subClassOf imdrf:E10,
        imdrf:E2324 .

imdrf:E232402 a owl:Class ;
    rdfs:label "Urinary Incontinence" ;
    ex:nonIMDRFCode "MedDRA:10046543:Urinary incontinence" ;
    ex:statusDescription """Editorial change to add Kidney and Urinary Tract as Secondary Category. For details, see comment No. 100 of the Change Log (Release Number 2023). Amended in Version 1 on 23 February 2023.
Code hierarchy adjusted for secondary category to prevent primary parent term appearing in three places. Release No. 2024""" ;
    rdfs:comment "Inability to control voluntary passage of urine from the body." ;
    rdfs:subClassOf imdrf:E13,
        imdrf:E2324 .

imdrf:E2325 a owl:Class ;
    rdfs:label "Infiltration into Tissue" ;
    ex:nonIMDRFCode "MedDRA:10080901:Tissue infiltration" ;
    rdfs:comment "Permeation of foreign substances into tissues or cells." ;
    rdfs:subClassOf imdrf:E23 .

imdrf:E2326 a owl:Class ;
    rdfs:label "Inflammation" ;
    ex:nonIMDRFCode "MedDRA:10061218:Inflammation" ;
    rdfs:comment "A localized physical condition in which part of the body becomes reddened, swollen, or hot and often painful." ;
    rdfs:subClassOf imdrf:E23 .

imdrf:E2327 a owl:Class ;
    rdfs:label "Necrosis" ;
    ex:nonIMDRFCode "MedDRA:10028851:Necrosis" ;
    rdfs:comment "The pathologic death of cells or of a portion of tissue or organ resulting from irreversible damage." ;
    rdfs:subClassOf imdrf:E23 .

imdrf:E2328 a owl:Class ;
    rdfs:label "Obstruction/Occlusion" ;
    ex:nonIMDRFCode "MedDRA:10061876:Obstruction" ;
    rdfs:comment "Blockage or closing of the normal flow of the contents of an anatomical passageway." ;
    rdfs:subClassOf imdrf:E23 .

imdrf:E2329 a owl:Class ;
    rdfs:label "Organ Dehiscence" ;
    ex:nonIMDRFCode "MedDRA:10080904:Dehiscence" ;
    rdfs:comment "A splitting open or rupture of an internal organ with the exposure or discharge of its content." ;
    rdfs:subClassOf imdrf:E23 .

imdrf:E233001 a owl:Class ;
    rdfs:label "Chest Pain" ;
    ex:nonIMDRFCode "MedDRA:10008479:Chest pain" ;
    rdfs:comment "Pain in the chest." ;
    rdfs:subClassOf imdrf:E2330 .

imdrf:E2331 a owl:Class ;
    rdfs:label "Pallor" ;
    ex:nonIMDRFCode "MedDRA:10033546:Pallor" ;
    rdfs:comment "Unhealthy, pale or white appearance of the face." ;
    rdfs:subClassOf imdrf:E23 .

imdrf:E2332 a owl:Class ;
    rdfs:label "Physical Asymmetry" ;
    rdfs:comment "Lack or absence of balanced proportions between parts or organs of the body." ;
    rdfs:subClassOf imdrf:E21,
        imdrf:E23 .

imdrf:E2333 a owl:Class ;
    rdfs:label "Prolapse" ;
    ex:nonIMDRFCode "MedDRA:10076708:Prolapse" ;
    rdfs:comment "A condition in which an organ or body tissue drops or bulges out of place." ;
    rdfs:subClassOf imdrf:E23 .

imdrf:E2334 a owl:Class ;
    rdfs:label "Ptosis" ;
    ex:nonIMDRFCode "MedDRA:10037272:Ptosis" ;
    rdfs:comment "The drooping or downward displacement of a body part." ;
    rdfs:subClassOf imdrf:E23 .

imdrf:E2335 a owl:Class ;
    rdfs:label "Reaction to Medicinal Component of Device" ;
    ex:nonIMDRFCode "MedDRA:10067484:Adverse reaction" ;
    rdfs:comment "Any local or systemic adverse reaction to the medicinal component of a combination product." ;
    rdfs:subClassOf imdrf:E23 .

imdrf:E233601 a owl:Class ;
    rdfs:label "Cardiogenic Shock" ;
    ex:nonIMDRFCode "MedDRA:10007625:Cardiogenic shock" ;
    rdfs:comment "Shock resulting from primary failure of the heart in its pumping function, as in myocardial infarction, severe cardiomyopathy, or mechanical obstruction or compression of the heart." ;
    rdfs:subClassOf imdrf:E2336 .

imdrf:E233602 a owl:Class ;
    rdfs:label "Hypoglycemic Shock" ;
    ex:nonIMDRFCode "MedDRA:10060493:Hypoglycemic shock" ;
    rdfs:comment "A hypoglycemic reaction to overdosage of insulin, a skipped meal, or strenuous exercise in an insulin-dependent diabetic." ;
    rdfs:subClassOf imdrf:E2336 .

imdrf:E233603 a owl:Class ;
    rdfs:label "Hypovolemic Shock" ;
    ex:nonIMDRFCode "MedDRA:10021140:Hypovolemic shock" ;
    rdfs:comment "Shock resulting from insufficient blood volume for the maintenance of adequate cardiac output, blood pressure and tissue perfusion." ;
    rdfs:subClassOf imdrf:E2336 .

imdrf:E233604 a owl:Class ;
    rdfs:label "Neurogenic Shock" ;
    ex:nonIMDRFCode "MedDRA:10058119:Neurogenic shock" ;
    rdfs:comment "Shock resulting from neurogenic vasodilation, which can be produced by cerebral trauma or hemorrhage, spinal cord injury, deep general or spinal anesthesia, or toxic central nervous system depression." ;
    rdfs:subClassOf imdrf:E2336 .

imdrf:E233605 a owl:Class ;
    rdfs:label "Septic Shock" ;
    ex:nonIMDRFCode "MedDRA:10040070:Septic shock" ;
    rdfs:comment "A state of acute circulatory failure resulting from organ injury or damage in response to infection that results in dangerously low blood pressure." ;
    rdfs:subClassOf imdrf:E2336 .

imdrf:E233701 a owl:Class ;
    rdfs:label "Restenosis" ;
    ex:nonIMDRFCode "MedDRA:10082493:Restenosis" ;
    rdfs:comment "The reoccurrence of stenosis after it has been treated." ;
    rdfs:subClassOf imdrf:E2337 .

imdrf:E233801 a owl:Class ;
    rdfs:label "Peripheral Edema" ;
    ex:nonIMDRFCode "MedDRA:10034570:Peripheral edema" ;
    rdfs:comment "accumulation of fluid in tissues perfused by the peripheral vascular system." ;
    rdfs:subClassOf imdrf:E2338 .

imdrf:E233802 a owl:Class ;
    rdfs:label "Joint effusion" ;
    ex:nonIMDRFCode "MedDRA:10023215:Joint effusion" ;
    ex:statusDescription "Term was added on 27 January 2022. For details, see comment No. 115 of the Change Log (Release Number 2022)." ;
    rdfs:comment "An abnormal collection of fluid in hollow spaces or between tissues of the joints." ;
    rdfs:subClassOf imdrf:E2338 .

imdrf:E2339 a owl:Class ;
    rdfs:label "Ulcer" ;
    ex:nonIMDRFCode "MedDRA:10045285:Ulcer" ;
    rdfs:comment "An open sore on an external or internal surface of the body caused by a break in the skin or mucous membrane that fails to heal." ;
    rdfs:subClassOf imdrf:E23 .

imdrf:E2340 a owl:Class ;
    rdfs:label "Wound Dehiscence" ;
    ex:nonIMDRFCode "MedDRA:10048031:Wound dehiscence" ;
    rdfs:comment "A complication in which the wound splits or separates after being surgically closed." ;
    rdfs:subClassOf imdrf:E21,
        imdrf:E23 .

imdrf:E2341 a owl:Class ;
    rdfs:label "Double Capsule" ;
    ex:statusDescription "Term was added on 18 March 2020 as an additional level 2 term for \"Generalized Disorders\"." ;
    rdfs:comment "The presence of two distinct capsular layers around an implant with an intercapsular space" ;
    rdfs:subClassOf imdrf:E14,
        imdrf:E23 .

imdrf:E2342 a owl:Class ;
    rdfs:label "Multiple Organ Dysfunction Syndrome" ;
    ex:nonIMDRFCode "MedDRA:10077361:Multiple organ dysfunction syndrome" ;
    ex:statusDescription "Term was added on 21 January 2021. For details, refer to comment No. 34 of the Change Log." ;
    rdfs:comment "Complete impairment of two or more organs or organ systems. Also known as multiple organ failure." ;
    rdfs:subClassOf imdrf:E23 .

imdrf:E2343 a owl:Class ;
    rdfs:label "Hemodynamic instability" ;
    ex:nonIMDRFCode "MedDRA:10058270:Hemodynamic instability" ;
    ex:statusDescription "Term was added on 31 January 2023. For details, see comment No. 101 of the Change Log (Release Number 2023)." ;
    rdfs:comment "Abnormal or unstable blood pressure" ;
    rdfs:subClassOf imdrf:E23 .

imdrf:E2344 a owl:Class ;
    rdfs:label "Voice alteration" ;
    ex:nonIMDRFCode "MedDRA:10047681:Voice alteration" ;
    ex:statusDescription "Term added for Release Number 2024. See no. 3 of Change Log" ;
    rdfs:comment "Changes in the pitch or quality of the voice, which may sound weak, scratchy, raspy, or otherwise out of the ordinary." ;
    rdfs:subClassOf imdrf:E23 .

imdrf:E2345 a owl:Class ;
    rdfs:label "Heat illness" ;
    ex:nonIMDRFCode "MedDRA:10068188:Heat illness" ;
    ex:statusDescription "Term added for Release Number 2024. See no. 4 of Change Log" ;
    rdfs:comment "A set of symptoms brought on by exposure to heat that can include confusion, hot dry skin, seizures, elevated body temperature, altered mental status, etc.  Includes heat stroke and heat exhaustion." ;
    rdfs:subClassOf imdrf:E23 .

imdrf:E2346 a owl:Class ;
    rdfs:label "Hypertrophy" ;
    ex:nonIMDRFCode "MedDRA:10020880:Hypertrophy" ;
    ex:statusDescription "Term added for Release Number 2024. See no. 11 of Change Log" ;
    rdfs:comment "An increase in organ size via increase in cell size rather than cell number" ;
    rdfs:subClassOf imdrf:E23 .

imdrf:E2347 a owl:Class ;
    rdfs:label "Breath odor" ;
    ex:nonIMDRFCode "MedDRA:10006325:Breath odor" ;
    ex:statusDescription "Term added for Release Number 2024. See no. 16 of Change Log" ;
    rdfs:comment "Unusual breath odor (e.g., halitosis, fruity/sweet breath)" ;
    rdfs:subClassOf imdrf:E23 .

imdrf:E2348 a owl:Class ;
    rdfs:label "Abnormal mucus discharge" ;
    ex:nonIMDRFCode "MedDRA:10073765:Mucus discharge" ;
    ex:statusDescription "Term added for Release Number 2024. See no. 20 of Change Log" ;
    rdfs:comment "Any deviation from the normal quantity, consistency, and/or color of mucus produced by the mucous membranes." ;
    rdfs:subClassOf imdrf:E23 .

imdrf:E2349 a owl:Class ;
    rdfs:label "Withdrawal Syndrome" ;
    ex:nonIMDRFCode "MedDRA:10048010:Withdrawal syndrome" ;
    ex:statusDescription "Term added for Release Number 2024. See no. 24 of Change Log" ;
    rdfs:comment "The substance-specific organic brain syndrome that follows the discontinuation of, or reduction in, administration or intake of an addictive substance." ;
    rdfs:subClassOf imdrf:E23 .

imdrf:E2350 a owl:Class ;
    rdfs:label "Tissue Irritation" ;
    ex:nonIMDRFCode "MedDRA:10075582:Medical device site irritation" ;
    ex:statusDescription "Term added for Release Number 2024. See no. 89 of Change Log" ;
    rdfs:comment """Irritation of body tissue(s), other than skin.
For skin irritation use E1720 - Skin Inflammation/Irritation""" ;
    rdfs:subClassOf imdrf:E23 .

imdrf:E2351 a owl:Class ;
    rdfs:label "Atrophy" ;
    ex:nonIMDRFCode "MedDRA:10003694:Atrophy" ;
    ex:statusDescription "Term added for Release Number 2024. See no. 93 of Change Log" ;
    rdfs:comment """Decrease in size of a body part, cell, organ, or other tissue. 
For muscular atrophy use E1621 - Muscle Weakness/Atrophy""" ;
    rdfs:subClassOf imdrf:E23 .

imdrf:E2352 a owl:Class ;
    rdfs:label "Exercise capacity decreased" ;
    ex:nonIMDRFCode "MedDRA:10052325:Exercise capacity decreased" ;
    ex:status "New" ;
    ex:statusDescription "Term added for Release Number 2025. See no. 18 of Change Request Log" ;
    rdfs:comment "Reduced ability of the body to perform strenuous activities" ;
    rdfs:subClassOf imdrf:E23 .

imdrf:E2401 a owl:Class ;
    rdfs:label "Insufficient Information" ;
    ex:statusDescription "Definition was modified on 31 January 2023 (Old definition: Health effect appears to have occurred but there is not yet enough information available to classify the clinical signs, symptoms and conditions.). For details, see comment No. 102 of the Change Log (Release Number 2023)." ;
    rdfs:comment "It is not clear whether any health effects occurred, or health effect appears to have occurred but there is not yet enough information available to classify the clinical signs, symptoms and conditions." ;
    rdfs:subClassOf imdrf:E24 .

imdrf:E2402 a owl:Class ;
    rdfs:label "Appropriate Clinical Signs, Symptoms and Conditions Term/Code Not Available" ;
    ex:status "Modified (editorial)" ;
    ex:statusDescription "Term modified for Release Number 2025. Previous term was \"Appropriate Term / Code Not Available\". See no. 110 of Change Request Log." ;
    rdfs:comment "The clinical signs, symptoms and conditions are not adequately described by any other term. Note: this code must not be used unless there is no other feasible code. The preferred term should be documented when submitting an adverse event report. This information will be used to determine if a new term should be added to the code table." ;
    rdfs:subClassOf imdrf:E24 .

imdrf:E2403 a owl:Class ;
    rdfs:label "No Clinical Signs, Symptoms or Conditions" ;
    rdfs:comment "No patient involvement or, no observable clinical symptoms or a change in symptoms is identified in the patient." ;
    rdfs:subClassOf imdrf:E24 .

imdrf:F0101 a owl:Class ;
    rdfs:label "Therapeutic Response Decreased" ;
    rdfs:comment "A reduction in the desirable and beneficial effects resulting from a medical treatment." ;
    rdfs:subClassOf imdrf:F01 .

imdrf:F0102 a owl:Class ;
    rdfs:label "Therapeutic Response Increased" ;
    rdfs:comment "An increase in the desirable and beneficial effects resulting from a medical treatment." ;
    rdfs:subClassOf imdrf:F01 .

imdrf:F0103 a owl:Class ;
    rdfs:label "Unexpected Therapeutic Effects" ;
    rdfs:comment "Unanticipated desirable and beneficial effects resulting from a medical treatment." ;
    rdfs:subClassOf imdrf:F01 .

imdrf:F0201 a owl:Class ;
    rdfs:label "Intrauterine Fetal Death" ;
    rdfs:comment "Death in utero; failure of the product of conception to show evidence of respiration, heart beat, or definite movement of a voluntary muscle after expulsion from the uterus, with no possibility of resuscitation." ;
    rdfs:subClassOf imdrf:F02 .

imdrf:F03 a owl:Class ;
    rdfs:label "Brain Death" ;
    rdfs:comment "The cessation of life due to permanent loss of brain function and brainstem for absence of responsiveness to external stimuli, absence of reflex and apnea." .

imdrf:F04 a owl:Class ;
    rdfs:label "Delay to Diagnosis" ;
    rdfs:comment "Patient diagnosis was clinically significant delayed as a consequence of device performance." .

imdrf:F05 a owl:Class ;
    rdfs:label "Delay to Treatment/ Therapy" ;
    rdfs:comment "Patient treatment was delayed as a consequence of device performance." .

imdrf:F06 a owl:Class ;
    rdfs:label "Disruption of Subsequent Medical Procedure" ;
    rdfs:comment "Situation in which the use of the device impedes or affects a subsequent medical procedure or use of a medicine or device. The time elapsed between the use of the device and the medical procedure is not a factor. It is not necessary for the device to have broken or malfunctioned." .

imdrf:F07 a owl:Class ;
    rdfs:label "Exacerbation of Existing Condition" ;
    rdfs:comment "Use of the device has lead to worsening of the existing disease or condition." .

imdrf:F0801 a owl:Class ;
    rdfs:label "Intensive Care" ;
    rdfs:comment "Patient requires admission to or extension of stay in an intensive care unit." ;
    rdfs:subClassOf imdrf:F08 .

imdrf:F0802 a owl:Class ;
    rdfs:label "Emergency Hospital Transfer" ;
    ex:status "New" ;
    ex:statusDescription "Term added for Release Number 2025. See no. 28 of Change Request Log" ;
    rdfs:comment "Patient required emergency transfer to a different facility because of the need for an additional level of care." ;
    rdfs:subClassOf imdrf:F08 .

imdrf:F09 a owl:Class ;
    rdfs:label "Fetal Harm" ;
    rdfs:comment "Fetal distress, congenital physical or mental impairment or birth defect, excluding fetal death." .

imdrf:F1001 a owl:Class ;
    rdfs:label "Absence of Treatment" ;
    rdfs:comment "Patient treatment was absent as a consequence of device performance." ;
    rdfs:subClassOf imdrf:F10 .

imdrf:F1002 a owl:Class ;
    rdfs:label "Incompatible Blood Transfusion" ;
    rdfs:comment "Receiving incorrect or incompatible whole blood or a blood component." ;
    rdfs:subClassOf imdrf:F10 .

imdrf:F1003 a owl:Class ;
    rdfs:label "Missed Dose" ;
    rdfs:comment "A dose of medicine was not taken or delivered at the prescribed dosing interval." ;
    rdfs:subClassOf imdrf:F10 .

imdrf:F100401 a owl:Class ;
    rdfs:label "Radiation Underdose" ;
    rdfs:comment "A lower than intended dose of radiation to a single field." ;
    rdfs:subClassOf imdrf:F1004 .

imdrf:F100501 a owl:Class ;
    rdfs:label "Radiation Overdose" ;
    rdfs:comment "A higher than intended cumulative dose of radiation to a single field." ;
    rdfs:subClassOf imdrf:F1005 .

imdrf:F1006 a owl:Class ;
    rdfs:label "Inadequate Treatment/Disease Progression" ;
    ex:status "Retired" ;
    ex:statusDescription "Term was added on 27 January 2022. For details, see comment No. 191 of the Change Log (Release Number 2022). Term retired for Release Number 2025. Use F1010 \"Inadequate Treatment\" or F30 \"Disease Progression\". See no. 63 of Change Request Log" ;
    rdfs:comment "The worsening of a disease over time due to inadequate treatment." ;
    rdfs:subClassOf imdrf:F10 .

imdrf:F1007 a owl:Class ;
    rdfs:label "Exposure to Contaminated Device/Risk of Infection" ;
    ex:statusDescription "Term was added on 27 January 2022. For details, see comment No. 214 of the Change Log (Release Number 2022)." ;
    rdfs:comment "Exposure to a non-sterile device or conditions where infection is likely." ;
    rdfs:subClassOf imdrf:F10 .

imdrf:F1008 a owl:Class ;
    rdfs:label "Accidental Exposure to Substance" ;
    ex:status "Modified (editorial)" ;
    ex:statusDescription "Term added for Release Number 2024. See no. 25 of Change Log. Formatting change to Term for Release Number 2025. See no. 21 of Change Request Log" ;
    rdfs:comment "Unintended exposure of the patient and/or healthcare providers to drugs or other substances.  This can include any exposure routes such as skin, mucous membranes, and respiratory." ;
    rdfs:subClassOf imdrf:F10 .

imdrf:F1009 a owl:Class ;
    rdfs:label "Inappropriate Treatment" ;
    ex:status "New" ;
    ex:statusDescription "Term added for Release Number 2025. See no. 20 of Change Request Log" ;
    rdfs:comment "Patient received treatment which was unnecessary or excessive. This includes treatment following a false positive diagnosis and excessive stimulation or shock delivery.  For drug or radiation overdose use F1005 or child term." ;
    rdfs:subClassOf imdrf:F10 .

imdrf:F1010 a owl:Class ;
    rdfs:label "Inadequate Treatment" ;
    ex:status "New" ;
    ex:statusDescription "Term added for Release Number 2025. See no. 63 of Change Request Log" ;
    rdfs:comment "Patient received inadequate or insufficient treatment of an appropriate type.  This includes inadequate stimulation or shock delivery.   For inappropriate treatment use F1009. For drug or radiation underdose use F1004 or child term." ;
    rdfs:subClassOf imdrf:F10 .

imdrf:F11 a owl:Class ;
    rdfs:label "Non-Serious Injury/Illness/Impairment" ;
    ex:status "Modified (technical)" ;
    ex:statusDescription "Definition was modified on 31 January 2023 (Old definition: A mild injury, illness or impairment which can be treated with minimal or no intervention.). For details, see comment No. 143 of the Change Log (Release Number 2023). Term and Definition modified for Release Number 2025. Previous term was \"Minor Injury/ Illness / Impairment\". See no. 79 of Change Request Log." ;
    rdfs:comment "A non-serious injury, illness or impairment which can be treated with minimal or no intervention, including monitoring only." .

imdrf:F1201 a owl:Class ;
    rdfs:label "Chronic Disease" ;
    rdfs:comment "Disease that persists over a long period of time, cannot be prevented by vaccines or cured by medication, nor do they just disappear." ;
    rdfs:subClassOf imdrf:F12 .

imdrf:F1202 a owl:Class ;
    rdfs:label "Disability" ;
    rdfs:comment "Any physical or mental impairment that interferes with an individual's ability to perform desired activities." ;
    rdfs:subClassOf imdrf:F12 .

imdrf:F1203 a owl:Class ;
    rdfs:label "Life Threatening Illness or Injury" ;
    rdfs:comment "Patient suffered an illness or injury which if not treated would be fatal." ;
    rdfs:subClassOf imdrf:F12 .

imdrf:F1204 a owl:Class ;
    rdfs:label "Permanent Impairment" ;
    rdfs:comment "Irreversible deterioration of the state of health." ;
    rdfs:subClassOf imdrf:F12 .

imdrf:F1205 a owl:Class ;
    rdfs:label "Temporary Impairment" ;
    rdfs:comment "Reversible deterioration of the state of health." ;
    rdfs:subClassOf imdrf:F12 .

imdrf:F13 a owl:Class ;
    rdfs:label "Misdiagnosis/ Misclassification" ;
    rdfs:comment "An incorrect diagnosis or classification of an illness or other problem." .

imdrf:F14 a owl:Class ;
    rdfs:label "Prolonged Episode of Care" ;
    ex:statusDescription "Editorial change to the definition on 16 February 2021." ;
    rdfs:comment "Clinically significant extended treatment time or procedural time. Not to be used for prolonged hospitalization or prolonged surgery." .

imdrf:F15 a owl:Class ;
    rdfs:label "Recognised Device or Procedural Complication" ;
    rdfs:comment "Patient experiencing a complication that is well documented in association with the device or procedure." .

imdrf:F16 a owl:Class ;
    rdfs:label "Reduction in Life Expectancy" ;
    rdfs:comment "Decrease in lifetime/ lifespan of an individual. Decline in the normal duration or in average life." .

imdrf:F17 a owl:Class ;
    rdfs:label "Sedation" ;
    rdfs:comment "Patient required sedation or additional sedation." .

imdrf:F18 a owl:Class ;
    rdfs:label "Rehabilitation" ;
    rdfs:comment "Patient requires treatment to facilitate the process of recovery from injury, illness, or disease." .

imdrf:F1901 a owl:Class ;
    rdfs:label "Additional Surgery" ;
    rdfs:comment "Surgical intervention that was not planned and needed to be performed in addition to other interventions including surgical ones." ;
    rdfs:subClassOf imdrf:F19 .

imdrf:F1902 a owl:Class ;
    rdfs:label "Amputation" ;
    rdfs:comment "Patient required surgical removal of limb, extremities or other external body parts." ;
    rdfs:subClassOf imdrf:F19 .

imdrf:F1903 a owl:Class ;
    rdfs:label "Device Explantation" ;
    rdfs:comment "Patient required a corrective invasive procedure to remove a device, or parts/fragments of a device." ;
    rdfs:subClassOf imdrf:F19 .

imdrf:F1904 a owl:Class ;
    rdfs:label "Device Repositioning" ;
    rdfs:comment "Patient required a corrective invasive procedure in which a device was repositioned. This includes implantable, surgically invasive (penetration through the surface of the body) or invasive (penetration though a natural body orifice or permanent artificial opening, e.g. stoma) devices." ;
    rdfs:subClassOf imdrf:F19 .

imdrf:F1905 a owl:Class ;
    rdfs:label "Device Revision or Replacement" ;
    rdfs:comment "Patient required a corrective invasive procedure in which a device was replaced/revised. This includes implantable, surgically invasive (penetration through the surface of the body) or invasive (penetration though a natural body orifice or permanent artificial opening, e.g. stoma) devices." ;
    rdfs:subClassOf imdrf:F19 .

imdrf:F1906 a owl:Class ;
    rdfs:label "Modified Surgical Procedure" ;
    rdfs:comment "A change of surgical procedures from the original plan." ;
    rdfs:subClassOf imdrf:F19 .

imdrf:F1907 a owl:Class ;
    rdfs:label "More Complex Surgery" ;
    ex:statusDescription "Definition was modified on 31 January 2023 (Old definition: Patient required additional or unexpected endoscopic procedure). For details, see comment No. 139 of the Change Log (Release Number 2023)." ;
    rdfs:comment "Surgery that is more complicated, more comprehensive or more extensive than planned (e.g. percutaneous to open surgery)." ;
    rdfs:subClassOf imdrf:F19 .

imdrf:F1908 a owl:Class ;
    rdfs:label "Prolonged Surgery" ;
    ex:status "Modified (editorial)" ;
    ex:statusDescription "Formatting change to Term for Release Number 2025. See no. 21 of Change Request Log" ;
    rdfs:comment "Surgery that takes longer than anticipated." ;
    rdfs:subClassOf imdrf:F19 .

imdrf:F1909 a owl:Class ;
    rdfs:label "Surgical Procedure Delayed" ;
    rdfs:comment "Surgical procedure unable to be completed when originally scheduled and put off until some time in the future." ;
    rdfs:subClassOf imdrf:F19 .

imdrf:F1910 a owl:Class ;
    rdfs:label "Cancelled/Aborted Surgical Procedure" ;
    ex:status "Modified (editorial)" ;
    ex:statusDescription "Term added for Release Number 2024. See no. 110 of Change Log. Formatting change to Term for Release Number 2025. See no. 21 of Change Request Log" ;
    rdfs:comment """Surgical procedure aborted, or unable to be completed.
This applies to cases where there is no information whether the procedure will be carried out at a later time, or where it is known that surgery will not go ahead.
If it is known that the procedure has been, or will be, carried out later then use F1909 - Surgical Procedure Delayed""" ;
    rdfs:subClassOf imdrf:F19 .

imdrf:F20 a owl:Class ;
    rdfs:label "Serious Public Health Threat" ;
    rdfs:comment "Any event type, which results in imminent risk of death, serious injury, or serious illness to more than one individual, that requires prompt remedial action." .

imdrf:F21 a owl:Class ;
    rdfs:label "Unexpected Deterioration" ;
    rdfs:comment "Unexpected clinical deterioration of patient." .

imdrf:F2201 a owl:Class ;
    rdfs:label "Biopsy" ;
    rdfs:comment "Patient required removal of tissue or fluid specimen to establish a diagnosis." ;
    rdfs:subClassOf imdrf:F22 .

imdrf:F2202 a owl:Class ;
    rdfs:label "Endoscopic Diagnostic Procedure" ;
    ex:statusDescription "Definition was modified on 31 January 2023 (Old definition: Patient required additional or unexpected endoscopic procedure). For details, see comment No. 137 of the Change Log (Release Number 2023)." ;
    rdfs:comment "Patient required additional or unexpected endoscopic diagnostic procedure." ;
    rdfs:subClassOf imdrf:F22 .

imdrf:F2203 a owl:Class ;
    rdfs:label "Imaging Required" ;
    rdfs:comment "Requirement for imaging that was not originally planned." ;
    rdfs:subClassOf imdrf:F22 .

imdrf:F2204 a owl:Class ;
    rdfs:label "IVD Testing" ;
    ex:statusDescription "Editorial change to the definition on 16 February 2021." ;
    rdfs:comment "Patient required additional or unexpected IVD testing." ;
    rdfs:subClassOf imdrf:F22 .

imdrf:F2301 a owl:Class ;
    rdfs:label "Additional Device Required" ;
    rdfs:comment "Use of an additional or alternative device require to achieve optimal outcome." ;
    rdfs:subClassOf imdrf:F23 .

imdrf:F2302 a owl:Class ;
    rdfs:label "Blood Transfusion" ;
    rdfs:comment "Patient required an infusion of whole blood or a blood component directly into the bloodstream." ;
    rdfs:subClassOf imdrf:F23 .

imdrf:F2303 a owl:Class ;
    rdfs:label "Medication Required" ;
    ex:status "Modified (editorial)" ;
    ex:statusDescription "Definition modified for Release Number 2025. See no. 99 of Change Request Log" ;
    rdfs:comment "Patient required new/additional medication or additional dose of existing medication." ;
    rdfs:subClassOf imdrf:F23 .

imdrf:F2304 a owl:Class ;
    rdfs:label "Prophylactic Treatment" ;
    rdfs:comment "A medication or course of action used to prevent a possible disease or condition from occurring." ;
    rdfs:subClassOf imdrf:F23 .

imdrf:F2305 a owl:Class ;
    rdfs:label "Radiation Therapy" ;
    ex:statusDescription "Editorial change to the definition on 16 February 2021." ;
    rdfs:comment "Patient required additional radiation therapy." ;
    rdfs:subClassOf imdrf:F23 .

imdrf:F2306 a owl:Class ;
    rdfs:label "Resuscitation" ;
    rdfs:comment "Patient required resuscitation." ;
    rdfs:subClassOf imdrf:F23 .

imdrf:F2307 a owl:Class ;
    rdfs:label "Reprogramming of Device" ;
    ex:statusDescription "Term was added on 31 January 2023. For details, see comment No. 133 of the Change Log (Release Number 2023)." ;
    rdfs:comment "Patient required programming changes to be made to an implantable or other programmable device." ;
    rdfs:subClassOf imdrf:F23 .

imdrf:F2308 a owl:Class ;
    rdfs:label "Medical treatment under anaesthesia" ;
    ex:statusDescription "Term added for Release Number 2024. See no. 111 of Change Log" ;
    rdfs:comment "Patient required non-surgical treatment under anaesthesia." ;
    rdfs:subClassOf imdrf:F23 .

imdrf:F2309 a owl:Class ;
    rdfs:label "Ventilation" ;
    ex:status "New" ;
    ex:statusDescription "Term added for Release Number 2025. See no. 27 of Change Request Log" ;
    rdfs:comment "Patient required ventilation or clinically significant extension of existing ventilation" ;
    rdfs:subClassOf imdrf:F23 .

imdrf:F24 a owl:Class ;
    rdfs:label "Insufficient Health Impact Information" ;
    ex:status "Modified (editorial)" ;
    ex:statusDescription "Definition was modified on 31 January 2023 (Old definition: There is not yet enough information available to classify the health impact). For details, see comment No. 102 of the Change Log (Release Number 2023). Term and Definition modified for Release Number 2025. Previous term was \"Insufficient Information\". See no. 122 of Change Request Log." ;
    rdfs:comment "It is not clear whether any health impact occurred, or health impact appears to have occurred, but there is not yet enough information available to classify the health impact." .

imdrf:F25 a owl:Class ;
    rdfs:label "Unanticipated Adverse Device Effect" ;
    ex:statusDescription "Editorial change to the definition on 16 February 2021." ;
    rdfs:comment "Complication occurring in the patient that had not previously been identified or expected for this device." .

imdrf:F2601 a owl:Class ;
    rdfs:label "Problem identified before clinical use/exposure" ;
    ex:statusDescription "Term added for Release Number 2024. See no. 120 of Change Log" ;
    rdfs:comment """The adverse event occurred during or immediately prior to a clinical procedure, but the problem was identified and corrected before harm could be caused.
E.g.1. an IVD gave a false reading but it was recognized as incorrect before treatment decisions were made and without any clinically significant delay to diagnosis;
E.g.2. a surgical device malfunctioned during pre-use checks and the malfunction was corrected or an alternative device was available without any clinically significant delay to the procedure.""" ;
    rdfs:subClassOf imdrf:F26 .

imdrf:F27 a owl:Class ;
    rdfs:label "Problem identified during non-clinical procedure." ;
    ex:statusDescription "Term and Definition modified for Release Number 2024. Previous term was No Patient Involvement. See no. 121 of Change Log" ;
    rdfs:comment """The adverse event occurred while the device was being used in a non-clinical setting and/or procedure and could not have any impact on a patient
E.g.1. an IVD gave a false reading when testing an External Quality Assessment (EQA) sample;
E.g.2. a surgical device malfunctioned during cleaning and/or maintenance.""" .

imdrf:F28 a owl:Class ;
    rdfs:label "Appropriate Health Impact Term/Code Not Available" ;
    ex:status "Modified (editorial)" ;
    ex:statusDescription "Term and Definition modified for Release Number 2025. Previous term was \"Appropriate Term/Code Not Available\". See no. 111 of Change Request Log." ;
    rdfs:comment "The Health Impact is not adequately described by any other term. Note: this code must not be used unless there is no other feasible code. The preferred term should be documented when submitting an adverse event report. This information will be used to determine if a new term should be added to the code table." .

imdrf:F29 a owl:Class ;
    rdfs:label "Death not related to reported adverse event" ;
    ex:statusDescription "Term added for Release Number 2024. See no. 119 of Change Log" ;
    rdfs:comment "A death has occurred, but it was confirmed that the event did not contribute to the death.  Other terms may also be selected if it is possible to link the adverse event to other identifiable health impacts." .

imdrf:F30 a owl:Class ;
    rdfs:label "Disease Progression" ;
    ex:status "New" ;
    ex:statusDescription "Term added for Release Number 2025. See no. 63 of Change Request Log" ;
    rdfs:comment "The worsening of a disease over time related to device performance." .

imdrf:F31 a owl:Class ;
    rdfs:label "Cancelled/Aborted Treatment/Therapy" ;
    ex:status "New" ;
    ex:statusDescription "Term added for Release Number 2025. See no. 84 of Change Request Log" ;
    rdfs:comment "Patient treatment aborted, or unable to be completed. This applies to cases where there is no information whether the treatment will be carried out at a later time, or where it is known that treatment will not go ahead. If it is known that the treatment has been, or will be, carried out later then use F05 - Delay to Treatment/ Therapy" .

imdrf:G01001 a owl:Class ;
    rdfs:label "Absorber" ;
    rdfs:comment "A component or material designed to take in or attenuate a substance." ;
    rdfs:subClassOf imdrf:G01 .

imdrf:G01002 a owl:Class ;
    rdfs:label "Cautery Tip" ;
    rdfs:comment "A component designed to coagulate and seal blood vessels or to destroy tissue with heat or electric current." ;
    rdfs:subClassOf imdrf:G01 .

imdrf:G01003 a owl:Class ;
    rdfs:label "Device Ingredient or Reagent" ;
    rdfs:comment "A consumable material that is added to a device and is used to make a finished product or becomes part of a finished product." ;
    rdfs:subClassOf imdrf:G01 .

imdrf:G01004 a owl:Class ;
    rdfs:label "Gas Scavenging" ;
    rdfs:comment "A component designed to remove certain gases from a gas stream or environment." ;
    rdfs:subClassOf imdrf:G01 .

imdrf:G01005 a owl:Class ;
    rdfs:label "Monomer Liquid" ;
    rdfs:comment "The liquid that reacts with the polymer powder to form adhesive, resin, or cement." ;
    rdfs:subClassOf imdrf:G01 .

imdrf:G01006 a owl:Class ;
    rdfs:label "Test Strip" ;
    rdfs:comment "A piece of chemically treated medium designed to react in the presence of specific amounts of a trigger substance." ;
    rdfs:subClassOf imdrf:G01 .

imdrf:G01007 a owl:Class ;
    rdfs:label "Polymer Powder" ;
    rdfs:comment "The powder that reacts with the monomer liquid to form adhesive, resin, or cement." ;
    rdfs:subClassOf imdrf:G01 .

imdrf:G02001 a owl:Class ;
    rdfs:label "Antenna" ;
    rdfs:comment "A component designed to transmit or receive electromagnetic signals." ;
    rdfs:subClassOf imdrf:G02 .

imdrf:G02002 a owl:Class ;
    rdfs:label "Battery" ;
    rdfs:comment "A component designed to produce an electric current through chemical reaction." ;
    rdfs:subClassOf imdrf:G02 .

imdrf:G02003 a owl:Class ;
    rdfs:label "Battery Charger" ;
    rdfs:comment "A device designed to restore the capacity of a battery." ;
    rdfs:subClassOf imdrf:G02 .

imdrf:G0200401 a owl:Class ;
    rdfs:label "Cable Grip/Tie" ;
    ex:statusDescription "Term/definition was modified on 31 January 2023 (Old term/definition: Cable Grip: Component used for tensioning, pulling or stringing of wires and cables.). For details, see comment No. 151 of the Change Log (Release Number 2023)." ;
    rdfs:comment "Component used for tensioning, pulling, holding or stringing of wires and cables." ;
    rdfs:subClassOf imdrf:G02004 .

imdrf:G0200402 a owl:Class ;
    rdfs:label "Cable Sleeve" ;
    rdfs:comment "Component used to protect cables and wires from abrasion, moisture and the elements." ;
    rdfs:subClassOf imdrf:G02004 .

imdrf:G02005 a owl:Class ;
    rdfs:label "Circuit Board" ;
    rdfs:comment "A non-conducting board with conductive tracks and electronic components forming a circuit." ;
    rdfs:subClassOf imdrf:G02 .

imdrf:G02006 a owl:Class ;
    rdfs:label "Circuit Breaker" ;
    rdfs:comment "A component designed to open an electrical circuit when it becomes overloaded." ;
    rdfs:subClassOf imdrf:G02 .

imdrf:G0200701 a owl:Class ;
    rdfs:label "Computer Processor" ;
    rdfs:comment "Component that carries out the instructions of a computer program by performing the basic arithmetic, logic, controlling, and input/output operations specified by the instructions." ;
    rdfs:subClassOf imdrf:G02007 .

imdrf:G0200702 a owl:Class ;
    rdfs:label "Memory/Storage" ;
    rdfs:comment "Any component that can hold data in machine-readable format." ;
    rdfs:subClassOf imdrf:G02007 .

imdrf:G0200703 a owl:Class ;
    rdfs:label "Network Interface" ;
    rdfs:comment "Point of interconnection between a computer and other computer that are linked each other." ;
    rdfs:subClassOf imdrf:G02007 .

imdrf:G0200801 a owl:Class ;
    rdfs:label "Driver" ;
    rdfs:comment "A computer interface designed to control the interaction between a CPU and a peripheral device." ;
    rdfs:subClassOf imdrf:G02008 .

imdrf:G0200802 a owl:Class ;
    rdfs:label "Software Interface" ;
    rdfs:comment "Languages, codes and messages that programs use to communicate with each other and to the hardware." ;
    rdfs:subClassOf imdrf:G02008 .

imdrf:G0200803 a owl:Class ;
    rdfs:label "User Interface" ;
    rdfs:comment "A computer program that controls the interaction between a user and a system." ;
    rdfs:subClassOf imdrf:G02008 .

imdrf:G0200804 a owl:Class ;
    rdfs:label "Firmware" ;
    ex:statusDescription "Term was added on 31 January 2023. For details, see comment No. 144 of the Change Log (Release Number 2023)." ;
    rdfs:comment "Computer instructions and data that reside as read-only software on that device. The computer cannot modify such software during processing." ;
    rdfs:subClassOf imdrf:G02008 .

imdrf:G02009 a owl:Class ;
    rdfs:label "Cooling Module" ;
    rdfs:comment "A component designed to lower the temperature of a device or system." ;
    rdfs:subClassOf imdrf:G02 .

imdrf:G02010 a owl:Class ;
    rdfs:label "Device Programmer" ;
    rdfs:comment "A piece of hardware for transferring data onto programmable integrated circuits." ;
    rdfs:subClassOf imdrf:G02 .

imdrf:G02011 a owl:Class ;
    rdfs:label "Device Reader" ;
    ex:statusDescription "Editorial change to the definition on 16 February 2021." ;
    rdfs:comment "A piece of hardware used to read the memory and the properties of a device." ;
    rdfs:subClassOf imdrf:G02 .

imdrf:G0201201 a owl:Class ;
    rdfs:label "Capacitor" ;
    rdfs:comment "An electrical component designed to store an electric charge." ;
    rdfs:subClassOf imdrf:G02012 .

imdrf:G0201202 a owl:Class ;
    rdfs:label "Fuse" ;
    rdfs:comment "An electrical component designed to stop the flow of current when an overload condition exists." ;
    rdfs:subClassOf imdrf:G02012 .

imdrf:G0201203 a owl:Class ;
    rdfs:label "Inductor" ;
    rdfs:comment "A component designed to introduce electromotive force to a circuit, usually a coil surrounding a wire." ;
    rdfs:subClassOf imdrf:G02012 .

imdrf:G0201204 a owl:Class ;
    rdfs:label "Resistor" ;
    rdfs:comment "An electronic component that opposes the flow of current." ;
    rdfs:subClassOf imdrf:G02012 .

imdrf:G0201205 a owl:Class ;
    rdfs:label "Solenoid" ;
    rdfs:comment "An electronic component consisting of a coil surrounding a movable iron core that is designed to act as a switch or relay." ;
    rdfs:subClassOf imdrf:G02012 .

imdrf:G0201206 a owl:Class ;
    rdfs:label "Transducer" ;
    rdfs:comment "An electrical component that converts one form of energy into another." ;
    rdfs:subClassOf imdrf:G02012 .

imdrf:G0201207 a owl:Class ;
    rdfs:label "Semiconductor" ;
    rdfs:comment "A type of electronic component, including transistors and diodes, that make use of the variable conductivity of certain materials." ;
    rdfs:subClassOf imdrf:G02012 .

imdrf:G0201208 a owl:Class ;
    rdfs:label "Feedthrough Capacitor" ;
    ex:status "New" ;
    ex:statusDescription "Term added for Release Number 2025. See no. 29 of Change Request Log" ;
    rdfs:comment "A component used to carry a current from an enclosing. Ensures that hermeticity is maintained." ;
    rdfs:subClassOf imdrf:G02012 .

imdrf:G02013 a owl:Class ;
    rdfs:label "IC (Integrated Circuit) Chip" ;
    rdfs:comment "A microelectronic circuit that incorporates many interconnected transistors and other components." ;
    rdfs:subClassOf imdrf:G02 .

imdrf:G0201401 a owl:Class ;
    rdfs:label "Indicator" ;
    rdfs:comment "A component designed to show an operating condition of a system or to attract attention." ;
    rdfs:subClassOf imdrf:G02014 .

imdrf:G0201402 a owl:Class ;
    rdfs:label "Screen" ;
    rdfs:comment "A panel or area on an electronic device where images and data are displayed." ;
    rdfs:subClassOf imdrf:G02014 .

imdrf:G0201501 a owl:Class ;
    rdfs:label "Electrode" ;
    ex:statusDescription "Editorial change to the definition on 16 February 2021." ;
    rdfs:comment "A small piece of metal or other conductive substance this is used to take an electric current to or from a source of power, a piece of equipment. Not to be used for patient connection." ;
    rdfs:subClassOf imdrf:G02015 .

imdrf:G0201502 a owl:Class ;
    rdfs:label "Ground Strap/Wire" ;
    rdfs:comment "A wire cable or strap designed to carry current safely away from an electronic device under fault condition" ;
    rdfs:subClassOf imdrf:G02015 .

imdrf:G0201503 a owl:Class ;
    rdfs:label "Wiring Harness" ;
    rdfs:comment "A collection of grouped wires or cables designed to connect to a specific device." ;
    rdfs:subClassOf imdrf:G02015 .

imdrf:G02016 a owl:Class ;
    rdfs:label "Electrical Mixer" ;
    rdfs:comment "An electronic component designed to blend signals." ;
    rdfs:subClassOf imdrf:G02 .

imdrf:G02017 a owl:Class ;
    rdfs:label "Electrical Port" ;
    rdfs:comment "An electronic circuit that acts as a connection to another device or component." ;
    rdfs:subClassOf imdrf:G02 .

imdrf:G02018 a owl:Class ;
    rdfs:label "Emitter" ;
    rdfs:comment "The electron source electrode in a transistor or any source in a system." ;
    rdfs:subClassOf imdrf:G02 .

imdrf:G02019 a owl:Class ;
    rdfs:label "Headphone/Headset" ;
    rdfs:comment "A component that covers the ear through which you can listen to without other people hearing. Some headphones come with a microphone which is used to communicate with other people or the device." ;
    rdfs:subClassOf imdrf:G02 .

imdrf:G02020 a owl:Class ;
    rdfs:label "Heater" ;
    ex:statusDescription "Editorial change to the definition on 16 February 2021." ;
    rdfs:comment "A piece of equipment used to raise the temperature of air, gas or water or an object." ;
    rdfs:subClassOf imdrf:G02 .

imdrf:G02021 a owl:Class ;
    rdfs:label "Hub" ;
    rdfs:comment "An electronic component designed as a central connection for other devices or components." ;
    rdfs:subClassOf imdrf:G02 .

imdrf:G02022 a owl:Class ;
    rdfs:label "Inverter" ;
    rdfs:comment "An electrical component that converts direct current to alternating current." ;
    rdfs:subClassOf imdrf:G02 .

imdrf:G02023 a owl:Class ;
    rdfs:label "Magnet" ;
    rdfs:comment "A component that attracts iron and produces a magnetic field." ;
    rdfs:subClassOf imdrf:G02 .

imdrf:G02024 a owl:Class ;
    rdfs:label "Oscillator" ;
    rdfs:comment "An electronic component designed to produce a wave signal." ;
    rdfs:subClassOf imdrf:G02 .

imdrf:G0202501 a owl:Class ;
    rdfs:label "Lead Conductor" ;
    rdfs:comment "A cable designed to conduct electricity from the device to the lead." ;
    rdfs:subClassOf imdrf:G02025 .

imdrf:G0202502 a owl:Class ;
    rdfs:label "Patient Electrode" ;
    rdfs:comment "An electrical conductor that is designed to make contact with a patient including defibrillator paddles." ;
    rdfs:subClassOf imdrf:G02025 .

imdrf:G02026 a owl:Class ;
    rdfs:label "Power Cord" ;
    rdfs:comment "A flexible cable designed to connect an electrical device to a power outlet." ;
    rdfs:subClassOf imdrf:G02 .

imdrf:G02027 a owl:Class ;
    rdfs:label "Power Supply" ;
    rdfs:comment "Component designed to supply electrical power to devices." ;
    rdfs:subClassOf imdrf:G02 .

imdrf:G02028 a owl:Class ;
    rdfs:label "Pressure Transducer Probe" ;
    rdfs:comment "A probe component designed to convert a change in pressure into a varying electrical signal." ;
    rdfs:subClassOf imdrf:G02 .

imdrf:G02029 a owl:Class ;
    rdfs:label "Printer" ;
    rdfs:comment "An electronic component that is designed to transfer text or images to paper or other substrate." ;
    rdfs:subClassOf imdrf:G02 .

imdrf:G02030 a owl:Class ;
    rdfs:label "Receiver" ;
    rdfs:comment "An electronic component designed to capture an incoming electromagnetic signal and convert it to an audible or visual signal." ;
    rdfs:subClassOf imdrf:G02 .

imdrf:G02031 a owl:Class ;
    rdfs:label "Receiver Stimulator Unit" ;
    rdfs:comment "As part of a cochlear implant, an implanted component designed to receive signal from the external component and then decode the signal and transmit it to the brain." ;
    rdfs:subClassOf imdrf:G02 .

imdrf:G02032 a owl:Class ;
    rdfs:label "Scanner" ;
    rdfs:comment "An electronic component that generates a digital representation of an image for data input to a computer; or a receiver designed to search for a signal within a specified frequency range." ;
    rdfs:subClassOf imdrf:G02 .

imdrf:G02033 a owl:Class ;
    rdfs:label "Speaker/Sounder" ;
    rdfs:comment "A component designed to convert electrical signals to sounds that can be heard." ;
    rdfs:subClassOf imdrf:G02 .

imdrf:G0203401 a owl:Class ;
    rdfs:label "Power Switch" ;
    rdfs:comment "A switch designed to regulate the power to a device." ;
    rdfs:subClassOf imdrf:G02034 .

imdrf:G0203402 a owl:Class ;
    rdfs:label "Relay" ;
    rdfs:comment "A electronic component designed to break or change the connections in a circuit." ;
    rdfs:subClassOf imdrf:G02034 .

imdrf:G02035 a owl:Class ;
    rdfs:label "Telemetry" ;
    rdfs:comment "Component designed to transmit and receive data from a remote source using telecommunications methods." ;
    rdfs:subClassOf imdrf:G02 .

imdrf:G02036 a owl:Class ;
    rdfs:label "Temperature Compensator" ;
    rdfs:comment "A component designed to compensate the temperature of one system in response to temperature changes in another system or the environment." ;
    rdfs:subClassOf imdrf:G02 .

imdrf:G02037 a owl:Class ;
    rdfs:label "Thermostat" ;
    rdfs:comment "A component designed to regulate temperature by controlling the starting and stopping of a heating/cooling system." ;
    rdfs:subClassOf imdrf:G02 .

imdrf:G02038 a owl:Class ;
    rdfs:label "Transformer" ;
    rdfs:comment "A component that either steps up or steps down an alternating electrical current to an output that is suitable for another electrical device or component." ;
    rdfs:subClassOf imdrf:G02 .

imdrf:G02039 a owl:Class ;
    rdfs:label "Transmitter" ;
    rdfs:comment "A component to propagate electromagnetic waves." ;
    rdfs:subClassOf imdrf:G02 .

imdrf:G0204001 a owl:Class ;
    rdfs:label "Joystick" ;
    rdfs:comment "A control component that uses a movable handle to create two-axis input to a computer." ;
    rdfs:subClassOf imdrf:G02040 .

imdrf:G0204002 a owl:Class ;
    rdfs:label "Keyboard/Keypad" ;
    rdfs:comment "A component consisting of mechanical keys that are pressed to create input to a computer." ;
    rdfs:subClassOf imdrf:G02040 .

imdrf:G0204003 a owl:Class ;
    rdfs:label "Microphone" ;
    rdfs:comment "A component designed to convert sound to an electrical signal." ;
    rdfs:subClassOf imdrf:G02040 .

imdrf:G0204004 a owl:Class ;
    rdfs:label "Touchscreen" ;
    rdfs:comment "A control component that operates the device following pressing the display on the screen." ;
    rdfs:subClassOf imdrf:G02040 .

imdrf:G02041 a owl:Class ;
    rdfs:label "Solder Joint" ;
    ex:status "New" ;
    ex:statusDescription "Term added for Release Number 2025. See no. 30 of Change Request Log" ;
    rdfs:comment "Joint between electrical components, often to a printed circuit board" ;
    rdfs:subClassOf imdrf:G02 .

imdrf:G0300101 a owl:Class ;
    rdfs:label "Oxygen Analyzer" ;
    rdfs:comment "A component designed to measure the concentration of oxygen in a gas mixture." ;
    rdfs:subClassOf imdrf:G03001 .

imdrf:G03002 a owl:Class ;
    rdfs:label "Aperture" ;
    rdfs:comment "An instrument designed to measure the size of an opening or one used to increase the diameter of an opening" ;
    rdfs:subClassOf imdrf:G03 .

imdrf:G03003 a owl:Class ;
    rdfs:label "Calibrator" ;
    rdfs:comment "A standard or reference material used to set the operating parameters of an instrument." ;
    rdfs:subClassOf imdrf:G03 .

imdrf:G03004 a owl:Class ;
    rdfs:label "Clock" ;
    rdfs:comment "A component designed to indicate the time of day." ;
    rdfs:subClassOf imdrf:G03 .

imdrf:G03005 a owl:Class ;
    rdfs:label "Counter" ;
    rdfs:comment "A component designed to keep track of the number of times something happens." ;
    rdfs:subClassOf imdrf:G03 .

imdrf:G03006 a owl:Class ;
    rdfs:label "Cuvette" ;
    ex:statusDescription "Editorial change to the definition on 16 February 2021." ;
    rdfs:comment "A clear container designed to interface with an optical sensor in order to obtain an optical measurement of a contained substance." ;
    rdfs:subClassOf imdrf:G03 .

imdrf:G0300701 a owl:Class ;
    rdfs:label "Flowmeter" ;
    rdfs:comment "A component designed to measure the flow rate of a fluid." ;
    rdfs:subClassOf imdrf:G03007 .

imdrf:G0300702 a owl:Class ;
    rdfs:label "Manometer" ;
    rdfs:comment "A component designed to measure pressure." ;
    rdfs:subClassOf imdrf:G03007 .

imdrf:G0300703 a owl:Class ;
    rdfs:label "Thermometer" ;
    rdfs:comment "A component designed to measure temperature." ;
    rdfs:subClassOf imdrf:G03007 .

imdrf:G03008 a owl:Class ;
    rdfs:label "Marker" ;
    rdfs:comment "A visual indicator of position, place or route, including radiopaque markers." ;
    rdfs:subClassOf imdrf:G03 .

imdrf:G03009 a owl:Class ;
    rdfs:label "Pipette" ;
    rdfs:comment "A measuring component, traditionally including a graduated tube, designed for the accurate transfer of liquid volumes." ;
    rdfs:subClassOf imdrf:G03 .

imdrf:G03010 a owl:Class ;
    rdfs:label "Pointer" ;
    rdfs:comment "An indicator component designed to show a position on a scale." ;
    rdfs:subClassOf imdrf:G03 .

imdrf:G03011 a owl:Class ;
    rdfs:label "Scale" ;
    rdfs:comment "A component designed for weighing or an indicator component with a graduated sequence of divisions." ;
    rdfs:subClassOf imdrf:G03 .

imdrf:G0301201 a owl:Class ;
    rdfs:label "Bubble Sensor" ;
    rdfs:comment "A component designed to signal the presence of bubbles in a system." ;
    rdfs:subClassOf imdrf:G03012 .

imdrf:G0301202 a owl:Class ;
    rdfs:label "O2 Sensor" ;
    rdfs:comment "A sensor designed to respond to the presence or level of oxygen in a space or environment." ;
    rdfs:subClassOf imdrf:G03012 .

imdrf:G0301203 a owl:Class ;
    rdfs:label "Photodetector" ;
    rdfs:comment "A component designed to detect light." ;
    rdfs:subClassOf imdrf:G03012 .

imdrf:G0301204 a owl:Class ;
    rdfs:label "Pressure Sensor" ;
    rdfs:comment "A sensor designed to respond to the level of pressure in a space or pressing on a surface." ;
    rdfs:subClassOf imdrf:G03012 .

imdrf:G0301205 a owl:Class ;
    rdfs:label "Sensor Probe" ;
    rdfs:comment "A component designed to reach into a location for sensing. Should be used when the problem involves the probe, not the sensor." ;
    rdfs:subClassOf imdrf:G03012 .

imdrf:G0301206 a owl:Class ;
    rdfs:label "Temperature Sensor" ;
    rdfs:comment "A sensor designed to respond to the temperature of a space, surface, or environment." ;
    rdfs:subClassOf imdrf:G03012 .

imdrf:G03013 a owl:Class ;
    rdfs:label "Timer" ;
    rdfs:comment "A component designed to measure a time interval." ;
    rdfs:subClassOf imdrf:G03 .

imdrf:G03014 a owl:Class ;
    rdfs:label "Control Material" ;
    ex:statusDescription "Term was added on 31 January 2023. For details, see comment No. 145 of the Change Log (Release Number 2023)." ;
    rdfs:comment "A standard or reference material used for the purposes of comparative evaluations." ;
    rdfs:subClassOf imdrf:G03 .

imdrf:G03015 a owl:Class ;
    rdfs:label "Swab" ;
    ex:statusDescription "Term was added on 31 January 2023. For details, see comment No. 146 of the Change Log (Release Number 2023)." ;
    rdfs:comment "An absorbent pad or piece of material attached to the end of a stick typically used for applying medicines or taking specimens." ;
    rdfs:subClassOf imdrf:G03 .

imdrf:G03016 a owl:Class ;
    rdfs:label "Tray" ;
    ex:statusDescription "Term was added on 31 January 2023. For details, see comment No. 148 of the Change Log (Release Number 2023)." ;
    rdfs:comment "A flat, shallow container with a raised rim." ;
    rdfs:subClassOf imdrf:G03 .

imdrf:G04001 a owl:Class ;
    rdfs:label "Access Port" ;
    rdfs:comment "A component designed for the introduction or removal of medical equipment or any substance." ;
    rdfs:subClassOf imdrf:G04 .

imdrf:G04002 a owl:Class ;
    rdfs:label "Actuator" ;
    rdfs:comment "A component which moves or controls a mechanism or system." ;
    rdfs:subClassOf imdrf:G04 .

imdrf:G04003 a owl:Class ;
    rdfs:label "Adapter (Adaptor)" ;
    rdfs:comment "A component designed to make different pieces of apparatus compatible." ;
    rdfs:subClassOf imdrf:G04 .

imdrf:G04004 a owl:Class ;
    rdfs:label "Air Eliminator" ;
    rdfs:comment "A component designed to remove air from a space or fluid." ;
    rdfs:subClassOf imdrf:G04 .

imdrf:G0400501 a owl:Class ;
    rdfs:label "Fixation Tines" ;
    ex:statusDescription "Term added for Release Number 2024. See no. 114 of Change Log." ;
    rdfs:comment "Projections designed to fix a device inside a cavity of the human body" ;
    rdfs:subClassOf imdrf:G04005 .

imdrf:G04006 a owl:Class ;
    rdfs:label "Applicator" ;
    rdfs:comment "A component designed to transfer a substance to a surface." ;
    rdfs:subClassOf imdrf:G04 .

imdrf:G04007 a owl:Class ;
    rdfs:label "Automatic Injection System" ;
    rdfs:comment "A system designed to pump a gas or liquid into a space or environment without outside intervention." ;
    rdfs:subClassOf imdrf:G04 .

imdrf:G04008 a owl:Class ;
    rdfs:label "Bag" ;
    rdfs:comment "A flexible container, often with a single opening." ;
    rdfs:subClassOf imdrf:G04 .

imdrf:G04009 a owl:Class ;
    rdfs:label "Ball" ;
    rdfs:comment "Any component that is spherical in shape." ;
    rdfs:subClassOf imdrf:G04 .

imdrf:G04010 a owl:Class ;
    rdfs:label "Balloon" ;
    rdfs:comment "A sac designed to be inflated and deflated." ;
    rdfs:subClassOf imdrf:G04 .

imdrf:G04011 a owl:Class ;
    rdfs:label "Bearings" ;
    rdfs:comment "A point of contact between moving parts designed for support or to reduce friction." ;
    rdfs:subClassOf imdrf:G04 .

imdrf:G04012 a owl:Class ;
    rdfs:label "Bellows" ;
    rdfs:comment "A component that expands and contracts to draw in air through a valve or orifice and expels it through a tube." ;
    rdfs:subClassOf imdrf:G04 .

imdrf:G04013 a owl:Class ;
    rdfs:label "Belt" ;
    rdfs:comment "A component consisting of a narrow band of material moving over shafts or pulleys." ;
    rdfs:subClassOf imdrf:G04 .

imdrf:G04014 a owl:Class ;
    rdfs:label "Bottle" ;
    rdfs:comment "A rigid or semi-rigid container used to store liquid." ;
    rdfs:subClassOf imdrf:G04 .

imdrf:G04015 a owl:Class ;
    rdfs:label "Breathing Circuit" ;
    rdfs:comment "In an anesthesia machine, the pathway by which a gaseous anesthetic agent and oxygen are delivered to the patient and carbon dioxide is removed. The circuit can be open or closed." ;
    rdfs:subClassOf imdrf:G04 .

imdrf:G04016 a owl:Class ;
    rdfs:label "Brush" ;
    rdfs:comment "A component consisting of hairs or bristles set into a handle or holder." ;
    rdfs:subClassOf imdrf:G04 .

imdrf:G04017 a owl:Class ;
    rdfs:label "Bushing" ;
    rdfs:comment "A cylindrical metal sleeve designed to reduce the friction of a rotating shaft." ;
    rdfs:subClassOf imdrf:G04 .

imdrf:G04018 a owl:Class ;
    rdfs:label "Cable, Mechanical/Structural" ;
    rdfs:comment "A long, thin, multistranded rope or metallic wire to hold the subject." ;
    rdfs:subClassOf imdrf:G04 .

imdrf:G0401901 a owl:Class ;
    rdfs:label "Cannula Hub" ;
    rdfs:comment "A metal or plastic component that connects to the cannula." ;
    rdfs:subClassOf imdrf:G04019 .

imdrf:G04020 a owl:Class ;
    rdfs:label "Cap" ;
    rdfs:comment "A component designed to close an opening of a container or device." ;
    rdfs:subClassOf imdrf:G04 .

imdrf:G04021 a owl:Class ;
    rdfs:label "Carrier" ;
    rdfs:comment "A component designed to facilitate the support, movement, or transport of another device or object." ;
    rdfs:subClassOf imdrf:G04 .

imdrf:G04022 a owl:Class ;
    rdfs:label "Caster" ;
    rdfs:comment "A pivoting roller or wheel designed to attach to an object to make it movable." ;
    rdfs:subClassOf imdrf:G04 .

imdrf:G0402301 a owl:Class ;
    rdfs:label "Catheter Hub" ;
    rdfs:comment "A small metal or plastic component that connects to the catheter." ;
    rdfs:subClassOf imdrf:G04023 .

imdrf:G04024 a owl:Class ;
    rdfs:label "Cell" ;
    rdfs:comment "A component that is designed as a container to collect and/or transfer materials, reagents or specimens." ;
    rdfs:subClassOf imdrf:G04 .

imdrf:G04025 a owl:Class ;
    rdfs:label "Chain" ;
    rdfs:comment "Assembly of interconnected links, typically made of metal used for connecting other components." ;
    rdfs:subClassOf imdrf:G04 .

imdrf:G04026 a owl:Class ;
    rdfs:label "Chamber" ;
    rdfs:comment "A component designed as a reservoir/storage." ;
    rdfs:subClassOf imdrf:G04 .

imdrf:G04027 a owl:Class ;
    rdfs:label "Chassis/Frame" ;
    rdfs:comment "A supporting frame designed to hold other components or devices such as the internal frame of an electronic device." ;
    rdfs:subClassOf imdrf:G04 .

imdrf:G04028 a owl:Class ;
    rdfs:label "Clutch" ;
    rdfs:comment "A component that engages and disengages power transmission." ;
    rdfs:subClassOf imdrf:G04 .

imdrf:G04029 a owl:Class ;
    rdfs:label "Coating Material" ;
    rdfs:comment "A layer of material covering the surface of a device." ;
    rdfs:subClassOf imdrf:G04 .

imdrf:G0403001 a owl:Class ;
    rdfs:label "Fixation Helix" ;
    ex:statusDescription "Term and Definition modified for Release Number 2024. Previous term was Helifix Coil. See no. 113 of Change Log." ;
    rdfs:comment "A coil designed for fixing or anchoring a device in human tissue." ;
    rdfs:subClassOf imdrf:G04030 .

imdrf:G04031 a owl:Class ;
    rdfs:label "Collimator" ;
    rdfs:comment "A diaphragm or system of diaphragms made of an absorbing material, designed to define and restrict the dimensions and direction of a beam of radiation." ;
    rdfs:subClassOf imdrf:G04 .

imdrf:G04032 a owl:Class ;
    rdfs:label "Concentrator" ;
    rdfs:comment "A component designed to increase the weight per unit volume of a substance." ;
    rdfs:subClassOf imdrf:G04 .

imdrf:G04033 a owl:Class ;
    rdfs:label "Cone" ;
    rdfs:comment "A three-dimensional part that tapers smoothly from a flat circular shape at one end to a point at the other end." ;
    rdfs:subClassOf imdrf:G04 .

imdrf:G0403401 a owl:Class ;
    rdfs:label "Connector Pin" ;
    rdfs:comment "A projecting part of a device that allows it to be secured through an opening." ;
    rdfs:subClassOf imdrf:G04034 .

imdrf:G04035 a owl:Class ;
    rdfs:label "Controller" ;
    rdfs:comment "A component designed to control or regulate the operation of another device." ;
    rdfs:subClassOf imdrf:G04 .

imdrf:G04036 a owl:Class ;
    rdfs:label "Compressor" ;
    rdfs:comment "A component that increases the pressure of air or gas." ;
    rdfs:subClassOf imdrf:G04 .

imdrf:G04037 a owl:Class ;
    rdfs:label "Cover" ;
    rdfs:comment "An object designed to conceal, enclose, or protect something." ;
    rdfs:subClassOf imdrf:G04 .

imdrf:G04038 a owl:Class ;
    rdfs:label "Cuff" ;
    rdfs:comment "A bandlike structure that encircles a body part or another component or device." ;
    rdfs:subClassOf imdrf:G04 .

imdrf:G04039 a owl:Class ;
    rdfs:label "Cup" ;
    rdfs:comment "Part or design of a device with a concave hemispherical shape." ;
    rdfs:subClassOf imdrf:G04 .

imdrf:G04040 a owl:Class ;
    rdfs:label "Cusp/Leaflet" ;
    ex:statusDescription "Minor editorial change to the term on 25 June 2020." ;
    rdfs:comment "A thin blade-like component, typically used as part of a one-way valve." ;
    rdfs:subClassOf imdrf:G04 .

imdrf:G04041 a owl:Class ;
    rdfs:label "Cutter/Blade" ;
    rdfs:comment "A component designed for slicing or cutting." ;
    rdfs:subClassOf imdrf:G04 .

imdrf:G04042 a owl:Class ;
    rdfs:label "Cylinder" ;
    rdfs:comment "A three-dimensional part with flat circular ends and long straight sides." ;
    rdfs:subClassOf imdrf:G04 .

imdrf:G04043 a owl:Class ;
    rdfs:label "Device Collapser" ;
    rdfs:comment "A component designed to fold or collapse something." ;
    rdfs:subClassOf imdrf:G04 .

imdrf:G04044 a owl:Class ;
    rdfs:label "Device Deployer" ;
    rdfs:comment "A component designed to install something or distribute something in a systematic way." ;
    rdfs:subClassOf imdrf:G04 .

imdrf:G04045 a owl:Class ;
    rdfs:label "Diaphragm" ;
    rdfs:comment "A component consisting of a flexible sheet or partition." ;
    rdfs:subClassOf imdrf:G04 .

imdrf:G04046 a owl:Class ;
    rdfs:label "Dome" ;
    rdfs:comment "Part or design of a device with a convex hemispherical shape." ;
    rdfs:subClassOf imdrf:G04 .

imdrf:G04047 a owl:Class ;
    rdfs:label "Ejector" ;
    rdfs:comment "A mechanism that pushes a device or component out." ;
    rdfs:subClassOf imdrf:G04 .

imdrf:G04048 a owl:Class ;
    rdfs:label "Equipment Pole" ;
    rdfs:comment "A structural component designed to hang medical equipment." ;
    rdfs:subClassOf imdrf:G04 .

imdrf:G04049 a owl:Class ;
    rdfs:label "Extender" ;
    rdfs:comment "A component designed to lengthen a structure." ;
    rdfs:subClassOf imdrf:G04 .

imdrf:G04050 a owl:Class ;
    rdfs:label "Fabric" ;
    rdfs:comment "Cloth produced from textile fibers." ;
    rdfs:subClassOf imdrf:G04 .

imdrf:G04051 a owl:Class ;
    rdfs:label "Fan/Blower" ;
    rdfs:comment "A component designed to create an air current through the rotation of a planar surface." ;
    rdfs:subClassOf imdrf:G04 .

imdrf:G0405201 a owl:Class ;
    rdfs:label "Adhesive" ;
    rdfs:comment "Any substance that affixes 2 or more surfaces together. This may be supplied separately, or attached to another item such as tape." ;
    rdfs:subClassOf imdrf:G04052 .

imdrf:G0405202 a owl:Class ;
    rdfs:label "Bolt" ;
    ex:statusDescription "Editorial change to the definition on 16 February 2021." ;
    rdfs:comment "A cylindrical connector element which may have a thread/nut connection to form a fastener." ;
    rdfs:subClassOf imdrf:G04052 .

imdrf:G0405203 a owl:Class ;
    rdfs:label "Clamp" ;
    rdfs:comment "A component designed to mechanically hold items firmly together." ;
    rdfs:subClassOf imdrf:G04052 .

imdrf:G0405204 a owl:Class ;
    rdfs:label "Clip" ;
    rdfs:comment "A small component designed to hold and attach items together." ;
    rdfs:subClassOf imdrf:G04052 .

imdrf:G0405205 a owl:Class ;
    rdfs:label "Fixation Wire" ;
    rdfs:comment "A metal strand designed for structural or other purpose." ;
    rdfs:subClassOf imdrf:G04052 .

imdrf:G0405206 a owl:Class ;
    rdfs:label "Latch" ;
    rdfs:comment "A fastening component for a mobile part usually consisting of a bar that is retained in a slot." ;
    rdfs:subClassOf imdrf:G04052 .

imdrf:G0405207 a owl:Class ;
    rdfs:label "Nail" ;
    rdfs:comment "A pin-shaped fastener with a sharp point at one end and usually flat on the other end." ;
    rdfs:subClassOf imdrf:G04052 .

imdrf:G0405208 a owl:Class ;
    rdfs:label "Nut" ;
    rdfs:comment "A threaded fastener designed to engage a bolt." ;
    rdfs:subClassOf imdrf:G04052 .

imdrf:G0405209 a owl:Class ;
    rdfs:label "Pin" ;
    rdfs:comment "A small, slender separate component which is designed to secure another object." ;
    rdfs:subClassOf imdrf:G04052 .

imdrf:G0405210 a owl:Class ;
    rdfs:label "Prong" ;
    rdfs:comment "A projecting pointed part of a device, usually one designed to attach a device to something else." ;
    rdfs:subClassOf imdrf:G04052 .

imdrf:G0405211 a owl:Class ;
    rdfs:label "Retainer" ;
    rdfs:comment "A physical component designed to hold items in place." ;
    rdfs:subClassOf imdrf:G04052 .

imdrf:G0405212 a owl:Class ;
    rdfs:label "Rivet" ;
    rdfs:comment "A fastening component resembling a heavy pin, having a head on one end and designed to have the other end flattened after passing through the parts to be connected." ;
    rdfs:subClassOf imdrf:G04052 .

imdrf:G0405213 a owl:Class ;
    rdfs:label "Screw" ;
    rdfs:comment "A fastening component with a tapered threaded shaft and a head designed to engage with a driving tool." ;
    rdfs:subClassOf imdrf:G04052 .

imdrf:G0405214 a owl:Class ;
    rdfs:label "Staple" ;
    rdfs:comment "A fastening component consisting of a bent wire designed to pierce and hold two or more surfaces together." ;
    rdfs:subClassOf imdrf:G04052 .

imdrf:G0405215 a owl:Class ;
    rdfs:label "Suture Thread" ;
    rdfs:comment "A monofilament or multifilament material used surgically to close a wound, join tissues, or fasten components of a device (e.g. fabric to wire stent frame)." ;
    rdfs:subClassOf imdrf:G04052 .

imdrf:G0405216 a owl:Class ;
    rdfs:label "Tape for Fixation" ;
    rdfs:comment "A long, thin, flat, flexible material often used for binding or fastening." ;
    rdfs:subClassOf imdrf:G04052 .

imdrf:G04053 a owl:Class ;
    rdfs:label "Fiber" ;
    rdfs:comment "Any component made from a long, slender material." ;
    rdfs:subClassOf imdrf:G04 .

imdrf:G04054 a owl:Class ;
    rdfs:label "Filter" ;
    rdfs:comment "A component designed to remove something from whatever passes through it." ;
    rdfs:subClassOf imdrf:G04 .

imdrf:G04055 a owl:Class ;
    rdfs:label "Flange" ;
    rdfs:comment "A protruding edge designed to strengthen or stabilize a device or facilitate its attachment to a surface." ;
    rdfs:subClassOf imdrf:G04 .

imdrf:G04056 a owl:Class ;
    rdfs:label "Foil" ;
    rdfs:comment "A thin, flexible sheet of metal." ;
    rdfs:subClassOf imdrf:G04 .

imdrf:G04057 a owl:Class ;
    rdfs:label "Gas Exchanger" ;
    rdfs:comment "Component that is used to transfer gasses between two or more locations." ;
    rdfs:subClassOf imdrf:G04 .

imdrf:G04058 a owl:Class ;
    rdfs:label "Gasket" ;
    rdfs:comment "A preformed material designed to form a seal between connecting surfaces." ;
    rdfs:subClassOf imdrf:G04 .

imdrf:G04059 a owl:Class ;
    rdfs:label "Gears" ;
    rdfs:comment "A toothed wheel designed to mesh with another toothed object and transmit motion." ;
    rdfs:subClassOf imdrf:G04 .

imdrf:G04060 a owl:Class ;
    rdfs:label "Generator" ;
    rdfs:comment "A component designed to produce electricity, vapor or gas." ;
    rdfs:subClassOf imdrf:G04 .

imdrf:G04061 a owl:Class ;
    rdfs:label "Guide" ;
    rdfs:comment "A component designed to help direct the passage of another object." ;
    rdfs:subClassOf imdrf:G04 .

imdrf:G04062 a owl:Class ;
    rdfs:label "Guidewire" ;
    rdfs:comment "A flexible wire designed to help position medical devices within the body." ;
    rdfs:subClassOf imdrf:G04 .

imdrf:G04063 a owl:Class ;
    rdfs:label "Handpiece" ;
    rdfs:comment "A part of a device designed to be used while held in the hand." ;
    rdfs:subClassOf imdrf:G04 .

imdrf:G04064 a owl:Class ;
    rdfs:label "Header" ;
    rdfs:comment "The connection point between the leads and the generator." ;
    rdfs:subClassOf imdrf:G04 .

imdrf:G04065 a owl:Class ;
    rdfs:label "Sewing Ring" ;
    rdfs:comment "A ring of supportive material designed to provide a stable surface for attachment to surrounding tissues." ;
    rdfs:subClassOf imdrf:G04 .

imdrf:G04066 a owl:Class ;
    rdfs:label "Heat Exchanger" ;
    rdfs:comment "A component designed to transfer heat between fluids and/or gases across a barrier or to the environment." ;
    rdfs:subClassOf imdrf:G04 .

imdrf:G04067 a owl:Class ;
    rdfs:label "Hinge" ;
    rdfs:comment "A component designed to join two objects and allow them to swing relative to one another." ;
    rdfs:subClassOf imdrf:G04 .

imdrf:G04068 a owl:Class ;
    rdfs:label "Holder" ;
    rdfs:comment "A component designed to hold another object." ;
    rdfs:subClassOf imdrf:G04 .

imdrf:G04069 a owl:Class ;
    rdfs:label "Hose" ;
    rdfs:comment "A flexible tube designed to carry a fluid or gas." ;
    rdfs:subClassOf imdrf:G04 .

imdrf:G04070 a owl:Class ;
    rdfs:label "Housing" ;
    rdfs:comment "A rigid casing that encloses and protects a piece of equipment." ;
    rdfs:subClassOf imdrf:G04 .

imdrf:G04071 a owl:Class ;
    rdfs:label "Humidifier" ;
    rdfs:comment "A component used to increase moisture in a gas." ;
    rdfs:subClassOf imdrf:G04 .

imdrf:G04072 a owl:Class ;
    rdfs:label "Hydraulic System" ;
    rdfs:comment "A system designed to use fluid pressure to bring about movement." ;
    rdfs:subClassOf imdrf:G04 .

imdrf:G04073 a owl:Class ;
    rdfs:label "Impeller" ;
    rdfs:comment "The rotating component of a centrifugal pump, compressor, or other machine designed to move a fluid by rotation." ;
    rdfs:subClassOf imdrf:G04 .

imdrf:G04074 a owl:Class ;
    rdfs:label "Inserter" ;
    rdfs:comment "A component whose function is to facilitate the insertion of a particular device." ;
    rdfs:subClassOf imdrf:G04 .

imdrf:G04075 a owl:Class ;
    rdfs:label "Insulation" ;
    rdfs:comment "A material designed to reduce the transmission of heat, sound, or electricity." ;
    rdfs:subClassOf imdrf:G04 .

imdrf:G04076 a owl:Class ;
    rdfs:label "Isolator" ;
    rdfs:comment "Any material or structure designed to limit the interaction between two components." ;
    rdfs:subClassOf imdrf:G04 .

imdrf:G04077 a owl:Class ;
    rdfs:label "Jaw" ;
    rdfs:comment "A component designed to use opposing parts to close on and hold an object." ;
    rdfs:subClassOf imdrf:G04 .

imdrf:G04078 a owl:Class ;
    rdfs:label "Joint" ;
    rdfs:comment "A component designed as the junction between objects; it may be flexible or rigid." ;
    rdfs:subClassOf imdrf:G04 .

imdrf:G04079 a owl:Class ;
    rdfs:label "Knob" ;
    rdfs:comment "A rounded lump or ball used for adjusting or controlling." ;
    rdfs:subClassOf imdrf:G04 .

imdrf:G04080 a owl:Class ;
    rdfs:label "Label" ;
    rdfs:comment "Any written, printed, or graphic matter upon a device to identify its nature, ownership, or other characteristics of the device." ;
    rdfs:subClassOf imdrf:G04 .

imdrf:G04081 a owl:Class ;
    rdfs:label "Leaflet" ;
    ex:status "Retired" ;
    ex:statusDescription "Term was inactivated on 25 June 2020. Please use \"Cusp/Leaflet\" (G04040)." ;
    rdfs:comment "A device consisting of two thin blades hinged in the center; typically designed to control flow of fluids." ;
    rdfs:subClassOf imdrf:G04 .

imdrf:G0408201 a owl:Class ;
    rdfs:label "Foot Pedal" ;
    rdfs:comment "A lever designed to be operated with the foot." ;
    rdfs:subClassOf imdrf:G04082 .

imdrf:G04083 a owl:Class ;
    rdfs:label "Liner" ;
    rdfs:comment "A component placed the inside of the walls of a cavity or container for protection or insulation." ;
    rdfs:subClassOf imdrf:G04 .

imdrf:G04084 a owl:Class ;
    rdfs:label "Magazine/Cassette" ;
    rdfs:comment "A compartment in a device designed to house a consumable material for feeding into a mechanism." ;
    rdfs:subClassOf imdrf:G04 .

imdrf:G04085 a owl:Class ;
    rdfs:label "Manifold" ;
    rdfs:comment "A branched system of pipes or channels; typically to funnel the flow of liquids or gases." ;
    rdfs:subClassOf imdrf:G04 .

imdrf:G04086 a owl:Class ;
    rdfs:label "Mask" ;
    rdfs:comment "A flexible, form-shaped component designed to be placed over the nose and/or mouth." ;
    rdfs:subClassOf imdrf:G04 .

imdrf:G04087 a owl:Class ;
    rdfs:label "Mechanical Mixer" ;
    rdfs:comment "A mechanical component designed to blend materials." ;
    rdfs:subClassOf imdrf:G04 .

imdrf:G04088 a owl:Class ;
    rdfs:label "Membrane" ;
    rdfs:comment "A component that is made from or resembles a thin flexible sheet of material acting as a boundary or separating two chambers." ;
    rdfs:subClassOf imdrf:G04 .

imdrf:G04089 a owl:Class ;
    rdfs:label "Mesh" ;
    rdfs:comment "Component made of overlapping strands forming a fine net-like structure." ;
    rdfs:subClassOf imdrf:G04 .

imdrf:G04090 a owl:Class ;
    rdfs:label "Motor(s)" ;
    rdfs:comment "A machine that converts any form of energy to produce or impart motion (kinetic energy)." ;
    rdfs:subClassOf imdrf:G04 .

imdrf:G04091 a owl:Class ;
    rdfs:label "Mount" ;
    rdfs:comment "A structural component designed to facilitate the attachment of one object to another." ;
    rdfs:subClassOf imdrf:G04 .

imdrf:G04092 a owl:Class ;
    rdfs:label "Needle" ;
    rdfs:comment "A component with a long, slender, pointed shape." ;
    rdfs:subClassOf imdrf:G04 .

imdrf:G04093 a owl:Class ;
    rdfs:label "Nozzle" ;
    rdfs:comment "A component designed to regulate and direct the flow of a fluid or gas." ;
    rdfs:subClassOf imdrf:G04 .

imdrf:G04094 a owl:Class ;
    rdfs:label "Packaging" ;
    rdfs:comment "The outer wrapping around a device which serves to contain, identify, and protect it prior to use." ;
    rdfs:subClassOf imdrf:G04 .

imdrf:G04095 a owl:Class ;
    rdfs:label "Pad" ;
    ex:statusDescription "Editorial change to the definition on 16 February 2021." ;
    rdfs:comment "Typically a soft, cushion-like material used to prevent injury or damage to a person or device. Can also be made of an absorbent material to absorb liquid." ;
    rdfs:subClassOf imdrf:G04 .

imdrf:G04096 a owl:Class ;
    rdfs:label "Panel" ;
    rdfs:comment "A rigid sheet that forms a surface of a device or component." ;
    rdfs:subClassOf imdrf:G04 .

imdrf:G04097 a owl:Class ;
    rdfs:label "Plate" ;
    ex:statusDescription "Definition was modified on 31 January 2023 (Old definition: A thin, flat sheet or strip used to join, strengthen or to form parts of another structure). For details, see comment No. 148 of the Change Log (Release Number 2023)." ;
    rdfs:comment "A thin, flat sheet or strip used to join, strengthen or to form parts of another structure. For a flat, shallow container with a raised rim, use G03016 - Tray." ;
    rdfs:subClassOf imdrf:G04 .

imdrf:G04098 a owl:Class ;
    rdfs:label "Plug" ;
    rdfs:comment "A component designed to seat into an opening in a device or other object." ;
    rdfs:subClassOf imdrf:G04 .

imdrf:G04099 a owl:Class ;
    rdfs:label "Plunger" ;
    rdfs:comment "A component of a machine, tool or device that pushes or thrusts another object, liquid or gas." ;
    rdfs:subClassOf imdrf:G04 .

imdrf:G04100 a owl:Class ;
    rdfs:label "Post" ;
    rdfs:comment "An upright piece that is fixed firmly that supports, place or aligns other parts." ;
    rdfs:subClassOf imdrf:G04 .

imdrf:G04101 a owl:Class ;
    rdfs:label "Potting" ;
    rdfs:comment "The resin, glue or other substance used to seal other components together." ;
    rdfs:subClassOf imdrf:G04 .

imdrf:G04102 a owl:Class ;
    rdfs:label "Probe" ;
    rdfs:comment "A component designed to reach into a location for manipulating or for measuring." ;
    rdfs:subClassOf imdrf:G04 .

imdrf:G04103 a owl:Class ;
    rdfs:label "Processor" ;
    rdfs:comment "A component designed for preparing or treating a material. Should not be used for computer processors." ;
    rdfs:subClassOf imdrf:G04 .

imdrf:G04104 a owl:Class ;
    rdfs:label "Pulley" ;
    rdfs:comment "A component which changes the direction of a force (e.g. belt or chain)." ;
    rdfs:subClassOf imdrf:G04 .

imdrf:G04105 a owl:Class ;
    rdfs:label "Pump" ;
    rdfs:comment "A component designed to facilitate the movement of a fluid." ;
    rdfs:subClassOf imdrf:G04 .

imdrf:G04106 a owl:Class ;
    rdfs:label "Pusher" ;
    rdfs:comment "A component designed to advance something by pushing it." ;
    rdfs:subClassOf imdrf:G04 .

imdrf:G04107 a owl:Class ;
    rdfs:label "Rachet" ;
    rdfs:comment "A part that allows or forces another part's movement in a single direction." ;
    rdfs:subClassOf imdrf:G04 .

imdrf:G0410801 a owl:Class ;
    rdfs:label "Side Rail" ;
    rdfs:comment "A supportive or protective rail attached to the side of something." ;
    rdfs:subClassOf imdrf:G04108 .

imdrf:G04109 a owl:Class ;
    rdfs:label "Regulator" ;
    rdfs:comment "A component designed to control a process or condition." ;
    rdfs:subClassOf imdrf:G04 .

imdrf:G04110 a owl:Class ;
    rdfs:label "Reservoir" ;
    rdfs:comment "A vessel designed to store a fluid." ;
    rdfs:subClassOf imdrf:G04 .

imdrf:G04111 a owl:Class ;
    rdfs:label "Ring" ;
    rdfs:comment "A circular band-shaped component." ;
    rdfs:subClassOf imdrf:G04 .

imdrf:G04112 a owl:Class ;
    rdfs:label "Rod/Shaft" ;
    rdfs:comment "A long cylindrical bar used to transmit motion or connect other components." ;
    rdfs:subClassOf imdrf:G04 .

imdrf:G04113 a owl:Class ;
    rdfs:label "Seal" ;
    rdfs:comment "A component designed to prevent passage of material through a joint or opening." ;
    rdfs:subClassOf imdrf:G04 .

imdrf:G04114 a owl:Class ;
    rdfs:label "Shock Absorber" ;
    rdfs:comment "A mechanical component designed to dampen or attenuate a force." ;
    rdfs:subClassOf imdrf:G04 .

imdrf:G04115 a owl:Class ;
    rdfs:label "Sleeve" ;
    rdfs:comment "A cylindrical fitting that slides over another part of a device or other object." ;
    rdfs:subClassOf imdrf:G04 .

imdrf:G04116 a owl:Class ;
    rdfs:label "Slide" ;
    rdfs:comment "A flat rectangular piece of glass on which specimens can be mounted for microscopic study." ;
    rdfs:subClassOf imdrf:G04 .

imdrf:G04117 a owl:Class ;
    rdfs:label "Socket" ;
    rdfs:comment "A component designed as an opening into which something else fits." ;
    rdfs:subClassOf imdrf:G04 .

imdrf:G04118 a owl:Class ;
    rdfs:label "Spacer" ;
    rdfs:comment "A component designed to position objects further apart." ;
    rdfs:subClassOf imdrf:G04 .

imdrf:G04119 a owl:Class ;
    rdfs:label "Spring" ;
    rdfs:comment "An elastic component designed to bend under a load and then return to its shape when unloaded." ;
    rdfs:subClassOf imdrf:G04 .

imdrf:G04120 a owl:Class ;
    rdfs:label "Stand" ;
    rdfs:comment "A support component designed to hold an object." ;
    rdfs:subClassOf imdrf:G04 .

imdrf:G04121 a owl:Class ;
    rdfs:label "Steering Wire" ;
    rdfs:comment "A wire designed to enable a device to be maneuvered." ;
    rdfs:subClassOf imdrf:G04 .

imdrf:G04122 a owl:Class ;
    rdfs:label "Stent" ;
    rdfs:comment "Tubular support placed inside a blood vessel, canal, or duct to aid healing or relieve an obstruction." ;
    rdfs:subClassOf imdrf:G04 .

imdrf:G04123 a owl:Class ;
    rdfs:label "Stopcock" ;
    rdfs:comment "A rotating component designed to act like a tap for regulating the flow of a fluid, and to completely stop the flow when closed fully." ;
    rdfs:subClassOf imdrf:G04 .

imdrf:G04124 a owl:Class ;
    rdfs:label "Stopper" ;
    rdfs:comment "Component designed to close an opening." ;
    rdfs:subClassOf imdrf:G04 .

imdrf:G04125 a owl:Class ;
    rdfs:label "Strain Relief" ;
    rdfs:comment "A structure designed to function with a connector to prevent damage to a hose or cable from excess flexing." ;
    rdfs:subClassOf imdrf:G04 .

imdrf:G04126 a owl:Class ;
    rdfs:label "Stylet" ;
    rdfs:comment "A thin metal wire designed to be passed through a needle, catheter, or cannula to stiffen it or clear it of debris." ;
    rdfs:subClassOf imdrf:G04 .

imdrf:G04127 a owl:Class ;
    rdfs:label "Syringe" ;
    rdfs:comment "A component designed as a rigid cylinder with a plunger at one end and a delivery opening at the other." ;
    rdfs:subClassOf imdrf:G04 .

imdrf:G04128 a owl:Class ;
    rdfs:label "Table" ;
    rdfs:comment "A component having a smooth flat surface that is usually supported by one or more vertical legs." ;
    rdfs:subClassOf imdrf:G04 .

imdrf:G04129 a owl:Class ;
    rdfs:label "Tip" ;
    rdfs:comment "Pointed or rounded end of an object." ;
    rdfs:subClassOf imdrf:G04 .

imdrf:G04130 a owl:Class ;
    rdfs:label "Tool" ;
    ex:statusDescription "Editorial change to the definition on 16 February 2021." ;
    rdfs:comment "A component that is delivered with a device to support its assembly or operation, and is not part of the device. Use only in the case there are no other terms to describe the component." ;
    rdfs:subClassOf imdrf:G04 .

imdrf:G04131 a owl:Class ;
    rdfs:label "Translational Motion Component" ;
    rdfs:comment "A rotating part which is intended to transfer rotational movement or motion to another type of movement (e.g. excenters)." ;
    rdfs:subClassOf imdrf:G04 .

imdrf:G04132 a owl:Class ;
    rdfs:label "Trap" ;
    rdfs:comment "A component designed to capture or remove bubbles or fluid." ;
    rdfs:subClassOf imdrf:G04 .

imdrf:G04133 a owl:Class ;
    rdfs:label "Trocar" ;
    rdfs:comment "A sharp, pointed rod designed to pierce the wall of a body cavity to withdraw fluid or allow placement of a catheter or other device." ;
    rdfs:subClassOf imdrf:G04 .

imdrf:G0413401 a owl:Class ;
    rdfs:label "Capillary Tube" ;
    rdfs:comment "A narrow tube in which a liquid flows up against gravity." ;
    rdfs:subClassOf imdrf:G04134 .

imdrf:G0413501 a owl:Class ;
    rdfs:label "Control Valve" ;
    rdfs:comment "A valve designed to regulate the flow of a fluid or gas." ;
    rdfs:subClassOf imdrf:G04135 .

imdrf:G0413502 a owl:Class ;
    rdfs:label "Luer Valve" ;
    rdfs:comment "A valve that incorporates a Luer fitting." ;
    rdfs:subClassOf imdrf:G04135 .

imdrf:G0413503 a owl:Class ;
    rdfs:label "One-Way Valve" ;
    rdfs:comment "A valve designed to allow flow in only one direction." ;
    rdfs:subClassOf imdrf:G04135 .

imdrf:G04136 a owl:Class ;
    rdfs:label "Vaporiser" ;
    rdfs:comment "A component for gasifying liquids such as drugs." ;
    rdfs:subClassOf imdrf:G04 .

imdrf:G04137 a owl:Class ;
    rdfs:label "Vibrator" ;
    rdfs:comment "A mechanical component designed to create a vibratory motion." ;
    rdfs:subClassOf imdrf:G04 .

imdrf:G04138 a owl:Class ;
    rdfs:label "Washer" ;
    rdfs:comment "A flattened disk used as a mechanical seal between objects." ;
    rdfs:subClassOf imdrf:G04 .

imdrf:G04139 a owl:Class ;
    rdfs:label "Weld" ;
    rdfs:comment "Any joining connection that is the result of welding 2 or more parts." ;
    rdfs:subClassOf imdrf:G04 .

imdrf:G04140 a owl:Class ;
    rdfs:label "Wheel" ;
    rdfs:comment "A mechanical component consisting of a spoked, circular rim or solid disk designed to rotate on an axle or shaft." ;
    rdfs:subClassOf imdrf:G04 .

imdrf:G04141 a owl:Class ;
    rdfs:label "Window" ;
    rdfs:comment "A transparent panel in a device designed for visual inspection or to let light pass." ;
    rdfs:subClassOf imdrf:G04 .

imdrf:G04142 a owl:Class ;
    rdfs:label "Shutter" ;
    rdfs:comment "Aperture that controls or blocks light or radiation passing through." ;
    rdfs:subClassOf imdrf:G04 .

imdrf:G05001 a owl:Class ;
    rdfs:label "Camera" ;
    rdfs:comment "An apparatus for taking photographs, generally consisting of a lightproof enclosure having an aperture with a shuttered lens through which the image of an object is focused and recorded." ;
    rdfs:subClassOf imdrf:G05 .

imdrf:G05002 a owl:Class ;
    rdfs:label "Film" ;
    rdfs:comment "A photographic material designed to capture an image upon exposure to electromagnetic radiation." ;
    rdfs:subClassOf imdrf:G05 .

imdrf:G05003 a owl:Class ;
    rdfs:label "Imager" ;
    rdfs:comment "A component designed to create or record a visual representation." ;
    rdfs:subClassOf imdrf:G05 .

imdrf:G05004 a owl:Class ;
    rdfs:label "Laser" ;
    rdfs:comment "A component designed to emit a monochromatic beam of coherent light." ;
    rdfs:subClassOf imdrf:G05 .

imdrf:G05005 a owl:Class ;
    rdfs:label "LED (Light Emitting Diode)" ;
    rdfs:comment "A type of diode designed to emit light when a current passes through it." ;
    rdfs:subClassOf imdrf:G05 .

imdrf:G05006 a owl:Class ;
    rdfs:label "Lenses" ;
    rdfs:comment "An electric or optical component designed to focus (concentrate) or disperse electromagnetic radiation." ;
    rdfs:subClassOf imdrf:G05 .

imdrf:G0500701 a owl:Class ;
    rdfs:label "Bulb" ;
    rdfs:comment "A component designed to produce light or heat." ;
    rdfs:subClassOf imdrf:G05007 .

imdrf:G05008 a owl:Class ;
    rdfs:label "Mirror" ;
    rdfs:comment "A component consisting of a polished surface designed to reflect light." ;
    rdfs:subClassOf imdrf:G05 .

imdrf:G05009 a owl:Class ;
    rdfs:label "Optical Fiber" ;
    rdfs:comment "A component made with thin glass fibers as a conduit for transmission of light." ;
    rdfs:subClassOf imdrf:G05 .

imdrf:G0600101 a owl:Class ;
    rdfs:label "Alarm, Audible" ;
    rdfs:comment "A component designed to signal the occurrence of a particular event by making a sound." ;
    rdfs:subClassOf imdrf:G06001 .

imdrf:G0600102 a owl:Class ;
    rdfs:label "Alarm, Visual" ;
    ex:statusDescription "Editorial change to the definition on 16 February 2021." ;
    rdfs:comment "A component designed to signal the occurrence of a particular event in a way that can be seen." ;
    rdfs:subClassOf imdrf:G06001 .

imdrf:G06002 a owl:Class ;
    rdfs:label "Emergency Button Or Switch" ;
    rdfs:comment "A button and circuits designed to force the shutdown of a machine or device." ;
    rdfs:subClassOf imdrf:G06 .

imdrf:G06003 a owl:Class ;
    rdfs:label "Fail-Safe System" ;
    rdfs:comment "A component designed to prevent malfunction, unsafe, or unauthorized operation of a device or system." ;
    rdfs:subClassOf imdrf:G06 .

imdrf:G06004 a owl:Class ;
    rdfs:label "Locking Mechanism" ;
    rdfs:comment "A fastening component designed to hold, close, or secure." ;
    rdfs:subClassOf imdrf:G06 .

imdrf:G06005 a owl:Class ;
    rdfs:label "Protector/Shield" ;
    rdfs:comment "A component designed to prevent harm or protect against damage to other components." ;
    rdfs:subClassOf imdrf:G06 .

imdrf:G0600601 a owl:Class ;
    rdfs:label "Needle Stick Prevention Mechanism" ;
    ex:statusDescription "Editorial change to the definition on 16 February 2021." ;
    rdfs:comment "A mechanism integrated into a device to prevent needle stick injuries." ;
    rdfs:subClassOf imdrf:G06006 .

imdrf:G06007 a owl:Class ;
    rdfs:label "Safety Valve" ;
    rdfs:comment "A valve designed to automatically open in order to maintain the pressure in a system below a specified pressure." ;
    rdfs:subClassOf imdrf:G06 .

imdrf:G07001 a owl:Class ;
    rdfs:label "Part/Component/Sub-assembly Term not Applicable" ;
    rdfs:comment "The device does not have distinct parts, components, or sub-assemblies, or it would not be appropriate to link the reported incident to a single part, component, or sub-assembly. Use this term if the problem involves or affects the overall device rather than a specific component." ;
    rdfs:subClassOf imdrf:G07 .

imdrf:G07002 a owl:Class ;
    rdfs:label "Appropriate Component Term/Code Not Available" ;
    ex:status "Modified (editorial)" ;
    ex:statusDescription "Editorial change to term for Release Number 2025. See no. 112 of Change Log." ;
    rdfs:comment "The parts, components, or sub-assemblies are not adequately described by any other term. Note: this code must not be used unless there is no other feasible code. The preferred term should be documented when submitting an adverse event report. This information will be used to determine if a new term should be added to the code table." ;
    rdfs:subClassOf imdrf:G07 .

imdrf:G07003 a owl:Class ;
    rdfs:label "Insufficient Component Information" ;
    ex:status "Modified (editorial)" ;
    ex:statusDescription "Term was added on 27 January 2022. For details, see comment No. 192 of the Change Log (Release Number 2022). Editorial change to term for Release Number 2025. See no. 123 of Change Log." ;
    rdfs:comment "There is not yet enough information available to classify the medical device component." ;
    rdfs:subClassOf imdrf:G07 .

imdrf:A0207 a owl:Class ;
    rdfs:label "Device Damaged Prior to Receipt by User" ;
    ex:status "Modified (technical)" ;
    ex:statusDescription "Term and Definition modified for Release Number 2025. Previous term was \"Shipping Damage or Problem\". See no. 106 of Change Request Log." ;
    rdfs:comment "Problem associated with packaging or shipping damage prior to receipt by the user." ;
    rdfs:subClassOf imdrf:A02 .

imdrf:A0410 a owl:Class ;
    rdfs:label "Material Perforation" ;
    rdfs:comment "Material constituting device is perforated possibly compromising the device's intended purpose." ;
    rdfs:subClassOf imdrf:A04 .

imdrf:A0509 a owl:Class ;
    rdfs:label "Physical Resistance/Sticking" ;
    rdfs:comment "Problem associated with the lack of movement in the device due parts sticking or seizing." ;
    rdfs:subClassOf imdrf:A05 .

imdrf:A0718 a owl:Class ;
    rdfs:label "Failure to Shut Off" ;
    rdfs:comment "Problem associated with the device not powering off when a shut down was requested." ;
    rdfs:subClassOf imdrf:A07 .

imdrf:A1905 a owl:Class ;
    rdfs:label "Moisture or Humidity Problem" ;
    rdfs:comment "Problem associated with an unsatisfactory humidity level in the storage or use environment which affects the device performance." ;
    rdfs:subClassOf imdrf:A19 .

imdrf:A1906 a owl:Class ;
    rdfs:label "Ventilation Problem in Device Environment" ;
    rdfs:comment "Problem associated with the circulation of fresh air in the immediate atmosphere in which the device is being used." ;
    rdfs:subClassOf imdrf:A19 .

imdrf:A20 a owl:Class ;
    rdfs:label "Installation-Related Problem" ;
    rdfs:comment "Problem associated with unsatisfactory installation, configuration, and/or setup of a specific device." .

imdrf:A25 a owl:Class ;
    rdfs:label "No Apparent Adverse Event" ;
    rdfs:comment "A report has been received but the description provided does not appear to relate to an adverse event. This code allows a report to be recorded for administration purposes, even if it doesn't meet the requirements for adverse event reporting." .

imdrf:C17 a owl:Class ;
    rdfs:label "Maintenance Problem Identified" ;
    rdfs:comment "A device malfunction or problem that occurs after production because the device was not properly maintained according to the instructions (e.g. maintenance may be performed by user facility, distributor, or service provider)." .

imdrf:D15 a owl:Class ;
    rdfs:label "Cause Not Established" ;
    rdfs:comment "The investigation findings do not lead to a clear conclusion about the cause of the reported adverse event." .

imdrf:E0102 a owl:Class ;
    rdfs:label "Brain Injury" ;
    ex:nonIMDRFCode "MedDRA:10060690:Traumatic brain injury" ;
    rdfs:comment "Damage to the brain." ;
    rdfs:subClassOf imdrf:E01,
        imdrf:E20 .

imdrf:E0113 a owl:Class ;
    rdfs:label "Dysphasia" ;
    ex:nonIMDRFCode "MedDRA:10013951:Dysphasia" ;
    rdfs:comment "Impairment of verbal communication skills, often resulting from brain damage." ;
    rdfs:subClassOf imdrf:E01 .

imdrf:E0123 a owl:Class ;
    rdfs:label "Nerve Damage" ;
    ex:nonIMDRFCode "MedDRA:10029177:Nerve damage" ;
    rdfs:comment "Injury to nervous tissue." ;
    rdfs:subClassOf imdrf:E01,
        imdrf:E20 .

imdrf:E0124 a owl:Class ;
    rdfs:label "Nervous System Injury" ;
    ex:nonIMDRFCode "MedDRA:10080898:Nervous system injury" ;
    rdfs:comment "Injury to the central or peripheral nervous system." ;
    rdfs:subClassOf imdrf:E01,
        imdrf:E20 .

imdrf:E0301 a owl:Class ;
    rdfs:label "Anemia" ;
    ex:nonIMDRFCode "MedDRA:10002272:Anemia" ;
    rdfs:comment "A reduction in the number of red blood cells, the amount of hemoglobin, and/or the volume of packed red blood cells." ;
    rdfs:subClassOf imdrf:E03 .

imdrf:E0511 a owl:Class ;
    rdfs:label "Perforation of Vessels" ;
    ex:nonIMDRFCode "MedDRA:10068149:Vessel perforation" ;
    rdfs:comment "Damage to a blood vessel resulting from a full thickness disruption in the integrity of the vessel wall." ;
    rdfs:subClassOf imdrf:E05,
        imdrf:E2114 .

imdrf:E0515 a owl:Class ;
    rdfs:label "Vascular Dissection" ;
    ex:nonIMDRFCode "MedDRA:10070693:Vascular dissection" ;
    rdfs:comment "Spontaneous or induced tear within the wall of a blood vessel." ;
    rdfs:subClassOf imdrf:E05 .

imdrf:E0711 a owl:Class ;
    rdfs:label "Chronic Obstructive Pulmonary Disease (COPD)" ;
    ex:nonIMDRFCode "MedDRA:10009033:Chronic obstructive pulmonary disease" ;
    rdfs:comment "A chronic and progressive lung disorder characterized by the loss of elasticity of the bronchial tree and the air sacs, destruction of the air sacs wall, thickening of the bronchial wall, and mucous accumulation in the bronchial tree. The pathologic changes result in the disruption of the air flow in the bronchial airways. Signs and symptoms include shortness of breath, wheezing, productive cough, and chest tightness. The two main types of chronic obstructive pulmonary disease are chronic obstructive bronchitis and emphysema." ;
    rdfs:subClassOf imdrf:E07 .

imdrf:E0733 a owl:Class ;
    rdfs:label "Pneumonia" ;
    ex:nonIMDRFCode "MedDRA:10035664:Pneumonia" ;
    rdfs:comment "An acute and/or chronic inflammation focally or diffusely affecting the lung parenchyma." ;
    rdfs:subClassOf imdrf:E07,
        imdrf:E19 .

imdrf:E0818 a owl:Class ;
    rdfs:label "Eye Infections" ;
    ex:nonIMDRFCode "MedDRA:10015929:Eye infection" ;
    rdfs:comment "An infection of any part of the eye, including the eyelid." ;
    rdfs:subClassOf imdrf:E08,
        imdrf:E19 .

imdrf:E0829 a owl:Class ;
    rdfs:label "Keratitis" ;
    ex:nonIMDRFCode "MedDRA:10023332:Keratitis" ;
    rdfs:comment "Inflammation of the cornea." ;
    rdfs:subClassOf imdrf:E08 .

imdrf:E1031 a owl:Class ;
    rdfs:label "Stomatitis" ;
    ex:nonIMDRFCode "MedDRA:10042128:Stomatitis" ;
    rdfs:comment "Inflammation of the oral mucosa." ;
    rdfs:subClassOf imdrf:E10 .

imdrf:E1205 a owl:Class ;
    rdfs:label "Hyperglycemia" ;
    ex:nonIMDRFCode "MedDRA:10020639:Hyperglycemia" ;
    rdfs:comment "Abnormally high level of glucose in the blood." ;
    rdfs:subClassOf imdrf:E12,
        imdrf:E22 .

imdrf:E1305 a owl:Class ;
    rdfs:label "Renal Impairment" ;
    ex:nonIMDRFCode "MedDRA:10062237:Renal impairment" ;
    ex:statusDescription "Editorial change to the definition on 16 February 2021." ;
    rdfs:comment "An acute or chronic condition where the kidneys are not functioning normally." ;
    rdfs:subClassOf imdrf:E13 .

imdrf:E1310 a owl:Class ;
    rdfs:label "Urinary Tract Infection" ;
    ex:nonIMDRFCode "MedDRA:10046571:Urinary tract infection" ;
    rdfs:comment "An inflammatory process affecting any part of the urinary tract, most commonly the bladder or the urethra." ;
    rdfs:subClassOf imdrf:E13,
        imdrf:E19 .

imdrf:E1413 a owl:Class ;
    rdfs:label "Sexual Dysfunction" ;
    ex:nonIMDRFCode "MedDRA:10040477:Sexual dysfunction" ;
    rdfs:comment "Difficulty, lack of desire, or pain associated with coitus." ;
    rdfs:subClassOf imdrf:E14 .

imdrf:E1602 a owl:Class ;
    rdfs:label "Arthritis" ;
    ex:nonIMDRFCode "MedDRA:10003246:Arthritis" ;
    rdfs:comment "An inflammatory process affecting a joint." ;
    rdfs:subClassOf imdrf:E16 .

imdrf:E1605 a owl:Class ;
    rdfs:label "Cramp(s) /Muscle Spasm(s)" ;
    ex:nonIMDRFCode "MedDRA:10011285:Cramp" ;
    rdfs:comment "A sustained, sudden and involuntary contraction of a muscle or group of muscles." ;
    rdfs:subClassOf imdrf:E16 .

imdrf:E1614 a owl:Class ;
    rdfs:label "Joint Dislocation" ;
    ex:nonIMDRFCode "MedDRA:10023204:Joint dislocation" ;
    rdfs:comment "An abnormal separation where two or more bones meet." ;
    rdfs:subClassOf imdrf:E16,
        imdrf:E20 .

imdrf:E1705 a owl:Class ;
    rdfs:label "Burning Sensation" ;
    ex:nonIMDRFCode "MedDRA:10006784:Burning sensation" ;
    rdfs:comment "A sensation of stinging or heat, not necessarily accompanied by redness or physical signs of irritation." ;
    rdfs:subClassOf imdrf:E17,
        imdrf:E23 .

imdrf:E1715 a owl:Class ;
    rdfs:label "Scar Tissue" ;
    ex:nonIMDRFCode "MedDRA:10039580:Scar" ;
    rdfs:comment "Formation of new tissue formed in the healing of a wound." ;
    rdfs:subClassOf imdrf:E17 .

imdrf:E1907 a owl:Class ;
    rdfs:label "Viral Infection" ;
    ex:nonIMDRFCode "MedDRA:10047461:Viral infection" ;
    rdfs:comment "Any disease caused by a virus." ;
    rdfs:subClassOf imdrf:E19 .

imdrf:E2002 a owl:Class ;
    rdfs:label "Bruise/Contusion" ;
    ex:nonIMDRFCode "MedDRA:10006502:Bruise" ;
    rdfs:comment "Injury of the soft tissues without breaking the skin that is characterized by blood leakage into the surrounding area." ;
    rdfs:subClassOf imdrf:E20 .

imdrf:E2008 a owl:Class ;
    rdfs:label "Foreign Body In Patient" ;
    ex:nonIMDRFCode "MedDRA:10070245:Foreign body" ;
    ex:status "Modified (technical)" ;
    ex:statusDescription "Definition modified for Release Number 2025. See no. 25 of Change Request Log" ;
    rdfs:comment "An occurrence involving any object including device and/or fragments of device being left unintentionally in the body. This includes devices left in the body as part of risk mitigation or surgical bailout procedures since their presence or location is not as originally intended." ;
    rdfs:subClassOf imdrf:E20,
        imdrf:E21 .

imdrf:E2014 a owl:Class ;
    rdfs:label "Tissue Breakdown" ;
    ex:nonIMDRFCode "MedDRA:10068521:Tissue breakdown associated with device" ;
    rdfs:comment "A process caused by injury or disease or aging and characterized by a partial/complete disruption of tissue. The disruption may be temporary or permanent and may be associated with either (1) impairment or (2) loss of function of the affected organ(s) or system(s)." ;
    rdfs:subClassOf imdrf:E20 .

imdrf:E2104 a owl:Class ;
    rdfs:label "Electric Shock" ;
    ex:nonIMDRFCode "MedDRA:10014357:Electric shock" ;
    rdfs:comment "A shock caused by a brief, unintentional exposure to an electric current from a device." ;
    rdfs:subClassOf imdrf:E20,
        imdrf:E21 .

imdrf:E2309 a owl:Class ;
    rdfs:label "Deposits" ;
    ex:nonIMDRFCode "MedDRA:10070692:Device deposit issue" ;
    rdfs:comment "Accumulation of extraneous inorganic matter in tissues or cavities." ;
    rdfs:subClassOf imdrf:E23 .

imdrf:E2312 a owl:Class ;
    rdfs:label "Fatigue" ;
    ex:nonIMDRFCode "MedDRA:10016256:Fatigue" ;
    rdfs:comment "A state of generalized weakness with a pronounced inability to summon sufficient energy to accomplish daily activities." ;
    rdfs:subClassOf imdrf:E23 .

imdrf:E2313 a owl:Class ;
    rdfs:label "Fibrosis" ;
    ex:nonIMDRFCode "MedDRA:10016642:Fibrosis" ;
    rdfs:comment "The formation of fibrous tissue." ;
    rdfs:subClassOf imdrf:E23 .

imdrf:E2315 a owl:Class ;
    rdfs:label "Fluid Discharge" ;
    ex:nonIMDRFCode "MedDRA:10080911:Fluid discharge" ;
    rdfs:comment "Flow or leakage of fluid other than blood, from an orifice, wound or tissue." ;
    rdfs:subClassOf imdrf:E23 .

imdrf:E2337 a owl:Class ;
    rdfs:label "Stenosis" ;
    ex:nonIMDRFCode "MedDRA:10076711:Stenosis" ;
    ex:statusDescription "Secondary category was added on 27 January 2022. For details, see comment No. 234 / 235 of the Change Log (Release Number 2022). Error in CodeHierarchy corrected for Release No. 2024" ;
    rdfs:comment "Narrowing or stricture of a vessel, duct or canal." ;
    rdfs:subClassOf imdrf:E05,
        imdrf:E23 .

imdrf:F02 a owl:Class ;
    rdfs:label "Death" ;
    rdfs:comment "The cessation of life." .

imdrf:F1004 a owl:Class ;
    rdfs:label "Underdose" ;
    rdfs:comment "Exposure to, or intake of, an insufficient amount of a substance." ;
    rdfs:subClassOf imdrf:F10 .

imdrf:F1005 a owl:Class ;
    rdfs:label "Overdose" ;
    rdfs:comment "Exposure to, or intake of, an excessive amount of a substance." ;
    rdfs:subClassOf imdrf:F10 .

imdrf:F26 a owl:Class ;
    rdfs:label "No Health Consequences or Impact" ;
    ex:statusDescription "Editorial change to the definition on 16 February 2021." ;
    rdfs:comment "No apparent harm occurred in relation to the adverse event." .

imdrf:G03001 a owl:Class ;
    rdfs:label "Analyzer" ;
    rdfs:comment "Any component designed to perform an analysis." ;
    rdfs:subClassOf imdrf:G03 .

imdrf:G04005 a owl:Class ;
    rdfs:label "Anchor" ;
    rdfs:comment "A component designed to fix the device or a portion of the device in place." ;
    rdfs:subClassOf imdrf:G04 .

imdrf:G04019 a owl:Class ;
    rdfs:label "Cannula" ;
    rdfs:comment "A rigid or semi-rigid tube inserted into the body." ;
    rdfs:subClassOf imdrf:G04 .

imdrf:G04023 a owl:Class ;
    rdfs:label "Catheter" ;
    rdfs:comment "A flexible tube inserted into the body designed to permit injection or withdrawal of fluids or to keep passage open." ;
    rdfs:subClassOf imdrf:G04 .

imdrf:G04030 a owl:Class ;
    rdfs:label "Coil" ;
    rdfs:comment "A structure consisting of something wrapped in a continuous series of loops." ;
    rdfs:subClassOf imdrf:G04 .

imdrf:G04034 a owl:Class ;
    rdfs:label "Connector/Coupler" ;
    rdfs:comment "A component designed to serve as a link between parts allowing easy disconnection and reconnection when necessary." ;
    rdfs:subClassOf imdrf:G04 .

imdrf:G04082 a owl:Class ;
    rdfs:label "Lever" ;
    rdfs:comment "A rigid bar that rotates around a fixed point." ;
    rdfs:subClassOf imdrf:G04 .

imdrf:G04108 a owl:Class ;
    rdfs:label "Rail" ;
    rdfs:comment "A bar designed for support, attachment, guidance, or protection from falling." ;
    rdfs:subClassOf imdrf:G04 .

imdrf:G04134 a owl:Class ;
    rdfs:label "Tube" ;
    rdfs:comment "A long hollow cylinder, either rigid or flexible, for holding or transporting liquids or gasses." ;
    rdfs:subClassOf imdrf:G04 .

imdrf:G05007 a owl:Class ;
    rdfs:label "Light Source" ;
    rdfs:comment "A component that produces visible light." ;
    rdfs:subClassOf imdrf:G05 .

imdrf:G06006 a owl:Class ;
    rdfs:label "Safety Interlock" ;
    rdfs:comment "A mechanical or electronic component designed to prevent undesired actions due to the changing state of a device, typically to prevent harm to an operator or damage to the device itself." ;
    rdfs:subClassOf imdrf:G06 .

imdrf:A0102 a owl:Class ;
    rdfs:label "Osseointegration Problem" ;
    rdfs:comment "Problem associated with interconnection between the bone tissue and the implanted device." ;
    rdfs:subClassOf imdrf:A01 .

imdrf:A0104 a owl:Class ;
    rdfs:label "Migration or Expulsion of Device" ;
    rdfs:comment "Problem with an implanted or invasive device moving within the body, or being completely expelled from the body." ;
    rdfs:subClassOf imdrf:A01 .

imdrf:A0201 a owl:Class ;
    rdfs:label "Product Quality Problem" ;
    rdfs:comment "Problem associated with an inherent device characteristic that is not satisfactory as specified or delivered." ;
    rdfs:subClassOf imdrf:A02 .

imdrf:A0503 a owl:Class ;
    rdfs:label "Ejection Problem" ;
    ex:statusDescription "Editorial change to the definition on 18 March 2020." ;
    rdfs:comment "Problems associated with the inability or unexpected ejection or discharge of the device from its physical location." ;
    rdfs:subClassOf imdrf:A05 .

imdrf:A0505 a owl:Class ;
    rdfs:label "Firing Problem" ;
    rdfs:comment "Problem associated with the device not discharging as intended." ;
    rdfs:subClassOf imdrf:A05 .

imdrf:A0703 a owl:Class ;
    rdfs:label "Arcing" ;
    rdfs:comment "Problem associated with electrical current flowing through a gap between two conductive surfaces, typically resulting in a visible flash of light." ;
    rdfs:subClassOf imdrf:A07 .

imdrf:A0711 a owl:Class ;
    rdfs:label "Interrogation Problem" ;
    rdfs:comment "Problems associated with the device's ability to respond to signals from a system designed to interrogate its status." ;
    rdfs:subClassOf imdrf:A07 .

imdrf:A0720 a owl:Class ;
    rdfs:label "Electromagnetic Compatibility Problem" ;
    rdfs:comment "Problem associated with the ability of a system to function in its electromagnetic environment without introducing intolerable disturbances to anything in its environment." ;
    rdfs:subClassOf imdrf:A07 .

imdrf:A0903 a owl:Class ;
    rdfs:label "Tactile Prompts/Feedback" ;
    rdfs:comment "Problem with any deviation from the documented specifications of the device that relate to tactile feedback. e.g device vibrational prompt." ;
    rdfs:subClassOf imdrf:A09 .

imdrf:A1104 a owl:Class ;
    rdfs:label "Computer Operating System Problem" ;
    rdfs:comment "Problem associated with software, firmware, and/or hardware elements that control the execution of computer programs and provides such services as computer resource allocation, job control, input/output control, and file management in a computer system." ;
    rdfs:subClassOf imdrf:A11 .

imdrf:A1105 a owl:Class ;
    rdfs:label "Computer System Security Problem" ;
    rdfs:comment "Problem associated with unauthorized access to or modification of a software system resulting in a loss of confidentiality, integrity, or availability of written program code, application software, or data or entire device." ;
    rdfs:subClassOf imdrf:A11 .

imdrf:A1106 a owl:Class ;
    rdfs:label "Data Back-Up Problem" ;
    rdfs:comment "Problems relating to a system, component, file, procedure, or person available to replace or help restore a primary item in the event of a failure or externally caused disaster." ;
    rdfs:subClassOf imdrf:A11 .

imdrf:A1107 a owl:Class ;
    rdfs:label "Data Problem" ;
    rdfs:comment "Event in which data (charting, orders, results) is not correctly stored, transferred, updated, or displayed." ;
    rdfs:subClassOf imdrf:A11 .

imdrf:A1401 a owl:Class ;
    rdfs:label "Deflation Problem" ;
    ex:statusDescription "Technical change to the definition on 18 March 2020 to accommodate additional level 3 terms." ;
    rdfs:comment "Problem associated with the deflation of the device including unintended deflation or inadequate deflation." ;
    rdfs:subClassOf imdrf:A14 .

imdrf:A1404 a owl:Class ;
    rdfs:label "Filtration Problem" ;
    rdfs:comment "Problem associated with the process of passing a substance through a porous medium, e.g., a blood clot filter for the removal of suspended matter." ;
    rdfs:subClassOf imdrf:A14 .

imdrf:A1409 a owl:Class ;
    rdfs:label "Obstruction of Flow" ;
    ex:statusDescription "Technical change to the definition on 18 March 2020 to clarify that the term includes problems related to blood clotting." ;
    rdfs:comment "Problem related to an obstruction or blockage within the device component (e.g. tube, opening, pipe) that results in restriction of flow (including blood clotting)." ;
    rdfs:subClassOf imdrf:A14 .

imdrf:A1414 a owl:Class ;
    rdfs:label "Priming Problem" ;
    rdfs:comment "Problem associated with the preparation of the device to begin pumping." ;
    rdfs:subClassOf imdrf:A14 .

imdrf:A1602 a owl:Class ;
    rdfs:label "Fail-Safe Problem" ;
    rdfs:comment "Problem associated with the feature that prevents the unsafe use of the device." ;
    rdfs:subClassOf imdrf:A16 .

imdrf:A1606 a owl:Class ;
    rdfs:label "Premature Indicator Activation" ;
    rdfs:comment "Problems with the activation of a protective measure indicator earlier than expected." ;
    rdfs:subClassOf imdrf:A16 .

imdrf:A1701 a owl:Class ;
    rdfs:label "Component or Accessory Incompatibility" ;
    rdfs:comment "Problem associated with the incompatibility of any device while being operated in the same use environment thereby leading to a dysfunction between the devices." ;
    rdfs:subClassOf imdrf:A17 .

imdrf:A2305 a owl:Class ;
    rdfs:label "Misassembled" ;
    rdfs:comment "Problem associated with incorrect assembly of the device or constituents after being put into use." ;
    rdfs:subClassOf imdrf:A23 .

imdrf:C0102 a owl:Class ;
    rdfs:label "Biological Contamination" ;
    rdfs:comment "The undesirable presence of living organisms such as bacteria, fungi, or viruses or their products (enzymes or toxins)." ;
    rdfs:subClassOf imdrf:C01 .

imdrf:C0105 a owl:Class ;
    rdfs:label "Genotoxicity Problem Identified" ;
    rdfs:comment "The device's ability to cause damage to genetic material (e.g. leading to malignant tumors). (See ISO 10993)" ;
    rdfs:subClassOf imdrf:C01 .

imdrf:C08 a owl:Class ;
    rdfs:label "Optical Problem Identified" ;
    rdfs:comment "Problems related to the optical properties of a device." .

imdrf:C18 a owl:Class ;
    rdfs:label "Transport/Storage Problem Identified" ;
    rdfs:comment "Problems was caused by transport or storage conditions." .

imdrf:C23 a owl:Class ;
    rdfs:label "Usage Problem Identified" ;
    ex:statusDescription "Term was added on 21 January 2021 for coding device usage problems. For details, refer to comment No. 32 of the Change Log." ;
    rdfs:comment "Problems that occurred related to the actions of a healthcare professional, patient, or other device user." .

imdrf:D03 a owl:Class ;
    rdfs:label "Cause Traced to Manufacturing" ;
    rdfs:comment "A defect in the processes or systems used in the manufacture of the device. Examples include problems within the change control, production, or quality control processes." .

imdrf:D14 a owl:Class ;
    rdfs:label "No Problem Detected" ;
    ex:statusDescription "Definition modified for Release Number 2024. See no. 53 of Change Log" ;
    rdfs:comment "Either it was not confirmed that there was a problem with the device, or it was confirmed that there was no problem with the device." .

imdrf:E0107 a owl:Class ;
    rdfs:label "Cognitive Changes" ;
    ex:nonIMDRFCode "MedDRA:10057668:Cognitive disorder" ;
    rdfs:comment "Changes in perception, thinking, or remembering." ;
    rdfs:subClassOf imdrf:E01 .

imdrf:E0133 a owl:Class ;
    rdfs:label "Stroke/CVA" ;
    ex:nonIMDRFCode "MedDRA:10042244:Stroke" ;
    rdfs:comment "A sudden loss of neurological function secondary to hemorrhage or ischemia in the brain parenchyma due to a vascular event." ;
    rdfs:subClassOf imdrf:E01 .

imdrf:E0135 a owl:Class ;
    rdfs:label "Taste Disorder" ;
    ex:nonIMDRFCode "MedDRA:10082490:Taste disorder" ;
    ex:statusDescription "Editorial change to the definition on 16 February 2021." ;
    rdfs:comment "Conditions characterized by an alteration in taste function or perception" ;
    rdfs:subClassOf imdrf:E01 .

imdrf:E0143 a owl:Class ;
    rdfs:label "Altered State of Consciousness" ;
    ex:nonIMDRFCode "MedDRA:10001854:Altered state of consciousness" ;
    ex:statusDescription "Term was added on 27 January 2022. For details, see comment No. 77 of the Change Log (Release Number 2022)." ;
    rdfs:comment "A level of awareness and arousal other than normal." ;
    rdfs:subClassOf imdrf:E01 .

imdrf:E0302 a owl:Class ;
    rdfs:label "Coagulation Disorder" ;
    ex:nonIMDRFCode "MedDRA:10009731:Coagulation disorder" ;
    rdfs:comment "A condition in which there is a deviation from or interruption of the normal coagulation properties of the blood." ;
    rdfs:subClassOf imdrf:E03 .

imdrf:E0501 a owl:Class ;
    rdfs:label "Aneurysm" ;
    ex:nonIMDRFCode "MedDRA:10002329:Aneurysm" ;
    rdfs:comment "Bulging or ballooning in an area of an artery secondary to arterial wall weakening." ;
    rdfs:subClassOf imdrf:E05 .

imdrf:E0506 a owl:Class ;
    rdfs:label "Hemorrhage/Blood Loss/Bleeding" ;
    ex:nonIMDRFCode "MedDRA:10019524:Hemorrhage" ;
    ex:statusDescription "Term and definition was modified on 27 January 2022 (Old term/definition: Hemorrhage/Bleeding: The loss of blood from a ruptured blood vessel.). For details, see comment No. 87 / 199 of the Change Log (Release Number 2022)." ;
    rdfs:comment "The loss of blood from the circulation, including blood loss from a device connected to a patient." ;
    rdfs:subClassOf imdrf:E05 .

imdrf:E0612 a owl:Class ;
    rdfs:label "Ischemic Heart Disease" ;
    ex:nonIMDRFCode "MedDRA:10055218:Ischemic heart disease" ;
    rdfs:comment "A disorder of cardiac function caused by insufficient blood flow to the muscle tissue of the heart. The decreased blood flow may be due to narrowing of the coronary arteries, to obstruction by a thrombus, or less commonly, to diffuse narrowing of arterioles and other small vessels within the heart. Severe interruption of the blood supply to the myocardial tissue may result in necrosis of cardiac muscle (myocardial infarction)." ;
    rdfs:subClassOf imdrf:E06 .

imdrf:E0807 a owl:Class ;
    rdfs:label "Corneal Edema" ;
    ex:nonIMDRFCode "MedDRA:10011007:Corneal edema" ;
    rdfs:comment "Hazy, swollen cornea." ;
    rdfs:subClassOf imdrf:E08,
        imdrf:E2338 .

imdrf:E0903 a owl:Class ;
    rdfs:label "Hearing Impairment" ;
    ex:nonIMDRFCode "MedDRA:10019245:Hearing impaired" ;
    rdfs:comment "Partial or complete loss of the ability to detect or understand sounds resulting from damage to the outer, middle, or inner ear structures." ;
    rdfs:subClassOf imdrf:E09 .

imdrf:E0908 a owl:Class ;
    rdfs:label "Ear infection" ;
    ex:nonIMDRFCode "MedDRA:10014011:Ear infection" ;
    ex:statusDescription "Term was added on 27 January 2022. For details, see comment No. 223 of the Change Log (Release Number 2022)." ;
    rdfs:comment "Infection of the ear." ;
    rdfs:subClassOf imdrf:E09,
        imdrf:E19 .

imdrf:E1028 a owl:Class ;
    rdfs:label "Salivary Gland Problem" ;
    ex:nonIMDRFCode "MedDRA:10061935:Salivary gland disorder" ;
    rdfs:comment "A non-neoplastic or neoplastic (benign or malignant) disorder involving a salivary gland." ;
    rdfs:subClassOf imdrf:E10 .

imdrf:E1407 a owl:Class ;
    rdfs:label "Genital Bleeding" ;
    ex:nonIMDRFCode "MedDRA:10071812:Genital bleeding" ;
    rdfs:comment "Abnormal bleeding from the genitalia." ;
    rdfs:subClassOf imdrf:E14 .

imdrf:E1512 a owl:Class ;
    rdfs:label "Neonatal Hearing Impairment" ;
    ex:nonIMDRFCode "MedDRA:10080921:Neonatal hearing impairment" ;
    rdfs:comment "An abnormality that affects hearing within the first month after birth." ;
    rdfs:subClassOf imdrf:E09,
        imdrf:E15 .

imdrf:E1612 a owl:Class ;
    rdfs:label "Inadequate Osseointegration" ;
    ex:nonIMDRFCode "MedDRA:10068157:Inadequate osteointegration" ;
    rdfs:comment "Insufficient structural and functional connection between living bone and the surface of a synthetic implant." ;
    rdfs:subClassOf imdrf:E16 .

imdrf:E2006 a owl:Class ;
    rdfs:label "Erosion" ;
    ex:nonIMDRFCode "MedDRA:10068527:Tissue erosion associated with device" ;
    rdfs:comment "An eating away or breakdown of any type of external or internal human tissue including but not limited to skin, teeth, mucosa, or somatic, which involves only the outer tissue layer. When tissue surrounds an implanted device, the tissue breakdown may result in migration and loss of the implant material and may result in further complications such as infection or abscess." ;
    rdfs:subClassOf imdrf:E20 .

imdrf:E2324 a owl:Class ;
    rdfs:label "Incontinence" ;
    ex:nonIMDRFCode "MedDRA:10021639:Incontinence" ;
    rdfs:comment "Involuntary passage of feces and/or urine from the body." ;
    rdfs:subClassOf imdrf:E23 .

imdrf:F08 a owl:Class ;
    rdfs:label "Hospitalization or Prolonged Hospitalization" ;
    rdfs:comment "Hospitalization or prolonged hospitalization due to the health damage accompanying the use of device." .

imdrf:G02004 a owl:Class ;
    rdfs:label "Cable, Electrical" ;
    rdfs:comment "A long, thin, multistranded electrical wire designed to carry signals or power over a distance." ;
    rdfs:subClassOf imdrf:G02 .

imdrf:G02014 a owl:Class ;
    rdfs:label "Display" ;
    rdfs:comment "A component designed to present information visually. In the case of Touchscreen, use G0204004." ;
    rdfs:subClassOf imdrf:G02 .

imdrf:G02025 a owl:Class ;
    rdfs:label "Patient Lead" ;
    rdfs:comment "An insulated electrical cable designed to connect to an electrical device to a patient." ;
    rdfs:subClassOf imdrf:G02 .

imdrf:G02034 a owl:Class ;
    rdfs:label "Switch/Relay" ;
    rdfs:comment "A mechanical or electronic component designed to break or change the connections in a circuit (e.g. button)." ;
    rdfs:subClassOf imdrf:G02 .

imdrf:G06001 a owl:Class ;
    rdfs:label "Alarm" ;
    rdfs:comment "A component designed to signal the occurrence of a particular event." ;
    rdfs:subClassOf imdrf:G06 .

imdrf:A0101 a owl:Class ;
    rdfs:label "Patient-Device Incompatibility" ;
    rdfs:comment "Problem associated with the interaction between the patient's physiology or anatomy and the device that affects the patient and/or the device." ;
    rdfs:subClassOf imdrf:A01 .

imdrf:A0206 a owl:Class ;
    rdfs:label "Device Misassembled During Manufacturing /Shipping" ;
    rdfs:comment "A device found incorrectly assembled when delivered to the user facility." ;
    rdfs:subClassOf imdrf:A02 .

imdrf:A03 a owl:Class ;
    rdfs:label "Chemical Problem" ;
    rdfs:comment "Problem associated with any from the documented specifications of the device that relate to any chemical characterization, i.e., element, compound, or mixture." .

imdrf:A0706 a owl:Class ;
    rdfs:label "Charging Problem" ;
    rdfs:comment "Problem associated with the inability of the device to successfully charge an electrical source." ;
    rdfs:subClassOf imdrf:A07 .

imdrf:A0713 a owl:Class ;
    rdfs:label "Defibrillation/Stimulation Problem" ;
    ex:statusDescription "Technical change to the term and definition on 18 March 2020 to include stimulation and to differentiate this term with \"Unintended Electrical Shock\" (A0714)." ;
    rdfs:comment "Problem associated with the delivery of electrical shock/stimulation by a device intended to deliver shocks/stimulation." ;
    rdfs:subClassOf imdrf:A07 .

imdrf:A0721 a owl:Class ;
    rdfs:label "Circuit Failure" ;
    rdfs:comment "Problem associated with a failure of the internal network paths or electrical circuitry (i.e. electrical components, circuit boards, wiring)" ;
    rdfs:subClassOf imdrf:A07 .

imdrf:A0722 a owl:Class ;
    rdfs:label "Impedance Problem" ;
    rdfs:comment "Problem associated with electrical impedance levels between device and patient connections." ;
    rdfs:subClassOf imdrf:A07 .

imdrf:A0901 a owl:Class ;
    rdfs:label "Audible Prompt/Feedback Problem" ;
    ex:statusDescription "Editorial change to the term on 18 March 2020." ;
    rdfs:comment "Problem with any deviation from the documented specifications of the device that relate to audible feedback. e.g. voice prompts or beeps, but not safety related alarms which are covered under \"Protective Measures Problem\"." ;
    rdfs:subClassOf imdrf:A09 .

imdrf:A1103 a owl:Class ;
    rdfs:label "Program or Algorithm Execution Problem" ;
    rdfs:comment "Problem associated with execution problems relating to program or algorithm." ;
    rdfs:subClassOf imdrf:A11 .

imdrf:A1408 a owl:Class ;
    rdfs:label "No Flow" ;
    rdfs:comment "Problem arising from the device failing to deliver the specified liquid or gas." ;
    rdfs:subClassOf imdrf:A14 .

imdrf:A1411 a owl:Class ;
    rdfs:label "Pressure Problem" ;
    rdfs:comment "Problem associated with the application of a force either internal or external to device that compromises the flow of fluid or gas." ;
    rdfs:subClassOf imdrf:A14 .

imdrf:A1413 a owl:Class ;
    rdfs:label "Suction Problem" ;
    rdfs:comment "Problem associated with suction equipment, which may be a manual, electrical, vacuum or pressure source operated to evacuate and remove undesired substances (air, gas, fluid, or particulates) via tubing and collection bag." ;
    rdfs:subClassOf imdrf:A14 .

imdrf:A15 a owl:Class ;
    rdfs:label "Activation, Positioning or Separation Problem" ;
    ex:status "Modified (technical)" ;
    ex:statusDescription "Editorial change to the term on 16 Feburary 2021. Definition modified for Release Number 2025. See no. 43 of Change Request Log" ;
    rdfs:comment "Problem associated with any deviations from the intended performance of the device that relate to the sequence of events for activation, positioning or separation of device. Note: Deployment is synonymous with activation." .

imdrf:A1503 a owl:Class ;
    rdfs:label "Separation Problem" ;
    rdfs:comment "Problem associated with the detachment or separation of the device." ;
    rdfs:subClassOf imdrf:A15 .

imdrf:A1605 a owl:Class ;
    rdfs:label "Reset Problem" ;
    rdfs:comment "Problem associated with setting a variable, register, or other storage location back to a prescribed state." ;
    rdfs:subClassOf imdrf:A16 .

imdrf:A1910 a owl:Class ;
    rdfs:label "Electrical Power Problem" ;
    rdfs:comment "Problem associated with the quality of the facility-supplied power." ;
    rdfs:subClassOf imdrf:A19 .

imdrf:C0207 a owl:Class ;
    rdfs:label "Power Source Problem Identified" ;
    rdfs:comment "Problems related to the source that provides electrical power to the device." ;
    rdfs:subClassOf imdrf:C02 .

imdrf:C0401 a owl:Class ;
    rdfs:label "Communications Problem Identified" ;
    rdfs:comment "Devices that do not send or receive adequate signals (this speaks to the interoperability between devices)." ;
    rdfs:subClassOf imdrf:C04 .

imdrf:C05 a owl:Class ;
    rdfs:label "Labeling and Instructions for Use/Maintenance" ;
    rdfs:comment "Insufficient, inadequate, or incorrect information provided on a device's label or documentation regarding e.g. its intended use, directions for use, and characteristics of the device, including its maintenance." .

imdrf:C0602 a owl:Class ;
    rdfs:label "Inappropriate Material" ;
    rdfs:comment "Problems that occur due to the presence of a material that should not be present or part of the device." ;
    rdfs:subClassOf imdrf:C06 .

imdrf:C1301 a owl:Class ;
    rdfs:label "Device Incorrectly Reprocessed" ;
    rdfs:comment "Problems associated with the failure to properly and adequately reprocess the device." ;
    rdfs:subClassOf imdrf:C13 .

imdrf:D10 a owl:Class ;
    rdfs:label "Cause Traced to Non-Device Related Factors" ;
    ex:statusDescription "The term and definition were modified on 21 January 2021. (Old term/definition: Cause Cannot be Traced to Device/The adverse event that occurred is not attributable to a device.). For details, refer to comment No. 28 of the Change Log." ;
    rdfs:comment "The adverse event that occurred is confirmed to have been caused by something other than the device or usage." .

imdrf:E0119 a owl:Class ;
    rdfs:label "Loss of consciousness" ;
    ex:nonIMDRFCode "MedDRA:10024855:Loss of consciousness" ;
    rdfs:comment "A level of awareness that can be described as consistently not responsive to stimuli." ;
    rdfs:subClassOf imdrf:E01 .

imdrf:E0134 a owl:Class ;
    rdfs:label "Tactile Disorders" ;
    ex:nonIMDRFCode "MedDRA:10062872:Dysesthesia" ;
    rdfs:comment "conditions characterized by an alteration in the ability to or perception of touch." ;
    rdfs:subClassOf imdrf:E01 .

imdrf:E0402 a owl:Class ;
    rdfs:label "Hypersensitivity/Allergic reaction" ;
    ex:nonIMDRFCode "MedDRA:10020751:Hypersensitivity" ;
    rdfs:comment "A local or general reaction of an organism following contact with a specific allergen to which it has been previously exposed and to which it has become sensitized." ;
    rdfs:subClassOf imdrf:E04 .

imdrf:E0839 a owl:Class ;
    rdfs:label "Visual Impairment" ;
    ex:nonIMDRFCode "MedDRA:10047571:Visual impairment" ;
    rdfs:comment "Decreased ability to see to a degree that requires corrective measures" ;
    rdfs:subClassOf imdrf:E08 .

imdrf:E1716 a owl:Class ;
    rdfs:label "Skin Discoloration" ;
    ex:nonIMDRFCode "MedDRA:10040828:Skin discoloration" ;
    rdfs:comment "any abnormal change in skin coloration." ;
    rdfs:subClassOf imdrf:E17 .

imdrf:E1901 a owl:Class ;
    rdfs:label "Bacterial Infection" ;
    ex:nonIMDRFCode "MedDRA:10060945:Bacterial infection" ;
    rdfs:comment "An acute infectious disorder caused by gram positive or gram negative bacteria." ;
    rdfs:subClassOf imdrf:E19 .

imdrf:E2301 a owl:Class ;
    rdfs:label "Alteration in Body Temperature" ;
    ex:nonIMDRFCode "MedDRA:10063488:Body temperature fluctuation" ;
    rdfs:comment "A Change or alteration of Body Temperature to a temperature outside the range of normal body temperature." ;
    rdfs:subClassOf imdrf:E23 .

imdrf:E24 a owl:Class ;
    rdfs:label "Other Terms/Codes Related to Clinical Signs and Symptoms or Conditions" ;
    ex:status "Not selectable, Modified (editorial)" ;
    ex:statusDescription "Please use more detailed term within the hierarchy. NOTE: Term modified for Release Number 2025. Previous term was \"Others\". See no. 141 of Change Request Log." ;
    rdfs:comment "Others" .

imdrf:F01 a owl:Class ;
    rdfs:label "Change in Therapeutic Response" ;
    rdfs:comment "Change in response to treatment or cure of a disorder or disease." .

imdrf:G02007 a owl:Class ;
    rdfs:label "Computer Hardware" ;
    rdfs:comment "The physical components from which a computer is constructed (electronic circuits and input/output devices)." ;
    rdfs:subClassOf imdrf:G02 .

imdrf:G02015 a owl:Class ;
    rdfs:label "Electrical Lead/Wire" ;
    rdfs:comment "A coated or uncoated wire used to connect two locations electronically. Not to be used for patient connection." ;
    rdfs:subClassOf imdrf:G02 .

imdrf:G03007 a owl:Class ;
    rdfs:label "Gauges/Meters" ;
    rdfs:comment "A component designed to give a visual indication of the condition of a system." ;
    rdfs:subClassOf imdrf:G03 .

imdrf:G04135 a owl:Class ;
    rdfs:label "Valve(s)" ;
    rdfs:comment "A mechanical component designed to control the flow of a fluid or gas." ;
    rdfs:subClassOf imdrf:G04 .

imdrf:G07 a owl:Class ;
    rdfs:label "Other Terms/Codes Related to Components" ;
    ex:status "Not selectable, Modified (editorial)" ;
    ex:statusDescription "Please use more detailed term within the hierarchy. NOTE: Definition changed to update a working note on 16 Feb. 2021. Editorial change to term for Release Number 2025. See no. 123 of Change Log." ;
    rdfs:comment "Others." .

imdrf:A0401 a owl:Class ;
    rdfs:label "Break" ;
    rdfs:comment "Problem associated with undesired damage or breakage of those materials used in the device construction." ;
    rdfs:subClassOf imdrf:A04 .

imdrf:A0701 a owl:Class ;
    rdfs:label "Capturing Problem" ;
    rdfs:comment "Problem associated with the inability of the device to achieve successful depolarization and contraction of a cardiac chamber caused by a pacemaker output pulse." ;
    rdfs:subClassOf imdrf:A07 .

imdrf:A0705 a owl:Class ;
    rdfs:label "Battery Problem" ;
    rdfs:comment "Problem associated with the internal power of the device (e.g. battery, transformer, fuel cell or other power sources)." ;
    rdfs:subClassOf imdrf:A07 .

imdrf:A0708 a owl:Class ;
    rdfs:label "Power Problem" ;
    rdfs:comment "Problem associated with the energy to operate the device." ;
    rdfs:subClassOf imdrf:A07 .

imdrf:A0905 a owl:Class ;
    rdfs:label "Radiation Output Problem" ;
    rdfs:comment "Problem with the device's intended output of radiation." ;
    rdfs:subClassOf imdrf:A09 .

imdrf:A1403 a owl:Class ;
    rdfs:label "Filling Problem" ;
    rdfs:comment "Problem associated with the method or amount of time associated with the delivery of a fluid. Time to delivery or amount of delivered entity may be affected." ;
    rdfs:subClassOf imdrf:A14 .

imdrf:A1412 a owl:Class ;
    rdfs:label "Pumping Problem" ;
    ex:statusDescription "Definition was modified on 31 January 2023 (Old definition: Problem associated with pump performance deviating from specifications in a way to compromise flow or infusion). For details, see comment No. 35 of the Change Log (Release Number 2023)." ;
    rdfs:comment "Problem associated with pump performance deviating from specifications in a way to compromise flow or infusion or dispensing." ;
    rdfs:subClassOf imdrf:A14 .

imdrf:A17 a owl:Class ;
    rdfs:label "Compatibility Problem" ;
    rdfs:comment "Problem associated with compatibility between device, patients or substances (medication, body fluid, etc.)" .

imdrf:A18 a owl:Class ;
    rdfs:label "Contamination /Decontamination Problem" ;
    rdfs:comment "Problem associated with the presence of any unexpected foreign substance found in the device, on its surface or in the package materials, which may affect performance or intended use of the device, or problem that compromise effective decontamination of the device." .

imdrf:C0106 a owl:Class ;
    rdfs:label "Hematological Problem Identified" ;
    rdfs:comment "The device affects or impacts the blood or its components. (See ISO 10993 all parts)" ;
    rdfs:subClassOf imdrf:C01 .

imdrf:C04 a owl:Class ;
    rdfs:label "Interoperability Problem Identified" ;
    rdfs:comment "Problems with the mechanical, electrical, or communication interface between two or more separate devices." .

imdrf:C09 a owl:Class ;
    rdfs:label "Clinical Imaging Problem Identified" ;
    rdfs:comment "Problems that occur with devices used for radiographic or imaging procedures e.g. CT scanners, magnetic resonance imaging." .

imdrf:C11 a owl:Class ;
    rdfs:label "Thermal Problem" ;
    rdfs:comment "Problems related to the temperature of the device. Note: For problems related to environmental temperature use ''Environment Problem Identified''." .

imdrf:C13 a owl:Class ;
    rdfs:label "Operational Problem Identified" ;
    rdfs:comment "Problems that occur during the performance, use, or functioning of the device." .

imdrf:C14 a owl:Class ;
    rdfs:label "Patient Sample Problem" ;
    rdfs:comment "Problems that occurred due to endogenous or exogenous interferent in the sample, or unexpected variation in the target analyte/marker." .

imdrf:C1605 a owl:Class ;
    rdfs:label "Packaging Problem Identified" ;
    rdfs:comment "Problems that occurred because of the device packaging." ;
    rdfs:subClassOf imdrf:C16 .

imdrf:E0109 a owl:Class ;
    rdfs:label "Convulsion/Seizure" ;
    ex:nonIMDRFCode "MedDRA:10010904:Convulsion" ;
    rdfs:comment "Sudden, involuntary skeletal muscular contractions of cerebral or brain stem origin." ;
    rdfs:subClassOf imdrf:E01 .

imdrf:E0621 a owl:Class ;
    rdfs:label "Valvular Insufficiency/ Regurgitation" ;
    ex:nonIMDRFCode "MedDRA:10058086:Heart valve insufficiency" ;
    rdfs:comment "Dysfunction of one of the cardiac valves, with incomplete valve closure or damage to a valve leaflet resulting in valvular backflow." ;
    rdfs:subClassOf imdrf:E06 .

imdrf:E0622 a owl:Class ;
    rdfs:label "Valvular Stenosis" ;
    ex:nonIMDRFCode "MedDRA:10061996:Heart valve stenosis" ;
    rdfs:comment "Obstruction of flow across a heart valve due to immobility of the leaflets and/or a restricted orifice." ;
    rdfs:subClassOf imdrf:E06 .

imdrf:E0838 a owl:Class ;
    rdfs:label "Visual Disturbances" ;
    ex:nonIMDRFCode "MedDRA:10047545:Visual disturbances" ;
    rdfs:comment "An interference to normal eyesight without necessarily affecting visual acuity." ;
    rdfs:subClassOf imdrf:E08 .

imdrf:E1801 a owl:Class ;
    rdfs:label "Cancer" ;
    ex:nonIMDRFCode "MedDRA:10007050:Cancer" ;
    rdfs:comment "A group of diseases in which abnormal cells divide without control, invade nearby tissues and may also spread to other parts of the body through the blood and lymph systems." ;
    rdfs:subClassOf imdrf:E18 .

imdrf:F22 a owl:Class ;
    rdfs:label "Unexpected Diagnostic Intervention" ;
    rdfs:comment "Diagnostic intervention needed to be completed that was not originally planned." .

imdrf:G02008 a owl:Class ;
    rdfs:label "Computer Software" ;
    rdfs:comment "A collection of data or computer instructions that tell the computer how to work." ;
    rdfs:subClassOf imdrf:G02 .

imdrf:G02040 a owl:Class ;
    rdfs:label "User Input Device" ;
    rdfs:comment "A component that uses a movable handle to create two-axis input to a computer." ;
    rdfs:subClassOf imdrf:G02 .

imdrf:A0205 a owl:Class ;
    rdfs:label "Packaging Problem" ;
    rdfs:comment "Problem associated with the materials used to construct the cover or outer wrapping of the device." ;
    rdfs:subClassOf imdrf:A02 .

imdrf:A0507 a owl:Class ;
    rdfs:label "Mechanics Altered" ;
    rdfs:comment "Problem associated with a device mechanical functioning of machinery, moving parts or tools of device being changed or modified." ;
    rdfs:subClassOf imdrf:A05 .

imdrf:A0511 a owl:Class ;
    rdfs:label "Structural Problem" ;
    rdfs:comment "Problem associated with the basic physical construction or physical make up of the device." ;
    rdfs:subClassOf imdrf:A05 .

imdrf:A06 a owl:Class ;
    rdfs:label "Optical Problem" ;
    rdfs:comment "Problem associated with transmission of visible light affecting the quality of the image transmitted or otherwise affecting the intended application of the visible light path." .

imdrf:A08 a owl:Class ;
    rdfs:label "Calibration Problem" ;
    rdfs:comment "Problem associated with the operation of the device, related to its accuracy, and associated with the calibration of the device." .

imdrf:A13 a owl:Class ;
    rdfs:label "Communication or Transmission Problem" ;
    rdfs:comment "Problem associated with the device sending or receiving signals or data. This includes transmission among internal components of the device to which the device is intended to communicate." .

imdrf:A1801 a owl:Class ;
    rdfs:label "Contamination" ;
    ex:statusDescription "Technical change to the term on 18 March 2020 to separate when/where contamination occurred from type of contamination (\"During Use\" was removed). NOTE: This change affects all lower level terms (A180101 - A180105) which are also no longer limited to contamination during use." ;
    rdfs:comment "Problem associated with the undesired introduction of impurities either chemical or microbiological in nature, or of foreign matter into or onto the device." ;
    rdfs:subClassOf imdrf:A18 .

imdrf:A21 a owl:Class ;
    rdfs:label "Labelling, Instructions for Use or Training Problem" ;
    rdfs:comment "Problem associated with device markings/labelling, instructions for use, training and maintenance documentation or guidelines." .

imdrf:A23 a owl:Class ;
    rdfs:label "Use of Device Problem" ;
    rdfs:comment "Problem associated with failure to process, service, or operate the device according to the manufacturer's recommendations or recognized best practices." .

imdrf:C03 a owl:Class ;
    rdfs:label "Electromagnetic Compatibility Problem Identified" ;
    rdfs:comment "Device-to-device or device-environment problem resulting from electromagnetic disturbances." .

imdrf:C16 a owl:Class ;
    rdfs:label "Manufacturing Process Problem Identified" ;
    rdfs:comment "Problems with a device that can be traced to a problem in the manufacturing and/or production process." .

imdrf:E0202 a owl:Class ;
    rdfs:label "Emotional Changes" ;
    ex:nonIMDRFCode "MedDRA:10014551:Emotional disorder" ;
    rdfs:comment "Change from the affected person's usual emotional state." ;
    rdfs:subClassOf imdrf:E02 .

imdrf:E04 a owl:Class ;
    rdfs:label "Immune System" ;
    ex:status "Not selectable" ;
    ex:statusDescription "Please use more detailed term within the hierarchy" ;
    rdfs:comment "Immune System" .

imdrf:E0503 a owl:Class ;
    rdfs:label "Embolism/Embolus" ;
    ex:nonIMDRFCode "MedDRA:10061169:Embolism" ;
    rdfs:comment "The blockage of a blood vessel lumen by air or solid material such as blood clot or other tissues (e.g., adipose tissue, cancer cells) that have migrated from another anatomic site." ;
    rdfs:subClassOf imdrf:E05 .

imdrf:E1501 a owl:Class ;
    rdfs:label "Abortion" ;
    ex:nonIMDRFCode "MedDRA:10000210:Abortion" ;
    rdfs:comment "The unintentional or intentional loss of a pregnancy before 22 weeks gestation." ;
    rdfs:subClassOf imdrf:E15 .

imdrf:E1603 a owl:Class ;
    rdfs:label "Bone Fracture(s)" ;
    ex:nonIMDRFCode "MedDRA:10017076:Fracture" ;
    rdfs:comment "A traumatic or pathological injury to the bone in which the continuity of the bone is broken." ;
    rdfs:subClassOf imdrf:E16,
        imdrf:E20 .

imdrf:E1616 a owl:Class ;
    rdfs:label "Loss of Range of Motion" ;
    ex:nonIMDRFCode "MedDRA:10048706:Joint range of motion decreased" ;
    rdfs:comment "A finding that the flexibility of a joint is below the expected range of normal for that individual." ;
    rdfs:subClassOf imdrf:E16 .

imdrf:E18 a owl:Class ;
    rdfs:label "Neoplasms Benign, Malignant and Unspecified" ;
    ex:status "Not selectable" ;
    ex:statusDescription "Please use more detailed term within the hierarchy" ;
    rdfs:comment "Neoplasms Benign, Malignant and Unspecified" .

imdrf:F12 a owl:Class ;
    rdfs:label "Serious Injury/ Illness/ Impairment" ;
    rdfs:comment "A severe injury, illness or impairment which requires hospitalization or medical intervention." .

imdrf:A1501 a owl:Class ;
    rdfs:label "Activation Problem" ;
    ex:statusDescription "Technical change to the definition on 18 March 2020 to clarify that activation includes expansion." ;
    rdfs:comment "Problem associated with the activation of the device. Note: Activation includes expansion." ;
    rdfs:subClassOf imdrf:A15 .

imdrf:A1601 a owl:Class ;
    rdfs:label "Device Alarm System" ;
    rdfs:comment "Problem associated with the alarm system of the device." ;
    rdfs:subClassOf imdrf:A16 .

imdrf:A1803 a owl:Class ;
    rdfs:label "Device Reprocessing Problem" ;
    rdfs:comment "Problem associated with a failure during any step of reprocessing process (cleaning, disinfection, packaging, labeling, sterilization) of a used or opened from its original packaging, but unused, device." ;
    rdfs:subClassOf imdrf:A18 .

imdrf:A22 a owl:Class ;
    rdfs:label "Human-Device Interface Problem" ;
    ex:status "Modified (technical)" ;
    ex:statusDescription "Definition modified for Release Number 2025. See no. 45 of Change Request Log." ;
    rdfs:comment "Problem associated with the user experiencing difficulty operating or otherwise interacting with the device, even if the operation is being performed according to labeled instructions for use." .

imdrf:C06 a owl:Class ;
    rdfs:label "Material and/or Chemical Problem Identified" ;
    rdfs:comment "Problems with the device materials or how its materials react to other elements either within the device or within the environment." .

imdrf:C0706 a owl:Class ;
    rdfs:label "Stress Problem Identified" ;
    rdfs:comment "Problems caused by either excessive or inadequate physical force exerted on it by another object resulting in problems e.g. wear, bending, deformation, fracture, fatigue." ;
    rdfs:subClassOf imdrf:C07 .

imdrf:C1002 a owl:Class ;
    rdfs:label "Design Error" ;
    rdfs:comment "The device had faulty (incomplete or incorrect) software design." ;
    rdfs:subClassOf imdrf:C10 .

imdrf:C15 a owl:Class ;
    rdfs:label "Environment Problem Identified" ;
    rdfs:comment "Problems that occurred due to factors within the environment e.g. dust, dirt, humidity, temperature." .

imdrf:E0819 a owl:Class ;
    rdfs:label "Eye Injury" ;
    ex:nonIMDRFCode "MedDRA:10061128:Eye injury" ;
    rdfs:comment "Damage to the eye." ;
    rdfs:subClassOf imdrf:E08,
        imdrf:E20 .

imdrf:E2336 a owl:Class ;
    rdfs:label "Shock" ;
    ex:nonIMDRFCode "MedDRA:10040560:Shock" ;
    ex:statusDescription "Editorial change to the definition on 16 February 2021." ;
    rdfs:comment "A life-threatening condition that requires immediate medical intervention. It is characterized by reduced blood flow that may result in damage of multiple organs." ;
    rdfs:subClassOf imdrf:E23 .

imdrf:G03012 a owl:Class ;
    rdfs:label "Sensor" ;
    rdfs:comment "A component designed to respond to a stimulus by generating a signal that can be measured or interpreted." ;
    rdfs:subClassOf imdrf:G03 .

imdrf:A01 a owl:Class ;
    rdfs:label "Patient Device Interaction Problem" ;
    rdfs:comment "Problem related to the interaction between the patient and the device." .

imdrf:A02 a owl:Class ;
    rdfs:label "Manufacturing, Packaging or Shipping Problem" ;
    ex:status "Modified (technical)" ;
    ex:statusDescription "Definition modified for Release Number 2025. See no. 42 of Change Request Log" ;
    rdfs:comment "Problem associated with any deviations from the intended performance of the device that appear to relate to the manufacturing, packaging or shipping processes." .

imdrf:A0904 a owl:Class ;
    rdfs:label "Energy Output Problem" ;
    rdfs:comment "Problem with the device's intended output of energy." ;
    rdfs:subClassOf imdrf:A09 .

imdrf:A16 a owl:Class ;
    rdfs:label "Protective Measures Problem" ;
    rdfs:comment "Problem associated with any deviations from the documented specifications of the device that relate to the implemented and inherited design features specific to devices used for reducing risks to patient or caregiver or maintaining risks within specified levels." .

imdrf:A2101 a owl:Class ;
    rdfs:label "Device Markings/Labelling Problem" ;
    rdfs:comment "Problem associated with the written, printed or graphic material accompanying or affixed to the device or any of its packaging. This includes verbal instructions relating to identification, technical description, and usage provided by the device manufacturers. Problems can include but are not limited to this material being unclear, missing, worn out, incorrect or inaccurate." ;
    rdfs:subClassOf imdrf:A21 .

imdrf:G01 a owl:Class ;
    rdfs:label "Biological and Chemical" ;
    ex:status "Not selectable" ;
    ex:statusDescription "Please use more detailed term within the hierarchy" ;
    rdfs:comment "Component whose mode of action involves a biological process (ex. test strip which acts on antibodies) and chemical reaction or transformation (ex. activated charcoal absorber)." .

imdrf:G06 a owl:Class ;
    rdfs:label "Safety" ;
    ex:status "Not selectable" ;
    ex:statusDescription "Please use more detailed term within the hierarchy" ;
    rdfs:comment "Safety related component" .

imdrf:A0302 a owl:Class ;
    rdfs:label "Device Ingredient or Reagent Problem" ;
    rdfs:comment "Problem associated with any deviations from the documented specifications of the device that relate to any ingredient or reagent characterization." ;
    rdfs:subClassOf imdrf:A03 .

imdrf:A0405 a owl:Class ;
    rdfs:label "Degraded" ;
    rdfs:comment "Problem associated with a undesired change in the chemical structure, physical properties, or appearance in the materials that are used in the device construction." ;
    rdfs:subClassOf imdrf:A04 .

imdrf:A0512 a owl:Class ;
    rdfs:label "Unintended Movement" ;
    rdfs:comment "Problem associated with an undesired movement of the device, which may be related to the device malfunction, misdiagnosis, or mistreatment." ;
    rdfs:subClassOf imdrf:A05 .

imdrf:A11 a owl:Class ;
    rdfs:label "Computer Software Problem" ;
    rdfs:comment "Problem associated with written programs, codes, and/or software system that affects device performance or communication with another device." .

imdrf:A1102 a owl:Class ;
    rdfs:label "Application Program Problem" ;
    rdfs:comment "Problem associated with the requirement for software to fulfill its function within an intended use or application." ;
    rdfs:subClassOf imdrf:A11 .

imdrf:A12 a owl:Class ;
    rdfs:label "Connection Problem" ;
    rdfs:comment "Problem associated with linking of the device and/or the functional units set up to provide means for a transfer of liquid, gas, electricity or data." .

imdrf:A1502 a owl:Class ;
    rdfs:label "Positioning Problem" ;
    rdfs:comment "Problem associated with the movement of the device to an intended location." ;
    rdfs:subClassOf imdrf:A15 .

imdrf:C07 a owl:Class ;
    rdfs:label "Mechanical Problem Identified" ;
    rdfs:comment "Problems that result from internal or external forces including fluids, other objects, or environmental or physiologic influences." .

imdrf:C12 a owl:Class ;
    rdfs:label "Protective System Problem Identified" ;
    rdfs:comment "Problems related to the system(s) designed to prevent or warn about unsafe operation of the device." .

imdrf:D01 a owl:Class ;
    rdfs:label "Cause Traced to Device Design" ;
    rdfs:comment "Problems traced to the design specifications (e.g. in the requirements, testing processes, hazard analysis, implementation strategy)." .

imdrf:D11 a owl:Class ;
    rdfs:label "Cause Traced to User" ;
    rdfs:comment "The adverse event caused partially or wholly by the user of the device including sample handling." .

imdrf:E1704 a owl:Class ;
    rdfs:label "Burn(s)" ;
    ex:nonIMDRFCode "MedDRA:10006634:Burn" ;
    rdfs:comment "An injury or tissue damage caused by exposure to caustic chemicals, extreme heat, extreme cold or excessive radiation." ;
    rdfs:subClassOf imdrf:E17,
        imdrf:E20 .

imdrf:E1720 a owl:Class ;
    rdfs:label "Skin Inflammation/ Irritation" ;
    ex:nonIMDRFCode "MedDRA:10062249:Skin inflammation" ;
    rdfs:comment "An inflammatory process affecting the skin. Signs include red rash, itching, and blister formation. Representative examples are contact dermatitis, atopic dermatitis, and seborrheic dermatitis." ;
    rdfs:subClassOf imdrf:E17 .

imdrf:G02012 a owl:Class ;
    rdfs:label "Discrete Electrical Component" ;
    rdfs:comment "An electrical component which is just one circuit, either passive or active, that is not an integrated circuit." ;
    rdfs:subClassOf imdrf:G02 .

imdrf:A0504 a owl:Class ;
    rdfs:label "Leak/Splash" ;
    ex:status "Modified (technical)" ;
    ex:statusDescription "Definition was modified on 27 January 2022 (Old definition: Leak/Splash: Problem associated with the escape of a liquid, gas or radiation from the vessel or container in which it is housed). For details, see comment No. 14 of the Change Log (Release Number 2022).  Definition modified for Release Number 2025. See no. 2 of Change Request Log." ;
    rdfs:comment "Problem associated with the escape or ingress of a liquid (including blood and bodily fluids), gas or radiation from or into a vessel or container." ;
    rdfs:subClassOf imdrf:A05 .

imdrf:A0712 a owl:Class ;
    rdfs:label "Pacing Problem" ;
    rdfs:comment "Problem associated with the inability of the device to generate a therapeutic simulated heart beat via electrical impulses." ;
    rdfs:subClassOf imdrf:A07 .

imdrf:A09 a owl:Class ;
    rdfs:label "Output Problem" ;
    rdfs:comment "Problem associated with any deviation from the documented specifications of the device that relate to the end result, data, or test results provided by the device." .

imdrf:A0902 a owl:Class ;
    rdfs:label "Display or Visual Feedback Problem" ;
    rdfs:comment "Problem with any deviation from the documented specifications of the device that relate to visual feedback. e.g. the display of information, images on a screen, or output from the device." ;
    rdfs:subClassOf imdrf:A09 .

imdrf:A10 a owl:Class ;
    rdfs:label "Temperature Problem" ;
    rdfs:comment "Problem associated with the device producing unintended temperatures." .

imdrf:A1405 a owl:Class ;
    rdfs:label "Improper Flow or Infusion" ;
    rdfs:comment "Problem associated with the regulation and delivery of therapeutic agents (e.g. air, gas, drugs or fluids into a device or a patient under positive pressure)." ;
    rdfs:subClassOf imdrf:A14 .

imdrf:C01 a owl:Class ;
    rdfs:label "Biological Problem Identified" ;
    rdfs:comment "Problems relating to, caused by or affecting biological processes or living organisms." .

imdrf:E0122 a owl:Class ;
    rdfs:label "Movement Disorder" ;
    ex:nonIMDRFCode "MedDRA:10028035:Movement disorder" ;
    rdfs:comment "Neurological conditions resulting in abnormal voluntary or involuntary movement, which may impact the speed, fluency, quality and ease of movement." ;
    rdfs:subClassOf imdrf:E01 .

imdrf:E02 a owl:Class ;
    rdfs:label "Mental, Emotional and Behavioural Disorders" ;
    ex:status "Not selectable" ;
    ex:statusDescription "Please use more detailed term within the hierarchy" ;
    rdfs:comment "Mental, Emotional and Behavioural Disorders" .

imdrf:E11 a owl:Class ;
    rdfs:label "Hepatic and Biliary System" ;
    ex:status "Not selectable" ;
    ex:statusDescription "Please use more detailed term within the hierarchy" ;
    rdfs:comment "Hepatic and Biliary System" .

imdrf:E1202 a owl:Class ;
    rdfs:label "Electrolyte Imbalance" ;
    ex:nonIMDRFCode "MedDRA:10014418:Electrolyte imbalance" ;
    rdfs:comment "Higher or lower than normal values for the serum electrolytes; usually affecting Na, K, Cl, Ca, CO2, BUN." ;
    rdfs:subClassOf imdrf:E03,
        imdrf:E12 .

imdrf:E2338 a owl:Class ;
    rdfs:label "Swelling/ Edema" ;
    ex:nonIMDRFCode "MedDRA:10014210:Edema" ;
    rdfs:comment "Enlargement or expansion in size of a body part from injury or inflammation." ;
    rdfs:subClassOf imdrf:E23 .

imdrf:F23 a owl:Class ;
    rdfs:label "Unexpected Medical Intervention" ;
    rdfs:comment "Patient required an unforeseen medical intervention, excluding surgery, which was not on the original treatment plan." .

imdrf:G05 a owl:Class ;
    rdfs:label "Optical" ;
    ex:status "Not selectable" ;
    ex:statusDescription "Please use more detailed term within the hierarchy" ;
    rdfs:comment "Component which involves or relates to vision, light, or images." .

imdrf:A19 a owl:Class ;
    rdfs:label "Environmental Compatibility Problem" ;
    rdfs:comment "Problem associated with the surrounding conditions in which the device is being used such as temperature, noise, lighting, ventilation, or other external factors such as power supply." .

imdrf:C02 a owl:Class ;
    rdfs:label "Electrical Problem Identified" ;
    rdfs:comment "Events associated with an electrically powered device where an electrical malfunction results in a device problem (e.g. electrical circuitry, contact or component failed) even if the problem is intermittent." .

imdrf:E0601 a owl:Class ;
    rdfs:label "Arrhythmia" ;
    ex:nonIMDRFCode "MedDRA:10003119:Arrhythmia" ;
    rdfs:comment "Any variation from the normal rate or rhythm (which may include the origin of the impulse and/or its subsequent propagation) in the heart." ;
    rdfs:subClassOf imdrf:E06 .

imdrf:F10 a owl:Class ;
    rdfs:label "Inadequate/Inappropriate Treatment or Diagnostic Exposure" ;
    ex:status "Modified (technical)" ;
    ex:statusDescription "Definition modified for Release Number 2025. See no. 19 of Change Request Log" ;
    rdfs:comment "Patient did not receive intended treatment from a device or received inadequate treatment as a consequence of device performance. This includes inadequate/inappropriate electrical stimulation or radiation dosage during procedures." .

imdrf:F19 a owl:Class ;
    rdfs:label "Surgical Intervention" ;
    ex:statusDescription "Definition was modified on 31 January 2023 (Old definition: One or more surgical procedures was required, or an existing procedure changed). For details, see comment No. 135 /137/138 /139 /140/141 of the Change Log (Release Number 2023)." ;
    rdfs:comment "One or more surgical procedures, including percutaneous or minimally invasive procedures, were required, or an existing procedure changed." .

imdrf:C10 a owl:Class ;
    rdfs:label "Software Problem Identified" ;
    rdfs:comment "Problems related to the device software." .

imdrf:E2114 a owl:Class ;
    rdfs:label "Perforation" ;
    ex:nonIMDRFCode "MedDRA:10076705:Perforation" ;
    rdfs:comment "A hole or opening made through a membrane or other tissue or material." ;
    rdfs:subClassOf imdrf:E21 .

imdrf:A0406 a owl:Class ;
    rdfs:label "Material Deformation" ;
    rdfs:comment "Problem associated with an undesired material change in shape or property caused by external forces." ;
    rdfs:subClassOf imdrf:A04 .

imdrf:A0709 a owl:Class ;
    rdfs:label "Device Sensing Problem" ;
    rdfs:comment "Problem associated with the device feature that are designed to respond to a physical stimulus (temperature, illumination, motion, cardiac rhythms) and that do not transmit a resulting signal for interpretation or measurement." ;
    rdfs:subClassOf imdrf:A07 .

imdrf:E2330 a owl:Class ;
    rdfs:label "Pain" ;
    ex:nonIMDRFCode "MedDRA:10033371:Pain" ;
    rdfs:comment "An unpleasant sensory and emotional experience that is associated with actual or potential tissue damage or described in such terms." ;
    rdfs:subClassOf imdrf:E23 .

imdrf:A05 a owl:Class ;
    rdfs:label "Mechanical Problem" ;
    rdfs:comment "Problems associated with mechanical actions or defects, including moving parts or subassemblies, etc." .

imdrf:A0908 a owl:Class ;
    rdfs:label "Incorrect, Inadequate or Imprecise Result or Readings" ;
    ex:statusDescription "Editorial change to the term on 16 Feburary 2021." ;
    rdfs:comment "Problem associated with a nonconforming end result, data, or test results provided by the device to its performance specifications." ;
    rdfs:subClassOf imdrf:A09 .

imdrf:E03 a owl:Class ;
    rdfs:label "Blood and Lymphatic System" ;
    ex:status "Not selectable" ;
    ex:statusDescription "Please use more detailed term within the hierarchy" ;
    rdfs:comment "Blood and Lymphatic System" .

imdrf:E09 a owl:Class ;
    rdfs:label "Ear and Labyrinth" ;
    ex:status "Not selectable" ;
    ex:statusDescription "Please use more detailed term within the hierarchy" ;
    rdfs:comment "Ear and Labyrinth" .

imdrf:A14 a owl:Class ;
    rdfs:label "Infusion or Flow Problem" ;
    ex:statusDescription "Definition was modified on 31 January 2023 (Old definition: Problem associated with the device failing to deliver or draw liquids or gases as intended (e.g. delivering drugs at incorrect rate, Problems with drawing fluid from a system). This includes vacuum collection devices.). For details, see comment No. 35 of the Change Log (Release Number 2023)." ;
    rdfs:comment "Problem associated with the device failing to deliver or draw liquids or gases as intended (e.g. delivering drugs at incorrect rate, problems with drawing fluid from a system). This includes vacuum collection devices and manual or mechanical pumps." .

imdrf:A04 a owl:Class ;
    rdfs:label "Material Integrity Problem" ;
    rdfs:comment "Problem associated with any deviations from the documented specifications of the device that relate to the limited durability of all material used to construct device." .

imdrf:G03 a owl:Class ;
    rdfs:label "Measurement" ;
    ex:status "Not selectable" ;
    ex:statusDescription "Please use more detailed term within the hierarchy" ;
    rdfs:comment "Component capable of measuring something in order to obtain a result." .

imdrf:G04052 a owl:Class ;
    rdfs:label "Fastener" ;
    rdfs:comment "A component designed to hold items in place." ;
    rdfs:subClassOf imdrf:G04 .

imdrf:E13 a owl:Class ;
    rdfs:label "Kidney and Urinary Tract" ;
    ex:status "Not selectable" ;
    ex:statusDescription "Please use more detailed term within the hierarchy" ;
    rdfs:comment "Kidney and Urinary Tract" .

imdrf:E12 a owl:Class ;
    rdfs:label "Endocrine, Metabolism and Nutrition" ;
    ex:status "Not selectable" ;
    ex:statusDescription "Please use more detailed term within the hierarchy. NOTE: Term was modified on 18 March 2020 to include Endocrine." ;
    rdfs:comment "Endocrine, Metabolism and Nutrition" .

imdrf:E15 a owl:Class ;
    rdfs:label "Pregnancy, Childbirth and the Puerperium" ;
    ex:status "Not selectable" ;
    ex:statusDescription "Please use more detailed term within the hierarchy" ;
    rdfs:comment "Pregnancy, Childbirth and the Puerperium" .

imdrf:E22 a owl:Class ;
    rdfs:label "Investigations and Diagnostic Tests" ;
    ex:status "Not selectable" ;
    ex:statusDescription "Please use more detailed term within the hierarchy" ;
    rdfs:comment "Investigations and Diagnostic Tests" .

imdrf:A07 a owl:Class ;
    rdfs:label "Electrical /Electronic Property Problem" ;
    ex:statusDescription "Definition was modified on 31 January 2023 to replace \"a failure\" with \"the function\". For details, see comment No. 8 of the Change Log (Release Number 2023)." ;
    rdfs:comment "Problem associated with the function of the electrical circuitry of the device." .

imdrf:E14 a owl:Class ;
    rdfs:label "Reproductive System and Breast" ;
    ex:status "Not selectable" ;
    ex:statusDescription "Please use more detailed term within the hierarchy" ;
    rdfs:comment "Reproductive System and Breast" .

imdrf:E17 a owl:Class ;
    rdfs:label "Skin and Subcutaneous Tissue" ;
    ex:status "Not selectable" ;
    ex:statusDescription "Please use more detailed term within the hierarchy" ;
    rdfs:comment "Skin and Subcutaneous Tissue" .

imdrf:E06 a owl:Class ;
    rdfs:label "Heart" ;
    ex:status "Not selectable" ;
    ex:statusDescription "Please use more detailed term within the hierarchy" ;
    rdfs:comment "Heart" .

imdrf:E05 a owl:Class ;
    rdfs:label "Vascular System" ;
    ex:status "Not selectable" ;
    ex:statusDescription "Please use more detailed term within the hierarchy" ;
    rdfs:comment "Vascular System" .

imdrf:E19 a owl:Class ;
    rdfs:label "Infections" ;
    ex:status "Not selectable" ;
    ex:statusDescription "Please use more detailed term within the hierarchy" ;
    rdfs:comment "Infections" .

imdrf:E20 a owl:Class ;
    rdfs:label "Injury" ;
    ex:status "Not selectable" ;
    ex:statusDescription "Please use more detailed term within the hierarchy" ;
    rdfs:comment "Injury" .

imdrf:E10 a owl:Class ;
    rdfs:label "Gastrointestinal System" ;
    ex:status "Not selectable" ;
    ex:statusDescription "Please use more detailed term within the hierarchy" ;
    rdfs:comment "Gastrointestinal System" .

imdrf:G02 a owl:Class ;
    rdfs:label "Electrical and Magnetic" ;
    ex:status "Not selectable" ;
    ex:statusDescription "Please use more detailed term within the hierarchy" ;
    rdfs:comment "Components which relates to the force of magnetism or such as microchips and transistors which control and direct electric currents. Also includes components involved in the representation, storage, or transmission of information by electronic systems." .

imdrf:E21 a owl:Class ;
    rdfs:label "Procedural Complications" ;
    ex:status "Not selectable" ;
    ex:statusDescription "Please use more detailed term within the hierarchy" ;
    rdfs:comment "Procedural Complications" .

imdrf:E01 a owl:Class ;
    rdfs:label "Nervous System" ;
    ex:status "Not selectable" ;
    ex:statusDescription "Please use more detailed term within the hierarchy" ;
    rdfs:comment "Nervous System" .

imdrf:E16 a owl:Class ;
    rdfs:label "Musculoskeletal System" ;
    ex:status "Not selectable" ;
    ex:statusDescription "Please use more detailed term within the hierarchy" ;
    rdfs:comment "Musculoskeletal System" .

imdrf:E23 a owl:Class ;
    rdfs:label "Generalized Disorders" ;
    ex:status "Not selectable" ;
    ex:statusDescription "Please use more detailed term within the hierarchy" ;
    rdfs:comment "Generalized Disorders" .

imdrf:E08 a owl:Class ;
    rdfs:label "Eye" ;
    ex:status "Not selectable" ;
    ex:statusDescription "Please use more detailed term within the hierarchy" ;
    rdfs:comment "Eye" .

imdrf:E07 a owl:Class ;
    rdfs:label "Respiratory System" ;
    ex:status "Not selectable" ;
    ex:statusDescription "Please use more detailed term within the hierarchy" ;
    rdfs:comment "Respiratory System" .

imdrf:G04 a owl:Class ;
    rdfs:label "Mechanical" ;
    ex:status "Not selectable" ;
    ex:statusDescription "Please use more detailed term within the hierarchy" ;
    rdfs:comment "Component of a device when it is working, often using power from an engine or from electricity." .

